format-version: 1.2
auto-generated-by: java
default-namespace: BananaTrait
namespace-id-rule: * CO_325:$sequence(7,0000000,0009999)$
ontology: CO_325

[Term]
id: CO_325:0000000
name: time from planting to shooting
namespace: BananaTrait
def: "The time elapsed from planting to shooting (when the inflorescence emerges from the pseudostem)." []
synonym: "Length of vegetative stage" EXACT []
synonym: "plant2shoot" EXACT []
is_a: CO_325:1000002

[Term]
id: CO_325:0000003
name: time from shooting to harvest
namespace: BananaTrait
def: "The time elapsed from shooting (when the inflorescence emerges from the pseudostem) to the harvest of the bunch." []
synonym: "shoot2harvest" EXACT []
synonym: "Time of fruit-filling, Fruit-filling period, Bunch maturity period, Length of reproductive stage, Bunch maturation period" EXACT []
is_a: CO_325:1000002

[Term]
id: CO_325:0000006
name: plant crop cycle
namespace: BananaTrait
def: "The time elapsed from planting to the harvest of the bunch." []
synonym: "Crop cycle, Mother plant crop cycle, Time from planting to harvest" EXACT []
synonym: "plant2harvest" EXACT []
is_a: CO_325:1000002

[Term]
id: CO_325:0000009
name: plant height
namespace: BananaTrait
def: "The height of the pseudostem of the plant." []
synonym: "plantheight" EXACT []
synonym: "Pseudostem height" EXACT []
is_a: CO_325:1000005

[Term]
id: CO_325:0000012
name: plant circumference
namespace: BananaTrait
def: "The circumference of the pseudostem of the plant at 1 m from the ground." []
synonym: "plantcircumf" EXACT []
synonym: "Pseudostem girth, Plant circumference, Pseudostem circumference, Plant girth" EXACT []
is_a: CO_325:1000005

[Term]
id: CO_325:0000021
name: leaf emission rate
namespace: BananaTrait
def: "A rate that expresses the number of leaves that have emerged from the pseudostem in a given period of time." []
synonym: "LER" EXACT []
is_a: CO_325:1000000

[Term]
id: CO_325:0000024
name: number of suckers
namespace: BananaTrait
def: "The number of all types of suckers in the mat." []
synonym: "numsuckers" EXACT []
is_a: CO_325:1000005

[Term]
id: CO_325:0000027
name: tallest sucker height
namespace: BananaTrait
def: "The height of the pseudostem of the tallest sucker within the same mat as the plant (the sucker that will become the next plant with a bunch, once the bunch from the current plant is harvested)" []
synonym: "Height of tallest sucker, Following sucker height, Height of following sucker" EXACT []
synonym: "suckerheight" EXACT []
is_a: CO_325:1000005

[Term]
id: CO_325:0000033
name: bunch weight
namespace: BananaTrait
def: "The weight of the bunch, including the rachis." []
synonym: "bunchweight" EXACT []
is_a: CO_325:1000005

[Term]
id: CO_325:0000036
name: number of hands in bunch
namespace: BananaTrait
def: "The number of hands in the bunch." []
synonym: "numhands" EXACT []
is_a: CO_325:1000005

[Term]
id: CO_325:0000039
name: number of fingers in bunch
namespace: BananaTrait
def: "The number of fingers in the bunch." []
synonym: "numfingers" EXACT []
is_a: CO_325:1000005

[Term]
id: CO_325:0000042
name: number of fingers in hand
namespace: BananaTrait
def: "The number of fingers in a hand." []
synonym: "numfingershand" EXACT []
is_a: CO_325:1000005

[Term]
id: CO_325:0000045
name: hand weight
namespace: BananaTrait
def: "The weight of a hand." []
synonym: "handweight" EXACT []
is_a: CO_325:1000005

[Term]
id: CO_325:0000048
name: finger weight
namespace: BananaTrait
def: "The weight of a finger." []
synonym: "fingerweight" EXACT []
is_a: CO_325:1000005

[Term]
id: CO_325:0000051
name: finger external length
namespace: BananaTrait
def: "The length of a finger measured along the external (dorsal) arc, excluding the petiole and the flower tip." []
synonym: "Finger dorsal length" EXACT []
synonym: "fingerextlength" EXACT []
is_a: CO_325:1000005

[Term]
id: CO_325:0000054
name: finger circumference
namespace: BananaTrait
def: "The circumference of a finger." []
synonym: "fingercircumf" EXACT []
is_a: CO_325:1000005

[Term]
id: CO_325:0000057
name: black sigatoka incubation time
namespace: BananaTrait
def: "The time elapsed between a tagged cigar leaf at Brun's stage B of unrolling and the development of black Sigatoka disease symptoms at Foure's black leaf streak disease severity grade 1." []
synonym: "Black leaf streak incubation time" EXACT []
synonym: "DIT" EXACT []
is_a: CO_325:1000001

[Term]
id: CO_325:0000060
name: black sigatoka disease evolution time
namespace: BananaTrait
def: "The time elapsed between the development of black leaf streak disease symptoms at Foure's black Sigatoka disease severity grade 1, to 6." []
synonym: "Black leaf streak evolution time" EXACT []
synonym: "DET" EXACT []
is_a: CO_325:1000001

[Term]
id: CO_325:0000066
name: number of functional leaves
namespace: BananaTrait
def: "The number of leaves on the plant that have 50% or more of the leaf surface area as green, healthy, photosynthetic tissue." []
synonym: "functleaves" EXACT []
is_a: CO_325:1000005

[Term]
id: CO_325:0000069
name: number of standing leaves
namespace: BananaTrait
def: "The number of leaves attached to the plant that have an erect petiole (not bent or broken)." []
is_a: CO_325:1000001

[Term]
id: CO_325:0000072
name: extent of internal discolouration in corm of tallest sucker caused by fusarium wilt
namespace: BananaTrait
def: "The extent of discolouration in the corm of the tallest sucker caused by Fusarium wilt." []
is_a: CO_325:1000001

[Term]
id: CO_325:0000075
name: distance of internal discolouration in pseudostem of plant caused by fusarium wilt
namespace: BananaTrait
def: "The distance of discolouration in the pseudostem of the plant caused by Fusarium wilt." []
is_a: CO_325:1000001

[Term]
id: CO_325:0000078
name: percentage of plants with external disease symptoms caused by fusarium wilt
namespace: BananaTrait
def: "The percentage of plants with any or multiple of the external disease symptoms caused by Fusarium wilt - yellowing leaves, splitting of pseudostem base, changes in new leaves, petiole collapse." []
is_a: CO_325:1000001

[Term]
id: CO_325:0000081
name: percentage of plants with internal disease symptoms caused by fusarium wilt
namespace: BananaTrait
def: "The percentage of plants with any or multiple of the internal disease symptoms caused by Fusarium wilt - discolouration in the corm, and/or discolouration in the pseudostem." []
is_a: CO_325:1000001

[Term]
id: CO_325:0000084
name: time from start of crop cycle to first external disease symptoms caused by fusarium wilt
namespace: BananaTrait
def: "The time elapsed from the start of the crop cycle to the appearance on the plant of any of the external disease symptoms caused by Fusarium wilt - yellowing leaves, splitting pseudostem base, changes in new leaves, petiole collapse." []
is_a: CO_325:1000001

[Term]
id: CO_325:0000087
name: presence of yellowing leaves caused by fusarium wilt
namespace: BananaTrait
def: "The presence/absence of yellowing leaves caused by Fusarium wilt." []
synonym: "YL" EXACT []
is_a: CO_325:1000001

[Term]
id: CO_325:0000090
name: presence of splitting pseudostem base caused by fusarium wilt
namespace: BananaTrait
def: "The presence/absence of a splitting pseudostem base caused by Fusarium wilt." []
synonym: "SP" EXACT []
is_a: CO_325:1000001

[Term]
id: CO_325:0000093
name: presence of changes in new leaves caused by fusarium wilt
namespace: BananaTrait
def: "The presence/absence of changes in new leaves - irregular pale margins, narrowing of lamina, burning plus ripping of lamina, lamina becoming more erect - caused by Fusarium wilt." []
synonym: "CNL" EXACT []
is_a: CO_325:1000001

[Term]
id: CO_325:0000096
name: presence of petiole collapse caused by fusarium wilt
namespace: BananaTrait
def: "The presence/absence of petiole collapse caused by Fusarium wilt." []
synonym: "PC" EXACT []
is_a: CO_325:1000001

[Term]
id: CO_325:0000099
name: youngest leaf spotted
namespace: BananaTrait
def: "The rank of the first fully unfurled leaf with at least 10 discrete, mature, necrotic lesions or one large necrotic area with 10 leaf spot light-coloued dry centres, caused by black Sigatoka disease." []
synonym: "YLS" EXACT []
is_a: CO_325:1000001

[Term]
id: CO_325:0000102
name: index of non-spotted leaves
namespace: BananaTrait
def: "An index to express the proportion of standing leaves without the typical late-stage symptoms of black Sigatoka disease, i.e. a black spot with a necrotic centre. This index provides an estimation of available photosynthetic leaf area prior to fruit filling and is a measure of resistance. It also corrects for the difference in the number of leaves produced by different types of bananas." []
synonym: "INSL" EXACT []
is_a: CO_325:1000001

[Term]
id: CO_325:0000105
name: black sigatoka disease infection index
namespace: BananaTrait
def: "An index to express the degree of leaf area of all standing leaves on the plant affected by black Sigatoka disease." []
synonym: "Black leaf streak infection index" EXACT []
is_a: CO_325:1000001

[Term]
id: CO_325:0000108
name: number of dead roots
namespace: BananaTrait
def: "Number of dead roots" []
is_a: CO_325:1000001

[Term]
id: CO_325:0000111
name: number of functional roots
namespace: BananaTrait
def: "Number of functional roots" []
is_a: CO_325:1000001

[Term]
id: CO_325:0000123
name: root necrosis
namespace: BananaTrait
def: "Percenatge of root necrosis" []
is_a: CO_325:1000001

[Term]
id: CO_325:0000156
name: PlntShtTime_Comp_d
namespace: BananaTrait
def: "Calculate as: the time elapsed between the Date of planting and the Date of shooting  in days format (e.g. 24/09/2014 - 24/01/2014 = 243 days.)" []
synonym: "Time from planting to shooting" EXACT []
is_a: CO_325:1000020
relationship: variable_of CO_325:0000000 ! time from planting to shooting
relationship: variable_of CO_325:0010011 ! time from planting to shooting - computation
relationship: variable_of CO_325:0100003 ! day

[Term]
id: CO_325:0000157
name: ShtHvstTime_Comp_d
namespace: BananaTrait
def: "Calculate as: the time elapsed between the Date of shooting to the Date of harvest, in days format (e.g. 24/12/2014 - 24/09/2014 = 91 days.)" []
synonym: "Time from shooting to harvest" EXACT []
is_a: CO_325:1000020
relationship: variable_of CO_325:0000003 ! time from shooting to harvest
relationship: variable_of CO_325:0010013 ! time from shooting to harvest - computation
relationship: variable_of CO_325:0100003 ! day

[Term]
id: CO_325:0000158
name: CropCyc_Comp_d
namespace: BananaTrait
def: "Calculate as: the time elapsed between the Date of planting to the Date of harvest in days format (e.g. 24/12/2014 - 24/01/2014 = 334 days.)" []
synonym: "Plant crop cycle" EXACT []
is_a: CO_325:1000020
relationship: variable_of CO_325:0000006 ! plant crop cycle
relationship: variable_of CO_325:0010012 ! plant crop cycle - computation
relationship: variable_of CO_325:0100003 ! day

[Term]
id: CO_325:0000159
name: PStmHt_M1_cm
namespace: BananaTrait
def: "Measure the distance from the pseudostem base at the ground to the intersection of the petioles of the two youngest leaves (leaf ranks 1 and 2), using a measuring pole or sliding ruler, in centimeters." []
synonym: "Plant height @ Shooting, from ground to two youngest leaves" EXACT []
is_a: CO_325:1000020
relationship: variable_of CO_325:0000009 ! plant height
relationship: variable_of CO_325:0010020 ! plant height - petiole of two youngest leaves - measurement
relationship: variable_of CO_325:0100004 ! cm

[Term]
id: CO_325:0000160
name: PStmGrth_M_cm
namespace: BananaTrait
def: "Measure the [girth / circumference] of the pseudostem of the plant at 1 m from the ground, using a tape measure,  in centimeters" []
synonym: "Plant circumference @ Shooting" EXACT []
is_a: CO_325:1000020
relationship: variable_of CO_325:0000012 ! plant circumference
relationship: variable_of CO_325:0010023 ! plant circumference - measurement
relationship: variable_of CO_325:0100004 ! cm

[Term]
id: CO_325:0000165
name: LfEmRate_Comp_LfWk
namespace: BananaTrait
def: "Calculate as: the Rank of previously marked leaf at one point in time, minus 1 (equivalent to the Rank of marked youngest leaf), divided by the time elapsed between the two Date of data collection events when the marked leaf was recorded as 1) the Rank of youngest leaf and 2) the Rank of previously marked leaf, e.g. (4 - 1) / 4 weeks = LER of 0.75 leaves/week during a particular time period." []
synonym: "Weekly Leaf emission rate @ At regular intervals, usually from 7 months after planting until harvest, and including at the Date of shooting and at the Date of harvest" EXACT []
is_a: CO_325:1000020
relationship: variable_of CO_325:0000021 ! leaf emission rate
relationship: variable_of CO_325:0010175 ! leaf emission rate - computation
relationship: variable_of CO_325:0100091 ! leaves/week

[Term]
id: CO_325:0000166
name: SuckNum_Ct_Suck
namespace: BananaTrait
def: "Count how many of all types of suckers are in the mat. in sucker." []
synonym: "Number of suckers @ Shooting" EXACT []
is_a: CO_325:1000020
relationship: variable_of CO_325:0000024 ! number of suckers
relationship: variable_of CO_325:0010030 ! number of suckers - counting
relationship: variable_of CO_325:0100009 ! sucker

[Term]
id: CO_325:0000167
name: SuckHtShtStg_M_cm
namespace: BananaTrait
def: "On the tallest sucker, measure the distance from the pseudostem base at the ground to the intersection of the petioles of the two youngest leaves (leaf ranks 1 and 2), using a measuring pole or sliding ruler, in centimeters" []
synonym: "Tallest sucker height @ Shooting" EXACT []
is_a: CO_325:1000020
relationship: variable_of CO_325:0000027 ! tallest sucker height
relationship: variable_of CO_325:0010024 ! tallest sucker height - measurement
relationship: variable_of CO_325:0100004 ! cm

[Term]
id: CO_325:0000169
name: BnchWt_M_kg
namespace: BananaTrait
def: "Harvest the bunch stalk by cutting the peduncle above the most proximal hand (=first hand) and immediately after the last hand  weigh the bunch, including the rachis, using scales, in kilograms." []
synonym: "Bunch weight @ Harvest" EXACT []
is_a: CO_325:1000020
relationship: variable_of CO_325:0000033 ! bunch weight
relationship: variable_of CO_325:0010032 ! bunch weight - measurement
relationship: variable_of CO_325:0100011 ! kg

[Term]
id: CO_325:0000170
name: BnchHndNum_Ct_Hnd
namespace: BananaTrait
def: "Count how many hands are in the bunch." []
synonym: "Number of hands in bunch" EXACT []
is_a: CO_325:1000020
relationship: variable_of CO_325:0000036 ! number of hands in bunch
relationship: variable_of CO_325:0010035 ! number of hands in bunch - counting
relationship: variable_of CO_325:0100012 ! hand

[Term]
id: CO_325:0000171
name: BnchFrtNum_Ct_Frt
namespace: BananaTrait
def: "Count how many fingers are in the bunch." []
synonym: "Number of fingers in bunch, count" EXACT []
is_a: CO_325:1000020
relationship: variable_of CO_325:0000039 ! number of fingers in bunch
relationship: variable_of CO_325:0010036 ! number of fingers in bunch - counting
relationship: variable_of CO_325:0100013 ! finger

[Term]
id: CO_325:0000172
name: HndFrtNum_Ct_Frt
namespace: BananaTrait
def: "Count how many fingers are in a hand." []
synonym: "Number of fingers in hand" EXACT []
is_a: CO_325:1000019
relationship: variable_of CO_325:0000042 ! number of fingers in hand
relationship: variable_of CO_325:0010038 ! number of fingers in hand - counting
relationship: variable_of CO_325:0100013 ! finger

[Term]
id: CO_325:0000173
name: HandWt_M_kgPlnt
namespace: BananaTrait
def: "Cut a hand from the rachis and weigh the hand, in kilograms." []
synonym: "Hand weight @ Harvest" EXACT []
is_a: CO_325:1000019
relationship: variable_of CO_325:0000045 ! hand weight
relationship: variable_of CO_325:0010043 ! hand weight - measurement
relationship: variable_of CO_325:0100011 ! kg

[Term]
id: CO_325:0000174
name: FrtWt_M_gFruit
namespace: BananaTrait
def: "Weigh a finger, in grams." []
synonym: "Finger weight @ Harvest" EXACT []
is_a: CO_325:1000020
relationship: variable_of CO_325:0000048 ! finger weight
relationship: variable_of CO_325:0010046 ! finger weight - measurement
relationship: variable_of CO_325:0100015 ! g

[Term]
id: CO_325:0000175
name: FrtExtLng_M_cm
namespace: BananaTrait
def: "Measure the length of a finger, along the dorsal edge from XXX to XXX, using a tape measure.Record on second hand middle finger of the outern whorl circumference, in centimeters." []
synonym: "Finger external length @ Harvest" EXACT []
is_a: CO_325:1000020
relationship: variable_of CO_325:0000051 ! finger external length
relationship: variable_of CO_325:0010050 ! finger dorsal length - measurement
relationship: variable_of CO_325:0100004 ! cm

[Term]
id: CO_325:0000176
name: FrtGrth_M_cm
namespace: BananaTrait
def: "Measure the circumference (= girth) of a finger at its widest point, using a tape measure, in centimeters." []
synonym: "Finger circumference @ Harvest, in centimeters" EXACT []
is_a: CO_325:1000020
relationship: variable_of CO_325:0000054 ! finger circumference
relationship: variable_of CO_325:0010054 ! finger circumference - measurement
relationship: variable_of CO_325:0100004 ! cm

[Term]
id: CO_325:0000177
name: DIT_Comp_d
namespace: BananaTrait
def: "Calculate as: the time elapsed between the Date of tagged leaf presenting BLS disease symptoms at Foure's stage 1 and the Date of tagged cigar leaf unrolling at stage B, in days (e.g. 24/04/2014 - 24/03/2014 = 31 days.)" []
synonym: "Black Sigatoka incubation time" EXACT []
is_a: CO_325:1000019
relationship: variable_of CO_325:0000057 ! black sigatoka incubation time
relationship: variable_of CO_325:0010166 ! black sigatoka disease incubation time - computation
relationship: variable_of CO_325:0100003 ! day

[Term]
id: CO_325:0000178
name: DET_Comp_d
namespace: BananaTrait
def: "Calculate as: the time elapsed between the Date of tagged leaf presenting BLS disease symptoms at Foure's stage 6 and the Date of tagged leaf presenting BLS disease symptoms at Foure's stage 1, in days (e.g. 24/06/2014 - 24/04/2014 = 61 days)." []
synonym: "Black Sigatoka disease evolution time" EXACT []
is_a: CO_325:1000019
relationship: variable_of CO_325:0000060 ! black sigatoka disease evolution time
relationship: variable_of CO_325:0010167 ! black sigatoka disease evolution time - computation
relationship: variable_of CO_325:0100003 ! day

[Term]
id: CO_325:0000181
name: StdLf_Ct_leaf
namespace: BananaTrait
def: "Count how many standing leaves (with an erect petiole) are on the plant, considering all leaves in between and inclusive of, the NEWEST LEAF and the oldest STANDING LEAF. Do not count those leaves with the petiole bent back, other leaves should be recorded regardless of their colour or the colour of their petiole." []
synonym: "Number of standing leaves @ Monthly, from 6 months after planting until harvest, and including at the Date of shooting and at the Date of harvest" EXACT []
is_a: CO_325:1000019
relationship: variable_of CO_325:0000069 ! number of standing leaves
relationship: variable_of CO_325:0010179 ! number of standing leaves - counting
relationship: variable_of CO_325:0100092 ! leaf

[Term]
id: CO_325:0000182
name: CormDiscol_Est_1to6
namespace: BananaTrait
def: "Completely cut the pseudostem off at the base and ***                                             For the motherplant, at harvest the plant should be cut at the base of the pseudostem. The extent to which vascular discolouration extends up the pseudostem should be determined by making transverse cuts, from the base of the pseudostem upwards, and examining the internal tissues following each cut. The point at which discolouration is no longer visible should be noted and the distance from this point to the pseudostem base recorded. in 5 pt corm discolouration. In scale 1to5: 1=Corm completely clean, no discolouration in vascular tissue; 2=Isolated points of discolouration of vascular tissue; 3=Discolouration of up to one-third of vascular tissue; 4=Discolouration of between one-third and two-thirds of vascular tissue; 5=Discolouration of more than two-thirds of vascular tissue" []
synonym: "Extent of internal discolouration in corm of tallest sucker caused by Fusarium wilt @ Harvest" EXACT []
is_a: CO_325:1000019
relationship: variable_of CO_325:0000072 ! extent of internal discolouration in corm of tallest sucker caused by fusarium wilt
relationship: variable_of CO_325:0010170 ! extent of internal discolouration in corm of tallest sucker caused by fusarium wilt - estimation
relationship: variable_of CO_325:0100088 ! 5 pt corm discolouration scale

[Term]
id: CO_325:0000183
name: PStmDiscol_Est_cm
namespace: BananaTrait
def: "****For the first sucker, the complete corm should be removed from the soil, the roots cut off and excess soil removed. Transverse sections of the corm should be cut (using a guillotine or other suitable device) to obtain five slices of equal thickness. The upper surface of each cut section should be examined and visually evaluate the extent of the vascular discolouration. In centimeters" []
synonym: "Distance of internal discolouration in pseudostem of plant caused by Fusarium wilt @ Harvest" EXACT []
is_a: CO_325:1000020
relationship: variable_of CO_325:0000075 ! distance of internal discolouration in pseudostem of plant caused by fusarium wilt
relationship: variable_of CO_325:0010169 ! distance of internal discolouration in pseudostem of plant caused by fusarium wilt
relationship: variable_of CO_325:0100004 ! cm

[Term]
id: CO_325:0000184
name: ExtDisProp_Comp_pct
namespace: BananaTrait
def: "Calculate as: the sum of the number of plants with any or multiple of the external disease symptoms caused by Fusarium wilt - yellowing leaves, splitting of pseudostem base, changes in new leaves, petiole collapse - divided by the Number of plants planted * 100, e.g. 112 / 300 * 100 = 37%." []
synonym: "Percentage of plants with external disease symptoms caused by Fusarium wilt @ Monthly, from 3 months after planting until harvest, and including at the Date of shooting and at the Date of harvest" EXACT []
is_a: CO_325:1000019
relationship: variable_of CO_325:0000078 ! percentage of plants with external disease symptoms caused by fusarium wilt
relationship: variable_of CO_325:0010198 ! percentage of plants with external disease symptoms caused by fusarium wilt - computation
relationship: variable_of CO_325:0100081 ! %

[Term]
id: CO_325:0000185
name: IntDisProp_Comp_pct
namespace: BananaTrait
def: "Calculate as: the sum of the number of plants with any or multiple of the internal disease symptoms caused by Fusarium wilt - discolouration in the corm, and/or discolouration in the pseudostem - divided by the Number of plants planted * 100, e.g. 108 / 300 * 100 = 36%." []
synonym: "Percentage of plants with internal disease symptoms caused by Fusarium wilt @ Monthly, from 3 months after planting until harvest, and including at the Date of shooting and at the Date of harvest" EXACT []
is_a: CO_325:1000019
relationship: variable_of CO_325:0000081 ! percentage of plants with internal disease symptoms caused by fusarium wilt
relationship: variable_of CO_325:0010199 ! percentage of plants with internal disease symptoms caused by fusarium wilt - computation
relationship: variable_of CO_325:0100081 ! %

[Term]
id: CO_325:0000186
name: PlntgDisTim_Comp_d
namespace: BananaTrait
def: "Calculate as: the time elapsed between the Date of planting or the Date of harvest of the bunch from the plant of the previous crop cycle and the Date of first external disease symptoms caused by Fusarium wilt." []
synonym: "Time from start of crop cycle to first external disease symptoms caused by Fusarium wilt" EXACT []
is_a: CO_325:1000020
relationship: variable_of CO_325:0000084 ! time from start of crop cycle to first external disease symptoms caused by fusarium wilt
relationship: variable_of CO_325:0010193 ! time from start of crop cycle to first external disease symptoms caused by fusarium wilt - computation
relationship: variable_of CO_325:0100003 ! day

[Term]
id: CO_325:0000187
name: YellowPres_Est_1or2
namespace: BananaTrait
def: "Visual assessment. in Presence/absence scale: 1=Absent; 2=Present" []
synonym: "Presence of yellowing leaves caused by Fusarium wilt @ Monthly, from 3 months after planting until harvest, and including at the Date of shooting and at the Date of harvest, scale 1-2" EXACT []
is_a: CO_325:1000019
relationship: variable_of CO_325:0000087 ! presence of yellowing leaves caused by fusarium wilt
relationship: variable_of CO_325:0010190 ! presence of yellowing leaves caused by fusarium wilt - estimation
relationship: variable_of CO_325:0100089 ! presence/absence scale

[Term]
id: CO_325:0000188
name: PStmSplitPres_Est_1or2
namespace: BananaTrait
def: "Visual assessment. in Presence/absence scale: 1=Absent; 2=Present" []
synonym: "Presence of splitting pseudostem base caused by Fusarium wilt @ Monthly, from 3 months after planting until harvest, and including at the Date of shooting and at the Date of harvest, scale 1-2" EXACT []
is_a: CO_325:1000019
relationship: variable_of CO_325:0000090 ! presence of splitting pseudostem base caused by fusarium wilt
relationship: variable_of CO_325:0010191 ! presence of splitting pseudostem base caused by fusarium wilt - estimation
relationship: variable_of CO_325:0100089 ! presence/absence scale

[Term]
id: CO_325:0000189
name: LfChgPres_Est_1or2
namespace: BananaTrait
def: "Visual assessment. in Presence/absence scale: 1=Absent; 2=Present" []
synonym: "Presence of changes in new leaves caused by Fusarium wilt @ Monthly, from 3 months after planting until harvest, and including at the Date of shooting and at the Date of harvest, scale 1-2" EXACT []
is_a: CO_325:1000019
relationship: variable_of CO_325:0000093 ! presence of changes in new leaves caused by fusarium wilt
relationship: variable_of CO_325:0010192 ! presence of changes in new leaves caused by fusarium wilt - estimation
relationship: variable_of CO_325:0100089 ! presence/absence scale

[Term]
id: CO_325:0000190
name: PetColpPres_Est_1or2
namespace: BananaTrait
def: "Visual assessment. in Presence/absence scale: 1=Absent; 2=Present" []
synonym: "Presence of petiole collapse caused by Fusarium wilt @ Monthly, from 3 months after planting until harvest, and including at the Date of shooting and at the Date of harvest, scale 1-2" EXACT []
is_a: CO_325:1000019
relationship: variable_of CO_325:0000096 ! presence of petiole collapse caused by fusarium wilt
relationship: variable_of CO_325:0010171 ! presence of petiole collapse caused by fusarium wilt - estimation
relationship: variable_of CO_325:0100089 ! presence/absence scale

[Term]
id: CO_325:0000191
name: SpotLfNum_Ct_Lf
namespace: BananaTrait
def: "Record the rank of the youngest leaf spotted (the first fully unfurled leaf with at least 10 discrete, mature, necrotic lesions or one large necrotic area with 10 light-coloured dry centres), counting the rank by starting with the newest fully unrolled leaf as 1 and moving downwards, associating the data with the time of collection. in leaf rank." []
synonym: "Youngest leaf spotted @ Monthly once recognised, and including at the Date of shooting and at the Date of harvest" EXACT []
is_a: CO_325:1000020
relationship: variable_of CO_325:0000099 ! youngest leaf spotted
relationship: variable_of CO_325:0010159 ! youngest leaf spotted - counting
relationship: variable_of CO_325:0100086 ! leaf rank

[Term]
id: CO_325:0000192
name: NSpotLfProp_Comp_idx
namespace: BananaTrait
def: "Calculate as: 100 multiplied by (Youngest leaf spotted, minus 1), divided by Number of standing leaves (e.g. 100 * (6 - 1) / 12 = 42)." []
synonym: "Index of non-spotted leaves @ Most commonly calculated at harvest, can also be measured at shooting." EXACT []
is_a: CO_325:1000019
relationship: variable_of CO_325:0000102 ! index of non-spotted leaves
relationship: variable_of CO_325:0010180 ! index of non-spotted leaves - computation
relationship: variable_of CO_325:0100087 ! Index

[Term]
id: CO_325:0000193
name: BlkLfStrkInfIndex_Comp_Idx
namespace: BananaTrait
def: "Calculate as an Index: ((((Number of leaves with BLS disease severity grade 0, multiplied by 0), plus (Number of leaves with BLS disease severity grade 1, multiplied by 1), plus (Number of leaves with BLS disease severity grade 2, multiplied by 2), plus (Number of leaves with BLS disease severity grade 3, multiplied by 3), plus (Number of leaves with BLS disease severity grade 4, multiplied by 4), plus (Number of leaves with BLS disease severity grade 5, multiplied by 5), plus (Number of leaves with BLS disease severity grade 6, multiplied by 6)), divided by the number of grades in the scale minus 1 (i.e. 7-1)), divided by the Number of standing leaves), multipled by 100. For example, ((((3 * 0) + (1 * 1) + (1 * 2) + (3 * 3) + (5 * 4) + (0 * 5) + (0 * 6)) / 6) / 13) * 100 = ((32 / 6) / 13) * 100 = 41." []
synonym: "Black Sigatoka disease infection index @ Monthly, from 6 months after planting until harvest, and including at the Date of shooting and at the Date of harvest" EXACT []
is_a: CO_325:1000019
relationship: variable_of CO_325:0000105 ! black sigatoka disease infection index
relationship: variable_of CO_325:0010162 ! black sigatoka disease infection index - computation
relationship: variable_of CO_325:0100087 ! Index

[Term]
id: CO_325:0000194
name: DeadRtNum2_Ct_Rt
namespace: BananaTrait
def: "visual counting method  from a 30 cm square hole one meter from plant" []
synonym: "Number of dead roots @ recently flowered plant (less than 14 days) or plant with emerging flowers" EXACT []
is_a: CO_325:1000020
relationship: variable_of CO_325:0000108 ! number of dead roots
relationship: variable_of CO_325:0010142 ! number of dead roots - method
relationship: variable_of CO_325:0100083 ! Number

[Term]
id: CO_325:0000195
name: FuncRtNum2_Ct_Rt
namespace: BananaTrait
def: "visual counting method from  a 30 cm square hole one meter from plant" []
synonym: "Number of functional roots @ recently flowered plant (less than 14 days) or plant with emerging flowers" EXACT []
is_a: CO_325:1000020
relationship: variable_of CO_325:0000111 ! number of functional roots
relationship: variable_of CO_325:0010141 ! number of functional roots - method
relationship: variable_of CO_325:0100083 ! Number

[Term]
id: CO_325:0000199
name: RtCtxNecrProp2_Comp_pct
namespace: BananaTrait
def: "Visual observation on 5 roots of 10 cm length each from around the the plants, in percentage. Split lengthwise and % necross assessed. (each root 20% total)" []
synonym: "Root necrosis  @ recently flowered plant (less than 14 days) or plant with emerging flowers" EXACT []
is_a: CO_325:1000020
relationship: variable_of CO_325:0000123 ! root necrosis
relationship: variable_of CO_325:0010140 ! percentage of root necrosis - method
relationship: variable_of CO_325:0100081 ! %

[Term]
id: CO_325:0000202
name: RadoNumSlWt_Comp_Nema
namespace: BananaTrait
def: "Count from 100 ml of soil sample in No. per 10g" []
synonym: "Number of Radopholus similis per soil sample @ recently flowered plant (less than 14 days) or plant with emerging flowers" EXACT []
is_a: CO_325:1000019
relationship: variable_of CO_325:0000522 ! number of radopholus similis per soil sample
relationship: variable_of CO_325:0010144 ! number of nematodes (radopholus similis ) per  unit fresh root weight - method
relationship: variable_of CO_325:0100085 ! No. per 10g

[Term]
id: CO_325:0000203
name: HelicoNumSlWt_Comp_Nema
namespace: BananaTrait
def: "Count from 100 ml of soil sample in No. per 10g" []
synonym: "Number of Helicotylenchus multicinctus per soil sample @ recently flowered plant (less than 14 days) or plant with emerging flowers" EXACT []
is_a: CO_325:1000019
relationship: variable_of CO_325:0000523 ! number of helicotylenchus multicinctus per soil sample
relationship: variable_of CO_325:0010145 ! number of nematodes (helicotylenchus multicinctus) per  unit fresh root weight - method
relationship: variable_of CO_325:0100085 ! No. per 10g

[Term]
id: CO_325:0000204
name: MeloiNumSlWt_Comp_Nema
namespace: BananaTrait
def: "Count from 100 ml of soil sample in No. per 10g" []
synonym: "Number of Meloidogyne spp. per  soil sample @ recently flowered plant (less than 14 days) or plant with emerging flowers" EXACT []
is_a: CO_325:1000019
relationship: variable_of CO_325:0000526 ! number of meloidogyne spp. per  soil sample
relationship: variable_of CO_325:0010147 ! number of nematodes (meloidogyne spp.) per  unit fresh root weight - method
relationship: variable_of CO_325:0100085 ! No. per 10g

[Term]
id: CO_325:0000205
name: PratyNumSlWt_Comp_Nema
namespace: BananaTrait
def: "Count from 100 ml of soil sample in No. per 10g" []
synonym: "Number of Pratylenchus spp. per soil sample @ recently flowered plant (less than 14 days) or plant with emerging flowers" EXACT []
is_a: CO_325:1000019
relationship: variable_of CO_325:0000527 ! number of pratylenchus spp. per soil sample
relationship: variable_of CO_325:0010148 ! number of nematodes (pratylenchus spp.) per  unit fresh root weight - method
relationship: variable_of CO_325:0100085 ! No. per 10g

[Term]
id: CO_325:0000206
name: HoploNumSlWt_Comp_Nema
namespace: BananaTrait
def: "Count from 100 ml of soil sample in No. per 10g" []
synonym: "Number of Hoplolaimus spp. per soil sample @ recently flowered plant (less than 14 days) or plant with emerging flowers" EXACT []
is_a: CO_325:1000019
relationship: variable_of CO_325:0000528 ! number of hoplolaimus spp. per soil sample
relationship: variable_of CO_325:0010149 ! number of nematodes (hoplolaimus spp.) per  unit fresh root weight - method
relationship: variable_of CO_325:0100085 ! No. per 10g

[Term]
id: CO_325:0000207
name: PratyGooNumSlWt_Comp_Nema
namespace: BananaTrait
def: "Count from 100 ml of soil sample in No. per 10g" []
synonym: "Number of Pratylenchus goodeyi per soil sample @ recently flowered plant (less than 14 days) or plant with emerging flowers" EXACT []
is_a: CO_325:1000019
relationship: variable_of CO_325:0000529 ! number of pratylenchus goodeyi per soil sample
relationship: variable_of CO_325:0010150 ! number of nematodes (pratylenchus goodeyi) per  unit fresh root weight - method
relationship: variable_of CO_325:0100085 ! No. per 10g

[Term]
id: CO_325:0000208
name: PratyCofNumSlWt_Comp_Nema
namespace: BananaTrait
def: "Count from 100 ml of soil sample in No. per 10g" []
synonym: "Number of Pratylenchus coffeae per soil sample @ recently flowered plant (less than 14 days) or plant with emerging flowers" EXACT []
is_a: CO_325:1000019
relationship: variable_of CO_325:0000530 ! number of pratylenchus coffeae per soil sample
relationship: variable_of CO_325:0010151 ! number of nematodes (pratylenchus coffeae) per  unit fresh root weight - method
relationship: variable_of CO_325:0100085 ! No. per 10g

[Term]
id: CO_325:0000210
name: Shoot_Date_ymd
namespace: BananaTrait
def: "Record the date of event. in yyyy/mm/dd format" []
synonym: "Date of shooting, yyyy/mm/dd" EXACT []
is_a: CO_325:1000020
relationship: variable_of CO_325:0000211 ! date of shooting
relationship: variable_of CO_325:0010007 ! date of shooting - estimation
relationship: variable_of CO_325:0100001 ! yyyy/mm/dd

[Term]
id: CO_325:0000211
name: date of shooting
namespace: BananaTrait
def: "The date the inflorescence emerges from the pseudostem." []
synonym: "Date of bunch emergence, Date of bunching, Shooting time, Shooting date, Date of flowering (incorrect usage)" EXACT []
synonym: "dateshoot" EXACT []
is_a: CO_325:1000002

[Term]
id: CO_325:0000217
name: FlwT_Date_ymd
namespace: BananaTrait
def: "Record the date of event. in yyyy/mm/dd format" []
synonym: "Date of flowering, yyyy/mm/dd" EXACT []
is_a: CO_325:1000020
relationship: variable_of CO_325:0000218 ! date of flowering
relationship: variable_of CO_325:0010008 ! date of flowering - estimation
relationship: variable_of CO_325:0100001 ! yyyy/mm/dd

[Term]
id: CO_325:0000218
name: date of flowering
namespace: BananaTrait
def: "The date the last bracts fall from the most distal hand (closest to the male bud) to display the female flowers." []
synonym: "Date of bract fall, Flowering date" EXACT []
synonym: "dateflower" EXACT []
is_a: CO_325:1000002

[Term]
id: CO_325:0000220
name: MSuckN_Ct_MSuck
namespace: BananaTrait
def: "Count how many maiden suckers are in the mat. in maiden sucker." []
synonym: "Number of maiden suckers @ Shooting" EXACT []
is_a: CO_325:1000020
relationship: variable_of CO_325:0000221 ! number of maiden suckers
relationship: variable_of CO_325:0010026 ! number of maiden suckers - counting
relationship: variable_of CO_325:0100005 ! maiden sucker

[Term]
id: CO_325:0000221
name: number of maiden suckers
namespace: BananaTrait
def: "The number of maiden suckers (fully grown suckers with foliage leaves) in the mat." []
synonym: "nummaidensuckers" EXACT []
is_a: CO_325:1000005

[Term]
id: CO_325:0000224
name: SSuckN_Ct_SSuck
namespace: BananaTrait
def: "Count how many sword suckers are in the mat. in sword sucker." []
synonym: "Number of sword suckers @ Shooting" EXACT []
is_a: CO_325:1000020
relationship: variable_of CO_325:0000225 ! number of sword suckers
relationship: variable_of CO_325:0010027 ! number of sword suckers - counting
relationship: variable_of CO_325:0100006 ! sword sucker

[Term]
id: CO_325:0000225
name: number of sword suckers
namespace: BananaTrait
def: "The number of sword suckers (suckers with narrow leaves and a large rhizome) in the mat." []
synonym: "numswordsuckers" EXACT []
is_a: CO_325:1000005

[Term]
id: CO_325:0000228
name: PSuckN_Ct_PSuck
namespace: BananaTrait
def: "Count how many peeper suckers are in the mat. in peeper sucker." []
synonym: "Number of peeper suckers @ Shooting" EXACT []
is_a: CO_325:1000020
relationship: variable_of CO_325:0000229 ! number of peeper suckers
relationship: variable_of CO_325:0010028 ! number of peeper suckers - counting
relationship: variable_of CO_325:0100007 ! peeper sucker

[Term]
id: CO_325:0000229
name: number of peeper suckers
namespace: BananaTrait
def: "The number of peeper suckers (suckers less than 15 cm tall) in the mat." []
synonym: "numpeepersuckers" EXACT []
is_a: CO_325:1000005

[Term]
id: CO_325:0000232
name: FrtDiam_M_cm
namespace: BananaTrait
def: "Measure the lateral diameter of a finger, from the left to the right side (not from the ventral to the dorsal side), at the widest point, using calipers, in centimeters." []
synonym: "Finger lateral diameter @ Harvest, in centimeters" EXACT []
is_a: CO_325:1000020
relationship: variable_of CO_325:0000233 ! finger lateral diameter
relationship: variable_of CO_325:0010056 ! finger lateral diameter - measurement
relationship: variable_of CO_325:0100004 ! cm

[Term]
id: CO_325:0000233
name: finger lateral diameter
namespace: BananaTrait
def: "The lateral (side to side) diameter of a finger." []
synonym: "fingerlatdiam" EXACT []
synonym: "Fruit circumference, Finger grade, Fruit diameter, Fruit grade" EXACT []
is_a: CO_325:1000005

[Term]
id: CO_325:0000235
name: PeelThck_M_mm
namespace: BananaTrait
def: "Remove the peel from a fruit and measure the thickness of the peel, using calipers, in millimeters. (breeders: Fruit peel thickness (mm): Recorded at fruit maturity (?ready to eat? ripe, but not over-ripe; full yellow stage) on second hand middle finger of the outern whorl circumference)" []
synonym: "Finger peel thickness" EXACT []
is_a: CO_325:1000020
relationship: variable_of CO_325:0000236 ! finger peel thickness
relationship: variable_of CO_325:0010060 ! finger peel thickness - measurement
relationship: variable_of CO_325:0100016 ! mm

[Term]
id: CO_325:0000236
name: finger peel thickness
namespace: BananaTrait
def: "The thickness of the peel of a finger." []
synonym: "peelthickness" EXACT []
synonym: "Width of the peel, Width of the skin, Width of the exocarp, Finger peel thickness" EXACT []
is_a: CO_325:1000005

[Term]
id: CO_325:0000239
name: PulpDiam_M_cm
namespace: BananaTrait
def: "Remove the peel of a finger and measure the lateral diameter of the fruit pulp, from the left to the right side (not from the ventral to the dorsal side), at the widest point, using calipers, in centimeters" []
synonym: "Fruit pulp lateral diameter @ When fruit mature at ready-to-eat stage, in centimeters" EXACT []
is_a: CO_325:1000020
relationship: variable_of CO_325:0000240 ! fruit pulp lateral diameter
relationship: variable_of CO_325:0010058 ! fruit pulp lateral diameter - measurement
relationship: variable_of CO_325:0100004 ! cm

[Term]
id: CO_325:0000240
name: fruit pulp lateral diameter
namespace: BananaTrait
def: "The lateral (side to side) diameter of the pulp of a fruit." []
synonym: "Finger pulp diameter" EXACT []
synonym: "pulpdiam" EXACT []
is_a: CO_325:1000005

[Term]
id: CO_325:0000242
name: PStmCol_Est_1to16
namespace: BananaTrait
def: "Detach the outermost sheath from the pseudostem (the sheath should not be too dry). Record the overall impression of colour of the exposed surface of the underlying pseudostem. Note that this 'main colour' should cover more than 75% of the underlying pseudostem surface. Use colour chart A and observe out of direct sunlight. in BD colour chart A - 2016 In scale 1to16:  1=Cream; 2=Yellow; 3=Watery green; 4=Green yellow; 5=Light green; 6=Medium green; 7=Green; 8=Dark green; 9=Whitish; 10=Orange red; 11=Red; 12=Pink-purple; 13=Purple-brown; 14=Red-purple; 15=Purple; 16=Blue" []
synonym: "Main underlying colour of pseudostem @ Harvest, scale (1 to 16)" EXACT []
is_a: CO_325:1000020
relationship: variable_of CO_325:0000243 ! main underlying colour of pseudostem
relationship: variable_of CO_325:0010097 ! pseudostem colour - estimation
relationship: variable_of CO_325:0100043 ! bd colour chart a - 2016

[Term]
id: CO_325:0000243
name: main underlying colour of pseudostem
namespace: BananaTrait
def: "Main colour of the pseudostem under the outermost sheath." []
synonym: "Predominant underlying colour of the pseudostem" EXACT []
is_a: CO_325:1000007

[Term]
id: CO_325:0000247
name: PMargColL_Est_1or2
namespace: BananaTrait
def: "Observations on the margins and petiole wings should be made where the petiole and pseudostem meet at shooting. Record on the last developed leaf. In scale 1to2: 1=No contrast between margin and petiole (without a colour line along); 2=Contrast between margin and petiole (with a contrasting colour line along)" []
synonym: "Colour line along edge of petiole margin @ Shooting, scale 1 to 2" EXACT []
is_a: CO_325:1000020
relationship: variable_of CO_325:0000248 ! colour line along edge of petiole margin
relationship: variable_of CO_325:0010104 ! colour line along edge of petiole margin - estimation
relationship: variable_of CO_325:0100054 ! petiole-margin contrast

[Term]
id: CO_325:0000248
name: colour line along edge of petiole margin
namespace: BananaTrait
def: "Presence or absence of colour line along edge of petiole margin" []
synonym: "Edge of petiole margin" EXACT []
is_a: CO_325:1000007

[Term]
id: CO_325:0000251
name: CigLfPigm_Est_1to3
namespace: BananaTrait
def: "Visually observe the pigmentation of the outer surface of the cigar leaf of a developed sucker or on another plant of the same accession. [ Observation should be made before shooting, on a developed sucker or on another plant of the same accession.] in Banana Descriptors colour chart A - 2016 format: In scale 1to3: 1=Green; 2=Red-purple; 3=Other (specify on answer sheet)." []
synonym: "Pigmentation of outer surface of cigar leaf on sucker @ Before shooting, scale 1 to 3" EXACT []
is_a: CO_325:1000020
relationship: variable_of CO_325:0000252 ! pigmentation of outer surface of cigar leaf on sucker
relationship: variable_of CO_325:0010105 ! pigmentation of outer surface of cigar leaf - estimation
relationship: variable_of CO_325:0100043 ! bd colour chart a - 2016

[Term]
id: CO_325:0000252
name: pigmentation of outer surface of cigar leaf on sucker
namespace: BananaTrait
def: "Colour of pigmentation on outer surface of cigar leaf on a developed sucker" []
synonym: "Colour of cigar leaf dorsal surface" EXACT []
is_a: CO_325:1000007

[Term]
id: CO_325:0000255
name: PMargWing_Est_1or2
namespace: BananaTrait
def: "Observations on the margins and petiole wings should be made where the petiole and pseudostem meet at shooting. Margin is the part of the petiole that can be bent outwards/inwards. In wing presence/absence. In scale 1to2: Nominal 1=Winged; 2=Not winged Behaviour of the petiole margins - winged or not winged. The petiole and pseudostem meet at shooting. Margin is the part of the petiole that can be bent outwards/inwards." []
synonym: "Petiole margins winged @ Shooting, scale 1 to 2" EXACT []
is_a: CO_325:1000020
relationship: variable_of CO_325:0000256 ! petiole margins winged
relationship: variable_of CO_325:0010101 ! winged petiole margin - estimation
relationship: variable_of CO_325:0100050 ! wing presence/absence

[Term]
id: CO_325:0000256
name: petiole margins winged
namespace: BananaTrait
def: "Behaviour of the petiole margins - winged or not winged. The petiole and pseudostem meet at shooting. Margin is the part of the petiole that can be bent outwards/inwards." []
synonym: "Petiole margins" EXACT []
is_a: CO_325:1000007

[Term]
id: CO_325:0000259
name: PMargClasp_Est_1or2
namespace: BananaTrait
def: "Observations on the margins and petiole wings should be made where the petiole and pseudostem meet at shooting. Observation should be made at shooting on the neck, where the petiole and pseudostem meet. Margin is the part of the petiole that can be bent outwards/inwards. In clasping or not clasping. In scale 1to2: 1=Clasping; 2=Not clasping" []
synonym: "Petiole margins clasping @ Shooting, scale 1 to 2" EXACT []
is_a: CO_325:1000020
relationship: variable_of CO_325:0000260 ! petiole margins clasping
relationship: variable_of CO_325:0010102 ! petiole margin clasping - estimation
relationship: variable_of CO_325:0100052 ! clasping or not clasping

[Term]
id: CO_325:0000260
name: petiole margins clasping
namespace: BananaTrait
def: "Behaviour of the petiole margins - winged or not winged. the petiole and pseudostem meet at shooting. Margin is the part of the petiole that can be bent outwards/inwards" []
synonym: "Petiole margins" EXACT []
is_a: CO_325:1000007

[Term]
id: CO_325:0000263
name: PMargCol_Esr_1to16
namespace: BananaTrait
def: "Observations on the margins and petiole wings should be made where the petiole and pseudostem meet at shooting. Use colour chart A and observe out of direct sunlight. Record the colour of the margin (general colour is below the rim). in Banana Descriptors colour chart A -2016.  In scale 1to16: 1=Cream; 2=Yellow; 3=Watery green; 4=Green yellow; 5=Light green; 6=Medium green; 7=Green; 8=Dark green; 9=Whitish; 10=Orange red; 11=Red; 12=Pink-purple; 13=Purple-brown; 14=Red-purple; 15=Purple; 16=Blue" []
synonym: "Petiole margin colour @ Harvest, scale 1 to 16" EXACT []
is_a: CO_325:1000020
relationship: variable_of CO_325:0000264 ! petiole margin colour
relationship: variable_of CO_325:0010103 ! petiole margin colour - estimation
relationship: variable_of CO_325:0100043 ! bd colour chart a - 2016

[Term]
id: CO_325:0000264
name: petiole margin colour
namespace: BananaTrait
def: "Main colour of the petiole margin. Where the petiole and pseudostem meet at shooting. Margin is the part of the petiole that can be bent outwards/inwards" []
is_a: CO_325:1000007

[Term]
id: CO_325:0000266
name: date of planting
namespace: BananaTrait
def: "The date of planting the plant." []
synonym: "dateplant" EXACT []
synonym: "Planting date" EXACT []
is_a: CO_325:1000005

[Term]
id: CO_325:0000267
name: PltEst_Date_dmy
namespace: BananaTrait
def: "Record the date of event. in dd/mm/yyyy format" []
synonym: "Date of planting @ Planting dd/mm/yyyy" EXACT []
is_a: CO_325:1000020
relationship: variable_of CO_325:0000266 ! date of planting
relationship: variable_of CO_325:0010000 ! date of planting - estimation
relationship: variable_of CO_325:0100000 ! dd/mm/yyyy

[Term]
id: CO_325:0000268
name: PltEst_Date_ymd
namespace: BananaTrait
def: "Record the date of event. in yyyy/mm/dd format" []
synonym: "Date of planting @ Planting yyyy/mm/dd" EXACT []
is_a: CO_325:1000020
relationship: variable_of CO_325:0000266 ! date of planting
relationship: variable_of CO_325:0010000 ! date of planting - estimation
relationship: variable_of CO_325:0100001 ! yyyy/mm/dd

[Term]
id: CO_325:0000269
name: date of recognising off-type
namespace: BananaTrait
def: "The date the plant is first recognised as an off-type." []
synonym: "dateofftype" EXACT []
is_a: CO_325:1000005

[Term]
id: CO_325:0000270
name: OffTypEst_Date_dmy
namespace: BananaTrait
def: "Record the date of event. in dd/mm/yyyy format" []
synonym: "Date of recognising off-type  dd/mm/yyyy" EXACT []
is_a: CO_325:1000019
relationship: variable_of CO_325:0000269 ! date of recognising off-type
relationship: variable_of CO_325:0010001 ! date of recognising off-type - estimation
relationship: variable_of CO_325:0100000 ! dd/mm/yyyy

[Term]
id: CO_325:0000271
name: OffTypEst_Date_ymd
namespace: BananaTrait
def: "Record the date of event. in yyyy/mm/dd format" []
synonym: "Date of recognising off-type  yyyy/mm/dd" EXACT []
is_a: CO_325:1000019
relationship: variable_of CO_325:0000269 ! date of recognising off-type
relationship: variable_of CO_325:0010001 ! date of recognising off-type - estimation
relationship: variable_of CO_325:0100001 ! yyyy/mm/dd

[Term]
id: CO_325:0000272
name: date of damage
namespace: BananaTrait
def: "The date damage to the plant is first observed." []
synonym: "Damage date" EXACT []
synonym: "datedamage" EXACT []
is_a: CO_325:1000005

[Term]
id: CO_325:0000273
name: DamEst_Date_dmy
namespace: BananaTrait
def: "Record the date of event. in dd/mm/yyyy format" []
synonym: "Date of damage  dd/mm/yyyy" EXACT []
is_a: CO_325:1000019
relationship: variable_of CO_325:0000272 ! date of damage
relationship: variable_of CO_325:0010002 ! date of damage - estimation
relationship: variable_of CO_325:0100000 ! dd/mm/yyyy

[Term]
id: CO_325:0000274
name: DamEst_Date_ymd
namespace: BananaTrait
def: "Record the date of event. in yyyy/mm/dd format" []
synonym: "Date of damage  yyyy/mm/dd" EXACT []
is_a: CO_325:1000019
relationship: variable_of CO_325:0000272 ! date of damage
relationship: variable_of CO_325:0010002 ! date of damage - estimation
relationship: variable_of CO_325:0100001 ! yyyy/mm/dd

[Term]
id: CO_325:0000275
name: plant damage description
namespace: BananaTrait
def: "A description of the damage to the plant." []
synonym: "typedamage" EXACT []
is_a: CO_325:1000005

[Term]
id: CO_325:0000276
name: PltDamDesc_Est_txt
namespace: BananaTrait
def: "Record a description of the damage that occurred to the plant (e.g. leaves ripped, pseudostem snapped, plant toppled)" []
synonym: "Plant damage description" EXACT []
is_a: CO_325:1000019
relationship: variable_of CO_325:0000275 ! plant damage description
relationship: variable_of CO_325:0010003 ! plant damage description - estimation
relationship: variable_of CO_325:0100002 ! open answer

[Term]
id: CO_325:0000277
name: cause of damage
namespace: BananaTrait
def: "The apparent cause of damage." []
synonym: "causedamage" EXACT []
is_a: CO_325:1000005

[Term]
id: CO_325:0000278
name: CauDam_Est_txt
namespace: BananaTrait
def: "Record the apparent cause of the damage to the plant (e.g. strong winds, weevil damage, etc.)" []
synonym: "Cause of damage" EXACT []
is_a: CO_325:1000019
relationship: variable_of CO_325:0000277 ! cause of damage
relationship: variable_of CO_325:0010004 ! cause of damage - estimation
relationship: variable_of CO_325:0100002 ! open answer

[Term]
id: CO_325:0000279
name: date of death
namespace: BananaTrait
def: "The date of death of the plant." []
synonym: "datedeath" EXACT []
synonym: "Death date" EXACT []
is_a: CO_325:1000005

[Term]
id: CO_325:0000280
name: DateDeath_Est_dmy
namespace: BananaTrait
def: "Record the date of event. in dd/mm/yyyy format" []
synonym: "Date of death , dd/mm/yyyy" EXACT []
is_a: CO_325:1000019
relationship: variable_of CO_325:0000279 ! date of death
relationship: variable_of CO_325:0010005 ! date of death - estimation
relationship: variable_of CO_325:0100000 ! dd/mm/yyyy

[Term]
id: CO_325:0000281
name: DateDeath_Est_ymd
namespace: BananaTrait
def: "Record the date of event. in yyyy/mm/dd format" []
synonym: "Date of death , yyyy/mm/dd" EXACT []
is_a: CO_325:1000019
relationship: variable_of CO_325:0000279 ! date of death
relationship: variable_of CO_325:0010005 ! date of death - estimation
relationship: variable_of CO_325:0100001 ! yyyy/mm/dd

[Term]
id: CO_325:0000282
name: cause of death
namespace: BananaTrait
def: "The cause of death." []
synonym: "causedeath" EXACT []
is_a: CO_325:1000005

[Term]
id: CO_325:0000283
name: DeathCause_Est
namespace: BananaTrait
def: "Record the apparent cause of death of the plant (e.g. strong winds, Fusarium wilt, etc.)" []
synonym: "Cause of death" EXACT []
is_a: CO_325:1000019
relationship: variable_of CO_325:0000282 ! cause of death
relationship: variable_of CO_325:0010006 ! cause of death - estimation
relationship: variable_of CO_325:0100002 ! open answer

[Term]
id: CO_325:0000284
name: Shoot_Date_dmy
namespace: BananaTrait
def: "Record the date of event. in dd/mm/yyyy format" []
synonym: "Date of shooting, dd/mm/yyyy" EXACT []
is_a: CO_325:1000020
relationship: variable_of CO_325:0000211 ! date of shooting
relationship: variable_of CO_325:0010007 ! date of shooting - estimation
relationship: variable_of CO_325:0100000 ! dd/mm/yyyy

[Term]
id: CO_325:0000285
name: FlwT_Date_dmy
namespace: BananaTrait
def: "Record the date of event. in dd/mm/yyyy format" []
synonym: "Date of flowering, dd/mm/yyyy" EXACT []
is_a: CO_325:1000020
relationship: variable_of CO_325:0000218 ! date of flowering
relationship: variable_of CO_325:0010008 ! date of flowering - estimation
relationship: variable_of CO_325:0100000 ! dd/mm/yyyy

[Term]
id: CO_325:0000286
name: date of harvest
namespace: BananaTrait
def: "The date the bunch is harvested from the plant." []
synonym: "dateharvest" EXACT []
synonym: "Harvest date" EXACT []
is_a: CO_325:1000005

[Term]
id: CO_325:0000287
name: DateHarv_Date_dmy
namespace: BananaTrait
def: "Record the date of event. in dd/mm/yyyy format" []
synonym: "Date of harvest, dd/mm/yyyy" EXACT []
is_a: CO_325:1000020
relationship: variable_of CO_325:0000286 ! date of harvest
relationship: variable_of CO_325:0010009 ! date of harvest - estimation
relationship: variable_of CO_325:0100000 ! dd/mm/yyyy

[Term]
id: CO_325:0000288
name: DateHarv_Date_ymd
namespace: BananaTrait
def: "Record the date of event. in yyyy/mm/dd format" []
synonym: "Date of harvest, yyyy/mm/dd" EXACT []
is_a: CO_325:1000020
relationship: variable_of CO_325:0000286 ! date of harvest
relationship: variable_of CO_325:0010009 ! date of harvest - estimation
relationship: variable_of CO_325:0100001 ! yyyy/mm/dd

[Term]
id: CO_325:0000289
name: date of data collection
namespace: BananaTrait
def: "The date of data collection." []
synonym: "datedatacoll" EXACT []
is_a: CO_325:1000005

[Term]
id: CO_325:0000290
name: DateColl_Date_dmy
namespace: BananaTrait
def: "Record the date of event. in dd/mm/yyyy format" []
synonym: "Date of data collection dd/mm/yyyy" EXACT []
is_a: CO_325:1000020
relationship: variable_of CO_325:0000289 ! date of data collection
relationship: variable_of CO_325:0010010 ! date of data collection - estimation
relationship: variable_of CO_325:0100000 ! dd/mm/yyyy

[Term]
id: CO_325:0000291
name: DateColl_Date_ymd
namespace: BananaTrait
def: "Record the date of event. in yyyy/mm/dd format" []
synonym: "Date of data collection, yyyy/mm/dd" EXACT []
is_a: CO_325:1000020
relationship: variable_of CO_325:0000289 ! date of data collection
relationship: variable_of CO_325:0010010 ! date of data collection - estimation
relationship: variable_of CO_325:0100001 ! yyyy/mm/dd

[Term]
id: CO_325:0000292
name: time from flowering to harvest
namespace: BananaTrait
def: "The time elapsed from flowering (when the last bracts fall from the most distal hand to display the female flowers) to the harvest of the bunch." []
synonym: "flower2harvest" EXACT []
is_a: CO_325:1000002

[Term]
id: CO_325:0000293
name: FlwHvstTime_Comp_d
namespace: BananaTrait
def: "Calculate as: the time elapsed between the Date of flowering to the Date of harvest, in days format (e.g. 24/12/2014 - 24/10/2014 = 91 days.)" []
synonym: "Time from flowering to harvest" EXACT []
is_a: CO_325:1000020
relationship: variable_of CO_325:0000292 ! time from flowering to harvest
relationship: variable_of CO_325:0010014 ! time from flowering to harvest - computation
relationship: variable_of CO_325:0100003 ! day

[Term]
id: CO_325:0000294
name: time from planting to death
namespace: BananaTrait
def: "The time elapsed from planting to the death of the plant." []
synonym: "plant2death" EXACT []
synonym: "Time to death" EXACT []
is_a: CO_325:1000005

[Term]
id: CO_325:0000295
name: PltDth_Comp_d
namespace: BananaTrait
def: "Calculate as: the time elapsed between the Date of planting and the Date of observed death,in days format (e.g. 24/05/2014 - 24/01/2014 = 120 days)" []
synonym: "Time from planting to death" EXACT []
is_a: CO_325:1000019
relationship: variable_of CO_325:0000294 ! time from planting to death
relationship: variable_of CO_325:0010015 ! time from planting to death - computation
relationship: variable_of CO_325:0100003 ! day

[Term]
id: CO_325:0000296
name: time from harvest to death
namespace: BananaTrait
def: "The time elapsed from the harvest of the bunch of the plant from the preceding crop cycle to the death of the plant from the current crop cycle." []
synonym: "harvest2death" EXACT []
synonym: "Time to death of the ratoon plant" EXACT []
is_a: CO_325:1000005

[Term]
id: CO_325:0000297
name: HvstDth_Comp_d
namespace: BananaTrait
def: "Calculate as: the time elapsed between the Date of harvest of the preceding CROP CYCLE and the Date of observed death of the subsequent CROP CYCLE PLANT, in days format (e.g. 24/03/2015 - 24/12/2014 = 90 days)" []
synonym: "Time from harvest to death" EXACT []
is_a: CO_325:1000019
relationship: variable_of CO_325:0000296 ! time from harvest to death
relationship: variable_of CO_325:0010016 ! time from harvest to death - computation
relationship: variable_of CO_325:0100003 ! day

[Term]
id: CO_325:0000298
name: ratoon crop cycle
namespace: BananaTrait
def: "The time elapsed from the harvest of the bunch of the plant from the preceding crop cycle to the harvest of the bunch of the plant from the current crop cycle." []
synonym: "harvest2harvest" EXACT []
synonym: "Time from harvest to harvest" EXACT []
is_a: CO_325:1000002

[Term]
id: CO_325:0000299
name: RtnCrpCyc_Comp_d
namespace: BananaTrait
def: "Calculate as: the time elapsed between the Date of harvest of the preceding CROP CYCLE and the Date of harvest of the subsequent CROP CYCLE PLANT in days format (e.g. 24/11/2015 - 24/12/2014 = 335 days)" []
synonym: "Ratoon crop cycle" EXACT []
is_a: CO_325:1000020
relationship: variable_of CO_325:0000298 ! ratoon crop cycle
relationship: variable_of CO_325:0010017 ! ratoon crop cycle - computation
relationship: variable_of CO_325:0100003 ! day

[Term]
id: CO_325:0000300
name: date of marking youngest leaf
namespace: BananaTrait
def: "The date of marking the youngest leaf." []
synonym: "dateyoungleaf" EXACT []
synonym: "Marking youngest leaf date" EXACT []
is_a: CO_325:1000002

[Term]
id: CO_325:0000301
name: DateMkYL_Date_dmy
namespace: BananaTrait
def: "Calculate as: the time elapsed between the Date of harvest of the preceding CROP CYCLE and the Date of harvest of the subsequent CROP CYCLE PLANT in days format (e.g. 24/11/2015 - 24/12/2014 = 335 days)" []
synonym: "Date of marking youngest leaf  dd/mm/yyyy" EXACT []
is_a: CO_325:1000019
relationship: variable_of CO_325:0000300 ! date of marking youngest leaf
relationship: variable_of CO_325:0010018 ! date of marking youngest leaf - estimation
relationship: variable_of CO_325:0100000 ! dd/mm/yyyy

[Term]
id: CO_325:0000302
name: DateMkYL_Date_ymd
namespace: BananaTrait
def: "Calculate as: the time elapsed between the Date of harvest of the preceding CROP CYCLE and the Date of harvest of the subsequent CROP CYCLE PLANT in days format (e.g. 24/11/2015 - 24/12/2014 = 335 days)" []
synonym: "Date of marking youngest leaf , yyyy/mm/dd" EXACT []
is_a: CO_325:1000019
relationship: variable_of CO_325:0000300 ! date of marking youngest leaf
relationship: variable_of CO_325:0010018 ! date of marking youngest leaf - estimation
relationship: variable_of CO_325:0100001 ! yyyy/mm/dd

[Term]
id: CO_325:0000303
name: date of recording rank of previously marked leaf
namespace: BananaTrait
def: "The date of recording the rank of the previously marked leaf." []
synonym: "dateprevleaf" EXACT []
synonym: "Recording rank of previously marked leaf date" EXACT []
is_a: CO_325:1000002

[Term]
id: CO_325:0000304
name: DateRkPMkLf_Date_dmy
namespace: BananaTrait
def: "Record the rank of the youngest, completely unrolled, leaf, which is always 1, in dd/mm/yyyy format" []
synonym: "Date of recording rank of previously marked leaf, in dd/mm/yyyy format" EXACT []
is_a: CO_325:1000019
relationship: variable_of CO_325:0000303 ! date of recording rank of previously marked leaf
relationship: variable_of CO_325:0010019 ! date of recording rank of previously marked leaf - estimation
relationship: variable_of CO_325:0100000 ! dd/mm/yyyy

[Term]
id: CO_325:0000305
name: DateRkPMkLf_Date_ymd
namespace: BananaTrait
def: "Record the rank of the youngest, completely unrolled, leaf, which is always 1, in yyyy/mm/dd format" []
synonym: "Date of recording rank of previously marked leaf, in yyyy/mm/dd format" EXACT []
is_a: CO_325:1000019
relationship: variable_of CO_325:0000303 ! date of recording rank of previously marked leaf
relationship: variable_of CO_325:0010019 ! date of recording rank of previously marked leaf - estimation
relationship: variable_of CO_325:0100001 ! yyyy/mm/dd

[Term]
id: CO_325:0000306
name: PStmHt_M3breeder_cm
namespace: BananaTrait
def: "Measure of the distance from the ground to the angle made between the bunch stalk and bunch cover leaf, in centimeters." []
synonym: "Plant height @ Shooting, breeder protocol" EXACT []
is_a: CO_325:1000020
relationship: variable_of CO_325:0000009 ! plant height
relationship: variable_of CO_325:0010021 ! plant height - angle made between the bunch stalk and bunch cover leaf. -measurement
relationship: variable_of CO_325:0100004 ! cm

[Term]
id: CO_325:0000307
name: plant height to neck of peduncle
namespace: BananaTrait
def: "The height of the pseudostem of the plant from the pseudostem base at the ground to the curved neck of the peduncle." []
synonym: "plantheightneck" EXACT []
synonym: "Pseudostem height, Plant height" EXACT []
is_a: CO_325:1000005

[Term]
id: CO_325:0000308
name: PStmHt_M2_cm
namespace: BananaTrait
def: "Measure the distance from the pseudostem base at the ground to under the curved peduncle, using a measuring pole or sliding ruler, in centimeters" []
synonym: "Plant height to neck of peduncle @ Shooting, from ground to under the curved peduncle" EXACT []
is_a: CO_325:1000020
relationship: variable_of CO_325:0000307 ! plant height to neck of peduncle
relationship: variable_of CO_325:0010022 ! plant height - neck of peduncle - measurement
relationship: variable_of CO_325:0100004 ! cm

[Term]
id: CO_325:0000309
name: SuckHtHvstStg_M_cm
namespace: BananaTrait
def: "On the tallest sucker, measure the distance from the pseudostem base at the ground to the intersection of the petioles of the two youngest leaves (leaf ranks 1 and 2), using a measuring pole or sliding ruler, in centimeters" []
synonym: "Tallest sucker height @ Harvest" EXACT []
is_a: CO_325:1000020
relationship: variable_of CO_325:0000027 ! tallest sucker height
relationship: variable_of CO_325:0010025 ! tallest sucker height - measurement at harvest
relationship: variable_of CO_325:0100004 ! cm

[Term]
id: CO_325:0000310
name: number of water suckers
namespace: BananaTrait
def: "The number of water suckers (suckers with broad leaves, a small rhizome, and a weak connection to the plant) in the mat." []
synonym: "numwatersuckers" EXACT []
is_a: CO_325:1000005

[Term]
id: CO_325:0000311
name: WSuckN_Ct_WSuck
namespace: BananaTrait
def: "Count how many water suckers are in the mat. in water sucker." []
synonym: "Number of water suckers @ Shooting" EXACT []
is_a: CO_325:1000020
relationship: variable_of CO_325:0000310 ! number of water suckers
relationship: variable_of CO_325:0010029 ! number of water suckers - counting
relationship: variable_of CO_325:0100008 ! water suckers

[Term]
id: CO_325:0000312
name: bunch maturity stage
namespace: BananaTrait
def: "The stage of maturity of the bunch." []
synonym: "bunchmaturity" EXACT []
synonym: "stage of harvesting" EXACT []
is_a: CO_325:1000005

[Term]
id: CO_325:0000313
name: BnchMatStg_Est_1to2
namespace: BananaTrait
def: "The visual observation of bunch maturity stage using a 1 to 2 scale: 1:full green  2:first finger yellow" []
synonym: "Bunch maturity stage @ Harvest scale 1 to 2" EXACT []
is_a: CO_325:1000020
relationship: variable_of CO_325:0000312 ! bunch maturity stage
relationship: variable_of CO_325:0010031 ! bunch maturity stage - estimation
relationship: variable_of CO_325:0100010 ! maturity

[Term]
id: CO_325:0000314
name: rachis weight
namespace: BananaTrait
def: "The weight of the rachis." []
synonym: "rachisweight" EXACT []
is_a: CO_325:1000005

[Term]
id: CO_325:0000315
name: RchsWt_M_kg
namespace: BananaTrait
def: "Cut the hands off the rachis and weigh the rachis, using scales, in kilograms." []
synonym: "Rachis weight @ Harvest" EXACT []
is_a: CO_325:1000020
relationship: variable_of CO_325:0000314 ! rachis weight
relationship: variable_of CO_325:0010033 ! rachis weight - measurement
relationship: variable_of CO_325:0100011 ! kg

[Term]
id: CO_325:0000316
name: total finger weight **check on name jeff daniells
namespace: BananaTrait
def: "The weight of all the hands of the bunch, excluding the rachis." []
synonym: "Total finger weight, Total hand weight" EXACT []
synonym: "totalfingerweight" EXACT []
is_a: CO_325:1000005

[Term]
id: CO_325:0000317
name: FngWtTtl_Comp_kg
namespace: BananaTrait
def: "Calculate as: the Bunch weight, minus the Rachis weight,in kilograms e.g. 50 - 2 = 48 kg)." []
synonym: "Total finger weight **check on name Jeff Daniells @ Harvest" EXACT []
is_a: CO_325:1000020
relationship: variable_of CO_325:0000316 ! total finger weight **check on name jeff daniells
relationship: variable_of CO_325:0010034 ! total finger weight - computation
relationship: variable_of CO_325:0100011 ! kg

[Term]
id: CO_325:0000318
name: hand rank
namespace: BananaTrait
def: "The rank (position) of a hand in the bunch." []
synonym: "handid" EXACT []
is_a: CO_325:1000005

[Term]
id: CO_325:0000319
name: HndRnk_Ct_HndRnk
namespace: BananaTrait
def: "Label each hand with an identifier of its rank (position) in the bunch, starting with the hand at the proximal (top) end of the bunch as 1 and continuing downwards to the last hand at the most-distal end." []
synonym: "Hand rank" EXACT []
is_a: CO_325:1000019
relationship: variable_of CO_325:0000318 ! hand rank
relationship: variable_of CO_325:0010037 ! hand rank - counting
relationship: variable_of CO_325:0100014 ! hand rank

[Term]
id: CO_325:0000320
name: multiple number of fingers in hand
namespace: BananaTrait
def: "The number of fingers in multiple hands." []
synonym: "multnumfingshand" EXACT []
is_a: CO_325:1000005

[Term]
id: CO_325:0000321
name: HndMltpFrtNum_Ct_Frt
namespace: BananaTrait
def: "Count how many fingers are in multiple hands. Associate the data with the Hand rank and the Number of hands measured. The recommendation is to collect this data from the third and seventh hand, or in cases where there are few hands, from the second and second-most distal hands." []
synonym: "Multiple number of fingers in hand" EXACT []
is_a: CO_325:1000019
relationship: variable_of CO_325:0000320 ! multiple number of fingers in hand
relationship: variable_of CO_325:0010039 ! multiple number of fingers in hand - counting
relationship: variable_of CO_325:0100013 ! finger

[Term]
id: CO_325:0000322
name: number of hands measured
namespace: BananaTrait
def: "The number of hands used to obtain a measurement." []
synonym: "numhandsmeas" EXACT []
is_a: CO_325:1000005

[Term]
id: CO_325:0000323
name: HndNumMsrd_Ct_Hnd
namespace: BananaTrait
def: "Count how many hands are used to obtain a measurement." []
synonym: "Number of hands measured @ Harvest" EXACT []
is_a: CO_325:1000019
relationship: variable_of CO_325:0000322 ! number of hands measured
relationship: variable_of CO_325:0010040 ! number of hands measured - counting
relationship: variable_of CO_325:0100012 ! hand

[Term]
id: CO_325:0000324
name: average number of fingers in hand
namespace: BananaTrait
def: "The average number of fingers in a hand." []
synonym: "avenumfingshand" EXACT []
is_a: CO_325:1000005

[Term]
id: CO_325:0000325
name: HndFrtAvgNum_Ct_Frt
namespace: BananaTrait
def: "Calculate as: the Multiple number of fingers in hand, divided by the Number of hands measured (e.g. 40 / 2 = 20.)" []
synonym: "Average number of fingers in hand" EXACT []
is_a: CO_325:1000020
relationship: variable_of CO_325:0000324 ! average number of fingers in hand
relationship: variable_of CO_325:0010041 ! average number of fingers in hand - computation
relationship: variable_of CO_325:0100013 ! finger

[Term]
id: CO_325:0000326
name: BnchFrtNum_Comp_Frt
namespace: BananaTrait
def: "Calculate as: divide the sum of the Number of fingers in the third hand and the Number of fingers in second-most distal hand by 2, and multiply by the Number of hands in bunch (e.g. (16 + 12) / 2 * 8 = 112)." []
synonym: "Estimated number of fingers in bunch, calculation" EXACT []
is_a: CO_325:1000020
relationship: variable_of CO_325:0000039 ! number of fingers in bunch
relationship: variable_of CO_325:0010042 ! number of fingers in bunch - estimation
relationship: variable_of CO_325:0100013 ! finger

[Term]
id: CO_325:0000327
name: multiple hand weight
namespace: BananaTrait
def: "The weight of multiple hands." []
synonym: "multhandweight" EXACT []
is_a: CO_325:1000005

[Term]
id: CO_325:0000328
name: MltHandWt_M_kgPlnt
namespace: BananaTrait
def: "Cut multiple hands from the rachis and weigh them together, in kilograms. Associate the data with the Hank rank and the Number of hands measured." []
synonym: "Multiple hand weight @ Harvest" EXACT []
is_a: CO_325:1000019
relationship: variable_of CO_325:0000327 ! multiple hand weight
relationship: variable_of CO_325:0010044 ! multiple hand weight - measurement
relationship: variable_of CO_325:0100011 ! kg

[Term]
id: CO_325:0000329
name: average hand weight
namespace: BananaTrait
def: "The average weight of a hand." []
synonym: "avehandweight" EXACT []
is_a: CO_325:1000005

[Term]
id: CO_325:0000330
name: HandAvgWt_M_kgPlnt
namespace: BananaTrait
def: "Calculate as: the Multiple hand weight in kilograms , divided by the Number of hands measured ( e.g. 5.6 / 2 = 2.8)" []
synonym: "Average hand weight @ Harvest" EXACT []
is_a: CO_325:1000019
relationship: variable_of CO_325:0000329 ! average hand weight
relationship: variable_of CO_325:0010045 ! average hand weight - computation
relationship: variable_of CO_325:0100011 ! kg

[Term]
id: CO_325:0000331
name: multiple finger weight
namespace: BananaTrait
def: "The weight of multiple fingers." []
synonym: "multfingerweight" EXACT []
is_a: CO_325:1000005

[Term]
id: CO_325:0000332
name: MltFrtWt_M_gFruit
namespace: BananaTrait
def: "Weight multiple fingers together, in grams. Associate the data with the Hank rank and the Number of fingers measured. The recommendation is to collect this data from three fingers in the middle of the outer whorl from both the third and of the seventh hand, or in cases where there are few hands, from the second and second-most distal hands." []
synonym: "Multiple finger weight @ Harvest" EXACT []
is_a: CO_325:1000019
relationship: variable_of CO_325:0000331 ! multiple finger weight
relationship: variable_of CO_325:0010047 ! multiple finger weight - measurement
relationship: variable_of CO_325:0100015 ! g

[Term]
id: CO_325:0000333
name: number of fingers measured
namespace: BananaTrait
def: "The number of fingers used to obtain a measurement." []
synonym: "numfingersmeas" EXACT []
is_a: CO_325:1000005

[Term]
id: CO_325:0000334
name: FrtNb_Ct_gFruit
namespace: BananaTrait
def: "Count how many fingers are used to obtain a measurement." []
synonym: "Number of fingers measured @ Harvest" EXACT []
is_a: CO_325:1000019
relationship: variable_of CO_325:0000333 ! number of fingers measured
relationship: variable_of CO_325:0010048 ! number of fingers measured - counting
relationship: variable_of CO_325:0100013 ! finger

[Term]
id: CO_325:0000335
name: average finger weight
namespace: BananaTrait
def: "The average weight of a finger." []
synonym: "avefingerweight" EXACT []
is_a: CO_325:1000005

[Term]
id: CO_325:0000336
name: FrtWtAvg_M_g
namespace: BananaTrait
def: "Calculate as: the Multiple finger weight, divided by the Number of fingers measured, e.g. 1633 / 6 = 272." []
synonym: "Average finger weight" EXACT []
is_a: CO_325:1000020
relationship: variable_of CO_325:0000335 ! average finger weight
relationship: variable_of CO_325:0010049 ! average finger weight - computation
relationship: variable_of CO_325:0100015 ! g

[Term]
id: CO_325:0000337
name: average finger external length
namespace: BananaTrait
def: "The average length of a finger measured along the external (dorsal) arc, excluding the petiole and the flower tip." []
synonym: "avefingerextlength" EXACT []
synonym: "Average finger dorsal length" EXACT []
is_a: CO_325:1000005

[Term]
id: CO_325:0000338
name: AvgFrtExtLng_M_cm
namespace: BananaTrait
def: "Calculate as: the sum of the Finger external length measurements, divided by the Number of fingers measured (e.g. (30 + 34 + 32 + 33 + 33 + 31) / 6 = 32.1.)" []
synonym: "Average finger external length @ Harvest" EXACT []
is_a: CO_325:1000020
relationship: variable_of CO_325:0000337 ! average finger external length
relationship: variable_of CO_325:0010051 ! average finger external length - computation
relationship: variable_of CO_325:0100004 ! cm

[Term]
id: CO_325:0000339
name: finger internal length
namespace: BananaTrait
def: "The length of a finger measured along the internal (ventral) arc, excluding the petiole and the flower tip." []
synonym: "Finger ventral length" EXACT []
synonym: "fingerintlength" EXACT []
is_a: CO_325:1000005

[Term]
id: CO_325:0000340
name: FrtIntLng_M_cm
namespace: BananaTrait
def: "Measure the length of the internal arc of the fruit, without pedicel. record on second hand middle finger on the outer whorl circumference, in centimeters." []
synonym: "Finger internal length @ Harvest" EXACT []
is_a: CO_325:1000020
relationship: variable_of CO_325:0000339 ! finger internal length
relationship: variable_of CO_325:0010052 ! finger internal length - measurement
relationship: variable_of CO_325:0100004 ! cm

[Term]
id: CO_325:0000341
name: average finger internal length
namespace: BananaTrait
def: "The average length of a finger measured along the internal (ventral) arc, excluding the petiole and the flower tip." []
synonym: "avefingerintlength" EXACT []
synonym: "Average finger ventral length" EXACT []
is_a: CO_325:1000005

[Term]
id: CO_325:0000342
name: AvgFrtIntLng_M_cm
namespace: BananaTrait
def: "Calculate as: the sum of the Finger internal length measurements, divided by the Number of fingers measured (e.g. (30 + 34 + 32 + 33 + 33 + 31) / 6 = 32.1.)" []
synonym: "Average finger internal length @ Harvest" EXACT []
is_a: CO_325:1000020
relationship: variable_of CO_325:0000341 ! average finger internal length
relationship: variable_of CO_325:0010053 ! average finger internal length - computation
relationship: variable_of CO_325:0100004 ! cm

[Term]
id: CO_325:0000343
name: FrtGrth_M_mm
namespace: BananaTrait
def: "Measure the circumference (= girth) of a finger at its widest point, using a tape measure, in millimeters." []
synonym: "Finger circumference @ Harvest, in millimeters" EXACT []
is_a: CO_325:1000020
relationship: variable_of CO_325:0000054 ! finger circumference
relationship: variable_of CO_325:0010054 ! finger circumference - measurement
relationship: variable_of CO_325:0100016 ! mm

[Term]
id: CO_325:0000344
name: average finger circumference
namespace: BananaTrait
def: "The average circumference of a finger." []
synonym: "avefingercircumf" EXACT []
synonym: "Average finger girth" EXACT []
is_a: CO_325:1000005

[Term]
id: CO_325:0000345
name: AvgFrtGrth_M_mm
namespace: BananaTrait
def: "Calculate as: the sum of the Finger circumference measurements, divided by the Number of fingers measured (e.g. (70 + 80 + 90 + 100 + 70 + 95) / 6 = 84.)" []
synonym: "Average finger circumference @ Harvest, in millimeters" EXACT []
is_a: CO_325:1000020
relationship: variable_of CO_325:0000344 ! average finger circumference
relationship: variable_of CO_325:0010055 ! average finger circumference - computation
relationship: variable_of CO_325:0100016 ! mm

[Term]
id: CO_325:0000346
name: AvgFrtGrth_M_cm
namespace: BananaTrait
def: "Calculate as: the sum of the Finger circumference measurements, divided by the Number of fingers measured, e.g. (7 + 8 + 9 + 10 + 7 + 9.5) / 6 = 8.4." []
synonym: "Average finger circumference @ Harvest, in centimeters" EXACT []
is_a: CO_325:1000020
relationship: variable_of CO_325:0000344 ! average finger circumference
relationship: variable_of CO_325:0010055 ! average finger circumference - computation
relationship: variable_of CO_325:0100004 ! cm

[Term]
id: CO_325:0000347
name: FrtDiam_M_mm
namespace: BananaTrait
def: "Measure the lateral diameter of a finger, from the left to the right side (not from the ventral to the dorsal side), at the widest point, using calipers, in millimeters." []
synonym: "Finger lateral diameter @ Harvest, in millimeters" EXACT []
is_a: CO_325:1000020
relationship: variable_of CO_325:0000233 ! finger lateral diameter
relationship: variable_of CO_325:0010056 ! finger lateral diameter - measurement
relationship: variable_of CO_325:0100016 ! mm

[Term]
id: CO_325:0000348
name: average finger lateral diameter
namespace: BananaTrait
def: "The average lateral (side to side) diameter of a finger." []
synonym: "avefingerlatdiam" EXACT []
is_a: CO_325:1000005

[Term]
id: CO_325:0000349
name: AvgFrtDiam_M_mm
namespace: BananaTrait
def: "Calculate as: the sum of the Finger lateral diameter measurements, divided by the Number of fingers measured, e.g. (35 + 52 + 41 + 5 + 6 + 68) / 6 = 51." []
synonym: "Average finger lateral diameter @ Harvest, in millimeters" EXACT []
is_a: CO_325:1000020
relationship: variable_of CO_325:0000348 ! average finger lateral diameter
relationship: variable_of CO_325:0010057 ! average finger lateral diameter - computation
relationship: variable_of CO_325:0100016 ! mm

[Term]
id: CO_325:0000350
name: AvgFrtDiam_M_cm
namespace: BananaTrait
def: "Calculate as: the sum of the Finger lateral diameter measurements, divided by the Number of fingers measured, e.g. (3.5 + 5.2 + 4.1 + 5 + 6 + 6.8) / 6 = 5.1." []
synonym: "Average finger lateral diameter @ Harvest, in centimeters" EXACT []
is_a: CO_325:1000020
relationship: variable_of CO_325:0000348 ! average finger lateral diameter
relationship: variable_of CO_325:0010057 ! average finger lateral diameter - computation
relationship: variable_of CO_325:0100004 ! cm

[Term]
id: CO_325:0000351
name: PulpDiam_M_mm
namespace: BananaTrait
def: "Remove the peel of a finger and measure the lateral diameter of the fruit pulp, from the left to the right side (not from the ventral to the dorsal side), at the widest point, using calipers, in millimeters." []
synonym: "Fruit pulp lateral diameter @ When fruit mature at ready-to-eat stage, in millimeters" EXACT []
is_a: CO_325:1000020
relationship: variable_of CO_325:0000240 ! fruit pulp lateral diameter
relationship: variable_of CO_325:0010058 ! fruit pulp lateral diameter - measurement
relationship: variable_of CO_325:0100016 ! mm

[Term]
id: CO_325:0000352
name: average fruit pulp lateral diameter
namespace: BananaTrait
def: "The average lateral (side to side) diameter of the pulp of a fruit." []
synonym: "avepulpdiam" EXACT []
is_a: CO_325:1000005

[Term]
id: CO_325:0000353
name: AvgPulpDiam_M_mm
namespace: BananaTrait
def: "Calculate as: the sum of the Fruit pulp lateral diameter measurements, divided by the Number of fingers measured, e.g. (31 + 48 + 37 + 46 + 56 + 64) / 6 = 47." []
synonym: "Average fruit pulp lateral diameter @ When fruit mature at ready-to-eat stage, in millimeters" EXACT []
is_a: CO_325:1000020
relationship: variable_of CO_325:0000352 ! average fruit pulp lateral diameter
relationship: variable_of CO_325:0010059 ! average fruit pulp lateral diameter - computation
relationship: variable_of CO_325:0100016 ! mm

[Term]
id: CO_325:0000354
name: AvgPulpDiam_M_cm
namespace: BananaTrait
def: "Calculate as: the sum of the Fruit pulp lateral diameter measurements, divided by the Number of fingers measured, e.g. (3.1 + 4.8 + 3.7 + 4.6 + 5.6 + 6.4) / 6 = 4.7." []
synonym: "Average fruit pulp lateral diameter @ When fruit mature at ready-to-eat stage, in centimeters" EXACT []
is_a: CO_325:1000020
relationship: variable_of CO_325:0000352 ! average fruit pulp lateral diameter
relationship: variable_of CO_325:0010059 ! average fruit pulp lateral diameter - computation
relationship: variable_of CO_325:0100004 ! cm

[Term]
id: CO_325:0000355
name: average finger peel thickness
namespace: BananaTrait
def: "The average thickness of the peel of a finger." []
synonym: "avepeelthickness" EXACT []
is_a: CO_325:1000005

[Term]
id: CO_325:0000356
name: AvgPeelThck_M_mm
namespace: BananaTrait
def: "Calculate as: the sum of the Finger peel thickness measurements, divided by the Number of fingers measured, e.g. (2 + 2 + 2 + 3 + 2 + 3 + 3) / 6 = 2." []
synonym: "Average finger peel thickness" EXACT []
is_a: CO_325:1000020
relationship: variable_of CO_325:0000355 ! average finger peel thickness
relationship: variable_of CO_325:0010061 ! average finger peel thickness - computation
relationship: variable_of CO_325:0100016 ! mm

[Term]
id: CO_325:0000357
name: number of plants planted
namespace: BananaTrait
def: "The number of plants that are planted." []
synonym: "numplanted" EXACT []
is_a: CO_325:1000005

[Term]
id: CO_325:0000358
name: PltPltd_Ct_Plnt
namespace: BananaTrait
def: "Calculate as: the sum of the number of plants at Date of planting." []
synonym: "Number of plants planted" EXACT []
is_a: CO_325:1000020
relationship: variable_of CO_325:0000357 ! number of plants planted
relationship: variable_of CO_325:0010062 ! number of plants planted - computation
relationship: variable_of CO_325:0100017 ! plant

[Term]
id: CO_325:0000359
name: plant spacing
namespace: BananaTrait
def: "The area allocated to one plant." []
synonym: "plantspacing" EXACT []
is_a: CO_325:1000005

[Term]
id: CO_325:0000360
name: PltSpcg_Comp_m2
namespace: BananaTrait
def: "Calculate as: multiply the distance of the spacing between the plants, both latitudinally and longitudinally. (e.g. 2 m x 3 m = 6 m2.)" []
synonym: "Plant spacing" EXACT []
is_a: CO_325:1000020
relationship: variable_of CO_325:0000359 ! plant spacing
relationship: variable_of CO_325:0010063 ! plant spacing - computation
relationship: variable_of CO_325:0100018 ! m2

[Term]
id: CO_325:0000361
name: plant density
namespace: BananaTrait
def: "The number of plants that are planted, in a defined area." []
synonym: "plantdens" EXACT []
is_a: CO_325:1000005

[Term]
id: CO_325:0000362
name: PltDnsty_Comp_PlntHa
namespace: BananaTrait
def: "Calculate as: number of square metres in the area unit of choice, divided by the Plant spacing, in plants/ha  (e.g. 10,000 square metres in 1 hectare / 6 = 1,667 plants/ha.)" []
synonym: "Plant density" EXACT []
is_a: CO_325:1000020
relationship: variable_of CO_325:0000361 ! plant density
relationship: variable_of CO_325:0010064 ! plant density - computation
relationship: variable_of CO_325:0100019 ! plants/unit of area

[Term]
id: CO_325:0000363
name: number of plants dead
namespace: BananaTrait
def: "The number of plants that are dead." []
synonym: "numdead" EXACT []
is_a: CO_325:1000005

[Term]
id: CO_325:0000364
name: PltDead_Ct_Plnt
namespace: BananaTrait
def: "Calculate as: the sum of the number of values for Date of death." []
synonym: "Number of plants dead" EXACT []
is_a: CO_325:1000020
relationship: variable_of CO_325:0000363 ! number of plants dead
relationship: variable_of CO_325:0010065 ! number of plants dead - computation
relationship: variable_of CO_325:0100017 ! plant

[Term]
id: CO_325:0000365
name: number of plants harvested
namespace: BananaTrait
def: "The number of plants that are harvested." []
synonym: "numharv" EXACT []
is_a: CO_325:1000005

[Term]
id: CO_325:0000366
name: PltHvstd_Ct_Plnt
namespace: BananaTrait
def: "Calculate as: the sum of the number of values for Date of harvest." []
synonym: "Number of plants harvested" EXACT []
is_a: CO_325:1000020
relationship: variable_of CO_325:0000365 ! number of plants harvested
relationship: variable_of CO_325:0010066 ! number of plants harvested - computation
relationship: variable_of CO_325:0100017 ! plant

[Term]
id: CO_325:0000367
name: number of plants not harvested
namespace: BananaTrait
def: "The number of plants that are alive but not harvested (e.g. due to slow or poor development)." []
synonym: "numnotharv" EXACT []
is_a: CO_325:1000005

[Term]
id: CO_325:0000368
name: PltNtHvstd_Ct_Plnt
namespace: BananaTrait
def: "Calculate as: the Number of plants planted, minus the Number of plants dead, minus the Number of plants harvested." []
synonym: "Number of plants not harvested" EXACT []
is_a: CO_325:1000020
relationship: variable_of CO_325:0000367 ! number of plants not harvested
relationship: variable_of CO_325:0010067 ! number of plants not harvested - computation
relationship: variable_of CO_325:0100017 ! plant

[Term]
id: CO_325:0000369
name: death proportion
namespace: BananaTrait
def: "The proportion of plants that are dead, from the number of plants planted." []
synonym: "deathprop" EXACT []
is_a: CO_325:1000005

[Term]
id: CO_325:0000370
name: DthPrp_Comp_DdPltRt
namespace: BananaTrait
def: "Calculate as: the Number of plants dead, divided by the Number of plants planted, in plants dead/plants planted  (e.g. 4 / 24 = 0.17.)" []
synonym: "Death proportion" EXACT []
is_a: CO_325:1000019
relationship: variable_of CO_325:0000369 ! death proportion
relationship: variable_of CO_325:0010068 ! death proportion - computation
relationship: variable_of CO_325:0100020 ! plants dead/plants planted

[Term]
id: CO_325:0000371
name: death density
namespace: BananaTrait
def: "The number of plants that are dead, in a defined area." []
synonym: "deathdens" EXACT []
is_a: CO_325:1000005

[Term]
id: CO_325:0000372
name: DthDnst_Comp_PlntHa
namespace: BananaTrait
def: "Calculate as: the Plant density multiplied by the Death proportion in plants/ha (e.g. 1,667 * 0.17 = 283 plants/ha)." []
synonym: "Death density" EXACT []
is_a: CO_325:1000019
relationship: variable_of CO_325:0000371 ! death density
relationship: variable_of CO_325:0010069 ! death density - computation
relationship: variable_of CO_325:0100019 ! plants/unit of area

[Term]
id: CO_325:0000373
name: harvest proportion
namespace: BananaTrait
def: "The proportion of plants that are harvested, from the number of plants planted." []
synonym: "harvprop" EXACT []
is_a: CO_325:1000005

[Term]
id: CO_325:0000374
name: HvstPrp_Comp_PlntNb
namespace: BananaTrait
def: "Calculate as: the Number of plants harvested, divided by the Number of plants planted, in plants harvested/plants planted. (e.g. 18 / 24 = 0.75.)" []
synonym: "Harvest proportion" EXACT []
is_a: CO_325:1000019
relationship: variable_of CO_325:0000373 ! harvest proportion
relationship: variable_of CO_325:0010070 ! harvest proportion - computation
relationship: variable_of CO_325:0100021 ! plants harvested/plants planted

[Term]
id: CO_325:0000375
name: harvest density
namespace: BananaTrait
def: "The number of plants that are harvested, in a defined area." []
synonym: "harvdens" EXACT []
is_a: CO_325:1000005

[Term]
id: CO_325:0000376
name: HvstDst_Comp_PlntHa
namespace: BananaTrait
def: "Calculate as: the Plant density multiplied by the Harvest proportion,in plants/ha (e.g. 1,667 * 0.75 = 1,250 plants/ha)." []
synonym: "Harvest density" EXACT []
is_a: CO_325:1000019
relationship: variable_of CO_325:0000375 ! harvest density
relationship: variable_of CO_325:0010071 ! harvest density - computation
relationship: variable_of CO_325:0100019 ! plants/unit of area

[Term]
id: CO_325:0000377
name: non-harvest proportion
namespace: BananaTrait
def: "The proportion of plants that are alive but not harvested (e.g. due to slow or poor development), from the number of plants planted." []
synonym: "nonharvprop" EXACT []
is_a: CO_325:1000005

[Term]
id: CO_325:0000378
name: NtHvstPrp_Comp_PlntNb
namespace: BananaTrait
def: "Calculate as: the Number of plants not harvested, divided by the Number of plants planted,in plants not harvested/plants planted (e.g. 2 / 24 = 0.08.)" []
synonym: "Non-harvest proportion" EXACT []
is_a: CO_325:1000019
relationship: variable_of CO_325:0000377 ! non-harvest proportion
relationship: variable_of CO_325:0010072 ! non-harvest proportion - computation
relationship: variable_of CO_325:0100022 ! plants not harvested/plants planted

[Term]
id: CO_325:0000379
name: non-harvest density
namespace: BananaTrait
def: "The number of plants that are alive but not harvested (e.g. due to slow or poor development), in a defined area." []
synonym: "nonharvdens" EXACT []
is_a: CO_325:1000005

[Term]
id: CO_325:0000380
name: NtHvstDst_Comp_PlntHa
namespace: BananaTrait
def: "Calculate as: the Plant density multiplied by the Non-harvest proportion,in plants/ha (e.g. 1,667 * 0.08 = 133 plants/ha.)" []
synonym: "Non-harvest density" EXACT []
is_a: CO_325:1000019
relationship: variable_of CO_325:0000379 ! non-harvest density
relationship: variable_of CO_325:0010073 ! non-harvest density - computation
relationship: variable_of CO_325:0100019 ! plants/unit of area

[Term]
id: CO_325:0000381
name: annual crop cycle proportion **ask jeff if this already has a different name
namespace: BananaTrait
def: "The proportion of the crop cycle that takes place in one year." []
synonym: "anncropcycprop" EXACT []
is_a: CO_325:1000005

[Term]
id: CO_325:0000382
name: AnCrpCyclPrp_Comp_CrpCclY
namespace: BananaTrait
def: "Calculate as: the number of days in a year (365) divided by the Time from planting to harvest/plant ratoon cycle, in crop cycle duration/year (e.g. 365 / 334 = 1.09.)" []
synonym: "Annual crop cycle proportion **ask Jeff if this already has a different name" EXACT []
is_a: CO_325:1000020
relationship: variable_of CO_325:0000381 ! annual crop cycle proportion **ask jeff if this already has a different name
relationship: variable_of CO_325:0010074 ! annual crop cycle proportion - computation
relationship: variable_of CO_325:0100023 ! crop cycle duration/year

[Term]
id: CO_325:0000383
name: plant annual yield
namespace: BananaTrait
def: "The bunch weight produced by the plant over the course of the crop cycle, averaged across one year." []
synonym: "plantannyield" EXACT []
is_a: CO_325:1000005

[Term]
id: CO_325:0000384
name: AnPltPrp_Comp_KgHaY
namespace: BananaTrait
def: "Calculate as: the Bunch weight multiplied by the Annual crop cycle proportion in kilograms/plant/year (e.g. 48 * 1.09 = 52.32 kg/plant/y)." []
synonym: "Plant annual yield" EXACT []
is_a: CO_325:1000020
relationship: variable_of CO_325:0000383 ! plant annual yield
relationship: variable_of CO_325:0010075 ! annual plant productivity - computation
relationship: variable_of CO_325:0100024 ! kg/plant/y

[Term]
id: CO_325:0000385
name: average actual annual yield
namespace: BananaTrait
def: "The average actual annual yield, taking into account the proportion of plants harvested, from the number of plants planted" []
synonym: "actualannyield" EXACT []
synonym: "Yield" EXACT []
is_a: CO_325:1000005

[Term]
id: CO_325:0000386
name: AcAnYd_Comp_TnHaY
namespace: BananaTrait
def: "Calculate as: the Bunch weight divided by 1,000, multiplied by the Annual crop cycle proportion, multiplied by the Harvest density in tons/hectare/year (e.g. (50 / 1,000) * 1.09 * 1,250 = 68.13 t/ha/y)." []
synonym: "Average actual annual yield" EXACT []
is_a: CO_325:1000020
relationship: variable_of CO_325:0000385 ! average actual annual yield
relationship: variable_of CO_325:0010076 ! actual annual yield - computation
relationship: variable_of CO_325:0100025 ! t/unit of area/y

[Term]
id: CO_325:0000387
name: average potential annual yield
namespace: BananaTrait
def: "The average potential annual yield, assuming that all plants are harvested, from the number of plants planted." []
synonym: "potannyield" EXACT []
synonym: "Yield" EXACT []
is_a: CO_325:1000005

[Term]
id: CO_325:0000388
name: PtYd_Comp_TnHaY
namespace: BananaTrait
def: "Calculate as: the Bunch weight divided by 1,000, multiplied by the Annual crop cycle proportion, multiplied by the Plant density, in tons/hectare/year (e.g. (50 / 1,000) * 1.09 * 1,667 = 90.85 t/ha/y)." []
synonym: "Average potential annual yield" EXACT []
is_a: CO_325:1000020
relationship: variable_of CO_325:0000387 ! average potential annual yield
relationship: variable_of CO_325:0010077 ! potential annual yield - computation
relationship: variable_of CO_325:0100025 ! t/unit of area/y

[Term]
id: CO_325:0000389
name: overall fruit pendulance
namespace: BananaTrait
def: "The overall estimation fruit pendulance on a bunch" []
synonym: "pendulantfruit" EXACT []
is_a: CO_325:1000005

[Term]
id: CO_325:0000390
name: PdltFrt_Est_1to2
namespace: BananaTrait
def: "The visual observation of fruit pendulance on a bunch using 1 to 2 scale: 1= bad ; 2= good" []
synonym: "Overall fruit pendulance" EXACT []
is_a: CO_325:1000020
relationship: variable_of CO_325:0000389 ! overall fruit pendulance
relationship: variable_of CO_325:0010078 ! fruit pendulance - estimation
relationship: variable_of CO_325:0100026 ! 1 to 2 acceptability score

[Term]
id: CO_325:0000391
name: overall bunch quality
namespace: BananaTrait
def: "The overall estimation of the bunch quality on a mat" []
synonym: "goodbunch" EXACT []
is_a: CO_325:1000005

[Term]
id: CO_325:0000392
name: GdBnch_Est_1to2
namespace: BananaTrait
def: "The visual observation  of the bunch quality on a mat using a 1 to 2 scale: 1= bad; 2= good" []
synonym: "Overall bunch quality" EXACT []
is_a: CO_325:1000020
relationship: variable_of CO_325:0000391 ! overall bunch quality
relationship: variable_of CO_325:0010079 ! bunch quality - estimation
relationship: variable_of CO_325:0100026 ! 1 to 2 acceptability score

[Term]
id: CO_325:0000393
name: partenocarpy
namespace: BananaTrait
def: "The overall estimation of fruit parthenocarpy level on a bunch" []
synonym: "goodfruitfill" EXACT []
is_a: CO_325:1000005

[Term]
id: CO_325:0000394
name: GdFrtFll_Est_1to2
namespace: BananaTrait
def: "The visual observation  of fruit parthenocarpy level on a bunch  using 1= Parthenocarpic; 2= Not parthenocarpic" []
synonym: "Partenocarpy" EXACT []
is_a: CO_325:1000020
relationship: variable_of CO_325:0000393 ! partenocarpy
relationship: variable_of CO_325:0010080 ! fruit parthenocarpy - estimation
relationship: variable_of CO_325:0100027 ! parthenocarpy presence

[Term]
id: CO_325:0000395
name: overall suckering quality
namespace: BananaTrait
def: "The overall estimation sucker quality on a mat" []
synonym: "suckering" EXACT []
is_a: CO_325:1000005

[Term]
id: CO_325:0000396
name: Sckr_Est_1to2
namespace: BananaTrait
def: "The visual observation  sucker quality on a mat using 1=bad; 2=good" []
synonym: "Overall suckering quality" EXACT []
is_a: CO_325:1000020
relationship: variable_of CO_325:0000395 ! overall suckering quality
relationship: variable_of CO_325:0010081 ! sucker quality - estimation
relationship: variable_of CO_325:0100026 ! 1 to 2 acceptability score

[Term]
id: CO_325:0000397
name: dwarfism
namespace: BananaTrait
def: "The presence or absence of dwarfism on a mat" []
synonym: "dwarfism" EXACT []
is_a: CO_325:1000005

[Term]
id: CO_325:0000398
name: Dwfsm_Est_1to2
namespace: BananaTrait
def: "The presence or absence of dwarfism on a mat using 1=Dwarf; 2=Not Dwarf" []
synonym: "Dwarfism" EXACT []
is_a: CO_325:1000020
relationship: variable_of CO_325:0000397 ! dwarfism
relationship: variable_of CO_325:0010082 ! dwarfism - estimation
relationship: variable_of CO_325:0100028 ! dwarfism presence

[Term]
id: CO_325:0000399
name: trial group id
namespace: BananaTrait
def: "The identifier of the trial group, if multiple field trials are being conducted with the same purpose." []
synonym: "trialgroup_id" EXACT []
is_a: CO_325:1000004

[Term]
id: CO_325:0000400
name: TrlGrpID
namespace: BananaTrait
def: "Assign the trial group a unique identifier, e.g. IMTP 3 in ??" []
synonym: "Trial group ID" EXACT []
is_a: CO_325:1000020
relationship: variable_of CO_325:0000399 ! trial group id
relationship: variable_of CO_325:0010083 ! trial group id -counting
relationship: variable_of CO_325:0100029 ! Trial group scale

[Term]
id: CO_325:0000401
name: trial id
namespace: BananaTrait
def: "The identifier of the field trial." []
synonym: "trial_id" EXACT []
is_a: CO_325:1000004

[Term]
id: CO_325:0000402
name: TrlID
namespace: BananaTrait
def: "Assign the field trial a unique identifier, e.g. IMTP 3 - Cameroon BLS in ??" []
synonym: "Trial ID" EXACT []
is_a: CO_325:1000020
relationship: variable_of CO_325:0000401 ! trial id
relationship: variable_of CO_325:0010084 ! trial id -counting
relationship: variable_of CO_325:0100030 ! Trial  scale

[Term]
id: CO_325:0000403
name: block id
namespace: BananaTrait
def: "The identifier of the experimental block within the field trial." []
synonym: "block_id" EXACT []
is_a: CO_325:1000004

[Term]
id: CO_325:0000404
name: BlkID
namespace: BananaTrait
def: "Assign each experimental block within the field trial a unique identifier, e.g. 1, 2, 3, 4, or A, B, C, D, etc. in ??" []
synonym: "Block ID" EXACT []
is_a: CO_325:1000020
relationship: variable_of CO_325:0000403 ! block id
relationship: variable_of CO_325:0010085 ! block id -counting
relationship: variable_of CO_325:0100031 ! Block  scale

[Term]
id: CO_325:0000405
name: row id
namespace: BananaTrait
def: "The identifier of the row within the field trial." []
synonym: "row_id" EXACT []
is_a: CO_325:1000004

[Term]
id: CO_325:0000406
name: RwID
namespace: BananaTrait
def: "Assign each row (latitudinally) within the field trial a unique identifier, e.g. 1, 2, 3, 4, or A, B, C, D, etc. in ??" []
synonym: "Row ID" EXACT []
is_a: CO_325:1000020
relationship: variable_of CO_325:0000405 ! row id
relationship: variable_of CO_325:0010086 ! row id -counting
relationship: variable_of CO_325:0100032 ! Row  scale

[Term]
id: CO_325:0000407
name: column id
namespace: BananaTrait
def: "The identifier of the column within the field trial." []
synonym: "column_id" EXACT []
is_a: CO_325:1000004

[Term]
id: CO_325:0000408
name: ClmnID
namespace: BananaTrait
def: "Assign each column (longitudinally) within the field trial a unique identifier, e.g. 1, 2, 3, 4, or A, B, C, D, etc. in ??" []
synonym: "Column ID" EXACT []
is_a: CO_325:1000020
relationship: variable_of CO_325:0000407 ! column id
relationship: variable_of CO_325:0010087 ! column id -counting
relationship: variable_of CO_325:0100033 ! Column  scale

[Term]
id: CO_325:0000409
name: spatial position id
namespace: BananaTrait
def: "The identifier of the plant-level spatial position within the field trial." []
synonym: "spatialpos_id" EXACT []
is_a: CO_325:1000004

[Term]
id: CO_325:0000410
name: SptPsID_Comp
namespace: BananaTrait
def: "Calculate as: the concatenation of Block ID, Row ID, and Column ID, e.g. 1_A_26 in ??" []
synonym: "Spatial position ID" EXACT []
is_a: CO_325:1000020
relationship: variable_of CO_325:0000409 ! spatial position id
relationship: variable_of CO_325:0010088 ! spatial position id -counting
relationship: variable_of CO_325:0100034 ! Spatial position  scale

[Term]
id: CO_325:0000411
name: accession id
namespace: BananaTrait
def: "The identifier of the genebank accession code of the plant." []
synonym: "acccode" EXACT []
is_a: CO_325:1000004

[Term]
id: CO_325:0000412
name: AccID
namespace: BananaTrait
def: "Record the genebank accession code of the genotype of the plant, if the planting material was sourced from a genebank either directly or secondarily through a tissue-culture provider. in ??" []
synonym: "Accession ID" EXACT []
is_a: CO_325:1000020
relationship: variable_of CO_325:0000411 ! accession id
relationship: variable_of CO_325:0010089 ! accession id -counting
relationship: variable_of CO_325:0100035 ! Accession  scale

[Term]
id: CO_325:0000413
name: genotype id
namespace: BananaTrait
def: "The identifier of the genotype of the plant." []
synonym: "geno_id" EXACT []
is_a: CO_325:1000004

[Term]
id: CO_325:0000414
name: GntpID
namespace: BananaTrait
def: "Assign the genotype a unique identifier" []
synonym: "Genotype ID" EXACT []
is_a: CO_325:1000020
relationship: variable_of CO_325:0000413 ! genotype id
relationship: variable_of CO_325:0010090 ! genotype id -counting
relationship: variable_of CO_325:0100036 ! Genotype ID scale

[Term]
id: CO_325:0000415
name: genotype purpose
namespace: BananaTrait
def: "The reason for including the genotype in the field trial." []
synonym: "genopurpose" EXACT []
is_a: CO_325:1000004

[Term]
id: CO_325:0000416
name: GntpPrp
namespace: BananaTrait
def: "Record the reason for including the genotype in the evaluation in folloowing format: Nominal 1=Test accession;2=Local check;3=Resistant/tolerant check;4=Susceptible check;5=Border row" []
synonym: "Genotype purpose" EXACT []
is_a: CO_325:1000020
relationship: variable_of CO_325:0000415 ! genotype purpose
relationship: variable_of CO_325:0010091 ! genotype purpose -counting
relationship: variable_of CO_325:0100037 ! genotype purpose scale

[Term]
id: CO_325:0000417
name: mat id
namespace: BananaTrait
def: "The identifier of the mat within the field trial." []
synonym: "mat_id" EXACT []
is_a: CO_325:1000004

[Term]
id: CO_325:0000418
name: MatID_Comp
namespace: BananaTrait
def: "Calculate as: ... = the spatial position ** but with an extra identifier to show whether it is the first, or whether plant has died and needed to be replanted, so is therefore the second...  Does that identifier need to have its own trait? in ??" []
synonym: "Mat ID" EXACT []
is_a: CO_325:1000020
relationship: variable_of CO_325:0000417 ! mat id
relationship: variable_of CO_325:0010092 ! mat id -counting
relationship: variable_of CO_325:0100038 ! Mat ID scale

[Term]
id: CO_325:0000419
name: crop cycle id
namespace: BananaTrait
def: "The identifier of the crop cycle that the plant being measured represents." []
synonym: "cropcycle_id" EXACT []
is_a: CO_325:1000004

[Term]
id: CO_325:0000420
name: CrpCyc_ID
namespace: BananaTrait
def: "Assign each crop cycle a unique identifier, e.g. 1 = first plant that is planted, 2 = first ratoon plant, 3 = second ratoon plant, etc. in following format: Ordinal 1=First plant planted;2=First ratoon plant;3=Second ratoon plant;4=Third ratoon plant;5=Fourth ratoon plant;6=Fifth ratoon plant" []
synonym: "Crop cycle ID" EXACT []
is_a: CO_325:1000020
relationship: variable_of CO_325:0000419 ! crop cycle id
relationship: variable_of CO_325:0010093 ! crop cycle id -counting
relationship: variable_of CO_325:0100039 ! crop cycle duration/year scale

[Term]
id: CO_325:0000421
name: plant id
namespace: BananaTrait
def: "The identifier of the plant." []
synonym: "plant_id" EXACT []
is_a: CO_325:1000004

[Term]
id: CO_325:0000422
name: PltID_Comp_
namespace: BananaTrait
def: "Calculate as: the concatenation of Spatial ID, Genotype ID, and Crop cycle ID, e.g. 1A26_3_1 in ??" []
synonym: "Plant ID" EXACT []
is_a: CO_325:1000020
relationship: variable_of CO_325:0000421 ! plant id
relationship: variable_of CO_325:0010094 ! plant id -counting
relationship: variable_of CO_325:0100040 ! Plant scale

[Term]
id: CO_325:0000423
name: plant barcode
namespace: BananaTrait
def: "The barcode of the plant." []
synonym: "plant_barcode" EXACT []
is_a: CO_325:1000004

[Term]
id: CO_325:0000424
name: PltBrcd
namespace: BananaTrait
def: "The barcode of the plant." []
synonym: "Plant barcode" EXACT []
is_a: CO_325:1000020
relationship: variable_of CO_325:0000423 ! plant barcode
relationship: variable_of CO_325:0010095 ! plant barcode -counting
relationship: variable_of CO_325:0100041 ! Plant barcode scale

[Term]
id: CO_325:0000425
name: pseudostem height
namespace: BananaTrait
def: "Distance from the base of the pseudostem to the emerging point of the peduncle." []
synonym: "Plant height" EXACT []
is_a: CO_325:1000007

[Term]
id: CO_325:0000426
name: PsdHght_E
namespace: BananaTrait
def: "Distance from the base of the pseudostem to the emerging point of the peduncle, with a height score (1 to 3): 1=Less than or equal to 2 m; 2=2.1-2.9 m; 3=Equal to or more than 3 m" []
synonym: "Pseudostem height @ Harvest" EXACT []
is_a: CO_325:1000019
relationship: variable_of CO_325:0000425 ! pseudostem height
relationship: variable_of CO_325:0010096 ! pseudostem height - estimation
relationship: variable_of CO_325:0100042 ! height score (1 to 3)

[Term]
id: CO_325:0000427
name: blotches relative area at petiole base
namespace: BananaTrait
def: "Percentage coverage of petiole base by blotches." []
synonym: "Blotches at the petiole base" EXACT []
is_a: CO_325:1000007

[Term]
id: CO_325:0000428
name: BlotchA_Est_1to4
namespace: BananaTrait
def: "Record the relative surface area coverage by blotches. [x Look at several plants if possible to get an overall idea. Observe at flowering time. In blotch pigmentation scale (1 to 4): 1=No pigmentation; 2=Sparse blotching (<20%); 3=Moderate blotching (20-50%); 4=Extensive pigmentation (>50%)" []
synonym: "Blotches relative area at petiole base @ Shooting, scale (1 to 4)" EXACT []
is_a: CO_325:1000020
relationship: variable_of CO_325:0000427 ! blotches relative area at petiole base
relationship: variable_of CO_325:0010098 ! blotches area - estimation
relationship: variable_of CO_325:0100044 ! blotch pigmentation scale (1 to 4)

[Term]
id: CO_325:0000429
name: BlotchA_Est_1to5
namespace: BananaTrait
def: "Record the relative surface area coverage by blotches. Look at several plants if possible to get an overall idea. Observe at flowering time. In blotch pigmentation scale (1 to 5): Ordinal 1=Sparse blotching; 2=Small blotches; 3=Large blotches; 4=Extensive pigmentation; 5=Without pigmentation" []
synonym: "Blotches relative area at petiole base @ Shooting, scale (1 to 5)" EXACT []
is_a: CO_325:1000020
relationship: variable_of CO_325:0000427 ! blotches relative area at petiole base
relationship: variable_of CO_325:0010098 ! blotches area - estimation
relationship: variable_of CO_325:0100045 ! blotch pigmentation scale (1 to 5)

[Term]
id: CO_325:0000430
name: blotches colour at the petiole base
namespace: BananaTrait
def: "Colour of the blotches on the upper leaf sheath of the petiole base." []
synonym: "Blotches colour" EXACT []
is_a: CO_325:1000007

[Term]
id: CO_325:0000431
name: BlotchCol_Est_1to4
namespace: BananaTrait
def: "Observe visually the colour of the blotches on the upper leaf sheath. In blotch color scale (1 to 4): 1=Orange-brown (mahogany, like in Pisang Mas); 2=Brown; 3=Black-purple; 4=Other" []
synonym: "Blotches colour at the petiole base @ Harvest, scale (1 to 4)" EXACT []
is_a: CO_325:1000020
relationship: variable_of CO_325:0000430 ! blotches colour at the petiole base
relationship: variable_of CO_325:0010099 ! blotches colour - estimation
relationship: variable_of CO_325:0100046 ! blotch color scale (1 to 4)

[Term]
id: CO_325:0000432
name: BlotchCol_Est_1to5
namespace: BananaTrait
def: "Observe visually the colour of the blotches on the upper leaf sheath. In blotch color scale (1 to 5): 1=Brown; 2=Dark brown; 3=Brown-black; 4=Black-purple; 5=Other" []
synonym: "Blotches colour at the petiole base @ Harvest, scale (1 to 5)" EXACT []
is_a: CO_325:1000020
relationship: variable_of CO_325:0000430 ! blotches colour at the petiole base
relationship: variable_of CO_325:0010099 ! blotches colour - estimation
relationship: variable_of CO_325:0100047 ! blotch color scale (1 to 5)

[Term]
id: CO_325:0000433
name: margin behaviour on petiole canal of third leaf
namespace: BananaTrait
def: "Margin behaviour of the petiole canal of the third leaf before bunch." []
synonym: "Petiole canal of the third leaf, Petiole canal leaf III" EXACT []
is_a: CO_325:1000007

[Term]
id: CO_325:0000434
name: MgnBhvPtCnlThrdLf_Est_1to4
namespace: BananaTrait
def: "The third leaf (Leaf III) is counted from the last leaf produced before shooting. Cut the petiole halfway between the pseudostem and the leaf blade and examine the cross section. [x Observe at flowering time]. In margin behaviour scale (1 to 4)  with the following format: Nominal 1=Margins spreading; 2=Margins erect; 3=Margins curved inward; 4=Margins overlapping" []
synonym: "Margin behaviour on petiole canal of third leaf @ Shooting, scale (1 to 4)" EXACT []
is_a: CO_325:1000020
relationship: variable_of CO_325:0000433 ! margin behaviour on petiole canal of third leaf
relationship: variable_of CO_325:0010100 ! margin behaviour on petiole canal of third leaf  - estimation
relationship: variable_of CO_325:0100048 ! margin behaviour scale (1 to 4)

[Term]
id: CO_325:0000435
name: MgnBhvPtCnlThrdLf_Est_1to5
namespace: BananaTrait
def: "The third leaf (Leaf III) is counted from the last leaf produced before shooting. Cut the petiole halfway between the pseudostem and the leaf blade and examine the cross section. [x Observe at flowering time]. In margin behaviour scale (1 to 5)  with the following format: Nominal 1=Open with margins spreading; 2=Wide with erect margins; 3=Straight with erect margins; 4=Margins curved inward; 5=Margins overlapping" []
synonym: "Margin behaviour on petiole canal of third leaf @ Shooting, scale 1 to 5" EXACT []
is_a: CO_325:1000020
relationship: variable_of CO_325:0000433 ! margin behaviour on petiole canal of third leaf
relationship: variable_of CO_325:0010100 ! margin behaviour on petiole canal of third leaf  - estimation
relationship: variable_of CO_325:0100049 ! margin behaviour scale (1 to 5)

[Term]
id: CO_325:0000436
name: PMargWing_Est_1or5
namespace: BananaTrait
def: "Observations on the margins and petiole wings should be made where the petiole and pseudostem meet at shooting. Margin is the part of the petiole that can be bent outwards/inwards. In wing presence/absence and clasping presence/absence scale 1 to 5 with format: Nominal 1=Winged and undulating; 2=Winged and not clasping the pseudostem; 3=Winged and clasping the pseudostem; 4=Not winged and clasping the pseudostem; 5=Not winged and not clasping the pseudostem" []
synonym: "Petiole margins winged @ Shooting, scale 1 to 5" EXACT []
is_a: CO_325:1000020
relationship: variable_of CO_325:0000256 ! petiole margins winged
relationship: variable_of CO_325:0010101 ! winged petiole margin - estimation
relationship: variable_of CO_325:0100051 ! wing presence/absence and clasping presence/absence scale 1 to 5

[Term]
id: CO_325:0000437
name: PMargCol_Esr_1to4
namespace: BananaTrait
def: "Observations on the margins and petiole wings should be made where the petiole and pseudostem meet at shooting. Use colour chart A and observe out of direct sunlight. Record the colour of the margin (general colour is below the rim). in Banana Descriptors colour chart A - 1996. In scale 1to4: 1=Green; 2=Pink-purple to red; 3=Purple to blue; 4=Other" []
synonym: "Petiole margin colour @ Shooting, scale 1 to 4" EXACT []
is_a: CO_325:1000020
relationship: variable_of CO_325:0000264 ! petiole margin colour
relationship: variable_of CO_325:0010103 ! petiole margin colour - estimation
relationship: variable_of CO_325:0100053 ! bd colour chart a - 1996

[Term]
id: CO_325:0000438
name: bunch position
namespace: BananaTrait
def: "Angle between the axis of the bunch and the vertical" []
is_a: CO_325:1000007

[Term]
id: CO_325:0000439
name: BnchPst_Estm_1to5
namespace: BananaTrait
def: "Visually observe the angle of the bunch and choose the option that is most similar, from the 5 schematic drawings of descriptor 6.4.6 in the reference material.In scale 1to5: 1=Hanging vertically; 2=Slightly angled; 3=Hanging at a 45 degree angle; 4=Horizontal; 5=Erect" []
synonym: "Bunch position @ Harvest, scale 1 to 5" EXACT []
is_a: CO_325:1000020
relationship: variable_of CO_325:0000438 ! bunch position
relationship: variable_of CO_325:0010106 ! bunch position - estimation
relationship: variable_of CO_325:0100055 ! bunch position scale(1 to 5)

[Term]
id: CO_325:0000440
name: bunch shape
namespace: BananaTrait
def: "Shape of the fully developed bunch on a plant" []
is_a: CO_325:1000007

[Term]
id: CO_325:0000441
name: BnchShp_Estm_1to5
namespace: BananaTrait
def: "Visually observe the shape of the mature bunch on a fully developed plant that is not experiencing environmental stress and choose the option that is most similar, from the 4 photos of descriptor 6.4.7. in the reference material.In scle 1to5:  Nominal 1=Cylindrical; 2=Truncate (=cone shaped); 3=Asymmetrical; 4=Spiral (all fruit are attached to a unique crown coiled around the stalk); 5=Other" []
synonym: "Bunch shape @ Harvest, scale 1 to 5" EXACT []
is_a: CO_325:1000020
relationship: variable_of CO_325:0000440 ! bunch shape
relationship: variable_of CO_325:0010107 ! bunch shape - estimation
relationship: variable_of CO_325:0100056 ! bunch shape scale (1 to 5)

[Term]
id: CO_325:0000442
name: male rachis type
namespace: BananaTrait
def: "Behaviour of male rachis - truncated or present. Truncated means there is no bract scar below the last hand. Present means there is a degenerated or persistent male bud" []
is_a: CO_325:1000007

[Term]
id: CO_325:0000443
name: MlRchsTp_Estm_1to2
namespace: BananaTrait
def: "Visually observe the part of the rachis between the last hand and the male bud. Truncated means there is no bract scar below the last hand. Present means there is a degenerated or persistent male bud.In scale 1to2: 1=Truncated; 2=Present" []
synonym: "Male rachis type @ Harvest, scale 1 to 2" EXACT []
is_a: CO_325:1000020
relationship: variable_of CO_325:0000442 ! male rachis type
relationship: variable_of CO_325:0010108 ! male rachis type - estimation
relationship: variable_of CO_325:0100057 ! rachis type scale (1 to 2)

[Term]
id: CO_325:0000444
name: male rachis position
namespace: BananaTrait
def: "Angle of the rachis between last hand and male bud" []
synonym: "Rachis angle" EXACT []
is_a: CO_325:1000007

[Term]
id: CO_325:0000445
name: MlRchsPst_Estm_1to5
namespace: BananaTrait
def: "Visually observe the male rachis position (the part between the last hand and the male bud) and choose the option that is most similar, from the 5 schematic drawings of descriptor 6.4.12 in the reference material. In scale 1to5: 1=Falling vertically; 2=At an angle; 3=With a curve; 4=Horizontal or supra-horizontal; 5=Erect" []
synonym: "Male rachis position @ Harvest, scale 1 to 5" EXACT []
is_a: CO_325:1000020
relationship: variable_of CO_325:0000444 ! male rachis position
relationship: variable_of CO_325:0010109 ! male rachis position - estimation
relationship: variable_of CO_325:0100058 ! rachis angle scale (1 to 2)

[Term]
id: CO_325:0000446
name: male rachis appearance
namespace: BananaTrait
def: "Appearance of flowers/bracts on the male rachis" []
synonym: "Rachis appearance" EXACT []
is_a: CO_325:1000007

[Term]
id: CO_325:0000447
name: MlRchsApp_Estm_1to7
namespace: BananaTrait
def: "Visually observe the male rachis appearance and choose the option that is most similar.In scale 1to7: 1=Bare; 2=Nuetral flowers on one to few hands only near the bunch (rest of stalk is bare); 3=Male flowers/bracts above the male bud (rest of stalk is bare); 4=Neutral/male flowers and presence of withered bracts on the entire stalk; 5=Neutral/male flowers on the whole stalk without persistent bracts (still firmly attached to the rachis); 6=Small bunch from neutral/hermaphrodite flowers just above the male bud; 7=Other" []
synonym: "Male rachis appearance @ Harvest, scale 1 to 7" EXACT []
is_a: CO_325:1000020
relationship: variable_of CO_325:0000446 ! male rachis appearance
relationship: variable_of CO_325:0010110 ! male rachis appearance - estimation
relationship: variable_of CO_325:0100059 ! rachis appearance scale (1 to 5)

[Term]
id: CO_325:0000448
name: male bud shape
namespace: BananaTrait
def: "Shape of the male bud defined as the ratio of male bud broadest width to total male bud length" []
is_a: CO_325:1000007

[Term]
id: CO_325:0000449
name: MlBdShp_Comp_1to3
namespace: BananaTrait
def: "Calculate the ratio w/y, i.e. the broadest width of the male bud to the total length of the male bud. Do not measure the dimensions along the bud but rather on a projection/outline of the bud (e.g. trace the outline of the bud on paper) and use ruler or measuring tape. In scale 1to3: 1=Skinny (w/y less than or equal to 0.45); 2=Medium (0.45 < w/y < 0.55); 3=Fat (w/y equal to or more than 0.55)" []
synonym: "Male bud shape @ Harvest, scale 1 to 3" EXACT []
is_a: CO_325:1000020
relationship: variable_of CO_325:0000448 ! male bud shape
relationship: variable_of CO_325:0010111 ! male bud shape - computation
relationship: variable_of CO_325:0100060 ! bud shape scale (1 to 3)

[Term]
id: CO_325:0000450
name: MlBdShp_Comp_1to5
namespace: BananaTrait
def: "Calculate the ratio w/y, i.e. the broadest width of the male bud to the total length of the male bud. Do not measure the dimensions along the bud but rather on a projection/outline of the bud (e.g. trace the outline of the bud on paper) and use ruler or measuring tape. in Scale 1 to 5: 1=Like a top; 2=Lanceolate; 3=Intermediate; 4=Ovoid; 5=Rounded" []
synonym: "Male bud shape @ Harvest, scale 1 to 5" EXACT []
is_a: CO_325:1000020
relationship: variable_of CO_325:0000448 ! male bud shape
relationship: variable_of CO_325:0010111 ! male bud shape - computation
relationship: variable_of CO_325:0100061 ! bud shape scale (1 to 5)

[Term]
id: CO_325:0000451
name: male bud length
namespace: BananaTrait
def: "Length of male bud from end of rachis to apex of the bud" []
synonym: "Male bud size" EXACT []
is_a: CO_325:1000007

[Term]
id: CO_325:0000452
name: MlBdLngth_M_1to3
namespace: BananaTrait
def: "Measure the length (y) of a projection/outline of the male bud on paper, with a measuring tape or ruler.In scale1to3: 1=Short (y less than or equal to 20 cm); 2=Medium (20 cm < y < 30 cm); 3=Long (equal to or more than 30 cm)" []
synonym: "Male bud length @ Harvest, scale 1 to 3" EXACT []
is_a: CO_325:1000020
relationship: variable_of CO_325:0000451 ! male bud length
relationship: variable_of CO_325:0010112 ! male bud length - measurement
relationship: variable_of CO_325:0100062 ! bud length scale (1 to 3)

[Term]
id: CO_325:0000453
name: MlBdLngthRt_M_1to3
namespace: BananaTrait
def: "Length and maximum diameter of male bud at harvest. scale 1 to 3: 1=Less than or equal to 20 cm; 2=21-30 cm; 3=Equal to or more than 31 cm" []
synonym: "Male bud length and diameter @ Harvest, scale 1 to 3" EXACT []
is_a: CO_325:1000020
relationship: variable_of CO_325:0000451 ! male bud length
relationship: variable_of CO_325:0010113 ! male bud size - measurement
relationship: variable_of CO_325:0100063 ! bud size scale (1 to 3)

[Term]
id: CO_325:0000454
name: male bud shoulder
namespace: BananaTrait
def: "Male bud shoulder description" []
synonym: "Male bud size" EXACT []
is_a: CO_325:1000007

[Term]
id: CO_325:0000455
name: MlBdShd_Comp_1to3
namespace: BananaTrait
def: "Calculate the ratio w/y, i.e. the broadest width of the male bud to the total length of the male bud. Do not measure the dimensions along the bud but rather on a projection/outline of the bud (e.g. trace the outline of the bud on paper) and use ruler or measuring tape in scale 1to3 :1=High shouldered (x/y less than or equal to 0.28); 2=Medium shouldered (0.28 < x/y < 0.30); 3=Low shouldered (x/y more than or equal to 0.30)" []
synonym: "Male bud shoulder @ Harvest, scale 1 to 3" EXACT []
is_a: CO_325:1000020
relationship: variable_of CO_325:0000454 ! male bud shoulder
relationship: variable_of CO_325:0010114 ! male bud shoulder - computation
relationship: variable_of CO_325:0100064 ! bud shoulder scale (1 to 3)

[Term]
id: CO_325:0000456
name: bract apex shape
namespace: BananaTrait
def: "Appearance of flowers/bracts on the male rachis" []
is_a: CO_325:1000007

[Term]
id: CO_325:0000457
name: FstBrctApxShp_Est_1to4
namespace: BananaTrait
def: "Refers to the first external unlifted bract. Visually observe the apex shape of flattened bracts to determine shape and choose the option that is most similar, from the 4 photos of descriptor 6.5.2. in the reference material. In scale 1to4: 1=Pointed; 2=Intermeditae; 3=Obtuse; 4=Obtuse and split" []
synonym: "Bract apex shape @ Harvest, scale 1 to 4" EXACT []
is_a: CO_325:1000020
relationship: variable_of CO_325:0000456 ! bract apex shape
relationship: variable_of CO_325:0010115 ! bract apex shape - estimation
relationship: variable_of CO_325:0100065 ! bract apex scale (1 to 4)

[Term]
id: CO_325:0000458
name: BrctApxShp_Est_1to5
namespace: BananaTrait
def: "Refers to the first external unlifted bract. Visually observe the apex shape of flattened bracts to determine shape and choose the option that is most similar, from the 4 photos of descriptor 6.5.2. in the reference material. In scale 1to5: 1=Pointed; 2=Slightly pointed; 3=Intermediate; 4=Obtuse; 5=Obtuse and split" []
synonym: "Bract apex shape @ Harvest, scale 1 to 5" EXACT []
is_a: CO_325:1000020
relationship: variable_of CO_325:0000456 ! bract apex shape
relationship: variable_of CO_325:0010115 ! bract apex shape - estimation
relationship: variable_of CO_325:0100066 ! bract apex scale (1 to 5)

[Term]
id: CO_325:0000459
name: bract imbrication at apex of male bud
namespace: BananaTrait
def: "Alignment of bracts at the apex of the male bud" []
synonym: "Bract imbrication" EXACT []
is_a: CO_325:1000007

[Term]
id: CO_325:0000460
name: BrctImbrcApxMlBd_Est_1to3
namespace: BananaTrait
def: "Visually observe the bract imbrication of the apex of the male bud and choose the option that is most similar, from the 3 photos of descriptor 6.5.3 in the reference material.In scale 1to3: 1=Convolute; 2=Moderately imbricate; 3=Highly imbricate" []
synonym: "Bract imbrication at apex of male bud @ Harvest, scale 1 to 3" EXACT []
is_a: CO_325:1000020
relationship: variable_of CO_325:0000459 ! bract imbrication at apex of male bud
relationship: variable_of CO_325:0010116 ! bract imbrication at apex of male bud - estimation
relationship: variable_of CO_325:0100067 ! bract imbrication scale (1 to 3)

[Term]
id: CO_325:0000461
name: bract behaviour before falling
namespace: BananaTrait
def: "Behaviour of the last lifted bract - revolute or not revolute" []
is_a: CO_325:1000007

[Term]
id: CO_325:0000462
name: BrctBhvBfFll_Est_1to2
namespace: BananaTrait
def: "Visually observe the last bract to lift from the hands, ideally when the bract has lifted to a horizontal position, and choose the option that is most similar, from the 2 photos of descriptpr 6.5.12 in the reference material.In scale 1to2: 1=Revolute (rolling); 2=Not revolute (not rolling)" []
synonym: "Bract behaviour before falling @ Harvest, scale 1 to 2" EXACT []
is_a: CO_325:1000020
relationship: variable_of CO_325:0000461 ! bract behaviour before falling
relationship: variable_of CO_325:0010117 ! bract behaviour before falling - estimation
relationship: variable_of CO_325:0100068 ! bract behaviour scale (1 to 2)

[Term]
id: CO_325:0000463
name: colour of bract external face
namespace: BananaTrait
def: "Main colour of the first external unlifted bract external face" []
synonym: "Colour of the bract external face" EXACT []
is_a: CO_325:1000007

[Term]
id: CO_325:0000464
name: BrctClExtFc_Est_1to16
namespace: BananaTrait
def: "Visually observe the colour of the external face of the first unlifted bract. Use colour chart A and observe out of direct sunlight. in BD colour chart A - 2016. In scale 1to16: 1=Cream; 2=Yellow; 3=Watery green; 4=Green yellow; 5=Light green; 6=Medium green; 7=Green; 8=Dark green; 9=Whitish; 10=Orange red; 11=Red; 12=Pink-purple; 13=Purple-brown; 14=Red-purple; 15=Purple; 16=Blue" []
synonym: "Colour of bract external face @ Harvest, scale 1 to 16" EXACT []
is_a: CO_325:1000020
relationship: variable_of CO_325:0000463 ! colour of bract external face
relationship: variable_of CO_325:0010118 ! colour of bract external face - estimation
relationship: variable_of CO_325:0100043 ! bd colour chart a - 2016

[Term]
id: CO_325:0000465
name: BrctClExtFc_Est_1to10
namespace: BananaTrait
def: "Visually observe the colour of the external face of the first unlifted bract. Use colour chart A and observe out of direct sunlight. in BD colour chart A - 1996. In  scale 1to10: : 1=Yellow; 2=Green; 3=Red; 4=Red-purple; 5=Purple-brown; 6=Purple; 7=Blue; 8=Pink-purple; 9=Orange-red; 10=Other" []
synonym: "Colour of bract external face @ Harvest, scale 1 to 10" EXACT []
is_a: CO_325:1000020
relationship: variable_of CO_325:0000463 ! colour of bract external face
relationship: variable_of CO_325:0010118 ! colour of bract external face - estimation
relationship: variable_of CO_325:0100053 ! bd colour chart a - 1996

[Term]
id: CO_325:0000466
name: colour of bract internal face
namespace: BananaTrait
def: "Main colour of the first external unlifted bract internal face" []
synonym: "Colour of the bract internal face" EXACT []
is_a: CO_325:1000007

[Term]
id: CO_325:0000467
name: BrctClExtFc_Int_1to16
namespace: BananaTrait
def: "Visually observe the colour of the internal face of the first unlifted bract. Use colour chart A and observe out of direct sunlight. in BD colour chart A - 2016. In scale 1to16: 1=Cream; 2=Yellow; 3=Watery green; 4=Green yellow; 5=Light green; 6=Medium green; 7=Green; 8=Dark green; 9=Whitish; 10=Orange red; 11=Red; 12=Pink-purple; 13=Purple-brown; 14=Red-purple; 15=Purple; 16=Blue" []
synonym: "Colour of bract internal face @ Harvest, scale 1 to 16" EXACT []
is_a: CO_325:1000020
relationship: variable_of CO_325:0000466 ! colour of bract internal face
relationship: variable_of CO_325:0010119 ! colour of bract internal face - estimation
relationship: variable_of CO_325:0100043 ! bd colour chart a - 2016

[Term]
id: CO_325:0000468
name: BrctClExtFc_Int_1to8
namespace: BananaTrait
def: "Visually observe the colour of the internal face of the first unlifted bract. Use colour chart A and observe out of direct sunlight. in BD colour chart A - 1996. In scale 1to8:  1=Whitish; 2=Yellow or green; 3=Orange red; 4=Red; 5=Purple; 6=Purple brown; 7=Pink-purple; 8=Other" []
synonym: "Colour of bract internal face @ Harvest, scale 1 to 8" EXACT []
is_a: CO_325:1000020
relationship: variable_of CO_325:0000466 ! colour of bract internal face
relationship: variable_of CO_325:0010119 ! colour of bract internal face - estimation
relationship: variable_of CO_325:0100053 ! bd colour chart a - 1996

[Term]
id: CO_325:0000469
name: compound tepal main colour
namespace: BananaTrait
def: "Main colour of the backside of the compound tepal" []
synonym: "Tepal colour, Compound tepal basic colour" EXACT []
is_a: CO_325:1000007

[Term]
id: CO_325:0000470
name: CmpdTplMnCl_Est_1to16
namespace: BananaTrait
def: "The following flower descriptors refer to the flowers at the axil of the first external unlifted bract. Fresh material must be used (make the observation as soon as you detach the bract/flower from the rachis). Visually observe the colour of the backside middle of tepal. Use colour chart B and observe out of direct sunlight. in BD colour chart B - 2016 In scale 1to16: 1=White; 2=Cream; 3=Ivory; 4=Yellow; 5=Bright yellow; 6=Orange; 7=Orange red; 8=Red; 9=Red-purple; 10=Pink/pink-purple; 11=Brown/Rusty-brown; 12=Beige-pink; 13=Silvery; 14=Light green; 15=Green; 16=Dark green" []
synonym: "Compound tepal main colour @ Shooting, scale 1 to 16" EXACT []
is_a: CO_325:1000020
relationship: variable_of CO_325:0000469 ! compound tepal main colour
relationship: variable_of CO_325:0010120 ! compound tepal main colour - estimation
relationship: variable_of CO_325:0100069 ! bd colour chart b - 2016

[Term]
id: CO_325:0000471
name: CmpdTplMnCl_Est_1to6
namespace: BananaTrait
def: "The following flower descriptors refer to the flowers at the axil of the first external unlifted bract. Fresh material must be used (make the observation as soon as you detach the bract/flower from the rachis). Visually observe the colour of the backside middle of tepal. Use colour chart B and observe out of direct sunlight. in BD colour chart B - 1996 In scale 1to6: Nominal 1=White; 2=Cream; 3=Yellow; 4=Orange; 5=Pink/pink-purple; 6=Other" []
synonym: "Compound tepal main colour @ Shooting, scale 1 to 6" EXACT []
is_a: CO_325:1000020
relationship: variable_of CO_325:0000469 ! compound tepal main colour
relationship: variable_of CO_325:0010120 ! compound tepal main colour - estimation
relationship: variable_of CO_325:0100070 ! bd colour chart b - 1996

[Term]
id: CO_325:0000472
name: lobe colour of tip of compound tepal
namespace: BananaTrait
def: "Main colour of the tip of the compound tepal (lobe)" []
synonym: "Lobe colour, Lobe colour of compound tepal" EXACT []
is_a: CO_325:1000007

[Term]
id: CO_325:0000473
name: CmpdTplLbCl_Est_1to16
namespace: BananaTrait
def: "The following flower descriptors refer to the flowers at the axil of the first external unlifted bract. Fresh material must be used (make the observation as soon as you detach the bract/flower from the rachis). Visually observe the colour of the lobe at the tip of the tepal. Use colour chart B and observe out of direct sunlight. in BD colour chart B - 2016. In scale 1to16: Nominal 1=White; 2=Cream; 3=Ivory; 4=Yellow; 5=Bright yellow; 6=Orange; 7=Orange red; 8=Red; 9=Red-purple; 10=Pink/pink-purple; 11=Brown/Rusty-brown; 12=Beige-pink; 13=Silvery; 14=Light green; 15=Green; 16=Dark green" []
synonym: "Lobe colour of tip of compound tepal @ Shooting, scale 1 to 16" EXACT []
is_a: CO_325:1000020
relationship: variable_of CO_325:0000472 ! lobe colour of tip of compound tepal
relationship: variable_of CO_325:0010121 ! lobe colour of tip of compound tepal - estimation
relationship: variable_of CO_325:0100069 ! bd colour chart b - 2016

[Term]
id: CO_325:0000474
name: CmpdTplLbCl_Est_1to5
namespace: BananaTrait
def: "The following flower descriptors refer to the flowers at the axil of the first external unlifted bract. Fresh material must be used (make the observation as soon as you detach the bract/flower from the rachis). Visually observe the colour of the lobe at the tip of the tepal. Use colour chart B and observe out of direct sunlight. in BD colour chart B - 1996. In scale 1to5: Nominal 1=Cream; 2=Yellow; 3=Orange; 4=Green; 5=Other" []
synonym: "Lobe colour of tip of compound tepal @ Shooting, scale 1 to 5" EXACT []
is_a: CO_325:1000020
relationship: variable_of CO_325:0000472 ! lobe colour of tip of compound tepal
relationship: variable_of CO_325:0010121 ! lobe colour of tip of compound tepal - estimation
relationship: variable_of CO_325:0100070 ! bd colour chart b - 1996

[Term]
id: CO_325:0000475
name: anther colour
namespace: BananaTrait
def: "Main colour of the face of anther opposite to dehiscence" []
is_a: CO_325:1000007

[Term]
id: CO_325:0000476
name: AnthrCl_Est_1to16
namespace: BananaTrait
def: "The following flower descriptors refer to the flowers at the axil of the first external unlifted bract. Fresh material must be used (make the observation as soon as you detach the bract/flower from the rachis). Visually observe the anther colour on the face opposite to the dehiscence split of the anther. Use colour chart B and observe out of direct sunlight. in BD colour chart B - 2016 In scale 1to16: Nominal 1=White; 2=Cream; 3=Ivory; 4=Yellow; 5=Bright yellow; 6=Orange; 7=Orange red; 8=Red; 9=Red-purple; 10=Pink/pink-purple; 11=Brown/Rusty-brown; 12=Beige-pink; 13=Silvery; 14=Light green; 15=Green; 16=Dark green" []
synonym: "Anther colour @ Shooting, scale 1 to 16" EXACT []
is_a: CO_325:1000020
relationship: variable_of CO_325:0000475 ! anther colour
relationship: variable_of CO_325:0010122 ! anther colour - estimation
relationship: variable_of CO_325:0100069 ! bd colour chart b - 2016

[Term]
id: CO_325:0000477
name: AnthrCl_Est_1to8
namespace: BananaTrait
def: "The following flower descriptors refer to the flowers at the axil of the first external unlifted bract. Fresh material must be used (make the observation as soon as you detach the bract/flower from the rachis). Visually observe the anther colour on the face opposite to the dehiscence split of the anther. Use colour chart B and observe out of direct sunlight. in BD colour chart B - 1996. In scale 1to8:: 1=White; 2=Cream; 3=Yellow; 4=Grey; 5=Brown/rusty brown; 6=Pink/pink-purple; 7=Black (anthers aborted); 8=Other" []
synonym: "Anther colour @ Shooting, scale 1 to 8" EXACT []
is_a: CO_325:1000020
relationship: variable_of CO_325:0000475 ! anther colour
relationship: variable_of CO_325:0010122 ! anther colour - estimation
relationship: variable_of CO_325:0100070 ! bd colour chart b - 1996

[Term]
id: CO_325:0000478
name: number of hands on whole bunch
namespace: BananaTrait
def: "Number of hands on bunch **subsume" []
synonym: "Number of hands" EXACT []
is_a: CO_325:1000007

[Term]
id: CO_325:0000479
name: HndNbWhlBnch_Ct_hands
namespace: BananaTrait
def: "On a bunch with mostly hands of > 10 fingers, a possible ultimate hand with 1-5 (rather smaller) fingers should not be counted." []
synonym: "Number of hands on whole bunch @ Harvest" EXACT []
is_a: CO_325:1000020
relationship: variable_of CO_325:0000478 ! number of hands on whole bunch
relationship: variable_of CO_325:0010123 ! number of hands on whole bunch - counting
relationship: variable_of CO_325:0100071 ! hands

[Term]
id: CO_325:0000480
name: number of fruits on mid-hand of the bunch
namespace: BananaTrait
def: "Number of fruits on the mid-hand of the bunch **subsume" []
synonym: "Number of fruits" EXACT []
is_a: CO_325:1000007

[Term]
id: CO_325:0000481
name: FrtNbMdHndBnch_Ct_ft
namespace: BananaTrait
def: "Count only fully developed fruit. If there is an even number of hands, there will be two middle hands. Count the middle hand that developed first. In scale 1to3: 1=Less than or equal to 12; 2=13-16; 3=Equal to or more than 17" []
synonym: "Number of fruits on mid-hand of the bunch @ Harvest" EXACT []
is_a: CO_325:1000020
relationship: variable_of CO_325:0000480 ! number of fruits on mid-hand of the bunch
relationship: variable_of CO_325:0010124 ! number of fruits on mid-hand of the bunch - counting
relationship: variable_of CO_325:0100013 ! finger

[Term]
id: CO_325:0000482
name: fruit length
namespace: BananaTrait
def: "Length of the internal arc of a finger ** subsume" []
synonym: "Fruit length" EXACT []
is_a: CO_325:1000007

[Term]
id: CO_325:0000483
name: FrtLngth_M_cm
namespace: BananaTrait
def: "Measure the length of the internal arc of a fruit, without pedicel in centimeters. Record on the inner fruit in the middle of the mid-hand of the bunch. If there is an even number of hands, there will be two middle hands so use the upper hand that developed first. Record the exact value." []
synonym: "Fruit length @ Harvest, in cm" EXACT []
is_a: CO_325:1000020
relationship: variable_of CO_325:0000482 ! fruit length
relationship: variable_of CO_325:0010125 ! fruit length - exact value - measurement
relationship: variable_of CO_325:0100004 ! cm

[Term]
id: CO_325:0000484
name: FrtLngth_M_1to5
namespace: BananaTrait
def: "Measure the length of the internal arc of a fruit, without pedicel. Record on the inner fruit in the middle of the mid-hand of the bunch. If there is an even number of hands, there will be two middle hands so use the upper hand that developed first. In scale 1to5:  1=Less than or equal to 15 cm; 2=16-20 cm; 3=21-25 cm; 4=26-30 cm; 5=Equal to or more than 31 cm" []
synonym: "Fruit length @ Harvest, scale 1 to 5" EXACT []
is_a: CO_325:1000020
relationship: variable_of CO_325:0000482 ! fruit length
relationship: variable_of CO_325:0010126 ! fruit length - range - measurement
relationship: variable_of CO_325:0100072 ! fruit length scale (1 to 5)

[Term]
id: CO_325:0000485
name: fruit shape of curve
namespace: BananaTrait
def: "Shape of a fruit (finger) in the middle of the bunch **subsume" []
synonym: "Fruit shape (longitudinal curve)" EXACT []
is_a: CO_325:1000007

[Term]
id: CO_325:0000486
name: FrtCvShp_Est_1to6
namespace: BananaTrait
def: "Visually observe the shape of the curve of the fruit and choose the option that is most similar, from the 5 photos of descriptor 6.7.4. in the reference material. Observe the inner fruit in the middle of the mid-hand of the bunch. In case of an asymmetric bunch that has straight and curved fruits, please indicate it in the note section and score only the fruit on the upper side of the bunch. In scale 1to6: 1=Straight; 2=Slightly curved; 3=Straight in the distal part; 4=Curved (sharp curve); 5=Curved in slight 'S' shape (double curvature); 6=Other" []
synonym: "Fruit shape of curve @ Harvest, scale 1 to 6" EXACT []
is_a: CO_325:1000020
relationship: variable_of CO_325:0000485 ! fruit shape of curve
relationship: variable_of CO_325:0010127 ! fruit shape of curve - estimation
relationship: variable_of CO_325:0100073 ! fruit curve shape (scale 1 to 6)

[Term]
id: CO_325:0000487
name: FrtCvShp_Est_1to5
namespace: BananaTrait
def: "Visually observe the shape of the curve of the fruit and choose the option that is most similar, from the 5 photos of descriptor 6.7.4. in the reference material. Observe the inner fruit in the middle of the mid-hand of the bunch. In case of an asymmetric bunch that has straight and curved fruits, please indicate it in the note section and score only the fruit on the upper side of the bunch. In scale 1to5: 1=Straight (or slightly curved); 2=Straight in the distal part; 3=Curved (sharp curve); 4=Curved in 'S' shape (double curvature); 5=Other" []
synonym: "Fruit shape of curve @ Harvest, scale 1 to 5" EXACT []
is_a: CO_325:1000020
relationship: variable_of CO_325:0000485 ! fruit shape of curve
relationship: variable_of CO_325:0010127 ! fruit shape of curve - estimation
relationship: variable_of CO_325:0100074 ! fruit curve shape (scale 1 to 5)

[Term]
id: CO_325:0000488
name: fruit apex point
namespace: BananaTrait
def: "Description of fruit apex" []
synonym: "Fruit apex" EXACT []
is_a: CO_325:1000007

[Term]
id: CO_325:0000489
name: FrtApxPt_Est_1to5
namespace: BananaTrait
def: "Visually observe the fruit apex point and choose the option that is most similar, from the 5 photos of descriptor 6.7.6 in the reference material. In scale 1to5: 1=Pointed; 2=Lengthily pointed (like plantain); 3=Blunt-tipped (plateau at tip); 4=Strongly bottle-necked (wider under tip than number 2); 5=Rounded" []
synonym: "Fruit apex point @ Harvest" EXACT []
is_a: CO_325:1000020
relationship: variable_of CO_325:0000488 ! fruit apex point
relationship: variable_of CO_325:0010128 ! fruit apex point - estimation
relationship: variable_of CO_325:0100075 ! fruit apex scale (1 to 5)

[Term]
id: CO_325:0000490
name: remains of flower relicts at fruit apex
namespace: BananaTrait
def: "Percentage of flower relicts at fruit apex" []
is_a: CO_325:1000007

[Term]
id: CO_325:0000491
name: FrtApxFlwRlt_Est_1to4
namespace: BananaTrait
def: "Visually observe the remains, or not, of flower relicts at the finger apex, and choose the option that is most similar, from the 4 photos of descriptor 6.7.7 in the reference materials. In scale 1to4:1=Without flower relicts; 2=Few flower relicts (< 20% of the fruits with relicts); 3=Persistent flower relicts (> 20% of the fruits with relicts); 4=Only base of the style persists" []
synonym: "Remains of flower relicts at fruit apex @ Harvest, scale 1 to 4" EXACT []
is_a: CO_325:1000020
relationship: variable_of CO_325:0000490 ! remains of flower relicts at fruit apex
relationship: variable_of CO_325:0010129 ! remains of flower relicts at fruit apex - estimation
relationship: variable_of CO_325:0100076 ! fruit relicts scale (1 to 4)

[Term]
id: CO_325:0000492
name: FrtApxFlwRlt_Est_1to3
namespace: BananaTrait
def: "Visually observe the remains, or not, of flower relicts at the finger apex, and choose the option that is most similar, from the 4 photos of descriptor 6.7.7 in the reference materials. In scale 1to3: 1=Without any floral relicts; 2=Persistent style; 3=Base of the style prominent" []
synonym: "Remains of flower relicts at fruit apex @ Harvest, scale 1 to 3" EXACT []
is_a: CO_325:1000020
relationship: variable_of CO_325:0000490 ! remains of flower relicts at fruit apex
relationship: variable_of CO_325:0010129 ! remains of flower relicts at fruit apex - estimation
relationship: variable_of CO_325:0100077 ! fruit relicts scale (1 to 3)

[Term]
id: CO_325:0000493
name: fruit pedicel length
namespace: BananaTrait
def: "Length of the fruit pedicel from rachis to the beginning of the pulp" []
is_a: CO_325:1000007

[Term]
id: CO_325:0000494
name: FrtftPdclLgth_M_mm
namespace: BananaTrait
def: "Measure from the scar on the rachis until the beginning of the fruit. Record on the inner fruit in the middle of the mid-hand of the bunch. Tip: use string to measure or trace outline of fruit on paper. Record the exact value in millimeters." []
synonym: "Fruit pedicel length @ Harvest, in mm" EXACT []
is_a: CO_325:1000020
relationship: variable_of CO_325:0000493 ! fruit pedicel length
relationship: variable_of CO_325:0010130 ! fruit pedicel length - exact value - measurement
relationship: variable_of CO_325:0100016 ! mm

[Term]
id: CO_325:0000495
name: FrtftPdclLgth_Est_1to3
namespace: BananaTrait
def: "Measure from the scar on the rachis until the beginning of the fruit in millimeters. Record on the inner fruit in the middle of the mid-hand of the bunch. Tip: use string to measure or trace outline of fruit on paper. Record the range in scale 1to3: Ordinal 1=Less than or equal to 10 mm; 2=11-20 mm; 3=Equal to or more than 21 mm" []
synonym: "Fruit pedicel length @ Harvest, scale 1 to 3" EXACT []
is_a: CO_325:1000020
relationship: variable_of CO_325:0000493 ! fruit pedicel length
relationship: variable_of CO_325:0010131 ! fruit pedical length - range - measurement
relationship: variable_of CO_325:0100078 ! fruit pedicel scale (1 to 3)

[Term]
id: CO_325:0000496
name: fusion of pedicels
namespace: BananaTrait
def: "Degree of fusion of the pedicels before they join the rachis" []
is_a: CO_325:1000007

[Term]
id: CO_325:0000497
name: PdcFsn_Est_1to2
namespace: BananaTrait
def: "Visually observe the fusion of pedicels and choose the option that is most similar, from the 3 photos of descriptor 6.7.11. in the reference materials. Observe before they join the rachis at the bract scar. Look upwards from the bottom of the bunch. In scale 1to2: 1=No visible sign of fusion; 2=Partially fused 9up to 50% of the length of the pedicel); Totally fused (more than 50% of the length of the pedicel)" []
synonym: "Fusion of pedicels  @ Harvest" EXACT []
is_a: CO_325:1000020
relationship: variable_of CO_325:0000496 ! fusion of pedicels
relationship: variable_of CO_325:0010132 ! fusion of pedicels - estimation
relationship: variable_of CO_325:0100079 ! fusion of pedicel scale (1 to 2)

[Term]
id: CO_325:0000498
name: fruit  smashed pulp colour
namespace: BananaTrait
def: "The color of the smashed pulp of a mature fruit" []
is_a: CO_325:1000003

[Term]
id: CO_325:0000499
name: FngSmshdPlpCl_Est_1to5
namespace: BananaTrait
def: "Subjective visual assessment of smashed and unsmashed fruit pulp in 1 to 5 acceptability score: 1 = Dislike very much; 2= Dislike; 3= Like fairly; 4= Like very much; 5 = Like extremely" []
synonym: "Fruit smashed pulp colour @ Post-harvest" EXACT []
is_a: CO_325:1000020
relationship: variable_of CO_325:0000498 ! fruit  smashed pulp colour
relationship: variable_of CO_325:0010133 ! visual appearance  - estimation
relationship: variable_of CO_325:0100080 ! 1 to 5 acceptability score

[Term]
id: CO_325:0000500
name: fruit  unsmashed pulp colour
namespace: BananaTrait
def: "The color of the unsmashed pulp of a mature  fruit" []
is_a: CO_325:1000003

[Term]
id: CO_325:0000501
name: FngUnSmshdPlpCl_Est_1to5
namespace: BananaTrait
def: "Subjective visual assessment of smashed and unsmashed fruit pulp in 1 to 5 acceptability score: 1 = Dislike very much; 2= Dislike; 3= Like fairly; 4= Like very much; 5 = Like extremely" []
synonym: "Fruit  unsmashed pulp colour @ Post-harvest" EXACT []
is_a: CO_325:1000020
relationship: variable_of CO_325:0000500 ! fruit  unsmashed pulp colour
relationship: variable_of CO_325:0010133 ! visual appearance  - estimation
relationship: variable_of CO_325:0100080 ! 1 to 5 acceptability score

[Term]
id: CO_325:0000502
name: fruit  smashed pulp taste
namespace: BananaTrait
def: "The taste of the smashed pulp of a mature  fruit" []
is_a: CO_325:1000003

[Term]
id: CO_325:0000503
name: FngSmshdPlpTst_Est_1to5
namespace: BananaTrait
def: "Subjective taste assessment of smashed and unsmashed fruit pulp in 1 to 5 acceptability score: 1 = Dislike very much; 2= Dislike; 3= Like fairly; 4= Like very much; 5 = Like extremely" []
synonym: "Fruit smashed pulp taste @ Post-harvest" EXACT []
is_a: CO_325:1000020
relationship: variable_of CO_325:0000502 ! fruit  smashed pulp taste
relationship: variable_of CO_325:0010134 ! taste  - estimation
relationship: variable_of CO_325:0100080 ! 1 to 5 acceptability score

[Term]
id: CO_325:0000504
name: fruit unsmashed pulp taste
namespace: BananaTrait
def: "The taste of the unsmashed pulp of a mature  fruit" []
is_a: CO_325:1000003

[Term]
id: CO_325:0000505
name: FngUnSmshdPlpTst_Est_1to5
namespace: BananaTrait
def: "Subjective taste assessment of smashed and unsmashed fruit pulp in 1 to 5 acceptability score: 1 = Dislike very much; 2= Dislike; 3= Like fairly; 4= Like very much; 5 = Like extremely" []
synonym: "Fruit  unsmashed pulp taste @ Post-harvest" EXACT []
is_a: CO_325:1000020
relationship: variable_of CO_325:0000504 ! fruit unsmashed pulp taste
relationship: variable_of CO_325:0010134 ! taste  - estimation
relationship: variable_of CO_325:0100080 ! 1 to 5 acceptability score

[Term]
id: CO_325:0000506
name: fruit  smashed pulp texture
namespace: BananaTrait
def: "The texture of the smashed pulp of a mature  fruit" []
is_a: CO_325:1000003

[Term]
id: CO_325:0000507
name: FngSmshdPlpTxt_Est_1to5
namespace: BananaTrait
def: "Finger feel assessment of smashed and unsmashed fruit pulp in 1 to 5 acceptability score: 1 = Dislike very much; 2= Dislike; 3= Like fairly; 4= Like very much; 5 = Like extremely" []
synonym: "Fruit  smashed pulp texture @ Post-harvest" EXACT []
is_a: CO_325:1000020
relationship: variable_of CO_325:0000506 ! fruit  smashed pulp texture
relationship: variable_of CO_325:0010135 ! finger feel  - estimation
relationship: variable_of CO_325:0100080 ! 1 to 5 acceptability score

[Term]
id: CO_325:0000508
name: fruit  unsmashed pulp texture
namespace: BananaTrait
def: "The texture of the unsmashed pulp  of a mature fruit" []
is_a: CO_325:1000003

[Term]
id: CO_325:0000509
name: FngUnSmshdPlpTxt_Est_1to5
namespace: BananaTrait
def: "Finger feel assessment of smashed and unsmashed fruit pulp in 1 to 5 acceptability score:1 = Dislike very much; 2= Dislike; 3= Like fairly; 4= Like very much; 5 = Like extremely" []
synonym: "Fruit  unsmashed pulp texture @ Post-harvest" EXACT []
is_a: CO_325:1000020
relationship: variable_of CO_325:0000508 ! fruit  unsmashed pulp texture
relationship: variable_of CO_325:0010135 ! finger feel  - estimation
relationship: variable_of CO_325:0100080 ! 1 to 5 acceptability score

[Term]
id: CO_325:0000510
name: fruit   smashed pulp smoothness-mouth feel
namespace: BananaTrait
def: "The smoothness-mouth feel of the smashed pulp  of a mature  fruit" []
is_a: CO_325:1000003

[Term]
id: CO_325:0000511
name: FngSmshdPlpSmth_Est_1to5
namespace: BananaTrait
def: "Mouth feel assessment of smashed and unsmashed fruit pulp in 1 to 5 acceptability score: 1 = Dislike very much; 2= Dislike; 3= Like fairly; 4= Like very much; 5 = Like extremely" []
synonym: "Fruit   smashed pulp smoothness-mouth feel @ Post-harvest" EXACT []
is_a: CO_325:1000020
relationship: variable_of CO_325:0000510 ! fruit   smashed pulp smoothness-mouth feel
relationship: variable_of CO_325:0010136 ! smoothness-mouth feel - estimation
relationship: variable_of CO_325:0100080 ! 1 to 5 acceptability score

[Term]
id: CO_325:0000512
name: fruit   unsmashed pulp smoothness-mouth feel
namespace: BananaTrait
def: "The smoothness-mouth feel of the unsmashed pulp of a mature  fruit" []
is_a: CO_325:1000003

[Term]
id: CO_325:0000513
name: FngUnSmshdPlpSmth_Est_1to5
namespace: BananaTrait
def: "Mouth feel assessment of smashed and unsmashed fruit pulp in 1 to 5 acceptability score: Dislike very much; 2= Dislike; 3= Like fairly; 4= Like very much; 5 = Like extremely" []
synonym: "Fruit   unsmashed pulp smoothness-mouth feel @ Post-harvest" EXACT []
is_a: CO_325:1000020
relationship: variable_of CO_325:0000512 ! fruit   unsmashed pulp smoothness-mouth feel
relationship: variable_of CO_325:0010136 ! smoothness-mouth feel - estimation
relationship: variable_of CO_325:0100080 ! 1 to 5 acceptability score

[Term]
id: CO_325:0000514
name: fruit smashed pulp aroma/smell
namespace: BananaTrait
def: "The pulp aroma  of the smashed pulp of a mature fruit" []
is_a: CO_325:1000003

[Term]
id: CO_325:0000515
name: FngSmshdPlpArm_Est_1to5
namespace: BananaTrait
def: "Nosal smell assessment of smashed and unsmashed fruit pulp aromas in 1 to 5 acceptability score: 1 = Dislike very much; 2= Dislike; 3= Like fairly; 4= Like very much; 5 = Like extremely" []
synonym: "Fruit  smashed pulp aroma/smell @ Post-harvest" EXACT []
is_a: CO_325:1000020
relationship: variable_of CO_325:0000514 ! fruit smashed pulp aroma/smell
relationship: variable_of CO_325:0010137 ! nosal smell  - estimation
relationship: variable_of CO_325:0100080 ! 1 to 5 acceptability score

[Term]
id: CO_325:0000516
name: percentage damage to periphery of peeled corm caused by weevils
namespace: BananaTrait
def: "The percentage of damage to the periphery of the peeled corm, assessed by tunnels caused by weevils" []
synonym: "peripheral damage" EXACT []
is_a: CO_325:1000001

[Term]
id: CO_325:0000517
name: DmgPrphl_M_%
namespace: BananaTrait
def: "Visual observation in %" []
synonym: "Percentage damage to periphery of peeled corm caused by weevils @ Harvest" EXACT []
is_a: CO_325:1000020
relationship: variable_of CO_325:0000516 ! percentage damage to periphery of peeled corm caused by weevils
relationship: variable_of CO_325:0010138 ! peripheral damage - measurement
relationship: variable_of CO_325:0100081 ! %

[Term]
id: CO_325:0000518
name: nematode reproduction factor (microplot screening)
namespace: BananaTrait
def: "Nematode multiplication from single root inoculation of 50 nematodes per 8 cm length after 12 weeks" []
is_a: CO_325:1000001

[Term]
id: CO_325:0000519
name: NmRpFctr_Ct_Nema
namespace: BananaTrait
def: "calculation from count  in multiplication factor" []
synonym: "Nematode reproduction factor (microplot screening) multiplication factor Numerical" EXACT []
is_a: CO_325:1000020
relationship: variable_of CO_325:0000518 ! nematode reproduction factor (microplot screening)
relationship: variable_of CO_325:0010139 ! nematode multiplication from single root inoculation - computation
relationship: variable_of CO_325:0100082 ! multiplication factor

[Term]
id: CO_325:0000520
name: nematode population density by species in soil
namespace: BananaTrait
def: "Number of nematodes in soil" []
is_a: CO_325:1000001

[Term]
id: CO_325:0000521
name: NmNumSlWt
namespace: BananaTrait
def: "Count from 100 ml of soil sample in No. per 100ml" []
synonym: "Nematode population density by species in soil @ recently flowered plant (less than 14 days) or plant with emerging flowers" EXACT []
is_a: CO_325:1000020
relationship: variable_of CO_325:0000520 ! nematode population density by species in soil
relationship: variable_of CO_325:0010143 ! number of nematodes (unclassified spp.) per unit fresh root weight - method
relationship: variable_of CO_325:0100084 ! No. per 100ml

[Term]
id: CO_325:0000522
name: number of radopholus similis per soil sample
namespace: BananaTrait
def: "Number of Radopholus similis in soil" []
is_a: CO_325:1000001

[Term]
id: CO_325:0000523
name: number of helicotylenchus multicinctus per soil sample
namespace: BananaTrait
def: "Number of Helicotylenchus multicinctus in soil" []
is_a: CO_325:1000001

[Term]
id: CO_325:0000524
name: number of rotylenchulus spp.per soil sample
namespace: BananaTrait
def: "Number of Rotylenchulus spp.in soil" []
is_a: CO_325:1000001

[Term]
id: CO_325:0000525
name: RotyNumSlWt_CompNema
namespace: BananaTrait
def: "Count from 100 ml of soil sample in No. per 10g" []
synonym: "Number of Rotylenchulus spp.per soil sample @ recently flowered plant (less than 14 days) or plant with emerging flowers" EXACT []
is_a: CO_325:1000019
relationship: variable_of CO_325:0000524 ! number of rotylenchulus spp.per soil sample
relationship: variable_of CO_325:0010146 ! number of nematodes (rotylenchulus spp.) per  unit fresh root weight - method
relationship: variable_of CO_325:0100085 ! No. per 10g

[Term]
id: CO_325:0000526
name: number of meloidogyne spp. per  soil sample
namespace: BananaTrait
def: "Number of Meloidogyne spp. in soil" []
is_a: CO_325:1000001

[Term]
id: CO_325:0000527
name: number of pratylenchus spp. per soil sample
namespace: BananaTrait
def: "Number of Pratylenchus spp. in soil" []
is_a: CO_325:1000001

[Term]
id: CO_325:0000528
name: number of hoplolaimus spp. per soil sample
namespace: BananaTrait
def: "Number of Hoplolaimus spp. in soil" []
is_a: CO_325:1000001

[Term]
id: CO_325:0000529
name: number of pratylenchus goodeyi per soil sample
namespace: BananaTrait
def: "Number of Pratylenchus goodeyi in soil" []
is_a: CO_325:1000001

[Term]
id: CO_325:0000530
name: number of pratylenchus coffeae per soil sample
namespace: BananaTrait
def: "Number of Pratylenchus coffeae in soil" []
is_a: CO_325:1000001

[Term]
id: CO_325:0000531
name: nematode population density by species in fresh roots
namespace: BananaTrait
def: "Number of nematode in roots" []
is_a: CO_325:1000001

[Term]
id: CO_325:0000532
name: NmNumRtWt
namespace: BananaTrait
def: "Count from 10 g of chopped roots from the tested banana plant sample in No. per 10g" []
synonym: "Nematode population density by species in fresh roots @ recently flowered plant (less than 14 days) or plant with emerging flowers" EXACT []
is_a: CO_325:1000019
relationship: variable_of CO_325:0000531 ! nematode population density by species in fresh roots
relationship: variable_of CO_325:0010152 ! number of nematodes per  unit fresh root weight
relationship: variable_of CO_325:0100085 ! No. per 10g

[Term]
id: CO_325:0000533
name: number of radopholus similis per fresh root weight
namespace: BananaTrait
def: "Number of Radopholus similis  in roots" []
is_a: CO_325:1000001

[Term]
id: CO_325:0000534
name: RadoNumRtWt2_Comp_Nema
namespace: BananaTrait
def: "Count from 10 g of chopped roots from the tested banana plant sample in No. per 10g" []
synonym: "Number of Radopholus similis per fresh root weight @ recently flowered plant (less than 14 days) or plant with emerging flowers" EXACT []
is_a: CO_325:1000019
relationship: variable_of CO_325:0000533 ! number of radopholus similis per fresh root weight
relationship: variable_of CO_325:0010153 ! number of nematodes (radopholus similis ) per  unit fresh root weight -method
relationship: variable_of CO_325:0100085 ! No. per 10g

[Term]
id: CO_325:0000535
name: number of meloidogyne spp. per fresh root weight
namespace: BananaTrait
def: "Number of Meloidogyne spp.  in roots" []
is_a: CO_325:1000001

[Term]
id: CO_325:0000536
name: MeloiNumRtWt2_Comp_Nema
namespace: BananaTrait
def: "Count from 10 g of chopped roots from the tested banana plant sample in No. per 10g" []
synonym: "Number of Meloidogyne spp. per fresh root weight @ recently flowered plant (less than 14 days) or plant with emerging flowers" EXACT []
is_a: CO_325:1000019
relationship: variable_of CO_325:0000535 ! number of meloidogyne spp. per fresh root weight
relationship: variable_of CO_325:0010154 ! number of nematodes (meloidogyne spp.)  per  unit fresh root weight -method
relationship: variable_of CO_325:0100085 ! No. per 10g

[Term]
id: CO_325:0000537
name: number of pratylenchus spp. per fresh root weight
namespace: BananaTrait
def: "Number of Pratylenchus spp.  in roots" []
is_a: CO_325:1000001

[Term]
id: CO_325:0000538
name: PratyNumRtWt2_Comp_Nema
namespace: BananaTrait
def: "Count from 10 g of chopped roots from the tested banana plant sample in No. per 10g" []
synonym: "Number of Pratylenchus spp. per fresh root weight @ recently flowered plant (less than 14 days) or plant with emerging flowers" EXACT []
is_a: CO_325:1000019
relationship: variable_of CO_325:0000537 ! number of pratylenchus spp. per fresh root weight
relationship: variable_of CO_325:0010155 ! number of nematodes (pratylenchus spp.)  per  unit fresh root weight -method
relationship: variable_of CO_325:0100085 ! No. per 10g

[Term]
id: CO_325:0000539
name: number of hoplolaimus spp. per fresh root weight
namespace: BananaTrait
def: "Number of Hoplolaimus spp.  in roots" []
is_a: CO_325:1000001

[Term]
id: CO_325:0000540
name: HoploNumRtWt2_Comp_Nema
namespace: BananaTrait
def: "Count from 10 g of chopped roots from the tested banana plant sample in No. per 10g" []
synonym: "Number of Hoplolaimus spp. per fresh root weight @ recently flowered plant (less than 14 days) or plant with emerging flowers" EXACT []
is_a: CO_325:1000019
relationship: variable_of CO_325:0000539 ! number of hoplolaimus spp. per fresh root weight
relationship: variable_of CO_325:0010156 ! number of nematodes (hoplolaimus spp.)  per  unit fresh root weight -method
relationship: variable_of CO_325:0100085 ! No. per 10g

[Term]
id: CO_325:0000541
name: number of pratylenchus goodeyi per fresh root weight
namespace: BananaTrait
def: "Number of Pratylenchus goodeyi  in roots" []
is_a: CO_325:1000001

[Term]
id: CO_325:0000542
name: PratyGooNumRtWt2_Comp_Nema
namespace: BananaTrait
def: "Count from 10 g of chopped roots from the tested banana plant sample in No. per 10g" []
synonym: "Number of Pratylenchus goodeyi per fresh root weight @ recently flowered plant (less than 14 days) or plant with emerging flowers" EXACT []
is_a: CO_325:1000019
relationship: variable_of CO_325:0000541 ! number of pratylenchus goodeyi per fresh root weight
relationship: variable_of CO_325:0010157 ! number of nematodes (pratylenchus goodeyi)  per  unit fresh root weight -method
relationship: variable_of CO_325:0100085 ! No. per 10g

[Term]
id: CO_325:0000543
name: number of pratylenchus coffeae per fresh root weight
namespace: BananaTrait
def: "Number of Pratylenchus coffeae  in roots" []
is_a: CO_325:1000001

[Term]
id: CO_325:0000544
name: PratyCofNumRtWt2_Comp_Nema
namespace: BananaTrait
def: "Count from 10 g of chopped roots from the tested banana plant sample in No. per 10g" []
synonym: "Number of Pratylenchus coffeae per fresh root weight @ recently flowered plant (less than 14 days) or plant with emerging flowers" EXACT []
is_a: CO_325:1000019
relationship: variable_of CO_325:0000543 ! number of pratylenchus coffeae per fresh root weight
relationship: variable_of CO_325:0010158 ! number of nematodes (pratylenchus coffeae)  per  unit fresh root weight -method
relationship: variable_of CO_325:0100085 ! No. per 10g

[Term]
id: CO_325:0000545
name: date of first youngest leaf spotted
namespace: BananaTrait
def: "The date a youngest leaf spotted is first observed on the plant, caused by black Sigatoka." []
is_a: CO_325:1000001

[Term]
id: CO_325:0000546
name: FstYngLfsptd_Est_dmy
namespace: BananaTrait
def: "Record the date of event, in dd/mm/yyyy format" []
synonym: "Date of first youngest leaf spotted, in dd/mm/yyyy" EXACT []
is_a: CO_325:1000019
relationship: variable_of CO_325:0000545 ! date of first youngest leaf spotted
relationship: variable_of CO_325:0010160 ! date of first youngest leaf spotted - estimation
relationship: variable_of CO_325:0100000 ! dd/mm/yyyy

[Term]
id: CO_325:0000547
name: FstYngLfsptd_Est_ymd
namespace: BananaTrait
def: "Record the date of event, in yyy/mm/dd format" []
synonym: "Date of first youngest leaf spotted, in yyyy/mm/dd" EXACT []
is_a: CO_325:1000019
relationship: variable_of CO_325:0000545 ! date of first youngest leaf spotted
relationship: variable_of CO_325:0010160 ! date of first youngest leaf spotted - estimation
relationship: variable_of CO_325:0100001 ! yyyy/mm/dd

[Term]
id: CO_325:0000548
name: rank of oldest standing leaf
namespace: BananaTrait
def: "The rank of the oldest (most-distal) standing leaf (with an erect petiole)." []
is_a: CO_325:1000001

[Term]
id: CO_325:0000549
name: OdStdLfRk_Ct_leaf
namespace: BananaTrait
def: "Record the rank of the oldest standing leaf (with an erect petiole), counting the rank by starting with the newest fully unrolled leaf as 1 and moving downwards, associating the data with the time of collection. in leaf rank format Numerical" []
synonym: "Rank of oldest standing leaf @ Monthly, from 6 months after planting until harvest, and including at the Date of shooting and at the Date of harvest" EXACT []
is_a: CO_325:1000019
relationship: variable_of CO_325:0000548 ! rank of oldest standing leaf
relationship: variable_of CO_325:0010161 ! rank of oldest standing leaf - counting
relationship: variable_of CO_325:0100086 ! leaf rank

[Term]
id: CO_325:0000550
name: date of tagged cigar leaf unrolling at brun's stage b
namespace: BananaTrait
def: "The date a tagged cigar leaf is at Brun's stage B of unrolling." []
is_a: CO_325:1000001

[Term]
id: CO_325:0000551
name: CigLfUnrBrnStgB_Date_dmy
namespace: BananaTrait
def: "Record the date of event. in dd/mm/yyyy" []
synonym: "Date of tagged cigar leaf unrolling at Brun's stage B , in dd/mm/yyyy format" EXACT []
is_a: CO_325:1000019
relationship: variable_of CO_325:0000550 ! date of tagged cigar leaf unrolling at brun's stage b
relationship: variable_of CO_325:0010163 ! date of tagged cigar leaf unrolling at brun's stage b - estimation
relationship: variable_of CO_325:0100000 ! dd/mm/yyyy

[Term]
id: CO_325:0000552
name: CigLfUnrBrnStgB_Date_ymd
namespace: BananaTrait
def: "Record the date of event. in yyyy/mm/dd" []
synonym: "Date of tagged cigar leaf unrolling at Brun's stage B , in yyyy/mm/dd format" EXACT []
is_a: CO_325:1000019
relationship: variable_of CO_325:0000550 ! date of tagged cigar leaf unrolling at brun's stage b
relationship: variable_of CO_325:0010163 ! date of tagged cigar leaf unrolling at brun's stage b - estimation
relationship: variable_of CO_325:0100001 ! yyyy/mm/dd

[Term]
id: CO_325:0000553
name: date of tagged leaf presenting black sigatoka disease symptoms at foure's stage 1
namespace: BananaTrait
def: "The date a tagged leaf presents black Sigatoka disease symptoms at Foure's black leaf streak disease severity grade 1." []
synonym: "Date of tagged leaf presenting black leaf streak symptoms at Foure's stage 1" EXACT []
is_a: CO_325:1000001

[Term]
id: CO_325:0000554
name: BlkLfStrkLfFrStg1_Date_dmy
namespace: BananaTrait
def: "Record the date of event. in dd/mm/yyyy" []
synonym: "Date of tagged leaf presenting black Sigatoka disease symptoms at Foure's stage 1 , in dd/mm/yyyy format" EXACT []
is_a: CO_325:1000019
relationship: variable_of CO_325:0000553 ! date of tagged leaf presenting black sigatoka disease symptoms at foure's stage 1
relationship: variable_of CO_325:0010164 ! date of tagged leaf presenting black sigatoka disease symptoms at foure's stage 1 - estimation
relationship: variable_of CO_325:0100000 ! dd/mm/yyyy

[Term]
id: CO_325:0000555
name: BlkLfStrkLfFrStg1_Date_ymd
namespace: BananaTrait
def: "Record the date of event. in yyyy/mm/dd" []
synonym: "Date of tagged leaf presenting black Sigatoka disease symptoms at Foure's stage 1 , in yyyy/mm/dd format" EXACT []
is_a: CO_325:1000019
relationship: variable_of CO_325:0000553 ! date of tagged leaf presenting black sigatoka disease symptoms at foure's stage 1
relationship: variable_of CO_325:0010164 ! date of tagged leaf presenting black sigatoka disease symptoms at foure's stage 1 - estimation
relationship: variable_of CO_325:0100001 ! yyyy/mm/dd

[Term]
id: CO_325:0000556
name: date of tagged leaf presenting black sigatoka disease symptoms at foure's stage 6
namespace: BananaTrait
def: "The date a tagged leaf presents black Sigatoka disease symptoms at Foure's black leaf streak disease severity grade 6." []
synonym: "Date of tagged leaf presenting black leaf streak symptoms at Foure's stage 6" EXACT []
is_a: CO_325:1000001

[Term]
id: CO_325:0000557
name: BlkLfStrkLfFrStg6_Date_dmy
namespace: BananaTrait
def: "Record the date of event. in dd/mm/yyyy" []
synonym: "Date of tagged leaf presenting black Sigatoka disease symptoms at Foure's stage 6 , in dd/mm/yyyy format" EXACT []
is_a: CO_325:1000019
relationship: variable_of CO_325:0000556 ! date of tagged leaf presenting black sigatoka disease symptoms at foure's stage 6
relationship: variable_of CO_325:0010165 ! date of tagged leaf presenting black sigatoka disease symptoms at foure's stage 6 - estimation
relationship: variable_of CO_325:0100000 ! dd/mm/yyyy

[Term]
id: CO_325:0000558
name: BlkLfStrkLfFrStg6_Date_ymd
namespace: BananaTrait
def: "Record the date of event. in yyyy/mm/dd" []
synonym: "Date of tagged leaf presenting black Sigatoka disease symptoms at Foure's stage 6 , in yyyy/mm/dd format" EXACT []
is_a: CO_325:1000019
relationship: variable_of CO_325:0000556 ! date of tagged leaf presenting black sigatoka disease symptoms at foure's stage 6
relationship: variable_of CO_325:0010165 ! date of tagged leaf presenting black sigatoka disease symptoms at foure's stage 6 - estimation
relationship: variable_of CO_325:0100001 ! yyyy/mm/dd

[Term]
id: CO_325:0000559
name: extent of internal discolouration in corm of plant caused by fusarium wilt
namespace: BananaTrait
def: "The extent of discolouration in the corm of the plant caused by Fusarium wilt." []
is_a: CO_325:1000001

[Term]
id: CO_325:0000560
name: CrmIntDiscFW_Est_1to5
namespace: BananaTrait
def: "Completely cut the pseudostem off at the base and ***                                             For the motherplant, at harvest the plant should be cut at the base of the pseudostem. The extent to which vascular discolouration extends up the pseudostem should be determined by making transverse cuts, from the base of the pseudostem upwards, and examining the internal tissues following each cut. The point at which discolouration is no longer visible should be noted and the distance from this point to the pseudostem base recorded. in 5 pt corm discolouration. In scale 1to5: 1=Corm completely clean, no discolouration in vascular tissue; 2=Isolated points of discolouration of vascular tissue; 3=Discolouration of up to one-third of vascular tissue; 4=Discolouration of between one-third and two-thirds of vascular tissue; 5=Discolouration of more than two-thirds of vascular tissue." []
synonym: "Extent of internal discolouration in corm of plant caused by Fusarium wilt @ Harvest" EXACT []
is_a: CO_325:1000020
relationship: variable_of CO_325:0000559 ! extent of internal discolouration in corm of plant caused by fusarium wilt
relationship: variable_of CO_325:0010168 ! extent of internal discolouration in corm of plant caused by fusarium wilt - estimation
relationship: variable_of CO_325:0100088 ! 5 pt corm discolouration scale

[Term]
id: CO_325:0000561
name: date of first external disease symptoms caused by fusarium wilt
namespace: BananaTrait
def: "The date of the appearance on the plant of any of the external disease symptoms caused by Fusarium wilt - yellowing leaves, splitting pseudostem base, changes in new leaves, petiole collapse." []
is_a: CO_325:1000001

[Term]
id: CO_325:0000562
name: FstExtDiSmptFW_Date_dmy
namespace: BananaTrait
def: "Record the date of event. in dd/mm/yyyy" []
synonym: "Date of first external disease symptoms caused by Fusarium wilt , in dd/mm/yyyy format" EXACT []
is_a: CO_325:1000020
relationship: variable_of CO_325:0000561 ! date of first external disease symptoms caused by fusarium wilt
relationship: variable_of CO_325:0010172 ! date of first external disease symptoms caused by fusarium wilt - estimation
relationship: variable_of CO_325:0100000 ! dd/mm/yyyy

[Term]
id: CO_325:0000563
name: FstExtDiSmptFW_Date_ymd
namespace: BananaTrait
def: "Record the date of event. in yyyymmdd" []
synonym: "Date of first external disease symptoms caused by Fusarium wilt , in yyyy/mm/dd format" EXACT []
is_a: CO_325:1000019
relationship: variable_of CO_325:0000561 ! date of first external disease symptoms caused by fusarium wilt
relationship: variable_of CO_325:0010172 ! date of first external disease symptoms caused by fusarium wilt - estimation
relationship: variable_of CO_325:0100001 ! yyyy/mm/dd

[Term]
id: CO_325:0000564
name: rank of marked youngest leaf
namespace: BananaTrait
def: "The rank (position) of the youngest completely unrolled leaf." []
synonym: "rankyoungleaf" EXACT []
is_a: CO_325:1000005

[Term]
id: CO_325:0000565
name: RkYgstLf_Comp_leafrank
namespace: BananaTrait
def: "Record the rank of the youngest, completely unrolled, leaf, which is always 1" []
synonym: "Rank of marked youngest leaf @ Monthly, from 6 months after planting until harvest, and including at the Date of shooting and at the Date of harvest" EXACT []
is_a: CO_325:1000019
relationship: variable_of CO_325:0000564 ! rank of marked youngest leaf
relationship: variable_of CO_325:0010173 ! rank of youngest leaf - counting
relationship: variable_of CO_325:0100086 ! leaf rank

[Term]
id: CO_325:0000566
name: rank of previously marked leaf
namespace: BananaTrait
def: "The current rank (position) of the leaf that was previously marked as the youngest leaf at the time of the last data collection event." []
synonym: "rankprevleaf" EXACT []
is_a: CO_325:1000005

[Term]
id: CO_325:0000567
name: RkPvsMktLf_Comp_leafrank
namespace: BananaTrait
def: "Record the rank of the leaf that was previously marked in the Rank of youngest leaf during the last data collection, counting the leaf rank by starting with the newest completely unrolled leaf as 1 and moving downwards, associating the data with the time of collection." []
synonym: "Rank of previously marked leaf @ Monthly, from 7 months after planting until harvest, and including at the Date of shooting and at the Date of harvest" EXACT []
is_a: CO_325:1000019
relationship: variable_of CO_325:0000566 ! rank of previously marked leaf
relationship: variable_of CO_325:0010174 ! rank of previously marked leaf - counting
relationship: variable_of CO_325:0100086 ! leaf rank

[Term]
id: CO_325:0000568
name: LfEmRate_Comp_LfMth
namespace: BananaTrait
def: "Calculate as: the Rank of previously marked leaf at one point in time, minus 1 (equivalent to the Rank of marked youngest leaf), divided by the time elapsed between the two Date of data collection events when the marked leaf was recorded as 1) the Rank of youngest leaf and 2) the Rank of previously marked leaf, e.g. (4 - 1) / 1 month = LER of 3 leaves/month during a particular time period." []
synonym: "Monthly Leaf emission rate @ At regular intervals, usually from 7 months after planting until harvest, and including at the Date of shooting and at the Date of harvest" EXACT []
is_a: CO_325:1000020
relationship: variable_of CO_325:0000021 ! leaf emission rate
relationship: variable_of CO_325:0010175 ! leaf emission rate - computation
relationship: variable_of CO_325:0100090 ! leaves/month

[Term]
id: CO_325:0000569
name: FnctLeav_Ct_Leaf
namespace: BananaTrait
def: "Count how many functional leaves (leaves that have 50% or more of their surface as green, healthy, photosynthetic tissue) are on the plant, considering all leaves in between and inclusive of, the youngest leaf (at leaf rank 1) and the oldest standing leaf" []
synonym: "Number of functional leaves @ Monthly, from 3 months after planting until harvest, and including at the Date of shooting and at the Date of harvest" EXACT []
is_a: CO_325:1000020
relationship: variable_of CO_325:0000066 ! number of functional leaves
relationship: variable_of CO_325:0010176 ! number of functional leaves - counting
relationship: variable_of CO_325:0100092 ! leaf

[Term]
id: CO_325:0000570
name: time from planting to first youngest leaf spotted
namespace: BananaTrait
def: "Time elapsed between planting and the appearance of the first youngest leaf spotted." []
is_a: CO_325:1000001

[Term]
id: CO_325:0000571
name: PltFstLfSptd_Ct_leaf
namespace: BananaTrait
def: "Calculate as: the time elapsed between the Date of planting and the Date of first youngest spotted leaf in days (e.g. 24/06/2014 - 24/01/2014 = 151 days.)" []
synonym: "Time from planting to first youngest leaf spotted" EXACT []
is_a: CO_325:1000019
relationship: variable_of CO_325:0000570 ! time from planting to first youngest leaf spotted
relationship: variable_of CO_325:0010177 ! time from planting to first youngest spotted leaf - computation
relationship: variable_of CO_325:0100003 ! day

[Term]
id: CO_325:0000572
name: number of spotted leaves
namespace: BananaTrait
def: "The number of leaves with at least 10 discrete, mature, necrotic lesions or one large necrotic area with 10 light-coloured dry centres, caused by black Sigatoka disease." []
synonym: "Number and severity of spotted leaves" EXACT []
is_a: CO_325:1000001

[Term]
id: CO_325:0000573
name: SptLfNb_Ct_leaf
namespace: BananaTrait
def: "Count how many of the standing leaves are spotted (with at least 10 discrete, mature, necrotic lesions or one large necrotic area with 10 light-coloured dry centres), considering all leaves in between and inclusive of, the NEWEST LEAF and the oldest STANDING LEAF." []
synonym: "Number of spotted leaves @ Monthly once recognised, and including at the Date of shooting and at the Date of harvest" EXACT []
is_a: CO_325:1000020
relationship: variable_of CO_325:0000572 ! number of spotted leaves
relationship: variable_of CO_325:0010178 ! number of spotted leaves - counting
relationship: variable_of CO_325:0100092 ! leaf

[Term]
id: CO_325:0000574
name: black sigatoka disease severity
namespace: BananaTrait
def: "An indication of the extent of damage on an individual leaf caused by black Sigatoka disease." []
synonym: "Black leaf streak disease severity" EXACT []
synonym: "BLS" EXACT []
is_a: CO_325:1000001

[Term]
id: CO_325:0000575
name: BlkLfStrkSvrt_Est_pct
namespace: BananaTrait
def: "Visually observe and record the amount of the surface area of a standing leaf that is affected by black leaf streak disease, in percentage." []
synonym: "Black Sigatoka disease severity @ Monthly, from 6 months after planting until harvest, and including at the Date of shooting and at the Date of harvest" EXACT []
is_a: CO_325:1000019
relationship: variable_of CO_325:0000574 ! black sigatoka disease severity
relationship: variable_of CO_325:0010181 ! black sigatoka disease severity - estimation
relationship: variable_of CO_325:0100081 ! %

[Term]
id: CO_325:0000576
name: BlkLfStrkSvrt_Est_Gauhl
namespace: BananaTrait
def: "Visually observe and record the amount of the surface area of a standing leaf that is affected by black leaf streak disease. in Gauhl's modification of Stover's severity scoring system (YYYY). In a 0to6 scale: 0=No symptoms; 1=Less than 1% of lamina with symptoms, only streaks and/or up to 10 spots; 2=1-5% of lamina with symptoms; 3=6-15% of lamina with symptoms; 4=16-33% of lamina with symptoms; 5=34-50% of lamina with symptoms; 6=51-100% of lamina with symptoms" []
synonym: "Black Sigatoka disease severity @ Monthly, from 6 months after planting until harvest, and including at the Date of shooting and at the Date of harvest, Gauhl method" EXACT []
is_a: CO_325:1000019
relationship: variable_of CO_325:0000574 ! black sigatoka disease severity
relationship: variable_of CO_325:0010181 ! black sigatoka disease severity - estimation
relationship: variable_of CO_325:0100093 ! gauhl's modification of stover's severity scoring system (yyyy)

[Term]
id: CO_325:0000577
name: BlkLfStrkSvrt_Est_Faure
namespace: BananaTrait
def: "Visually observe and record the stage of the symptoms of a standing leaf that is affected by black leaf streak disease. in Faure's stages of development of BLS disease scale (1987). In scale 1to6:  1=Stage 1 appears as a small depigmentation spot whose whitish or yellow colour resembles stage 1 of Yellow Sigatoka disease. These symptoms are not visible in transmitted light and can be observed only on the underside of the leaf.; 2=Stage 2 appears as a stripe, generally brown in colour and visible on the underside of the leaf; later the symptom also appears on the upper part of the limb as a stripe, the yellow colour of which resembles the stripe at stage 1 of Yellow Sigatoka. The colour of this stripe will change progressively from brown and later to black on the upper side of the limb, but will retain the brown colour on the underside.; 3=Stage 3 differs from the previous one by its dimensions. The stripe becomes longer, is enlarged and in certain conditions (weak inoculum and unfavourable climatic conditions) can reach 2 or 3 cm.; 4=Stage 4 appears on the underside as a brown spot and on the upper side as a black spot.; 5=Stage 5 is when the elliptical spot is totally black and has spread to the underside of the limb. It is surrounded by a yellow halo with the centre beginning to flatten out.; 6=Stage 6 is when the centre of the spot dries out, turns clear gray and is surrounded by a well-defined black ring, which is, in turn, surrounded by a bright yellow halo. These spots remain visible after the leaf has dried out because the ring persists." []
synonym: "Black Sigatoka disease severity @ Monthly, from 6 months after planting until harvest, and including at the Date of shooting and at the Date of harvest, Faure method" EXACT []
is_a: CO_325:1000019
relationship: variable_of CO_325:0000574 ! black sigatoka disease severity
relationship: variable_of CO_325:0010181 ! black sigatoka disease severity - estimation
relationship: variable_of CO_325:0100094 ! faure's stages of development of bls disease scale (1987)

[Term]
id: CO_325:0000578
name: BlkLfStrkSvrt_Est_MedLawCpt
namespace: BananaTrait
def: "Visually observe and record the stage of the symptoms of a standing leaf that is affected by black leaf streak disease. in Meredith & Lawrence (1969) - In 1to6 scale: 1=Initial speck stage: symptoms are first visible to the naked eye as faint, minute (less than 0.25 mm diam), reddish brown specks on the lower surface of the leaf. Specks are often most abundant near the margin of the left side of the leaf, particularly towards the tip. Where leaf spot is severe, specks have been observed on the second leaf of plants that have not yet produced a bunch. Elsewhere they usually appear on the third, fourth, or older leaves.; 2=First streak stage: the initial speck elongates, becoming slightly wider, to form a characteristic narrow, reddish brown streak up to 20 mm long and 2.0 mm wide, with the long axis parallel to the leaf venation. At this stage, streaks are more clearly visible on the lower surface of the leaf than on the upper one. The distribution of streaks is variable. Sometimes they are most numerous near the edge of the left side of the leaf. At other times they are equally numerous on both sides of the leaf, and more or less evenly distributed. Frequently they are densely aggregated in a band several cm wide on one side or both sides of the mid-rib, becoming less numerous towards the edge of the leaf. Streaks may be so numerous that every cm2 of leaf surface bears one or more. There is considerable variation in the length of individual streaks on a given leaf, and they frequently overlap to form larger, compound streaks.; 3=Second-streak stage: the streaks may elongate slightly, but the most notable change is that in colour from reddish brown to dark brown or almost black, sometimes with a purplish tinge. The streak is now clearly visible on the upper surface of the leaf. The distribution of streaks at this stage of development varies in the same way as mentioned above. When streaks are very numerous, and more or less evenly distributed, the entire leaf blackens.; 4=First-spot stage: the streak broadens and becomes more or less fusiform and elliptical in outline and similar to the 'first-spot stage' of Sigatoka (Leach 1946). The transition from streak to spot is further characterised by the development of a light brown, water-soaked border around the spot. This water-soaked effect is especially clear in the early morning, when dew is still present on the leaf, or after rain.; 5=Second-spot stage: the dark brown or black central area of the spot becomes slightly depressed and the water-soaked border becomes more pronounced due to darkening. At this stage, a slight yellowing of the leaf tissue immediately surrounding the water-soaked border may occur.; 6=Third or mature spot stage: the centre of the spot dries out, becoming light grey or buff-coloured, and further depressed. The spot is surrounded by a narrow, well-defined, dark brown or black border. between the latter and the normal green colour of the leaf, there is often a bright yellow transitional zone. After the leaf has collapsed and withered, spots remain clearly visible because of the light-coloured centre and dark border." []
synonym: "Black Sigatoka disease severity @ Monthly, from 6 months after planting until harvest, and including at the Date of shooting and at the Date of harvest, Meredith method -complete" EXACT []
is_a: CO_325:1000019
relationship: variable_of CO_325:0000574 ! black sigatoka disease severity
relationship: variable_of CO_325:0010181 ! black sigatoka disease severity - estimation
relationship: variable_of CO_325:0100095 ! meredith & lawrence (1969) - complete

[Term]
id: CO_325:0000579
name: BlkLfStrkSvrt_Est_MedLawCdsd
namespace: BananaTrait
def: "Visually observe and record the stage of the symptoms of a standing leaf that is affected by black leaf streak disease. in Meredith & Lawrence (1969) - condensed. In a 1to6 scale: 1=Initial speck stage: faint, minute, reddish-brown specks on the lower surface of the leaf.; 2=First streak stage: specks elongate, becoming slightly wider to form narrow reddish-brown streaks.; 3=Second-streak stage: streaks change colour from reddish brown to dark brown or black, sometimes with a purplish tinge, clearly visible at the upper surface of the leaf.; 4=First-spot stage: the streaks broaden and become more or less fusiform or elliptical in outline and a water soaked border appears around each lesion.; 5=Second-spot stage: the dark brown or black centre of each lesion becomes slightly depressed and water soaked border becomes more pronounced.; 6=Third or mature spot stage: the centres of the lesions dry out becoming light grey or buff coloured and a bright yellow transitional zone appears between them and the normal green colour of the leaf. The lesions remain clearly visible after the leaf has collapsed or withered because of their light coloured centre and dark border." []
synonym: "Black Sigatoka disease severity @ Monthly, from 6 months after planting until harvest, and including at the Date of shooting and at the Date of harvest, Meredith method -condensed" EXACT []
is_a: CO_325:1000019
relationship: variable_of CO_325:0000574 ! black sigatoka disease severity
relationship: variable_of CO_325:0010181 ! black sigatoka disease severity - estimation
relationship: variable_of CO_325:0100096 ! meredith & lawrence (1969) - condensed

[Term]
id: CO_325:0000580
name: number of leaves with black sigatoka disease severity grade 0
namespace: BananaTrait
def: "The number of leaves on a plant with a black Sigatoka disease severity grade of 0." []
synonym: "Number of leaves with black leaf streak disease severity grade 0" EXACT []
is_a: CO_325:1000001

[Term]
id: CO_325:0000581
name: BlkLfStrkSvrtLfNb_Ct_grd0
namespace: BananaTrait
def: "Calculate as: the sum of values for one plant with a BLS disease severity grade of 0. in leaf" []
synonym: "Number of leaves with black Sigatoka disease severity grade 0 @ Monthly, from 6 months after planting until harvest, and including at the Date of shooting and at the Date of harvest" EXACT []
is_a: CO_325:1000019
relationship: variable_of CO_325:0000580 ! number of leaves with black sigatoka disease severity grade 0
relationship: variable_of CO_325:0010182 ! number of leaves with black sigatoka disease severity grade 0 - computation
relationship: variable_of CO_325:0100092 ! leaf

[Term]
id: CO_325:0000582
name: number of leaves with black sigatoka disease severity grade 1
namespace: BananaTrait
def: "The number of leaves on a plant with a black Sigatoka disease severity grade of 1." []
synonym: "Number of leaves with black leaf streak disease severity grade 1" EXACT []
is_a: CO_325:1000001

[Term]
id: CO_325:0000583
name: BlkLfStrkSvrtLfNb_Ct_grd1
namespace: BananaTrait
def: "Calculate as: the sum of values for one plant with a BLS disease severity grade of 1. in leaf" []
synonym: "Number of leaves with black Sigatoka disease severity grade 1 @ Monthly, from 6 months after planting until harvest, and including at the Date of shooting and at the Date of harvest" EXACT []
is_a: CO_325:1000019
relationship: variable_of CO_325:0000582 ! number of leaves with black sigatoka disease severity grade 1
relationship: variable_of CO_325:0010183 ! number of leaves with black sigatoka disease severity grade 1 - computation
relationship: variable_of CO_325:0100092 ! leaf

[Term]
id: CO_325:0000584
name: number of leaves with black sigatoka disease severity grade 2
namespace: BananaTrait
def: "The number of leaves on a plant with a black Sigatoka disease severity grade of 2." []
synonym: "Number of leaves with black leaf streak disease severity grade 2" EXACT []
is_a: CO_325:1000001

[Term]
id: CO_325:0000585
name: BlkLfStrkSvrtLfNb_Ct_grd2
namespace: BananaTrait
def: "Calculate as: the sum of values for one plant with a BLS disease severity grade of 2. in leaf" []
synonym: "Number of leaves with black Sigatoka disease severity grade 2 @ Monthly, from 6 months after planting until harvest, and including at the Date of shooting and at the Date of harvest" EXACT []
is_a: CO_325:1000019
relationship: variable_of CO_325:0000584 ! number of leaves with black sigatoka disease severity grade 2
relationship: variable_of CO_325:0010184 ! number of leaves with black sigatoka disease severity grade 2 - computation
relationship: variable_of CO_325:0100092 ! leaf

[Term]
id: CO_325:0000586
name: number of leaves with black sigatoka disease severity grade 3
namespace: BananaTrait
def: "The number of leaves on a plant with a black Sigatoka disease severity grade of 3." []
synonym: "Number of leaves with black leaf streak disease severity grade 3" EXACT []
is_a: CO_325:1000001

[Term]
id: CO_325:0000587
name: BlkLfStrkSvrtLfNb_Ct_grd3
namespace: BananaTrait
def: "Calculate as: the sum of values for one plant with a BLS disease severity grade of 3. in leaf" []
synonym: "Number of leaves with black Sigatoka disease severity grade 3 @ Monthly, from 6 months after planting until harvest, and including at the Date of shooting and at the Date of harvest" EXACT []
is_a: CO_325:1000019
relationship: variable_of CO_325:0000586 ! number of leaves with black sigatoka disease severity grade 3
relationship: variable_of CO_325:0010185 ! number of leaves with black sigatoka disease severity grade 3 - computation
relationship: variable_of CO_325:0100092 ! leaf

[Term]
id: CO_325:0000588
name: number of leaves with black sigatoka disease severity grade 4
namespace: BananaTrait
def: "The number of leaves on a plant with a black Sigatoka disease severity grade of 4." []
synonym: "Number of leaves with black leaf streak disease severity grade 4" EXACT []
is_a: CO_325:1000001

[Term]
id: CO_325:0000589
name: BlkLfStrkSvrtLfNb_Ct_grd4
namespace: BananaTrait
def: "Calculate as: the sum of values for one plant with a BLS disease severity grade of 4. in leaf" []
synonym: "Number of leaves with black Sigatoka disease severity grade 4 @ Monthly, from 6 months after planting until harvest, and including at the Date of shooting and at the Date of harvest" EXACT []
is_a: CO_325:1000019
relationship: variable_of CO_325:0000588 ! number of leaves with black sigatoka disease severity grade 4
relationship: variable_of CO_325:0010186 ! number of leaves with black sigatoka disease severity grade 4 - computation
relationship: variable_of CO_325:0100092 ! leaf

[Term]
id: CO_325:0000590
name: number of leaves with black sigatoka disease severity grade 5
namespace: BananaTrait
def: "The number of leaves on a plant with a black Sigatoka disease severity grade of 5." []
synonym: "Number of leaves with black leaf streak disease severity grade 5" EXACT []
is_a: CO_325:1000001

[Term]
id: CO_325:0000591
name: BlkLfStrkSvrtLfNb_Ct_grd5
namespace: BananaTrait
def: "Calculate as: the sum of values for one plant with a BLS disease severity grade of 5. in leaf" []
synonym: "Number of leaves with black Sigatoka disease severity grade 5 @ Monthly, from 6 months after planting until harvest, and including at the Date of shooting and at the Date of harvest" EXACT []
is_a: CO_325:1000019
relationship: variable_of CO_325:0000590 ! number of leaves with black sigatoka disease severity grade 5
relationship: variable_of CO_325:0010187 ! number of leaves with black sigatoka disease severity grade 5 - computation
relationship: variable_of CO_325:0100092 ! leaf

[Term]
id: CO_325:0000592
name: number of leaves with black sigatoka disease severity grade 6
namespace: BananaTrait
def: "The number of leaves on a plant with a black Sigatoka disease severity grade of 6." []
synonym: "Number of leaves with black leaf streak disease severity grade 6" EXACT []
is_a: CO_325:1000001

[Term]
id: CO_325:0000593
name: BlkLfStrkSvrtLfNb_Ct_grd6
namespace: BananaTrait
def: "Calculate as: the sum of values for one plant with a BLS disease severity grade of 6. in leaf" []
synonym: "Number of leaves with black Sigatoka disease severity grade 6 @ Monthly, from 6 months after planting until harvest, and including at the Date of shooting and at the Date of harvest" EXACT []
is_a: CO_325:1000019
relationship: variable_of CO_325:0000592 ! number of leaves with black sigatoka disease severity grade 6
relationship: variable_of CO_325:0010188 ! number of leaves with black sigatoka disease severity grade 6 - computation
relationship: variable_of CO_325:0100092 ! leaf

[Term]
id: CO_325:0000594
name: distance of internal discolouration in pseudostem of tallest sucker caused by fusarium wilt
namespace: BananaTrait
def: "The distance of discolouration in the pseudostem of the tallest sucker caused by Fusarium wilt." []
is_a: CO_325:1000001

[Term]
id: CO_325:0000595
name: CrmDiscDistTlstSckFW_M_cm
namespace: BananaTrait
def: "****For the first sucker, the complete corm should be removed from the soil, the roots cut off and excess soil removed. Transverse sections of the corm should be cut (using a guillotine or other suitable device) to obtain five slices of equal thickness. The upper surface of each cut section should be examined and visually evaluate the extent of the vascular discolouration. In centimeters" []
synonym: "Distance of internal discolouration in pseudostem of tallest sucker caused by Fusarium wilt @ Harvest" EXACT []
is_a: CO_325:1000020
relationship: variable_of CO_325:0000594 ! distance of internal discolouration in pseudostem of tallest sucker caused by fusarium wilt
relationship: variable_of CO_325:0010189 ! distance of internal discolouration in pseudostem of tallest sucker caused by fusarium wilt
relationship: variable_of CO_325:0100004 ! cm

[Term]
id: CO_325:0000596
name: YellowPres_Est_0or1
namespace: BananaTrait
def: "Visual assessment. in Presence/absence scale: 0=Absent; 1=Present" []
synonym: "Presence of yellowing leaves caused by Fusarium wilt @ Monthly, from 3 months after planting until harvest, and including at the Date of shooting and at the Date of harvest, scale 0-1" EXACT []
is_a: CO_325:1000020
relationship: variable_of CO_325:0000087 ! presence of yellowing leaves caused by fusarium wilt
relationship: variable_of CO_325:0010190 ! presence of yellowing leaves caused by fusarium wilt - estimation
relationship: variable_of CO_325:0100089 ! presence/absence scale

[Term]
id: CO_325:0000597
name: PStmSplitPres_Est_0or1
namespace: BananaTrait
def: "Visual assessment. in Presence/absence scale: 0=Absent; 1=Present" []
synonym: "Presence of splitting pseudostem base caused by Fusarium wilt @ Monthly, from 3 months after planting until harvest, and including at the Date of shooting and at the Date of harvest, scale 0-1" EXACT []
is_a: CO_325:1000020
relationship: variable_of CO_325:0000090 ! presence of splitting pseudostem base caused by fusarium wilt
relationship: variable_of CO_325:0010191 ! presence of splitting pseudostem base caused by fusarium wilt - estimation
relationship: variable_of CO_325:0100089 ! presence/absence scale

[Term]
id: CO_325:0000598
name: LfChgPres_Est_0or1
namespace: BananaTrait
def: "Visual assessment. in Presence/absence scale: 0=Absent; 1=Present" []
synonym: "Presence of changes in new leaves caused by Fusarium wilt @ Monthly, from 3 months after planting until harvest, and including at the Date of shooting and at the Date of harvest, scale 0-1" EXACT []
is_a: CO_325:1000019
relationship: variable_of CO_325:0000093 ! presence of changes in new leaves caused by fusarium wilt
relationship: variable_of CO_325:0010192 ! presence of changes in new leaves caused by fusarium wilt - estimation
relationship: variable_of CO_325:0100089 ! presence/absence scale

[Term]
id: CO_325:0000599
name: PetColpPres_Est_0or1
namespace: BananaTrait
def: "Visual assessment. in Presence/absence scale:  0=Absent; 1=Present" []
synonym: "Presence of petiole collapse caused by Fusarium wilt @ Monthly, from 3 months after planting until harvest, and including at the Date of shooting and at the Date of harvest, scale 0-1" EXACT []
is_a: CO_325:1000019
relationship: variable_of CO_325:0000096 ! presence of petiole collapse caused by fusarium wilt
relationship: variable_of CO_325:0010171 ! presence of petiole collapse caused by fusarium wilt - estimation
relationship: variable_of CO_325:0100089 ! presence/absence scale

[Term]
id: CO_325:0000600
name: percentage of plants with yellowing leaves caused by fusarium wilt
namespace: BananaTrait
def: "Percentage of plants with yellowing leaves caused by Fusarium wilt." []
is_a: CO_325:1000001

[Term]
id: CO_325:0000601
name: YlLfPercFW_Comp_pct
namespace: BananaTrait
def: "Calculate as: the sum of the number of values for Presence of yellowing leaves caused by Fusarium wilt scored as Present, divided by the Number of plants planted, multiplied by 100, e.g. 78 / 300 * 100 = 26%." []
synonym: "Percentage of plants with yellowing leaves caused by Fusarium wilt @ Monthly, from 3 months after planting until harvest, and including at the Date of shooting and at the Date of harvest" EXACT []
is_a: CO_325:1000019
relationship: variable_of CO_325:0000600 ! percentage of plants with yellowing leaves caused by fusarium wilt
relationship: variable_of CO_325:0010194 ! percentage of plants with yellowing leaves caused by fusarium wilt - computation
relationship: variable_of CO_325:0100081 ! %

[Term]
id: CO_325:0000602
name: percentage of plants with a splitting pseudostem base caused by fusarium wilt
namespace: BananaTrait
def: "Percentage of plants with a splitting pseudostem base caused by Fusarium wilt." []
is_a: CO_325:1000001

[Term]
id: CO_325:0000603
name: SptPsdStmPercFW_Comp_pct
namespace: BananaTrait
def: "Calculate as: the sum of the number of values for Presence of splitting pseudostem base caused by Fusarium wilt scored as Present, divided by the Number of plants planted, multiplied by 100, e.g. 24 / 300 * 100 = 8%." []
synonym: "Percentage of plants with a splitting pseudostem base caused by Fusarium wilt @ Monthly, from 3 months after planting until harvest, and including at the Date of shooting and at the Date of harvest" EXACT []
is_a: CO_325:1000019
relationship: variable_of CO_325:0000602 ! percentage of plants with a splitting pseudostem base caused by fusarium wilt
relationship: variable_of CO_325:0010195 ! percentage of plants with a splitting pseudostem base caused by fusarium wilt - computation
relationship: variable_of CO_325:0100081 ! %

[Term]
id: CO_325:0000604
name: percentage of plants with changes in new leaves caused by fusarium wilt
namespace: BananaTrait
def: "Percentage of plants with changes in new leaves caused by Fusarium wilt." []
is_a: CO_325:1000001

[Term]
id: CO_325:0000605
name: ChgNwLfPercFW_Comp_pct
namespace: BananaTrait
def: "Calculate as: the sum of the number of values for Presence of changes in new leaves caused by Fusarium wilt scored as Present, divided by the Number of plants planted, multiplied by 100, e.g. 67 / 300 * 100 = 22%." []
synonym: "Percentage of plants with changes in new leaves caused by Fusarium wilt @ Monthly, from 3 months after planting until harvest, and including at the Date of shooting and at the Date of harvest" EXACT []
is_a: CO_325:1000019
relationship: variable_of CO_325:0000604 ! percentage of plants with changes in new leaves caused by fusarium wilt
relationship: variable_of CO_325:0010196 ! percentage of plants with changes in new leaves caused by fusarium wilt - computation
relationship: variable_of CO_325:0100081 ! %

[Term]
id: CO_325:0000606
name: percentage of plants with petiole collapse caused by fusarium wilt
namespace: BananaTrait
def: "Percentage of plants with petiole collapse caused by Fusarium wilt." []
is_a: CO_325:1000001

[Term]
id: CO_325:0000607
name: PtlClpFW_Comp_pct
namespace: BananaTrait
def: "Calculate as: the sum of the number of values for Presence of petiole collapse caused by Fusarium wilt scored as Present, divided by the Number of plants planted, multiplied by 100, e.g. 84 / 300 * 100 = 28%." []
synonym: "Percentage of plants with petiole collapse caused by Fusarium wilt @ Monthly, from 3 months after planting until harvest, and including at the Date of shooting and at the Date of harvest" EXACT []
is_a: CO_325:1000019
relationship: variable_of CO_325:0000606 ! percentage of plants with petiole collapse caused by fusarium wilt
relationship: variable_of CO_325:0010197 ! percentage of plants with petiole collapse caused by fusarium wilt - computation
relationship: variable_of CO_325:0100081 ! %

[Term]
id: CO_325:0000608
name: vitamin c content
namespace: BananaTrait
def: "The Vitamin C content of freeze-dried smashed pulp of a mature fruit" []
is_a: CO_325:1000006

[Term]
id: CO_325:0000609
name: VitCCnt_M_
namespace: BananaTrait
synonym: "Vitamin C content @ Post-harvest" EXACT []
is_a: CO_325:1000020
relationship: variable_of CO_325:0000608 ! vitamin c content
relationship: variable_of CO_325:0010200 ! vitamin c - measurement
relationship: variable_of CO_325:0100097 ! Ex: g/100 mL juice????

[Term]
id: CO_325:0000610
name: number of adult weevils per trap
namespace: BananaTrait
def: "The number of adult weevils per trap" []
is_a: CO_325:1000001

[Term]
id: CO_325:0000611
name: WvlAdltPrTrp_Ct_weevil
namespace: BananaTrait
def: "visual counting method in weevil" []
synonym: "Number of adult weevils per trap @ recently flowered plant (less than 14 days) or plant with emerging flowers" EXACT []
is_a: CO_325:1000019
relationship: variable_of CO_325:0000610 ! number of adult weevils per trap
relationship: variable_of CO_325:0010201 ! number of adult weevils - counting
relationship: variable_of CO_325:0100098 ! weevil

[Term]
id: CO_325:0000612
name: number of weevils traps used
namespace: BananaTrait
def: "The number of adult weevils traps" []
is_a: CO_325:1000001

[Term]
id: CO_325:0000613
name: TrpNum_Ct_weeviltrap
namespace: BananaTrait
def: "visual counting method in weevil" []
synonym: "Number of weevils traps used @ recently flowered plant (less than 14 days) or plant with emerging flowers" EXACT []
is_a: CO_325:1000019
relationship: variable_of CO_325:0000612 ! number of weevils traps used
relationship: variable_of CO_325:0010202 ! number of adult weevil trap - counting
relationship: variable_of CO_325:0100098 ! weevil

[Term]
id: CO_325:0000614
name: average number of adult weevils \{x per trap} per mat
namespace: BananaTrait
def: "The average number of adult weevils per trap per mat" []
is_a: CO_325:1000001

[Term]
id: CO_325:0000615
name: WvlAdlt_Ct_weevil
namespace: BananaTrait
def: "visual counting method in weevil" []
synonym: "Average number of adult weevils {x per trap} per mat @ recently flowered plant (less than 14 days) or plant with emerging flowers" EXACT []
is_a: CO_325:1000019
relationship: variable_of CO_325:0000614 ! average number of adult weevils {x per trap} per mat
relationship: variable_of CO_325:0010201 ! number of adult weevils - counting
relationship: variable_of CO_325:0100098 ! weevil

[Term]
id: CO_325:0000616
name: [number of weevil larvae per trap]
namespace: BananaTrait
def: "The number of weevil larvae per trap" []
is_a: CO_325:1000001

[Term]
id: CO_325:0000617
name: WvlLvPrTrp_Ct_weevil
namespace: BananaTrait
def: "visual counting method in weevil" []
synonym: "[Number of weevil larvae per trap] @ recently flowered plant (less than 14 days) or plant with emerging flowers" EXACT []
is_a: CO_325:1000019
relationship: variable_of CO_325:0000616 ! [number of weevil larvae per trap]
relationship: variable_of CO_325:0010203 ! number of weevil larvae - counting
relationship: variable_of CO_325:0100098 ! weevil

[Term]
id: CO_325:0000618
name: average number of weevil larvae per mat
namespace: BananaTrait
def: "The average number of weevil larvae per mat" []
is_a: CO_325:1000001

[Term]
id: CO_325:0000619
name: WvlLv_Ct_weevil
namespace: BananaTrait
def: "visual counting method in weevil" []
synonym: "Average number of weevil larvae per mat @ recently flowered plant (less than 14 days) or plant with emerging flowers" EXACT []
is_a: CO_325:1000019
relationship: variable_of CO_325:0000618 ! average number of weevil larvae per mat
relationship: variable_of CO_325:0010203 ! number of weevil larvae - counting
relationship: variable_of CO_325:0100098 ! weevil

[Term]
id: CO_325:0000620
name: number of adult weevils measured
namespace: BananaTrait
def: "The number of adult weevils used to obtain a measurement" []
is_a: CO_325:1000001

[Term]
id: CO_325:0000621
name: WvlAdltMsrd_Ct_weevil
namespace: BananaTrait
def: "visual counting method in weevil" []
synonym: "Number of adult weevils measured @ Detached corm Assay" EXACT []
is_a: CO_325:1000019
relationship: variable_of CO_325:0000620 ! number of adult weevils measured
relationship: variable_of CO_325:0010204 ! number of adult larvae - counting
relationship: variable_of CO_325:0100098 ! weevil

[Term]
id: CO_325:0000622
name: number of weevil larvae measured
namespace: BananaTrait
def: "The number of weevil larvae used to obtain a measurement" []
is_a: CO_325:1000001

[Term]
id: CO_325:0000623
name: WvlLvMsrd_Ct_weevil
namespace: BananaTrait
def: "visual counting method in weevil" []
synonym: "Number of weevil larvae measured @ Detached corm Assay" EXACT []
is_a: CO_325:1000019
relationship: variable_of CO_325:0000622 ! number of weevil larvae measured
relationship: variable_of CO_325:0010203 ! number of weevil larvae - counting
relationship: variable_of CO_325:0100098 ! weevil

[Term]
id: CO_325:0000624
name: adult weevil head capsule width
namespace: BananaTrait
def: "The width of the adult weevil head {x per trap per mat}" []
is_a: CO_325:1000001

[Term]
id: CO_325:0000625
name: WvlAdltHdCps_M_?M
namespace: BananaTrait
def: "Measurement under microscope in ?M" []
synonym: "Adult weevil head capsule width @ Detached corm Assay" EXACT []
is_a: CO_325:1000019
relationship: variable_of CO_325:0000624 ! adult weevil head capsule width
relationship: variable_of CO_325:0010205 ! adult weevil head capsule - measurement
relationship: variable_of CO_325:0100099 ! ?M

[Term]
id: CO_325:0000626
name: average adult weevil head capsule width
namespace: BananaTrait
def: "The average width of the adult weevil head" []
is_a: CO_325:1000001

[Term]
id: CO_325:0000627
name: AvgWvlAdltHdCps_M_?M
namespace: BananaTrait
def: "Measurement under microscope in ?M" []
synonym: "Average adult weevil head capsule width @ Detached corm Assay" EXACT []
is_a: CO_325:1000019
relationship: variable_of CO_325:0000626 ! average adult weevil head capsule width
relationship: variable_of CO_325:0010205 ! adult weevil head capsule - measurement
relationship: variable_of CO_325:0100099 ! ?M

[Term]
id: CO_325:0000628
name: adult weevil body length
namespace: BananaTrait
def: "The length of the adult weevil body, from the head to the tip of the abdomen" []
is_a: CO_325:1000001

[Term]
id: CO_325:0000629
name: WvlAdltBdLgt_M_?M
namespace: BananaTrait
def: "Measurement under microscope in ?M" []
synonym: "Adult weevil body length @ Detached corm Assay" EXACT []
is_a: CO_325:1000019
relationship: variable_of CO_325:0000628 ! adult weevil body length
relationship: variable_of CO_325:0010206 ! adult weevil body - measurement
relationship: variable_of CO_325:0100099 ! ?M

[Term]
id: CO_325:0000630
name: average adult weevil body length
namespace: BananaTrait
def: "The average length of the adult weevil body, from the head to the tip of the abdomen." []
is_a: CO_325:1000001

[Term]
id: CO_325:0000631
name: AvgWvlAdltBdLgt_M_?M
namespace: BananaTrait
def: "Measurement under microscope in ?M" []
synonym: "Average adult weevil body length @ Detached corm Assay" EXACT []
is_a: CO_325:1000019
relationship: variable_of CO_325:0000630 ! average adult weevil body length
relationship: variable_of CO_325:0010206 ! adult weevil body - measurement
relationship: variable_of CO_325:0100099 ! ?M

[Term]
id: CO_325:0000632
name: adult weevil body weight
namespace: BananaTrait
def: "The weight of the adult weevil" []
is_a: CO_325:1000001

[Term]
id: CO_325:0000633
name: WvlAdltBdWght_M_mg
namespace: BananaTrait
def: "electronic weighing method in mg" []
synonym: "Adult weevil body weight @ Detached corm Assay" EXACT []
is_a: CO_325:1000019
relationship: variable_of CO_325:0000632 ! adult weevil body weight
relationship: variable_of CO_325:0010206 ! adult weevil body - measurement
relationship: variable_of CO_325:0100100 ! mg

[Term]
id: CO_325:0000634
name: average adult weevil body weight
namespace: BananaTrait
def: "The average weight of the adult weevil" []
is_a: CO_325:1000001

[Term]
id: CO_325:0000635
name: AvgWvlAdltBdWght_M_mg
namespace: BananaTrait
def: "electronic weighing method in mg" []
synonym: "Average adult weevil body weight @ Detached corm Assay" EXACT []
is_a: CO_325:1000019
relationship: variable_of CO_325:0000634 ! average adult weevil body weight
relationship: variable_of CO_325:0010206 ! adult weevil body - measurement
relationship: variable_of CO_325:0100100 ! mg

[Term]
id: CO_325:0000636
name: weevil larvae head capsule width
namespace: BananaTrait
def: "The length of the weevil larvae head" []
is_a: CO_325:1000001

[Term]
id: CO_325:0000637
name: WvlLvHdCps_M_?M
namespace: BananaTrait
def: "Measurement under microscope in ?M" []
synonym: "Weevil larvae head capsule width @ Detached corm Assay" EXACT []
is_a: CO_325:1000019
relationship: variable_of CO_325:0000636 ! weevil larvae head capsule width
relationship: variable_of CO_325:0010207 ! weevil larvae head capsule - measurement
relationship: variable_of CO_325:0100099 ! ?M

[Term]
id: CO_325:0000638
name: average weevil larvae head capsule width
namespace: BananaTrait
def: "The average length of the weevil larvae head" []
is_a: CO_325:1000001

[Term]
id: CO_325:0000639
name: AvgWvlLvHdCps_M_?M
namespace: BananaTrait
def: "Measurement under microscope in ?M" []
synonym: "Average weevil larvae head capsule width @ Detached corm Assay" EXACT []
is_a: CO_325:1000019
relationship: variable_of CO_325:0000638 ! average weevil larvae head capsule width
relationship: variable_of CO_325:0010207 ! weevil larvae head capsule - measurement
relationship: variable_of CO_325:0100099 ! ?M

[Term]
id: CO_325:0000640
name: weevil larvae body length
namespace: BananaTrait
def: "The length of the weevil larvae body, from the weevil larvae head to the tip of the abdomen." []
is_a: CO_325:1000001

[Term]
id: CO_325:0000641
name: WvlLvBdLgt_M_?M
namespace: BananaTrait
def: "Measurement under microscope in ?M" []
synonym: "Weevil larvae body length @ Detached corm Assay" EXACT []
is_a: CO_325:1000019
relationship: variable_of CO_325:0000640 ! weevil larvae body length
relationship: variable_of CO_325:0010208 ! weevil larvae body length - measurement
relationship: variable_of CO_325:0100099 ! ?M

[Term]
id: CO_325:0000642
name: average weevil larvae body length
namespace: BananaTrait
def: "The average length of the weevil larvae body, from the head to the tip of the abdomen." []
is_a: CO_325:1000001

[Term]
id: CO_325:0000643
name: AvgWvlLvBdLgt_M_?M
namespace: BananaTrait
def: "Measurement under microscope in ?M" []
synonym: "Average weevil larvae body length @ Detached corm Assay" EXACT []
is_a: CO_325:1000019
relationship: variable_of CO_325:0000642 ! average weevil larvae body length
relationship: variable_of CO_325:0010208 ! weevil larvae body length - measurement
relationship: variable_of CO_325:0100099 ! ?M

[Term]
id: CO_325:0000644
name: weevil larvae weight
namespace: BananaTrait
def: "The weight of the weevil larvae" []
is_a: CO_325:1000001

[Term]
id: CO_325:0000645
name: WvlLvBdWght_M_mg
namespace: BananaTrait
def: "Measurement under microscope in mg" []
synonym: "Weevil larvae weight @ Detached corm Assay" EXACT []
is_a: CO_325:1000019
relationship: variable_of CO_325:0000644 ! weevil larvae weight
relationship: variable_of CO_325:0010209 ! weevil larvae body weight - measurement
relationship: variable_of CO_325:0100100 ! mg

[Term]
id: CO_325:0000646
name: average weevil larvae weight
namespace: BananaTrait
def: "The average weight of the adult weevil" []
is_a: CO_325:1000001

[Term]
id: CO_325:0000647
name: AvgWvlLvBdWght_M_mg
namespace: BananaTrait
def: "Measurement under microscope in mg" []
synonym: "Average weevil larvae weight @ Detached corm Assay" EXACT []
is_a: CO_325:1000019
relationship: variable_of CO_325:0000646 ! average weevil larvae weight
relationship: variable_of CO_325:0010209 ! weevil larvae body weight - measurement
relationship: variable_of CO_325:0100100 ! mg

[Term]
id: CO_325:0000648
name: percentage damage to corm cortex cross-section caused by weevils
namespace: BananaTrait
def: "The percentage of damage in the corm cortex cross-section, assessed by tunnels caused by weevils" []
synonym: "Damage index-X-inner" EXACT []
is_a: CO_325:1000001

[Term]
id: CO_325:0000649
name: DmgIdxInn_M_%
namespace: BananaTrait
def: "Visual observation in %" []
synonym: "Percentage damage to corm cortex cross-section caused by weevils @ Harvest" EXACT []
is_a: CO_325:1000020
relationship: variable_of CO_325:0000648 ! percentage damage to corm cortex cross-section caused by weevils
relationship: variable_of CO_325:0010210 ! damage index-x-inner - measurement
relationship: variable_of CO_325:0100081 ! %

[Term]
id: CO_325:0000650
name: percentage damage to corm outer cylinder cross-section caused by weevils
namespace: BananaTrait
def: "The percentage of damage in the corm outer cylinder cross-section, assessed by tunnels caused by weevils" []
synonym: "Damage index-X-outer" EXACT []
is_a: CO_325:1000001

[Term]
id: CO_325:0000651
name: DmgIdxOut_M_%
namespace: BananaTrait
def: "Visual observation in %" []
synonym: "Percentage damage to corm outer cylinder cross-section caused by weevils @ Harvest" EXACT []
is_a: CO_325:1000020
relationship: variable_of CO_325:0000650 ! percentage damage to corm outer cylinder cross-section caused by weevils
relationship: variable_of CO_325:0010211 ! damage index-x-outer - measurement
relationship: variable_of CO_325:0100081 ! %

[Term]
id: CO_325:0010000
name: date of planting - estimation
namespace: BananaMethod
def: "Record the date of event." []
is_a: CO_325:1000011
relationship: method_of CO_325:0000266 ! date of planting
relationship: method_of CO_325:0000266 ! date of planting

[Term]
id: CO_325:0010001
name: date of recognising off-type - estimation
namespace: BananaMethod
def: "Record the date of event." []
is_a: CO_325:1000011
relationship: method_of CO_325:0000269 ! date of recognising off-type
relationship: method_of CO_325:0000269 ! date of recognising off-type

[Term]
id: CO_325:0010002
name: date of damage - estimation
namespace: BananaMethod
def: "Record the date of event." []
is_a: CO_325:1000011
relationship: method_of CO_325:0000272 ! date of damage
relationship: method_of CO_325:0000272 ! date of damage

[Term]
id: CO_325:0010003
name: plant damage description - estimation
namespace: BananaMethod
def: "Record a description of the damage that occurred to the plant, e.g. leaves ripped, pseudostem snapped, plant toppled, etc." []
is_a: CO_325:1000011
relationship: method_of CO_325:0000275 ! plant damage description

[Term]
id: CO_325:0010004
name: cause of damage - estimation
namespace: BananaMethod
def: "Record the apparent cause of the damage to the plant, e.g. strong winds, weevil damage, etc." []
is_a: CO_325:1000011
relationship: method_of CO_325:0000277 ! cause of damage

[Term]
id: CO_325:0010005
name: date of death - estimation
namespace: BananaMethod
def: "Record the date of event." []
is_a: CO_325:1000011
relationship: method_of CO_325:0000279 ! date of death
relationship: method_of CO_325:0000279 ! date of death

[Term]
id: CO_325:0010006
name: cause of death - estimation
namespace: BananaMethod
def: "Record the apparent cause of death of the plant, e.g. strong winds, Fusarium wilt, etc." []
is_a: CO_325:1000011
relationship: method_of CO_325:0000282 ! cause of death

[Term]
id: CO_325:0010007
name: date of shooting - estimation
namespace: BananaMethod
def: "Record the date of event." []
is_a: CO_325:1000011
relationship: method_of CO_325:0000211 ! date of shooting
relationship: method_of CO_325:0000211 ! date of shooting

[Term]
id: CO_325:0010008
name: date of flowering - estimation
namespace: BananaMethod
def: "Record the date of event." []
is_a: CO_325:1000011
relationship: method_of CO_325:0000218 ! date of flowering
relationship: method_of CO_325:0000218 ! date of flowering

[Term]
id: CO_325:0010009
name: date of harvest - estimation
namespace: BananaMethod
def: "Record the date of event." []
is_a: CO_325:1000011
relationship: method_of CO_325:0000286 ! date of harvest
relationship: method_of CO_325:0000286 ! date of harvest

[Term]
id: CO_325:0010010
name: date of data collection - estimation
namespace: BananaMethod
def: "Record the date of event." []
is_a: CO_325:1000011
relationship: method_of CO_325:0000289 ! date of data collection
relationship: method_of CO_325:0000289 ! date of data collection

[Term]
id: CO_325:0010011
name: time from planting to shooting - computation
namespace: BananaMethod
def: "Calculate as: the time elapsed between the Date of planting and the Date of shooting, e.g. 24/09/2014 - 24/01/2014 = 243 days." []
is_a: CO_325:1000010
relationship: method_of CO_325:0000000 ! time from planting to shooting

[Term]
id: CO_325:0010012
name: plant crop cycle - computation
namespace: BananaMethod
def: "Calculate as: the time elapsed between the Date of planting to the Date of harvest, e.g. 24/12/2014 - 24/01/2014 = 334 days." []
is_a: CO_325:1000010
relationship: method_of CO_325:0000006 ! plant crop cycle

[Term]
id: CO_325:0010013
name: time from shooting to harvest - computation
namespace: BananaMethod
def: "Calculate as: the time elapsed between the Date of shooting to the Date of harvest, e.g. 24/12/2014 - 24/09/2014 = 91 days." []
is_a: CO_325:1000010
relationship: method_of CO_325:0000003 ! time from shooting to harvest

[Term]
id: CO_325:0010014
name: time from flowering to harvest - computation
namespace: BananaMethod
def: "Calculate as: the time elapsed between the Date of flowering to the Date of harvest, e.g. 24/12/2014 - 24/10/2014 = 91 days." []
is_a: CO_325:1000010
relationship: method_of CO_325:0000292 ! time from flowering to harvest

[Term]
id: CO_325:0010015
name: time from planting to death - computation
namespace: BananaMethod
def: "Calculate as: the time elapsed between the Date of planting and the Date of death, e.g. 24/05/2014 - 24/01/2014 = 120 days." []
is_a: CO_325:1000010
relationship: method_of CO_325:0000294 ! time from planting to death

[Term]
id: CO_325:0010016
name: time from harvest to death - computation
namespace: BananaMethod
def: "Calculate as: the time elapsed between the Date of harvest of the bunch of the plant from the preceeding crop cycle and the Date of observed death of the current plant, e.g. 24/03/2015 - 24/12/2014 = 90 days." []
is_a: CO_325:1000010
relationship: method_of CO_325:0000296 ! time from harvest to death

[Term]
id: CO_325:0010017
name: ratoon crop cycle - computation
namespace: BananaMethod
def: "Calculate as: the time elapsed between the Date of harvest of the bunch of the plant from the preceeding crop cycle and the Date of harvest of the bunch of the plant from the current crop cycle, e.g. 24/11/2015 - 24/12/2014 = 335 days." []
is_a: CO_325:1000010
relationship: method_of CO_325:0000298 ! ratoon crop cycle

[Term]
id: CO_325:0010018
name: date of marking youngest leaf - estimation
namespace: BananaMethod
def: "Record the date of event." []
is_a: CO_325:1000011
relationship: method_of CO_325:0000300 ! date of marking youngest leaf
relationship: method_of CO_325:0000300 ! date of marking youngest leaf

[Term]
id: CO_325:0010019
name: date of recording rank of previously marked leaf - estimation
namespace: BananaMethod
def: "Record the date of event." []
is_a: CO_325:1000011
relationship: method_of CO_325:0000303 ! date of recording rank of previously marked leaf
relationship: method_of CO_325:0000303 ! date of recording rank of previously marked leaf

[Term]
id: CO_325:0010020
name: plant height - petiole of two youngest leaves - measurement
namespace: BananaMethod
def: "Measure the distance from the pseudostem base at the ground to the intersection of the petioles of the two youngest leaves (leaf ranks 1 and 2), using a measuring pole or sliding ruler." []
is_a: CO_325:1000008
relationship: method_of CO_325:0000009 ! plant height

[Term]
id: CO_325:0010021
name: plant height - angle made between the bunch stalk and bunch cover leaf. -measurement
namespace: BananaMethod
def: "Measure of the distance from the ground to the angle made between the bunch stalk and bunch cover leaf." []
is_a: CO_325:1000008
relationship: method_of CO_325:0000009 ! plant height

[Term]
id: CO_325:0010022
name: plant height - neck of peduncle - measurement
namespace: BananaMethod
def: "Measure the distance from the pseudostem base at the ground to under the curved peduncle, using a measuring pole or sliding ruler." []
is_a: CO_325:1000008
relationship: method_of CO_325:0000307 ! plant height to neck of peduncle

[Term]
id: CO_325:0010023
name: plant circumference - measurement
namespace: BananaMethod
def: "Measure the circumference of the pseudostem of the plant at 1 m from the ground, using a tape measure." []
is_a: CO_325:1000008
relationship: method_of CO_325:0000012 ! plant circumference

[Term]
id: CO_325:0010024
name: tallest sucker height - measurement
namespace: BananaMethod
def: "On the tallest sucker, measure the distance from the pseudostem base at the ground to the intersection of the petioles of the two youngest leaves (leaf ranks 1 and 2), using a measuring pole or sliding ruler." []
is_a: CO_325:1000008
relationship: method_of CO_325:0000027 ! tallest sucker height

[Term]
id: CO_325:0010025
name: tallest sucker height - measurement at harvest
namespace: BananaMethod
def: "On the tallest sucker, measure the distance from the pseudostem base at the ground to the intersection of the petioles of the two youngest leaves (leaf ranks 1 and 2), using a measuring pole or sliding ruler." []
is_a: CO_325:1000008
relationship: method_of CO_325:0000027 ! tallest sucker height

[Term]
id: CO_325:0010026
name: number of maiden suckers - counting
namespace: BananaMethod
def: "Count how many maiden suckers are in the mat." []
is_a: CO_325:1000009
relationship: method_of CO_325:0000221 ! number of maiden suckers

[Term]
id: CO_325:0010027
name: number of sword suckers - counting
namespace: BananaMethod
def: "Count how many sword suckers are in the mat." []
is_a: CO_325:1000009
relationship: method_of CO_325:0000225 ! number of sword suckers

[Term]
id: CO_325:0010028
name: number of peeper suckers - counting
namespace: BananaMethod
def: "Count how many peeper suckers are in the mat." []
is_a: CO_325:1000009
relationship: method_of CO_325:0000229 ! number of peeper suckers

[Term]
id: CO_325:0010029
name: number of water suckers - counting
namespace: BananaMethod
def: "Count how many water suckers are in the mat." []
is_a: CO_325:1000009
relationship: method_of CO_325:0000310 ! number of water suckers

[Term]
id: CO_325:0010030
name: number of suckers - counting
namespace: BananaMethod
def: "Count how many of all types of suckers are in the mat." []
is_a: CO_325:1000009
relationship: method_of CO_325:0000024 ! number of suckers

[Term]
id: CO_325:0010031
name: bunch maturity stage - estimation
namespace: BananaMethod
def: "Estimate maturity stage of the bunch" []
is_a: CO_325:1000011
relationship: method_of CO_325:0000312 ! bunch maturity stage

[Term]
id: CO_325:0010032
name: bunch weight - measurement
namespace: BananaMethod
def: "Harvest the bunch by cutting the peduncle above the most proximal hand and immediately below the most distal hand and weigh the bunch (including the rachis), using scales." []
is_a: CO_325:1000008
relationship: method_of CO_325:0000033 ! bunch weight

[Term]
id: CO_325:0010033
name: rachis weight - measurement
namespace: BananaMethod
def: "Cut the hands off the rachis and weigh the rachis, using scales." []
is_a: CO_325:1000008
relationship: method_of CO_325:0000314 ! rachis weight

[Term]
id: CO_325:0010034
name: total finger weight - computation
namespace: BananaMethod
def: "Calculate as: the Bunch weight, minus the Rachis weight, e.g. 50 - 2 = 48." []
is_a: CO_325:1000010
relationship: method_of CO_325:0000316 ! total finger weight **check on name jeff daniells

[Term]
id: CO_325:0010035
name: number of hands in bunch - counting
namespace: BananaMethod
def: "Count how many hands are in the bunch." []
is_a: CO_325:1000009
relationship: method_of CO_325:0000036 ! number of hands in bunch

[Term]
id: CO_325:0010036
name: number of fingers in bunch - counting
namespace: BananaMethod
def: "Count how many fingers are in the bunch." []
is_a: CO_325:1000009
relationship: method_of CO_325:0000039 ! number of fingers in bunch

[Term]
id: CO_325:0010037
name: hand rank - counting
namespace: BananaMethod
def: "Record the rank (position) of a hand in the bunch, starting with the hand at the proximal end (closest to th pseudostem) of the bunch as 1 and continuing to the hand at the most distal end (closest to the male bud)." []
is_a: CO_325:1000009
relationship: method_of CO_325:0000318 ! hand rank

[Term]
id: CO_325:0010038
name: number of fingers in hand - counting
namespace: BananaMethod
def: "Count how many fingers are in a hand. Associate the data with the Hand rank. The recommendation is to collect this data from the third and seventh hand, or in cases where there are few hands, from the second and second-most distal hands." []
is_a: CO_325:1000009
relationship: method_of CO_325:0000042 ! number of fingers in hand

[Term]
id: CO_325:0010039
name: multiple number of fingers in hand - counting
namespace: BananaMethod
def: "Count how many fingers are in multiple hands. Associate the data with the Hand rank and the Number of hands measured. The recommendation is to collect this data from the third and seventh hand, or in cases where there are few hands, from the second and second-most distal hands." []
is_a: CO_325:1000009
relationship: method_of CO_325:0000320 ! multiple number of fingers in hand

[Term]
id: CO_325:0010040
name: number of hands measured - counting
namespace: BananaMethod
def: "Count how many hands are used to obtain a measurement." []
is_a: CO_325:1000009
relationship: method_of CO_325:0000322 ! number of hands measured

[Term]
id: CO_325:0010041
name: average number of fingers in hand - computation
namespace: BananaMethod
def: "Calculate as: the Multiple number of fingers in hand, divided by the Number of hands measured, e.g. 40 / 2 = 20." []
is_a: CO_325:1000010
relationship: method_of CO_325:0000324 ! average number of fingers in hand

[Term]
id: CO_325:0010042
name: number of fingers in bunch - estimation
namespace: BananaMethod
def: "Calculate as: the sum of the Number of fingers in hand from the the third and second-most distal hands (which would be Hand rank = '2' and the rank of the second-most distal hand which should be the equivalent to the Number of hands in bunch minus 1), divided by 2, and multiplied by the Number of hands in bunch, e.g. (16 + 12) / 2 * 8 = 112." []
is_a: CO_325:1000010
relationship: method_of CO_325:0000039 ! number of fingers in bunch

[Term]
id: CO_325:0010043
name: hand weight - measurement
namespace: BananaMethod
def: "Cut a hand from the rachis and weigh the hand, using scales. Associate the data with the Hand rank." []
is_a: CO_325:1000008
relationship: method_of CO_325:0000045 ! hand weight

[Term]
id: CO_325:0010044
name: multiple hand weight - measurement
namespace: BananaMethod
def: "Cut multiple hands from the rachis and weigh them together, using scales. Associate the data with the Hank rank and the Number of hands measured." []
is_a: CO_325:1000008
relationship: method_of CO_325:0000327 ! multiple hand weight

[Term]
id: CO_325:0010045
name: average hand weight - computation
namespace: BananaMethod
def: "Calculate as: the Multiple hand weight, divided by the Number of hands measured, e.g. 5.6 / 2 = 2.8." []
is_a: CO_325:1000010
relationship: method_of CO_325:0000329 ! average hand weight

[Term]
id: CO_325:0010046
name: finger weight - measurement
namespace: BananaMethod
def: "Weigh a finger, using scales. Associate the data with the Hand rank. The recommendation is to collect this data from three fingers in the middle of the outer whorl from both the third and of the seventh hand, or in cases where there are few hands, from the second and second-most distal hands." []
is_a: CO_325:1000008
relationship: method_of CO_325:0000048 ! finger weight

[Term]
id: CO_325:0010047
name: multiple finger weight - measurement
namespace: BananaMethod
def: "Weight multiple fingers together, using scales. Associate the data with the Hank rank and the Number of fingers measured. The recommendation is to collect this data from three fingers in the middle of the outer whorl from both the third and of the seventh hand, or in cases where there are few hands, from the second and second-most distal hands." []
is_a: CO_325:1000008
relationship: method_of CO_325:0000331 ! multiple finger weight

[Term]
id: CO_325:0010048
name: number of fingers measured - counting
namespace: BananaMethod
def: "Count how many fingers are used to obtain a measurement." []
is_a: CO_325:1000009
relationship: method_of CO_325:0000333 ! number of fingers measured

[Term]
id: CO_325:0010049
name: average finger weight - computation
namespace: BananaMethod
def: "Calculate as: the Multiple finger weight, divided by the Number of fingers measured, e.g. 1633 / 6 = 272." []
is_a: CO_325:1000010
relationship: method_of CO_325:0000335 ! average finger weight

[Term]
id: CO_325:0010050
name: finger dorsal length - measurement
namespace: BananaMethod
def: "Measure the length of a finger, along the external (dorsal) arc, excluding the petiole and the flower tip, using a tape measure. Associate the data with the Hand rank and the Number of fingers measured. The recommendation is to collect this data from three fingers in the middle of the outer whorl from both the third and of the seventh hand, or in cases where there are few hands, from the second and second-most distal hands." []
is_a: CO_325:1000008
relationship: method_of CO_325:0000051 ! finger external length

[Term]
id: CO_325:0010051
name: average finger external length - computation
namespace: BananaMethod
def: "Calculate as: the sum of the Finger external length measurements, divided by the Number of fingers measured, e.g. (30 + 34 + 32 + 33 + 33 + 31) / 6 = 32.1." []
is_a: CO_325:1000010
relationship: method_of CO_325:0000337 ! average finger external length

[Term]
id: CO_325:0010052
name: finger internal length - measurement
namespace: BananaMethod
def: "Measure the length of a finger, along the internal (ventral) arc, excluding the petiole and the flower tip, using a tape measure. Associate the data with the Hand rank and the Number of fingers measured. The recommendation is to collect this data from three fingers in the middle of the outer whorl from both the third and of the seventh hand, or in cases where there are few hands, from the second and second-most distal hands." []
is_a: CO_325:1000008
relationship: method_of CO_325:0000339 ! finger internal length

[Term]
id: CO_325:0010053
name: average finger internal length - computation
namespace: BananaMethod
def: "Calculate as: the sum of the Finger internal length measurements, divided by the Number of fingers measured, e.g. (27 + 31 + 29 + 30 + 30 + 28) / 6 = 29.2." []
is_a: CO_325:1000010
relationship: method_of CO_325:0000341 ! average finger internal length

[Term]
id: CO_325:0010054
name: finger circumference - measurement
namespace: BananaMethod
def: "Measure the circumference of a finger at its widest point, using a tape measure. Associate the data with the Hand rank. The recommendation is to collect this data from three fingers in the middle of the outer whorl from both the third and of the seventh hand, or in cases where there are few hands, from the second and second-most distal hands." []
is_a: CO_325:1000008
relationship: method_of CO_325:0000054 ! finger circumference
relationship: method_of CO_325:0000054 ! finger circumference

[Term]
id: CO_325:0010055
name: average finger circumference - computation
namespace: BananaMethod
def: "Calculate as: the sum of the Finger circumference measurements, divided by the Number of fingers measured, (e.g. (70 + 80 + 90 + 100 + 70 + 95) / 6 = 84.)" []
is_a: CO_325:1000010
relationship: method_of CO_325:0000344 ! average finger circumference
relationship: method_of CO_325:0000344 ! average finger circumference

[Term]
id: CO_325:0010056
name: finger lateral diameter - measurement
namespace: BananaMethod
def: "Measure the lateral diameter of a finger, from the left to the right side (not from the ventral to the dorsal side), at the widest point, using calipers. Associate the data with the Hand rank. The recommendation is to collect this data from three fingers in the middle of the outer whorl from both the third and of the seventh hand, or in cases where there are few hands, from the second and second-most distal hands." []
is_a: CO_325:1000008
relationship: method_of CO_325:0000233 ! finger lateral diameter
relationship: method_of CO_325:0000233 ! finger lateral diameter

[Term]
id: CO_325:0010057
name: average finger lateral diameter - computation
namespace: BananaMethod
def: "Calculate as: the sum of the Finger lateral diameter measurements, divided by the Number of fingers measured, e.g. (3.5 + 5.2 + 4.1 + 5 + 6 + 6.8) / 6 = 5.1." []
is_a: CO_325:1000010
relationship: method_of CO_325:0000348 ! average finger lateral diameter
relationship: method_of CO_325:0000348 ! average finger lateral diameter

[Term]
id: CO_325:0010058
name: fruit pulp lateral diameter - measurement
namespace: BananaMethod
def: "Remove the peel of a finger and measure the lateral diameter of the fruit pulp, from the left to the right side (not from the ventral to the dorsal side), at the widest point, using calipers. Associate the data with the Hand rank. The recommendation is to collect this data from three fingers in the middle of the outer whorl from both the third and of the seventh hand, or in cases where there are few hands, from the second and second-most distal hands." []
is_a: CO_325:1000008
relationship: method_of CO_325:0000240 ! fruit pulp lateral diameter
relationship: method_of CO_325:0000240 ! fruit pulp lateral diameter

[Term]
id: CO_325:0010059
name: average fruit pulp lateral diameter - computation
namespace: BananaMethod
def: "Calculate as: the sum of the Fruit pulp lateral diameter measurements, divided by the Number of fingers measured, e.g. (3.1 + 4.8 + 3.7 + 4.6 + 5.6 + 6.4) / 6 = 4.7." []
is_a: CO_325:1000010
relationship: method_of CO_325:0000352 ! average fruit pulp lateral diameter
relationship: method_of CO_325:0000352 ! average fruit pulp lateral diameter

[Term]
id: CO_325:0010060
name: finger peel thickness - measurement
namespace: BananaMethod
def: "Remove the peel of a finger that is at a 'ready to eat' stage, and measure the thickness of the peel, using calipers. Associate the data with the Hank rank. The recommendation is to collect this data from three fingers in the middle of the outer whorl from both the third and of the seventh hand, or in cases where there are few hands, from the second and second-most distal hands." []
is_a: CO_325:1000008
relationship: method_of CO_325:0000236 ! finger peel thickness

[Term]
id: CO_325:0010061
name: average finger peel thickness - computation
namespace: BananaMethod
def: "Calculate as: the sum of the Finger peel thickness measurements, divided by the Number of fingers measured, e.g. (2 + 2 + 2 + 3 + 2 + 3 + 3) / 6 = 2." []
is_a: CO_325:1000010
relationship: method_of CO_325:0000355 ! average finger peel thickness

[Term]
id: CO_325:0010062
name: number of plants planted - computation
namespace: BananaMethod
def: "Calculate as: the sum of the number of values for Date of planting." []
is_a: CO_325:1000010
relationship: method_of CO_325:0000357 ! number of plants planted

[Term]
id: CO_325:0010063
name: plant spacing - computation
namespace: BananaMethod
def: "Calculate as: multiply the distance of the spacing between the plants, both latitudinally and longitudinally, e.g. 2 m x 3 m = 6 m2." []
is_a: CO_325:1000010
relationship: method_of CO_325:0000359 ! plant spacing

[Term]
id: CO_325:0010064
name: plant density - computation
namespace: BananaMethod
def: "Calculate as: number of square metres in the area unit of choice, divided by the Plant spacing, e.g. 10,000 square metres in 1 hectare / 6 = 1,667 plants/ha." []
is_a: CO_325:1000010
relationship: method_of CO_325:0000361 ! plant density

[Term]
id: CO_325:0010065
name: number of plants dead - computation
namespace: BananaMethod
def: "Calculate as: the sum of the number of values for Date of death." []
is_a: CO_325:1000010
relationship: method_of CO_325:0000363 ! number of plants dead

[Term]
id: CO_325:0010066
name: number of plants harvested - computation
namespace: BananaMethod
def: "Calculate as: the sum of the number of values for Date of harvest." []
is_a: CO_325:1000010
relationship: method_of CO_325:0000365 ! number of plants harvested

[Term]
id: CO_325:0010067
name: number of plants not harvested - computation
namespace: BananaMethod
def: "Calculate as: the Number of plants planted, minus the Number of plants dead, minus the Number of plants harvested, e.g. 24 - 4 - 18 = 2." []
is_a: CO_325:1000010
relationship: method_of CO_325:0000367 ! number of plants not harvested

[Term]
id: CO_325:0010068
name: death proportion - computation
namespace: BananaMethod
def: "Calculate as: the Number of plants dead, divided by the Number of plants planted, e.g. 4 / 24 = 0.17." []
is_a: CO_325:1000010
relationship: method_of CO_325:0000369 ! death proportion

[Term]
id: CO_325:0010069
name: death density - computation
namespace: BananaMethod
def: "Calculate as: the Plant density multiplied by the Death proportion, e.g. 1,667 * 0.17 = 283." []
is_a: CO_325:1000010
relationship: method_of CO_325:0000371 ! death density

[Term]
id: CO_325:0010070
name: harvest proportion - computation
namespace: BananaMethod
def: "Calculate as: the Number of plants harvested, divided by the Number of plants planted, e.g. 18 / 24 = 0.75." []
is_a: CO_325:1000010
relationship: method_of CO_325:0000373 ! harvest proportion

[Term]
id: CO_325:0010071
name: harvest density - computation
namespace: BananaMethod
def: "Calculate as: the Plant density multiplied by the Harvest proportion, e.g. 1,667 * 0.75 = 1,250." []
is_a: CO_325:1000010
relationship: method_of CO_325:0000375 ! harvest density

[Term]
id: CO_325:0010072
name: non-harvest proportion - computation
namespace: BananaMethod
def: "Calculate as: the Number of plants not harvested, divided by the Number of plants planted, e.g. 2 / 24 = 0.08." []
is_a: CO_325:1000010
relationship: method_of CO_325:0000377 ! non-harvest proportion

[Term]
id: CO_325:0010073
name: non-harvest density - computation
namespace: BananaMethod
def: "Calculate as: the Plant density multiplied by the Non-harvest proportion, e.g. 1,667 * 0.08 = 133." []
is_a: CO_325:1000010
relationship: method_of CO_325:0000379 ! non-harvest density

[Term]
id: CO_325:0010074
name: annual crop cycle proportion - computation
namespace: BananaMethod
def: "Calculate as: the length of a year (e.g. 365 days) divided by the Plant crop cycle or the Ratoon crop cycle, e.g. 365 / 334 = 1.09." []
is_a: CO_325:1000010
relationship: method_of CO_325:0000381 ! annual crop cycle proportion **ask jeff if this already has a different name

[Term]
id: CO_325:0010075
name: annual plant productivity - computation
namespace: BananaMethod
def: "Calculate as: the Bunch weight multiplied by the Annual crop cycle proportion, e.g. 48 * 1.09 = 52.32." []
is_a: CO_325:1000010
relationship: method_of CO_325:0000383 ! plant annual yield

[Term]
id: CO_325:0010076
name: actual annual yield - computation
namespace: BananaMethod
def: "Calculate as: the Bunch weight divided by 1,000, multiplied by the Annual crop cycle proportion, multiplied by the Harvest density, e.g. (50 / 1,000) * 1.09 * 1,250 = 68.13." []
is_a: CO_325:1000010
relationship: method_of CO_325:0000385 ! average actual annual yield

[Term]
id: CO_325:0010077
name: potential annual yield - computation
namespace: BananaMethod
def: "Calculate as: the Bunch weight divided by 1,000, multiplied by the Annual crop cycle proportion, multiplied by the Plant density, e.g. (50 / 1,000) * 1.09 * 1,667 = 90.85." []
is_a: CO_325:1000010
relationship: method_of CO_325:0000387 ! average potential annual yield

[Term]
id: CO_325:0010078
name: fruit pendulance - estimation
namespace: BananaMethod
def: "Visual estimation of fruit pendulance on a bunch, for Early Evaluation Trial stage only." []
is_a: CO_325:1000011
relationship: method_of CO_325:0000389 ! overall fruit pendulance

[Term]
id: CO_325:0010079
name: bunch quality - estimation
namespace: BananaMethod
def: "Visual estimation of bunch quality, for Early Evaluation Trial stage only." []
is_a: CO_325:1000011
relationship: method_of CO_325:0000391 ! overall bunch quality

[Term]
id: CO_325:0010080
name: fruit parthenocarpy - estimation
namespace: BananaMethod
def: "Visual estimation of a fruit fill, (or parthenocarpic) for Early Evaluation Trial stage only." []
is_a: CO_325:1000011
relationship: method_of CO_325:0000393 ! partenocarpy

[Term]
id: CO_325:0010081
name: sucker quality - estimation
namespace: BananaMethod
def: "Visual estimation of suckering, for Early Evaluation Trial stage only." []
is_a: CO_325:1000011
relationship: method_of CO_325:0000395 ! overall suckering quality

[Term]
id: CO_325:0010082
name: dwarfism - estimation
namespace: BananaMethod
def: "Visual estimation of dwarfism, for Early Evaluation Trial stage only." []
is_a: CO_325:1000011
relationship: method_of CO_325:0000397 ! dwarfism

[Term]
id: CO_325:0010083
name: trial group id -counting
namespace: BananaMethod
def: "Assign the trial group a unique identifier, e.g. IMTP 3" []
is_a: CO_325:1000009
relationship: method_of CO_325:0000399 ! trial group id

[Term]
id: CO_325:0010084
name: trial id -counting
namespace: BananaMethod
def: "Assign the field trial a unique identifier, e.g. IMTP 3 - Cameroon BLS" []
is_a: CO_325:1000009
relationship: method_of CO_325:0000401 ! trial id

[Term]
id: CO_325:0010085
name: block id -counting
namespace: BananaMethod
def: "Assign each experimental block within the field trial a unique identifier, e.g. 1, 2, 3, 4, or A, B, C, D, etc." []
is_a: CO_325:1000009
relationship: method_of CO_325:0000403 ! block id

[Term]
id: CO_325:0010086
name: row id -counting
namespace: BananaMethod
def: "Assign each row (latitudinally) within the field trial a unique identifier, e.g. 1, 2, 3, 4, or A, B, C, D, etc." []
is_a: CO_325:1000009
relationship: method_of CO_325:0000405 ! row id

[Term]
id: CO_325:0010087
name: column id -counting
namespace: BananaMethod
def: "Assign each column (longitudinally) within the field trial a unique identifier, e.g. 1, 2, 3, 4, or A, B, C, D, etc." []
is_a: CO_325:1000009
relationship: method_of CO_325:0000407 ! column id

[Term]
id: CO_325:0010088
name: spatial position id -counting
namespace: BananaMethod
def: "Calculate as: the concatenation of Block ID, Row ID, and Column ID, e.g. 1_A_26" []
is_a: CO_325:1000009
relationship: method_of CO_325:0000409 ! spatial position id

[Term]
id: CO_325:0010089
name: accession id -counting
namespace: BananaMethod
def: "Record the genebank accession code of the genotype of the plant, if the planting material was sourced from a genebank either directly or secondarily through a tissue-culture provider." []
is_a: CO_325:1000009
relationship: method_of CO_325:0000411 ! accession id

[Term]
id: CO_325:0010090
name: genotype id -counting
namespace: BananaMethod
def: "Assign the genotype a unique identifier." []
is_a: CO_325:1000009
relationship: method_of CO_325:0000413 ! genotype id

[Term]
id: CO_325:0010091
name: genotype purpose -counting
namespace: BananaMethod
def: "Record the reason for including the genotype in the field trial." []
is_a: CO_325:1000009
relationship: method_of CO_325:0000415 ! genotype purpose

[Term]
id: CO_325:0010092
name: mat id -counting
namespace: BananaMethod
def: "Calculate as: ... = the spatial position ** but with an extra identifier to show whether it is the first, or whether plant has died and needed to be replanted, so is therefore the second...  Does that identifier need to have its own trait?" []
is_a: CO_325:1000009
relationship: method_of CO_325:0000417 ! mat id

[Term]
id: CO_325:0010093
name: crop cycle id -counting
namespace: BananaMethod
def: "Assign each crop cycle a unique identifier, e.g. 1 = first plant that is planted, 2 = first ratoon plant, 3 = second ratoon plant, etc." []
is_a: CO_325:1000009
relationship: method_of CO_325:0000419 ! crop cycle id

[Term]
id: CO_325:0010094
name: plant id -counting
namespace: BananaMethod
def: "Calculate as: the concatenation of Spatial ID, Genotype ID, and Crop cycle ID, e.g. 1A26_3_1" []
is_a: CO_325:1000009
relationship: method_of CO_325:0000421 ! plant id

[Term]
id: CO_325:0010095
name: plant barcode -counting
namespace: BananaMethod
def: "Assign the plant a unique identifier in the form of a barcode." []
is_a: CO_325:1000009
relationship: method_of CO_325:0000423 ! plant barcode

[Term]
id: CO_325:0010096
name: pseudostem height - estimation
namespace: BananaMethod
def: "Recorded from the base of the pseudostem to the emerging point of the peduncle." []
is_a: CO_325:1000011
relationship: method_of CO_325:0000425 ! pseudostem height

[Term]
id: CO_325:0010097
name: pseudostem colour - estimation
namespace: BananaMethod
def: "Detach the outermost sheath from the pseudostem (the sheath should not be too dry). Record the overall impression of colour of the exposed surface of the underlying pseudostem. Note that this 'main colour' should cover more than 75% of the underlying pseudostem surface. Use colour chart A and observe out of direct sunlight." []
is_a: CO_325:1000011
relationship: method_of CO_325:0000243 ! main underlying colour of pseudostem

[Term]
id: CO_325:0010098
name: blotches area - estimation
namespace: BananaMethod
def: "Record the relative surface area coverage by blotches. [x Look at several plants if possible to get an overall idea. Observe at flowering time]." []
is_a: CO_325:1000011
relationship: method_of CO_325:0000427 ! blotches relative area at petiole base
relationship: method_of CO_325:0000427 ! blotches relative area at petiole base

[Term]
id: CO_325:0010099
name: blotches colour - estimation
namespace: BananaMethod
def: "Observe visually the colour of the blotches on the upper leaf sheath." []
is_a: CO_325:1000011
relationship: method_of CO_325:0000430 ! blotches colour at the petiole base
relationship: method_of CO_325:0000430 ! blotches colour at the petiole base

[Term]
id: CO_325:0010100
name: margin behaviour on petiole canal of third leaf  - estimation
namespace: BananaMethod
def: "The third leaf (Leaf III) is counted from the last leaf produced before [x bunch emergence] [shooting]. Cut the petiole halfway between the pseudostem and the leaf blade and examine the cross section. [x Observe at flowering time]." []
is_a: CO_325:1000011
relationship: method_of CO_325:0000433 ! margin behaviour on petiole canal of third leaf
relationship: method_of CO_325:0000433 ! margin behaviour on petiole canal of third leaf

[Term]
id: CO_325:0010101
name: winged petiole margin - estimation
namespace: BananaMethod
def: "Observations on the margins and petiole wings should be made where the petiole and pseudostem meet at shooting. Margin is the part of the petiole that can be bent outwards/inwards. [x Observe at flowering time.]" []
is_a: CO_325:1000011
relationship: method_of CO_325:0000256 ! petiole margins winged
relationship: method_of CO_325:0000256 ! petiole margins winged

[Term]
id: CO_325:0010102
name: petiole margin clasping - estimation
namespace: BananaMethod
def: "Observations on the margins and petiole wings should be made where the petiole and pseudostem meet at shooting. Observation should be made at shooting on the neck, where the petiole and pseudostem meet. Margin is the part of the petiole that can be bent outwards/inwards. [x Observe at flowering time.]" []
is_a: CO_325:1000011
relationship: method_of CO_325:0000260 ! petiole margins clasping

[Term]
id: CO_325:0010103
name: petiole margin colour - estimation
namespace: BananaMethod
def: "Observations on the margins and petiole wings should be made where the petiole and pseudostem meet at shooting. Use colour chart A and observe out of direct sunlight. Record the colour of the margin (general colour is below the rim). [x Observe at flowering time.]" []
is_a: CO_325:1000011
relationship: method_of CO_325:0000264 ! petiole margin colour
relationship: method_of CO_325:0000264 ! petiole margin colour

[Term]
id: CO_325:0010104
name: colour line along edge of petiole margin - estimation
namespace: BananaMethod
def: "Observations on the margins and petiole wings should be made where the petiole and pseudostem meet at shooting. Record on the last developed leaf at [x flowering stage] [shooting]." []
is_a: CO_325:1000011
relationship: method_of CO_325:0000248 ! colour line along edge of petiole margin

[Term]
id: CO_325:0010105
name: pigmentation of outer surface of cigar leaf - estimation
namespace: BananaMethod
def: "Visually observe the pigmentation of the outer surface of the cigar leaf of a developed sucker or on another plant of the same accession. [x Observation should be made before shooting, on a developed sucker or on another plant of the same accession.]" []
is_a: CO_325:1000011
relationship: method_of CO_325:0000252 ! pigmentation of outer surface of cigar leaf on sucker

[Term]
id: CO_325:0010106
name: bunch position - estimation
namespace: BananaMethod
def: "Visually observe the angle of the bunch and choose the option that is most similar, from the 5 schematic drawings of descriptor 6.4.6 in the reference material." []
is_a: CO_325:1000011
relationship: method_of CO_325:0000438 ! bunch position

[Term]
id: CO_325:0010107
name: bunch shape - estimation
namespace: BananaMethod
def: "Visually observe the shape of the mature bunch on a fully developed plant that is not experiencing environmental stress and choose the option that is most similar, from the 4 photos of descriptor 6.4.7. in the reference material." []
is_a: CO_325:1000011
relationship: method_of CO_325:0000440 ! bunch shape

[Term]
id: CO_325:0010108
name: male rachis type - estimation
namespace: BananaMethod
def: "Visually observe the part of the rachis between the last hand and the male bud. Truncated means there is no bract scar below the last hand. Present means there is a degenerated or persistent male bud" []
is_a: CO_325:1000011
relationship: method_of CO_325:0000442 ! male rachis type

[Term]
id: CO_325:0010109
name: male rachis position - estimation
namespace: BananaMethod
def: "Visually observe the male rachis position (the part between the last hand and the male bud) and choose the option that is most similar, from the 5 schematic drawings of descriptor 6.4.12 in the reference material." []
is_a: CO_325:1000011
relationship: method_of CO_325:0000444 ! male rachis position

[Term]
id: CO_325:0010110
name: male rachis appearance - estimation
namespace: BananaMethod
def: "Visually observe the male rachis appearance and choose the option that is most similar." []
is_a: CO_325:1000011
relationship: method_of CO_325:0000446 ! male rachis appearance

[Term]
id: CO_325:0010111
name: male bud shape - computation
namespace: BananaMethod
def: "Calculate the ratio w/y, i.e. the broadest width of the male bud to the total length of the male bud. Do not measure the dimensions along the bud but rather on a projection/outline of the bud (e.g. trace the outline of the bud on paper) and use ruler or measuring tape." []
is_a: CO_325:1000010
relationship: method_of CO_325:0000448 ! male bud shape
relationship: method_of CO_325:0000448 ! male bud shape

[Term]
id: CO_325:0010112
name: male bud length - measurement
namespace: BananaMethod
def: "Measure the length (y) of a projection/outline of the male bud on paper, with a measuring tape or ruler." []
is_a: CO_325:1000008
relationship: method_of CO_325:0000451 ! male bud length

[Term]
id: CO_325:0010113
name: male bud size - measurement
namespace: BananaMethod
def: "Length and maximum diamter of male bud at harvest." []
is_a: CO_325:1000008
relationship: method_of CO_325:0000451 ! male bud length

[Term]
id: CO_325:0010114
name: male bud shoulder - computation
namespace: BananaMethod
def: "Calculate the ratio w/y, i.e. the broadest width of the male bud to the total length of the male bud. Do not measure the dimensions along the bud but rather on a projection/outline of the bud (e.g. trace the outline of the bud on paper) and use ruler or measuring tape" []
is_a: CO_325:1000010
relationship: method_of CO_325:0000454 ! male bud shoulder

[Term]
id: CO_325:0010115
name: bract apex shape - estimation
namespace: BananaMethod
def: "Refers to the first external unlifted bract. Visually observe the apex shape of flattened bracts to determine shape and choose the option that is most similar, from the 4 photos of descriptor 6.5.2. in the reference material." []
is_a: CO_325:1000011
relationship: method_of CO_325:0000456 ! bract apex shape
relationship: method_of CO_325:0000456 ! bract apex shape

[Term]
id: CO_325:0010116
name: bract imbrication at apex of male bud - estimation
namespace: BananaMethod
def: "Visually observe the bract imbrication of the apex of the male bud and choose the option that is most similar, from the 3 photos of descriptor 6.5.3 in the reference material." []
is_a: CO_325:1000011
relationship: method_of CO_325:0000459 ! bract imbrication at apex of male bud

[Term]
id: CO_325:0010117
name: bract behaviour before falling - estimation
namespace: BananaMethod
def: "Visually observe the last bract to lift from the hands, ideally when the bract has lifted to a horizontal position, and choose the option that is most similar, from the 2 photos of descriptpr 6.5.12 in the reference material." []
is_a: CO_325:1000011
relationship: method_of CO_325:0000461 ! bract behaviour before falling

[Term]
id: CO_325:0010118
name: colour of bract external face - estimation
namespace: BananaMethod
def: "Visually observe the colour of the external face of the first unlifted bract. Use colour chart A and observe out of direct sunlight." []
is_a: CO_325:1000011
relationship: method_of CO_325:0000463 ! colour of bract external face
relationship: method_of CO_325:0000463 ! colour of bract external face

[Term]
id: CO_325:0010119
name: colour of bract internal face - estimation
namespace: BananaMethod
def: "Visually observe the colour of the internal face of the first unlifted bract. Use colour chart A and observe out of direct sunlight." []
is_a: CO_325:1000011
relationship: method_of CO_325:0000466 ! colour of bract internal face
relationship: method_of CO_325:0000466 ! colour of bract internal face

[Term]
id: CO_325:0010120
name: compound tepal main colour - estimation
namespace: BananaMethod
def: "The following flower descriptors refer to the flowers at the axil of the first external unlifted bract. Fresh material must be used (make the observation as soon as you detach the bract/flower from the rachis). Visually observe the colour of the backside middle of tepal. Use colour chart B and observe out of direct sunlight." []
is_a: CO_325:1000011
relationship: method_of CO_325:0000469 ! compound tepal main colour
relationship: method_of CO_325:0000469 ! compound tepal main colour

[Term]
id: CO_325:0010121
name: lobe colour of tip of compound tepal - estimation
namespace: BananaMethod
def: "The following flower descriptors refer to the flowers at the axil of the first external unlifted bract. Fresh material must be used (make the observation as soon as you detach the bract/flower from the rachis). Visually observe the colour of the lobe at the tip of the tepal. Use colour chart B and observe out of direct sunlight." []
is_a: CO_325:1000011
relationship: method_of CO_325:0000472 ! lobe colour of tip of compound tepal
relationship: method_of CO_325:0000472 ! lobe colour of tip of compound tepal

[Term]
id: CO_325:0010122
name: anther colour - estimation
namespace: BananaMethod
def: "The following flower descriptors refer to the flowers at the axil of the first external unlifted bract. Fresh material must be used (make the observation as soon as you detach the bract/flower from the rachis). Visually observe the anther colour on the face opposite to the dehiscence split of the anther. Use colour chart B and observe out of direct sunlight." []
is_a: CO_325:1000011
relationship: method_of CO_325:0000475 ! anther colour
relationship: method_of CO_325:0000475 ! anther colour

[Term]
id: CO_325:0010123
name: number of hands on whole bunch - counting
namespace: BananaMethod
def: "On a bunch with mostly hands of > 10 fingers, a possible ultimate hand with 1-5 (rather smaller) fingers should not be counted." []
is_a: CO_325:1000009
relationship: method_of CO_325:0000478 ! number of hands on whole bunch

[Term]
id: CO_325:0010124
name: number of fruits on mid-hand of the bunch - counting
namespace: BananaMethod
def: "Count only fully developed fruit. If there is an even number of hands, there will be two middle hands. Count the middle hand that developed first." []
is_a: CO_325:1000009
relationship: method_of CO_325:0000480 ! number of fruits on mid-hand of the bunch

[Term]
id: CO_325:0010125
name: fruit length - exact value - measurement
namespace: BananaMethod
def: "Measure the length of the internal arc of a fruit, without pedicel. Record on the inner fruit in the middle of the mid-hand of the bunch. If there is an even number of hands, there will be two middle hands so use the upper hand that developed first. Record the exact value." []
is_a: CO_325:1000008
relationship: method_of CO_325:0000482 ! fruit length

[Term]
id: CO_325:0010126
name: fruit length - range - measurement
namespace: BananaMethod
def: "Measure the length of the internal arc of a fruit, without pedicel. Record on the inner fruit in the middle of the mid-hand of the bunch. If there is an even number of hands, there will be two middle hands so use the upper hand that developed first. Record the range." []
is_a: CO_325:1000008
relationship: method_of CO_325:0000482 ! fruit length

[Term]
id: CO_325:0010127
name: fruit shape of curve - estimation
namespace: BananaMethod
def: "Visually observe the shape of the curve of the fruit and choose the option that is most similar, from the 5 photos of descriptor 6.7.4. in the reference material. Observe the inner fruit in the middle of the mid-hand of the bunch. In case of an asymmetric bunch that has straight and curved fruits, please indicate it in the note section and score only the fruit on the upper side of the bunch." []
is_a: CO_325:1000011
relationship: method_of CO_325:0000485 ! fruit shape of curve
relationship: method_of CO_325:0000485 ! fruit shape of curve

[Term]
id: CO_325:0010128
name: fruit apex point - estimation
namespace: BananaMethod
def: "Visually observe the fruit apex point and choose the option that is most similar, from the 5 photos of descriptor 6.7.6 in the reference material." []
is_a: CO_325:1000011
relationship: method_of CO_325:0000488 ! fruit apex point

[Term]
id: CO_325:0010129
name: remains of flower relicts at fruit apex - estimation
namespace: BananaMethod
def: "Visually observe the remains, or not, of flower relicts at the finger apex, and choose the option that is most similar, from the 4 photos of descriptor 6.7.7 in the reference materials." []
is_a: CO_325:1000011
relationship: method_of CO_325:0000490 ! remains of flower relicts at fruit apex
relationship: method_of CO_325:0000490 ! remains of flower relicts at fruit apex

[Term]
id: CO_325:0010130
name: fruit pedicel length - exact value - measurement
namespace: BananaMethod
def: "Measure from the scar on the rachis until the beginning of the fruit. Record on the inner fruit in the middle of the mid-hand of the bunch. Tip: use string to measure or trace outline of fruit on paper. Record the exact value." []
is_a: CO_325:1000008
relationship: method_of CO_325:0000493 ! fruit pedicel length

[Term]
id: CO_325:0010131
name: fruit pedical length - range - measurement
namespace: BananaMethod
def: "Measure from the scar on the rachis until the beginning of the fruit. Record on the inner fruit in the middle of the mid-hand of the bunch. Tip: use string to measure or trace outline of fruit on paper. Record the range." []
is_a: CO_325:1000008
relationship: method_of CO_325:0000493 ! fruit pedicel length

[Term]
id: CO_325:0010132
name: fusion of pedicels - estimation
namespace: BananaMethod
def: "Visually observe the fusion of pedicels and choose the option that is most similar, from the 3 photos of descriptor 6.7.11. in the reference materials. Observe before they join the rachis at the bract scar. Look upwards from the bottom of the bunch." []
is_a: CO_325:1000011
relationship: method_of CO_325:0000496 ! fusion of pedicels

[Term]
id: CO_325:0010133
name: visual appearance  - estimation
namespace: BananaMethod
def: "Subjective visual assessment of smashed and unsmashed fruit pulp" []
is_a: CO_325:1000011
relationship: method_of CO_325:0000498 ! fruit  smashed pulp colour
relationship: method_of CO_325:0000500 ! fruit  unsmashed pulp colour

[Term]
id: CO_325:0010134
name: taste  - estimation
namespace: BananaMethod
def: "Subjective taste assessment of smashed and unsmashed fruit pulp" []
is_a: CO_325:1000011
relationship: method_of CO_325:0000502 ! fruit  smashed pulp taste
relationship: method_of CO_325:0000504 ! fruit unsmashed pulp taste

[Term]
id: CO_325:0010135
name: finger feel  - estimation
namespace: BananaMethod
def: "Finger feel assessment of smashed and unsmashed fruit pulp" []
is_a: CO_325:1000011
relationship: method_of CO_325:0000506 ! fruit  smashed pulp texture
relationship: method_of CO_325:0000508 ! fruit  unsmashed pulp texture

[Term]
id: CO_325:0010136
name: smoothness-mouth feel - estimation
namespace: BananaMethod
def: "Mouth feel assessment of smashed and unsmashed fruit pulp" []
is_a: CO_325:1000011
relationship: method_of CO_325:0000510 ! fruit   smashed pulp smoothness-mouth feel
relationship: method_of CO_325:0000512 ! fruit   unsmashed pulp smoothness-mouth feel

[Term]
id: CO_325:0010137
name: nosal smell  - estimation
namespace: BananaMethod
def: "Nosal smell assessment of smashed and unsmashed fruit pulp aromas" []
is_a: CO_325:1000011
relationship: method_of CO_325:0000514 ! fruit smashed pulp aroma/smell

[Term]
id: CO_325:0010138
name: peripheral damage - measurement
namespace: BananaMethod
def: "Visual observation" []
is_a: CO_325:1000008
relationship: method_of CO_325:0000516 ! percentage damage to periphery of peeled corm caused by weevils

[Term]
id: CO_325:0010139
name: nematode multiplication from single root inoculation - computation
namespace: BananaMethod
def: "calculation from count" []
is_a: CO_325:1000009
relationship: method_of CO_325:0000518 ! nematode reproduction factor (microplot screening)

[Term]
id: CO_325:0010140
name: percentage of root necrosis - method
namespace: BananaMethod
def: "Visual observation on 5 roots of 10 cm length each from around the the plants. Split lengthwise and % necross assessed. (each root 20% total)" []
is_a: CO_325:1000009
relationship: method_of CO_325:0000123 ! root necrosis

[Term]
id: CO_325:0010141
name: number of functional roots - method
namespace: BananaMethod
def: "visual counting method from  a 30 cm square hole one meter from plant" []
is_a: CO_325:1000009
relationship: method_of CO_325:0000111 ! number of functional roots

[Term]
id: CO_325:0010142
name: number of dead roots - method
namespace: BananaMethod
def: "visual counting method  from a 30 cm square hole one meter from plant" []
is_a: CO_325:1000009
relationship: method_of CO_325:0000108 ! number of dead roots

[Term]
id: CO_325:0010143
name: number of nematodes (unclassified spp.) per unit fresh root weight - method
namespace: BananaMethod
def: "Count from 100 ml of soil sample" []
is_a: CO_325:1000009
relationship: method_of CO_325:0000520 ! nematode population density by species in soil

[Term]
id: CO_325:0010144
name: number of nematodes (radopholus similis ) per  unit fresh root weight - method
namespace: BananaMethod
def: "Count from 100 ml of soil sample" []
is_a: CO_325:1000009
relationship: method_of CO_325:0000522 ! number of radopholus similis per soil sample

[Term]
id: CO_325:0010145
name: number of nematodes (helicotylenchus multicinctus) per  unit fresh root weight - method
namespace: BananaMethod
def: "Count from 100 ml of soil sample" []
is_a: CO_325:1000009
relationship: method_of CO_325:0000523 ! number of helicotylenchus multicinctus per soil sample

[Term]
id: CO_325:0010146
name: number of nematodes (rotylenchulus spp.) per  unit fresh root weight - method
namespace: BananaMethod
def: "Count from 100 ml of soil sample" []
is_a: CO_325:1000009
relationship: method_of CO_325:0000524 ! number of rotylenchulus spp.per soil sample

[Term]
id: CO_325:0010147
name: number of nematodes (meloidogyne spp.) per  unit fresh root weight - method
namespace: BananaMethod
def: "Count from 100 ml of soil sample" []
is_a: CO_325:1000009
relationship: method_of CO_325:0000526 ! number of meloidogyne spp. per  soil sample

[Term]
id: CO_325:0010148
name: number of nematodes (pratylenchus spp.) per  unit fresh root weight - method
namespace: BananaMethod
def: "Count from 100 ml of soil sample" []
is_a: CO_325:1000009
relationship: method_of CO_325:0000527 ! number of pratylenchus spp. per soil sample

[Term]
id: CO_325:0010149
name: number of nematodes (hoplolaimus spp.) per  unit fresh root weight - method
namespace: BananaMethod
def: "Count from 100 ml of soil sample" []
is_a: CO_325:1000009
relationship: method_of CO_325:0000528 ! number of hoplolaimus spp. per soil sample

[Term]
id: CO_325:0010150
name: number of nematodes (pratylenchus goodeyi) per  unit fresh root weight - method
namespace: BananaMethod
def: "Count from 100 ml of soil sample" []
is_a: CO_325:1000009
relationship: method_of CO_325:0000529 ! number of pratylenchus goodeyi per soil sample

[Term]
id: CO_325:0010151
name: number of nematodes (pratylenchus coffeae) per  unit fresh root weight - method
namespace: BananaMethod
def: "Count from 100 ml of soil sample" []
is_a: CO_325:1000009
relationship: method_of CO_325:0000530 ! number of pratylenchus coffeae per soil sample

[Term]
id: CO_325:0010152
name: number of nematodes per  unit fresh root weight
namespace: BananaMethod
def: "Count from 10 g of chopped roots from the tested banana plant sample" []
is_a: CO_325:1000009
relationship: method_of CO_325:0000531 ! nematode population density by species in fresh roots

[Term]
id: CO_325:0010153
name: number of nematodes (radopholus similis ) per  unit fresh root weight -method
namespace: BananaMethod
def: "Count from 10 g of chopped roots from the tested banana plant sample" []
is_a: CO_325:1000009
relationship: method_of CO_325:0000533 ! number of radopholus similis per fresh root weight

[Term]
id: CO_325:0010154
name: number of nematodes (meloidogyne spp.)  per  unit fresh root weight -method
namespace: BananaMethod
def: "Count from 10 g of chopped roots from the tested banana plant sample" []
is_a: CO_325:1000009
relationship: method_of CO_325:0000535 ! number of meloidogyne spp. per fresh root weight

[Term]
id: CO_325:0010155
name: number of nematodes (pratylenchus spp.)  per  unit fresh root weight -method
namespace: BananaMethod
def: "Count from 10 g of chopped roots from the tested banana plant sample" []
is_a: CO_325:1000009
relationship: method_of CO_325:0000537 ! number of pratylenchus spp. per fresh root weight

[Term]
id: CO_325:0010156
name: number of nematodes (hoplolaimus spp.)  per  unit fresh root weight -method
namespace: BananaMethod
def: "Count from 10 g of chopped roots from the tested banana plant sample" []
is_a: CO_325:1000009
relationship: method_of CO_325:0000539 ! number of hoplolaimus spp. per fresh root weight

[Term]
id: CO_325:0010157
name: number of nematodes (pratylenchus goodeyi)  per  unit fresh root weight -method
namespace: BananaMethod
def: "Count from 10 g of chopped roots from the tested banana plant sample" []
is_a: CO_325:1000009
relationship: method_of CO_325:0000541 ! number of pratylenchus goodeyi per fresh root weight

[Term]
id: CO_325:0010158
name: number of nematodes (pratylenchus coffeae)  per  unit fresh root weight -method
namespace: BananaMethod
def: "Count from 10 g of chopped roots from the tested banana plant sample" []
is_a: CO_325:1000009
relationship: method_of CO_325:0000543 ! number of pratylenchus coffeae per fresh root weight

[Term]
id: CO_325:0010159
name: youngest leaf spotted - counting
namespace: BananaMethod
def: "Record the rank of the youngest leaf spotted (the first fully unfurled leaf with at least 10 discrete, mature, necrotic lesions or one large necrotic area with 10 light-coloured dry centres), counting the rank by starting with the youngest completely unrolled leaf as 1 and moving downwards, associating the data with the Date of data collection." []
is_a: CO_325:1000009
relationship: method_of CO_325:0000099 ! youngest leaf spotted

[Term]
id: CO_325:0010160
name: date of first youngest leaf spotted - estimation
namespace: BananaMethod
def: "Record the date of event." []
is_a: CO_325:1000011
relationship: method_of CO_325:0000545 ! date of first youngest leaf spotted
relationship: method_of CO_325:0000545 ! date of first youngest leaf spotted

[Term]
id: CO_325:0010161
name: rank of oldest standing leaf - counting
namespace: BananaMethod
def: "Record the rank of the oldest standing leaf (with an erect petiole), counting the rank by starting with the youngest completely unrolled leaf as 1 and moving downwards, associating the data with the Date of data collection." []
is_a: CO_325:1000009
relationship: method_of CO_325:0000548 ! rank of oldest standing leaf

[Term]
id: CO_325:0010162
name: black sigatoka disease infection index - computation
namespace: BananaMethod
def: "Calculate as: ((((Number of leaves with black Sigatoka disease severity grade 0, multiplied by 0), plus (Number of leaves with black Sigatoka disease severity grade 1, multiplied by 1), plus (Number of leaves with black Sigatoka disease severity grade 2, multiplied by 2), plus (Number of leaves with black Sigatoka disease severity grade 3, multiplied by 3), plus (Number of leaves with black Sigatoka disease severity grade 4, multiplied by 4), plus (Number of leaves with black Sigatoka disease severity grade 5, multiplied by 5), plus (Number of leaves with black Sigatoka disease severity grade 6, multiplied by 6)), divided by the number of grades in the scale minus 1 (i.e. 7-1)), divided by the Number of standing leaves), multipled by 100. For example, ((((3 * 0) + (1 * 1) + (1 * 2) + (3 * 3) + (5 * 4) + (0 * 5) + (0 * 6)) / 6) / 13) * 100 = ((32 / 6) / 13) * 100 = 41." []
is_a: CO_325:1000010
relationship: method_of CO_325:0000105 ! black sigatoka disease infection index

[Term]
id: CO_325:0010163
name: date of tagged cigar leaf unrolling at brun's stage b - estimation
namespace: BananaMethod
def: "Record the date of event." []
is_a: CO_325:1000011
relationship: method_of CO_325:0000550 ! date of tagged cigar leaf unrolling at brun's stage b
relationship: method_of CO_325:0000550 ! date of tagged cigar leaf unrolling at brun's stage b

[Term]
id: CO_325:0010164
name: date of tagged leaf presenting black sigatoka disease symptoms at foure's stage 1 - estimation
namespace: BananaMethod
def: "Record the date of event." []
is_a: CO_325:1000011
relationship: method_of CO_325:0000553 ! date of tagged leaf presenting black sigatoka disease symptoms at foure's stage 1
relationship: method_of CO_325:0000553 ! date of tagged leaf presenting black sigatoka disease symptoms at foure's stage 1

[Term]
id: CO_325:0010165
name: date of tagged leaf presenting black sigatoka disease symptoms at foure's stage 6 - estimation
namespace: BananaMethod
def: "Record the date of event." []
is_a: CO_325:1000011
relationship: method_of CO_325:0000556 ! date of tagged leaf presenting black sigatoka disease symptoms at foure's stage 6
relationship: method_of CO_325:0000556 ! date of tagged leaf presenting black sigatoka disease symptoms at foure's stage 6

[Term]
id: CO_325:0010166
name: black sigatoka disease incubation time - computation
namespace: BananaMethod
def: "Calculate as: the time elapsed between the Date of tagged leaf presenting black Sigatoka disease symptoms at Foure's stage 1 and the Date of tagged cigar leaf unrolling at stage B, e.g. 24/04/2014 - 24/03/2014 = 31 days." []
is_a: CO_325:1000010
relationship: method_of CO_325:0000057 ! black sigatoka incubation time

[Term]
id: CO_325:0010167
name: black sigatoka disease evolution time - computation
namespace: BananaMethod
def: "Calculate as: the time elapsed between the Date of tagged leaf presenting black Sigatoka disease symptoms at Foure's stage 6 and the Date of tagged leaf presenting black Sigatoka disease symptoms at Foure's stage 1, e.g. 24/06/2014 - 24/04/2014 = 61 days." []
is_a: CO_325:1000010
relationship: method_of CO_325:0000060 ! black sigatoka disease evolution time

[Term]
id: CO_325:0010168
name: extent of internal discolouration in corm of plant caused by fusarium wilt - estimation
namespace: BananaMethod
def: "Completely cut the pseudostem off at the base and ***                                             For the motherplant, at harvest the plant should be cut at the base of the pseudostem. The extent to which vascular discolouration extends up the pseudostem should be determined by making transverse cuts, from the base of the pseudostem upwards, and examining the internal tissues following each cut. The point at which discolouration is no longer visible should be noted and the distance from this point to the pseudostem base recorded." []
is_a: CO_325:1000011
relationship: method_of CO_325:0000559 ! extent of internal discolouration in corm of plant caused by fusarium wilt

[Term]
id: CO_325:0010169
name: distance of internal discolouration in pseudostem of plant caused by fusarium wilt
namespace: BananaMethod
def: "****For the first sucker, the complete corm should be removed from the soil, the roots cut off and excess soil removed. Transverse sections of the corm should be cut (using a guillotine or other suitable device) to obtain five slices of equal thickness. The upper surface of each cut section should be examined and visually evaluate the extent of the vascular discolouration." []
is_a: CO_325:1000008
relationship: method_of CO_325:0000075 ! distance of internal discolouration in pseudostem of plant caused by fusarium wilt

[Term]
id: CO_325:0010170
name: extent of internal discolouration in corm of tallest sucker caused by fusarium wilt - estimation
namespace: BananaMethod
def: "Completely cut the pseudostem off at the base and ***                                             For the motherplant, at harvest the plant should be cut at the base of the pseudostem. The extent to which vascular discolouration extends up the pseudostem should be determined by making transverse cuts, from the base of the pseudostem upwards, and examining the internal tissues following each cut. The point at which discolouration is no longer visible should be noted and the distance from this point to the pseudostem base recorded." []
is_a: CO_325:1000011
relationship: method_of CO_325:0000072 ! extent of internal discolouration in corm of tallest sucker caused by fusarium wilt

[Term]
id: CO_325:0010171
name: presence of petiole collapse caused by fusarium wilt - estimation
namespace: BananaMethod
def: "Visual assessment." []
is_a: CO_325:1000011
relationship: method_of CO_325:0000096 ! presence of petiole collapse caused by fusarium wilt
relationship: method_of CO_325:0000096 ! presence of petiole collapse caused by fusarium wilt

[Term]
id: CO_325:0010172
name: date of first external disease symptoms caused by fusarium wilt - estimation
namespace: BananaMethod
def: "Record the date of event." []
is_a: CO_325:1000011
relationship: method_of CO_325:0000561 ! date of first external disease symptoms caused by fusarium wilt
relationship: method_of CO_325:0000561 ! date of first external disease symptoms caused by fusarium wilt

[Term]
id: CO_325:0010173
name: rank of youngest leaf - counting
namespace: BananaMethod
def: "Record the rank of the youngest completely unrolled leaf, which is always 1. Associate the data with the Date of data collection." []
is_a: CO_325:1000009
relationship: method_of CO_325:0000564 ! rank of marked youngest leaf

[Term]
id: CO_325:0010174
name: rank of previously marked leaf - counting
namespace: BananaMethod
def: "Record the rank of the previously marked leaf (the leaf that was marked in the Rank of marked youngest leaf during the last data collection), counting the leaf rank by starting with the newest completely unrolled leaf as 1 and moving downwards. Associate the data with the Date of data collection." []
is_a: CO_325:1000009
relationship: method_of CO_325:0000566 ! rank of previously marked leaf

[Term]
id: CO_325:0010175
name: leaf emission rate - computation
namespace: BananaMethod
def: "Calculate as: the Rank of previously marked leaf at one point in time, minus 1 (equivalent to the Rank of marked youngest leaf), divided by the time elapsed between the two Date of data collection events when the marked leaf was recorded as 1) the Rank of youngest leaf and 2) the Rank of previously marked leaf, e.g. (4 - 1) / 1 month = LER of 3 leaves/month during a particular time period." []
is_a: CO_325:1000010
relationship: method_of CO_325:0000021 ! leaf emission rate
relationship: method_of CO_325:0000021 ! leaf emission rate

[Term]
id: CO_325:0010176
name: number of functional leaves - counting
namespace: BananaMethod
def: "Count how many functional leaves (leaves that have 50% or more of their surface as green, healthy, photosynthetic tissue) are on the plant, considering all standing leaves in between and inclusive of, the youngest leaf (at leaf rank 1) and the oldest standing leaf." []
is_a: CO_325:1000009
relationship: method_of CO_325:0000066 ! number of functional leaves

[Term]
id: CO_325:0010177
name: time from planting to first youngest spotted leaf - computation
namespace: BananaMethod
def: "Calculate as: the time elapsed between the Date of planting and the Date of first youngest leaf spotted, e.g. 24/06/2014 - 24/01/2014 = 151 days." []
is_a: CO_325:1000010
relationship: method_of CO_325:0000570 ! time from planting to first youngest leaf spotted

[Term]
id: CO_325:0010178
name: number of spotted leaves - counting
namespace: BananaMethod
def: "Count how many of the standing leaves are spotted (with at least 10 discrete, mature, necrotic lesions or one large necrotic area with 10 light-coloured dry centres), considering all leaves in between and inclusive of, the youngest leaf and the oldest standing leaf." []
is_a: CO_325:1000009
relationship: method_of CO_325:0000572 ! number of spotted leaves

[Term]
id: CO_325:0010179
name: number of standing leaves - counting
namespace: BananaMethod
def: "Count how many standing leaves (with an erect petiole) are on the plant, considering all leaves in between and inclusive of, the youngest leaf and the oldest standing leaf. Do not count those leaves with the petiole bent back, other leaves should be recorded regardless of their colour or the colour of their petiole." []
is_a: CO_325:1000009
relationship: method_of CO_325:0000069 ! number of standing leaves

[Term]
id: CO_325:0010180
name: index of non-spotted leaves - computation
namespace: BananaMethod
def: "Calculate as: 100 multiplied by (Youngest leaf spotted, minus 1), divided by Number of standing leaves, e.g. 100 * (6 - 1) / 12 = 42." []
is_a: CO_325:1000010
relationship: method_of CO_325:0000102 ! index of non-spotted leaves

[Term]
id: CO_325:0010181
name: black sigatoka disease severity - estimation
namespace: BananaMethod
def: "Visually observe and record the amount of the surface area of a standing leaf that is affected by black Sigatoka disease." []
is_a: CO_325:1000011
relationship: method_of CO_325:0000574 ! black sigatoka disease severity
relationship: method_of CO_325:0000574 ! black sigatoka disease severity
relationship: method_of CO_325:0000574 ! black sigatoka disease severity
relationship: method_of CO_325:0000574 ! black sigatoka disease severity
relationship: method_of CO_325:0000574 ! black sigatoka disease severity

[Term]
id: CO_325:0010182
name: number of leaves with black sigatoka disease severity grade 0 - computation
namespace: BananaMethod
def: "Calculate as: the sum of values for one plant with a Black Sigatoka disease severity grade of 0." []
is_a: CO_325:1000010
relationship: method_of CO_325:0000580 ! number of leaves with black sigatoka disease severity grade 0

[Term]
id: CO_325:0010183
name: number of leaves with black sigatoka disease severity grade 1 - computation
namespace: BananaMethod
def: "Calculate as: the sum of values for one plant with a Black Sigatoka disease severity grade of 1." []
is_a: CO_325:1000010
relationship: method_of CO_325:0000582 ! number of leaves with black sigatoka disease severity grade 1

[Term]
id: CO_325:0010184
name: number of leaves with black sigatoka disease severity grade 2 - computation
namespace: BananaMethod
def: "Calculate as: the sum of values for one plant with a Black Sigatoka disease severity grade of 2." []
is_a: CO_325:1000010
relationship: method_of CO_325:0000584 ! number of leaves with black sigatoka disease severity grade 2

[Term]
id: CO_325:0010185
name: number of leaves with black sigatoka disease severity grade 3 - computation
namespace: BananaMethod
def: "Calculate as: the sum of values for one plant with a Black Sigatoka disease severity grade of 3." []
is_a: CO_325:1000010
relationship: method_of CO_325:0000586 ! number of leaves with black sigatoka disease severity grade 3

[Term]
id: CO_325:0010186
name: number of leaves with black sigatoka disease severity grade 4 - computation
namespace: BananaMethod
def: "Calculate as: the sum of values for one plant with a Black Sigatoka disease severity grade of 4." []
is_a: CO_325:1000010
relationship: method_of CO_325:0000588 ! number of leaves with black sigatoka disease severity grade 4

[Term]
id: CO_325:0010187
name: number of leaves with black sigatoka disease severity grade 5 - computation
namespace: BananaMethod
def: "Calculate as: the sum of values for one plant with a Black Sigatoka disease severity grade of 5." []
is_a: CO_325:1000010
relationship: method_of CO_325:0000590 ! number of leaves with black sigatoka disease severity grade 5

[Term]
id: CO_325:0010188
name: number of leaves with black sigatoka disease severity grade 6 - computation
namespace: BananaMethod
def: "Calculate as: the sum of values for one plant with a Black Sigatoka disease severity grade of 6." []
is_a: CO_325:1000010
relationship: method_of CO_325:0000592 ! number of leaves with black sigatoka disease severity grade 6

[Term]
id: CO_325:0010189
name: distance of internal discolouration in pseudostem of tallest sucker caused by fusarium wilt
namespace: BananaMethod
def: "****For the first sucker, the complete corm should be removed from the soil, the roots cut off and excess soil removed. Transverse sections of the corm should be cut (using a guillotine or other suitable device) to obtain five slices of equal thickness. The upper surface of each cut section should be examined and visually evaluate the extent of the vascular discolouration." []
is_a: CO_325:1000008
relationship: method_of CO_325:0000594 ! distance of internal discolouration in pseudostem of tallest sucker caused by fusarium wilt

[Term]
id: CO_325:0010190
name: presence of yellowing leaves caused by fusarium wilt - estimation
namespace: BananaMethod
def: "Visual assessment." []
is_a: CO_325:1000011
relationship: method_of CO_325:0000087 ! presence of yellowing leaves caused by fusarium wilt
relationship: method_of CO_325:0000087 ! presence of yellowing leaves caused by fusarium wilt

[Term]
id: CO_325:0010191
name: presence of splitting pseudostem base caused by fusarium wilt - estimation
namespace: BananaMethod
def: "Visual assessment." []
is_a: CO_325:1000011
relationship: method_of CO_325:0000090 ! presence of splitting pseudostem base caused by fusarium wilt
relationship: method_of CO_325:0000090 ! presence of splitting pseudostem base caused by fusarium wilt

[Term]
id: CO_325:0010192
name: presence of changes in new leaves caused by fusarium wilt - estimation
namespace: BananaMethod
def: "Visual assessment." []
is_a: CO_325:1000011
relationship: method_of CO_325:0000093 ! presence of changes in new leaves caused by fusarium wilt
relationship: method_of CO_325:0000093 ! presence of changes in new leaves caused by fusarium wilt

[Term]
id: CO_325:0010193
name: time from start of crop cycle to first external disease symptoms caused by fusarium wilt - computation
namespace: BananaMethod
def: "Calculate as: the time elapsed between the Date of planting or the Date of harvest of the bunch from the plant of the previous crop cycle and the Date of first external disease symptoms caused by Fusarium wilt." []
is_a: CO_325:1000010
relationship: method_of CO_325:0000084 ! time from start of crop cycle to first external disease symptoms caused by fusarium wilt

[Term]
id: CO_325:0010194
name: percentage of plants with yellowing leaves caused by fusarium wilt - computation
namespace: BananaMethod
def: "Calculate as: the sum of the number of values for Presence of yellowing leaves caused by Fusarium wilt scored as Present, divided by the Number of plants planted, multiplied by 100, e.g. 78 / 300 * 100 = 26%." []
is_a: CO_325:1000010
relationship: method_of CO_325:0000600 ! percentage of plants with yellowing leaves caused by fusarium wilt

[Term]
id: CO_325:0010195
name: percentage of plants with a splitting pseudostem base caused by fusarium wilt - computation
namespace: BananaMethod
def: "Calculate as: the sum of the number of values for Presence of splitting pseudostem base caused by Fusarium wilt scored as Present, divided by the Number of plants planted, multiplied by 100, e.g. 24 / 300 * 100 = 8%." []
is_a: CO_325:1000010
relationship: method_of CO_325:0000602 ! percentage of plants with a splitting pseudostem base caused by fusarium wilt

[Term]
id: CO_325:0010196
name: percentage of plants with changes in new leaves caused by fusarium wilt - computation
namespace: BananaMethod
def: "Calculate as: the sum of the number of values for Presence of changes in new leaves caused by Fusarium wilt scored as Present, divided by the Number of plants planted, multiplied by 100, e.g. 67 / 300 * 100 = 22%." []
is_a: CO_325:1000010
relationship: method_of CO_325:0000604 ! percentage of plants with changes in new leaves caused by fusarium wilt

[Term]
id: CO_325:0010197
name: percentage of plants with petiole collapse caused by fusarium wilt - computation
namespace: BananaMethod
def: "Calculate as: the sum of the number of values for Presence of petiole collapse caused by Fusarium wilt scored as Present, divided by the Number of plants planted, multiplied by 100, e.g. 84 / 300 * 100 = 28%." []
is_a: CO_325:1000010
relationship: method_of CO_325:0000606 ! percentage of plants with petiole collapse caused by fusarium wilt

[Term]
id: CO_325:0010198
name: percentage of plants with external disease symptoms caused by fusarium wilt - computation
namespace: BananaMethod
def: "Calculate as: the sum of the number of plants with any or multiple of the external disease symptoms caused by Fusarium wilt - yellowing leaves, splitting of pseudostem base, changes in new leaves, petiole collapse - divided by the Number of plants planted * 100, e.g. 112 / 300 * 100 = 37%." []
is_a: CO_325:1000010
relationship: method_of CO_325:0000078 ! percentage of plants with external disease symptoms caused by fusarium wilt

[Term]
id: CO_325:0010199
name: percentage of plants with internal disease symptoms caused by fusarium wilt - computation
namespace: BananaMethod
def: "Calculate as: the sum of the number of plants with any or multiple of the internal disease symptoms caused by Fusarium wilt - discolouration in the corm, and/or discolouration in the pseudostem - divided by the Number of plants planted * 100, e.g. 108 / 300 * 100 = 36%." []
is_a: CO_325:1000010
relationship: method_of CO_325:0000081 ! percentage of plants with internal disease symptoms caused by fusarium wilt

[Term]
id: CO_325:0010200
name: vitamin c - measurement
namespace: BananaMethod
def: "?" []
is_a: CO_325:1000008
relationship: method_of CO_325:0000608 ! vitamin c content

[Term]
id: CO_325:0010201
name: number of adult weevils - counting
namespace: BananaMethod
def: "visual counting method of Weevils per trap (the trap should be minimum 30 cm long)" []
is_a: CO_325:1000009
relationship: method_of CO_325:0000610 ! number of adult weevils per trap
relationship: method_of CO_325:0000614 ! average number of adult weevils {x per trap} per mat

[Term]
id: CO_325:0010202
name: number of adult weevil trap - counting
namespace: BananaMethod
def: "visual counting method of Weevil traps (the trap should be  minimum 30 cm long)." []
is_a: CO_325:1000009
relationship: method_of CO_325:0000612 ! number of weevils traps used

[Term]
id: CO_325:0010203
name: number of weevil larvae - counting
namespace: BananaMethod
def: "visual counting method" []
is_a: CO_325:1000009
relationship: method_of CO_325:0000616 ! [number of weevil larvae per trap]
relationship: method_of CO_325:0000618 ! average number of weevil larvae per mat
relationship: method_of CO_325:0000622 ! number of weevil larvae measured

[Term]
id: CO_325:0010204
name: number of adult larvae - counting
namespace: BananaMethod
def: "visual counting method" []
is_a: CO_325:1000009
relationship: method_of CO_325:0000620 ! number of adult weevils measured

[Term]
id: CO_325:0010205
name: adult weevil head capsule - measurement
namespace: BananaMethod
def: "Measurement under microscope" []
is_a: CO_325:1000008
relationship: method_of CO_325:0000624 ! adult weevil head capsule width
relationship: method_of CO_325:0000626 ! average adult weevil head capsule width

[Term]
id: CO_325:0010206
name: adult weevil body - measurement
namespace: BananaMethod
def: "Measurement under microscope" []
is_a: CO_325:1000008
relationship: method_of CO_325:0000628 ! adult weevil body length
relationship: method_of CO_325:0000630 ! average adult weevil body length
relationship: method_of CO_325:0000632 ! adult weevil body weight
relationship: method_of CO_325:0000634 ! average adult weevil body weight

[Term]
id: CO_325:0010207
name: weevil larvae head capsule - measurement
namespace: BananaMethod
def: "Measurement under microscope" []
is_a: CO_325:1000008
relationship: method_of CO_325:0000636 ! weevil larvae head capsule width
relationship: method_of CO_325:0000638 ! average weevil larvae head capsule width

[Term]
id: CO_325:0010208
name: weevil larvae body length - measurement
namespace: BananaMethod
def: "Measurement under microscope" []
is_a: CO_325:1000008
relationship: method_of CO_325:0000640 ! weevil larvae body length
relationship: method_of CO_325:0000642 ! average weevil larvae body length

[Term]
id: CO_325:0010209
name: weevil larvae body weight - measurement
namespace: BananaMethod
def: "Measurement under microscope" []
is_a: CO_325:1000008
relationship: method_of CO_325:0000644 ! weevil larvae weight
relationship: method_of CO_325:0000646 ! average weevil larvae weight

[Term]
id: CO_325:0010210
name: damage index-x-inner - measurement
namespace: BananaMethod
def: "Visual observation" []
is_a: CO_325:1000008
relationship: method_of CO_325:0000648 ! percentage damage to corm cortex cross-section caused by weevils

[Term]
id: CO_325:0010211
name: damage index-x-outer - measurement
namespace: BananaMethod
def: "Visual observation" []
is_a: CO_325:1000008
relationship: method_of CO_325:0000650 ! percentage damage to corm outer cylinder cross-section caused by weevils

[Term]
id: CO_325:0100000
name: dd/mm/yyyy
namespace: BananaScale
is_a: CO_325:1000018
relationship: scale_of CO_325:0010000 ! date of planting - estimation
relationship: scale_of CO_325:0010001 ! date of recognising off-type - estimation
relationship: scale_of CO_325:0010002 ! date of damage - estimation
relationship: scale_of CO_325:0010005 ! date of death - estimation
relationship: scale_of CO_325:0010007 ! date of shooting - estimation
relationship: scale_of CO_325:0010008 ! date of flowering - estimation
relationship: scale_of CO_325:0010009 ! date of harvest - estimation
relationship: scale_of CO_325:0010010 ! date of data collection - estimation
relationship: scale_of CO_325:0010018 ! date of marking youngest leaf - estimation
relationship: scale_of CO_325:0010019 ! date of recording rank of previously marked leaf - estimation
relationship: scale_of CO_325:0010160 ! date of first youngest leaf spotted - estimation
relationship: scale_of CO_325:0010163 ! date of tagged cigar leaf unrolling at brun's stage b - estimation
relationship: scale_of CO_325:0010164 ! date of tagged leaf presenting black sigatoka disease symptoms at foure's stage 1 - estimation
relationship: scale_of CO_325:0010165 ! date of tagged leaf presenting black sigatoka disease symptoms at foure's stage 6 - estimation
relationship: scale_of CO_325:0010172 ! date of first external disease symptoms caused by fusarium wilt - estimation

[Term]
id: CO_325:0100001
name: yyyy/mm/dd
namespace: BananaScale
is_a: CO_325:1000018
relationship: scale_of CO_325:0010000 ! date of planting - estimation
relationship: scale_of CO_325:0010001 ! date of recognising off-type - estimation
relationship: scale_of CO_325:0010002 ! date of damage - estimation
relationship: scale_of CO_325:0010005 ! date of death - estimation
relationship: scale_of CO_325:0010007 ! date of shooting - estimation
relationship: scale_of CO_325:0010008 ! date of flowering - estimation
relationship: scale_of CO_325:0010009 ! date of harvest - estimation
relationship: scale_of CO_325:0010010 ! date of data collection - estimation
relationship: scale_of CO_325:0010018 ! date of marking youngest leaf - estimation
relationship: scale_of CO_325:0010019 ! date of recording rank of previously marked leaf - estimation
relationship: scale_of CO_325:0010160 ! date of first youngest leaf spotted - estimation
relationship: scale_of CO_325:0010163 ! date of tagged cigar leaf unrolling at brun's stage b - estimation
relationship: scale_of CO_325:0010164 ! date of tagged leaf presenting black sigatoka disease symptoms at foure's stage 1 - estimation
relationship: scale_of CO_325:0010165 ! date of tagged leaf presenting black sigatoka disease symptoms at foure's stage 6 - estimation
relationship: scale_of CO_325:0010172 ! date of first external disease symptoms caused by fusarium wilt - estimation

[Term]
id: CO_325:0100002
name: open answer
namespace: BananaScale
is_a: CO_325:1000014
relationship: scale_of CO_325:0010003 ! plant damage description - estimation
relationship: scale_of CO_325:0010004 ! cause of damage - estimation
relationship: scale_of CO_325:0010006 ! cause of death - estimation

[Term]
id: CO_325:0100003
name: day
namespace: BananaScale
is_a: CO_325:1000016
relationship: scale_of CO_325:0010011 ! time from planting to shooting - computation
relationship: scale_of CO_325:0010012 ! plant crop cycle - computation
relationship: scale_of CO_325:0010013 ! time from shooting to harvest - computation
relationship: scale_of CO_325:0010014 ! time from flowering to harvest - computation
relationship: scale_of CO_325:0010015 ! time from planting to death - computation
relationship: scale_of CO_325:0010016 ! time from harvest to death - computation
relationship: scale_of CO_325:0010017 ! ratoon crop cycle - computation
relationship: scale_of CO_325:0010166 ! black sigatoka disease incubation time - computation
relationship: scale_of CO_325:0010167 ! black sigatoka disease evolution time - computation
relationship: scale_of CO_325:0010177 ! time from planting to first youngest spotted leaf - computation
relationship: scale_of CO_325:0010193 ! time from start of crop cycle to first external disease symptoms caused by fusarium wilt - computation

[Term]
id: CO_325:0100004
name: cm
namespace: BananaScale
is_a: CO_325:1000013
relationship: scale_of CO_325:0010020 ! plant height - petiole of two youngest leaves - measurement
relationship: scale_of CO_325:0010021 ! plant height - angle made between the bunch stalk and bunch cover leaf. -measurement
relationship: scale_of CO_325:0010022 ! plant height - neck of peduncle - measurement
relationship: scale_of CO_325:0010023 ! plant circumference - measurement
relationship: scale_of CO_325:0010024 ! tallest sucker height - measurement
relationship: scale_of CO_325:0010025 ! tallest sucker height - measurement at harvest
relationship: scale_of CO_325:0010050 ! finger dorsal length - measurement
relationship: scale_of CO_325:0010051 ! average finger external length - computation
relationship: scale_of CO_325:0010052 ! finger internal length - measurement
relationship: scale_of CO_325:0010053 ! average finger internal length - computation
relationship: scale_of CO_325:0010054 ! finger circumference - measurement
relationship: scale_of CO_325:0010055 ! average finger circumference - computation
relationship: scale_of CO_325:0010056 ! finger lateral diameter - measurement
relationship: scale_of CO_325:0010057 ! average finger lateral diameter - computation
relationship: scale_of CO_325:0010058 ! fruit pulp lateral diameter - measurement
relationship: scale_of CO_325:0010059 ! average fruit pulp lateral diameter - computation
relationship: scale_of CO_325:0010125 ! fruit length - exact value - measurement
relationship: scale_of CO_325:0010169 ! distance of internal discolouration in pseudostem of plant caused by fusarium wilt
relationship: scale_of CO_325:0010189 ! distance of internal discolouration in pseudostem of tallest sucker caused by fusarium wilt

[Term]
id: CO_325:0100005
name: maiden sucker
namespace: BananaScale
is_a: CO_325:1000013
relationship: scale_of CO_325:0010026 ! number of maiden suckers - counting

[Term]
id: CO_325:0100006
name: sword sucker
namespace: BananaScale
is_a: CO_325:1000013
relationship: scale_of CO_325:0010027 ! number of sword suckers - counting

[Term]
id: CO_325:0100007
name: peeper sucker
namespace: BananaScale
is_a: CO_325:1000013
relationship: scale_of CO_325:0010028 ! number of peeper suckers - counting

[Term]
id: CO_325:0100008
name: water suckers
namespace: BananaScale
is_a: CO_325:1000013
relationship: scale_of CO_325:0010029 ! number of water suckers - counting

[Term]
id: CO_325:0100009
name: sucker
namespace: BananaScale
is_a: CO_325:1000013
relationship: scale_of CO_325:0010030 ! number of suckers - counting

[Term]
id: CO_325:0100010
name: maturity
namespace: BananaScale
is_a: CO_325:1000012
relationship: scale_of CO_325:0010031 ! bunch maturity stage - estimation

[Term]
id: CO_325:0100010:0
name: full green
namespace: BananaScale
synonym: "0" EXACT []
is_a: CO_325:0100010 ! maturity

[Term]
id: CO_325:0100010:1
name: first finger yellow
namespace: BananaScale
synonym: "1" EXACT []
is_a: CO_325:0100010 ! maturity

[Term]
id: CO_325:0100011
name: kg
namespace: BananaScale
is_a: CO_325:1000013
relationship: scale_of CO_325:0010032 ! bunch weight - measurement
relationship: scale_of CO_325:0010033 ! rachis weight - measurement
relationship: scale_of CO_325:0010034 ! total finger weight - computation
relationship: scale_of CO_325:0010043 ! hand weight - measurement
relationship: scale_of CO_325:0010044 ! multiple hand weight - measurement
relationship: scale_of CO_325:0010045 ! average hand weight - computation

[Term]
id: CO_325:0100012
name: hand
namespace: BananaScale
is_a: CO_325:1000013
relationship: scale_of CO_325:0010035 ! number of hands in bunch - counting
relationship: scale_of CO_325:0010040 ! number of hands measured - counting

[Term]
id: CO_325:0100013
name: finger
namespace: BananaScale
is_a: CO_325:1000013
relationship: scale_of CO_325:0010036 ! number of fingers in bunch - counting
relationship: scale_of CO_325:0010038 ! number of fingers in hand - counting
relationship: scale_of CO_325:0010039 ! multiple number of fingers in hand - counting
relationship: scale_of CO_325:0010041 ! average number of fingers in hand - computation
relationship: scale_of CO_325:0010042 ! number of fingers in bunch - estimation
relationship: scale_of CO_325:0010048 ! number of fingers measured - counting
relationship: scale_of CO_325:0010124 ! number of fruits on mid-hand of the bunch - counting

[Term]
id: CO_325:0100014
name: hand rank
namespace: BananaScale
is_a: CO_325:1000013
relationship: scale_of CO_325:0010037 ! hand rank - counting

[Term]
id: CO_325:0100015
name: g
namespace: BananaScale
is_a: CO_325:1000013
relationship: scale_of CO_325:0010046 ! finger weight - measurement
relationship: scale_of CO_325:0010047 ! multiple finger weight - measurement
relationship: scale_of CO_325:0010049 ! average finger weight - computation

[Term]
id: CO_325:0100016
name: mm
namespace: BananaScale
is_a: CO_325:1000013
relationship: scale_of CO_325:0010054 ! finger circumference - measurement
relationship: scale_of CO_325:0010055 ! average finger circumference - computation
relationship: scale_of CO_325:0010056 ! finger lateral diameter - measurement
relationship: scale_of CO_325:0010057 ! average finger lateral diameter - computation
relationship: scale_of CO_325:0010058 ! fruit pulp lateral diameter - measurement
relationship: scale_of CO_325:0010059 ! average fruit pulp lateral diameter - computation
relationship: scale_of CO_325:0010060 ! finger peel thickness - measurement
relationship: scale_of CO_325:0010061 ! average finger peel thickness - computation
relationship: scale_of CO_325:0010130 ! fruit pedicel length - exact value - measurement

[Term]
id: CO_325:0100017
name: plant
namespace: BananaScale
is_a: CO_325:1000013
relationship: scale_of CO_325:0010062 ! number of plants planted - computation
relationship: scale_of CO_325:0010065 ! number of plants dead - computation
relationship: scale_of CO_325:0010066 ! number of plants harvested - computation
relationship: scale_of CO_325:0010067 ! number of plants not harvested - computation

[Term]
id: CO_325:0100018
name: m2
namespace: BananaScale
is_a: CO_325:1000013
relationship: scale_of CO_325:0010063 ! plant spacing - computation

[Term]
id: CO_325:0100019
name: plants/unit of area
namespace: BananaScale
is_a: CO_325:1000013
relationship: scale_of CO_325:0010064 ! plant density - computation
relationship: scale_of CO_325:0010069 ! death density - computation
relationship: scale_of CO_325:0010071 ! harvest density - computation
relationship: scale_of CO_325:0010073 ! non-harvest density - computation

[Term]
id: CO_325:0100020
name: plants dead/plants planted
namespace: BananaScale
is_a: CO_325:1000013
relationship: scale_of CO_325:0010068 ! death proportion - computation

[Term]
id: CO_325:0100021
name: plants harvested/plants planted
namespace: BananaScale
is_a: CO_325:1000013
relationship: scale_of CO_325:0010070 ! harvest proportion - computation

[Term]
id: CO_325:0100022
name: plants not harvested/plants planted
namespace: BananaScale
is_a: CO_325:1000013
relationship: scale_of CO_325:0010072 ! non-harvest proportion - computation

[Term]
id: CO_325:0100023
name: crop cycle duration/year
namespace: BananaScale
is_a: CO_325:1000013
relationship: scale_of CO_325:0010074 ! annual crop cycle proportion - computation

[Term]
id: CO_325:0100024
name: kg/plant/y
namespace: BananaScale
is_a: CO_325:1000013
relationship: scale_of CO_325:0010075 ! annual plant productivity - computation

[Term]
id: CO_325:0100025
name: t/unit of area/y
namespace: BananaScale
is_a: CO_325:1000013
relationship: scale_of CO_325:0010076 ! actual annual yield - computation
relationship: scale_of CO_325:0010077 ! potential annual yield - computation

[Term]
id: CO_325:0100026
name: 1 to 2 acceptability score
namespace: BananaScale
is_a: CO_325:1000012
relationship: scale_of CO_325:0010078 ! fruit pendulance - estimation
relationship: scale_of CO_325:0010079 ! bunch quality - estimation
relationship: scale_of CO_325:0010081 ! sucker quality - estimation

[Term]
id: CO_325:0100026:1
name: bad
namespace: BananaScale
synonym: "1" EXACT []
is_a: CO_325:0100026 ! 1 to 2 acceptability score

[Term]
id: CO_325:0100026:2
name: good
namespace: BananaScale
synonym: "2" EXACT []
is_a: CO_325:0100026 ! 1 to 2 acceptability score

[Term]
id: CO_325:0100027
name: parthenocarpy presence
namespace: BananaScale
is_a: CO_325:1000015
relationship: scale_of CO_325:0010080 ! fruit parthenocarpy - estimation

[Term]
id: CO_325:0100027:1
name: Parthenocarpic
namespace: BananaScale
synonym: "1" EXACT []
is_a: CO_325:0100027 ! parthenocarpy presence

[Term]
id: CO_325:0100027:2
name: Not parthenocarpic
namespace: BananaScale
synonym: "2" EXACT []
is_a: CO_325:0100027 ! parthenocarpy presence

[Term]
id: CO_325:0100028
name: dwarfism presence
namespace: BananaScale
is_a: CO_325:1000015
relationship: scale_of CO_325:0010082 ! dwarfism - estimation

[Term]
id: CO_325:0100028:1
name: Dwarf
namespace: BananaScale
synonym: "1" EXACT []
is_a: CO_325:0100028 ! dwarfism presence

[Term]
id: CO_325:0100028:2
name: Not Dwarf
namespace: BananaScale
synonym: "2" EXACT []
is_a: CO_325:0100028 ! dwarfism presence

[Term]
id: CO_325:0100029
name: Trial group scale
namespace: BananaScale
is_a: CO_325:1000013
relationship: scale_of CO_325:0010083 ! trial group id -counting

[Term]
id: CO_325:0100030
name: Trial  scale
namespace: BananaScale
is_a: CO_325:1000013
relationship: scale_of CO_325:0010084 ! trial id -counting

[Term]
id: CO_325:0100031
name: Block  scale
namespace: BananaScale
is_a: CO_325:1000013
relationship: scale_of CO_325:0010085 ! block id -counting

[Term]
id: CO_325:0100032
name: Row  scale
namespace: BananaScale
is_a: CO_325:1000013
relationship: scale_of CO_325:0010086 ! row id -counting

[Term]
id: CO_325:0100033
name: Column  scale
namespace: BananaScale
is_a: CO_325:1000013
relationship: scale_of CO_325:0010087 ! column id -counting

[Term]
id: CO_325:0100034
name: Spatial position  scale
namespace: BananaScale
is_a: CO_325:1000013
relationship: scale_of CO_325:0010088 ! spatial position id -counting

[Term]
id: CO_325:0100035
name: Accession  scale
namespace: BananaScale
is_a: CO_325:1000013
relationship: scale_of CO_325:0010089 ! accession id -counting

[Term]
id: CO_325:0100036
name: Genotype ID scale
namespace: BananaScale
is_a: CO_325:1000013
relationship: scale_of CO_325:0010090 ! genotype id -counting

[Term]
id: CO_325:0100037
name: genotype purpose scale
namespace: BananaScale
is_a: CO_325:1000012
relationship: scale_of CO_325:0010091 ! genotype purpose -counting

[Term]
id: CO_325:0100037:1
name: Test accession
namespace: BananaScale
synonym: "1" EXACT []
is_a: CO_325:0100037 ! genotype purpose scale

[Term]
id: CO_325:0100037:2
name: Local check
namespace: BananaScale
synonym: "2" EXACT []
is_a: CO_325:0100037 ! genotype purpose scale

[Term]
id: CO_325:0100037:3
name: Resistant/tolerant check
namespace: BananaScale
synonym: "3" EXACT []
is_a: CO_325:0100037 ! genotype purpose scale

[Term]
id: CO_325:0100037:4
name: Susceptible check
namespace: BananaScale
synonym: "4" EXACT []
is_a: CO_325:0100037 ! genotype purpose scale

[Term]
id: CO_325:0100037:5
name: Border row
namespace: BananaScale
synonym: "5" EXACT []
is_a: CO_325:0100037 ! genotype purpose scale

[Term]
id: CO_325:0100038
name: Mat ID scale
namespace: BananaScale
is_a: CO_325:1000013
relationship: scale_of CO_325:0010092 ! mat id -counting

[Term]
id: CO_325:0100039
name: crop cycle duration/year scale
namespace: BananaScale
is_a: CO_325:1000012
relationship: scale_of CO_325:0010093 ! crop cycle id -counting

[Term]
id: CO_325:0100039:1
name: First plant planted
namespace: BananaScale
synonym: "1" EXACT []
is_a: CO_325:0100039 ! crop cycle duration/year scale

[Term]
id: CO_325:0100039:2
name: First ratoon plant
namespace: BananaScale
synonym: "2" EXACT []
is_a: CO_325:0100039 ! crop cycle duration/year scale

[Term]
id: CO_325:0100039:3
name: Second ratoon plant
namespace: BananaScale
synonym: "3" EXACT []
is_a: CO_325:0100039 ! crop cycle duration/year scale

[Term]
id: CO_325:0100039:4
name: Third ratoon plant
namespace: BananaScale
synonym: "4" EXACT []
is_a: CO_325:0100039 ! crop cycle duration/year scale

[Term]
id: CO_325:0100039:5
name: Fourth ratoon plant
namespace: BananaScale
synonym: "5" EXACT []
is_a: CO_325:0100039 ! crop cycle duration/year scale

[Term]
id: CO_325:0100039:6
name: Fifth ratoon plant
namespace: BananaScale
synonym: "6" EXACT []
is_a: CO_325:0100039 ! crop cycle duration/year scale

[Term]
id: CO_325:0100040
name: Plant scale
namespace: BananaScale
is_a: CO_325:1000013
relationship: scale_of CO_325:0010094 ! plant id -counting

[Term]
id: CO_325:0100041
name: Plant barcode scale
namespace: BananaScale
is_a: CO_325:1000013
relationship: scale_of CO_325:0010095 ! plant barcode -counting

[Term]
id: CO_325:0100042
name: height score (1 to 3)
namespace: BananaScale
is_a: CO_325:1000012
relationship: scale_of CO_325:0010096 ! pseudostem height - estimation

[Term]
id: CO_325:0100042:1
name: Less than or equal to 2 m
namespace: BananaScale
synonym: "1" EXACT []
is_a: CO_325:0100042 ! height score (1 to 3)

[Term]
id: CO_325:0100042:2
name: 2.1-2.9 m
namespace: BananaScale
synonym: "2" EXACT []
is_a: CO_325:0100042 ! height score (1 to 3)

[Term]
id: CO_325:0100042:3
name: Equal to or more than 3 m
namespace: BananaScale
synonym: "3" EXACT []
is_a: CO_325:0100042 ! height score (1 to 3)

[Term]
id: CO_325:0100043
name: bd colour chart a - 2016
namespace: BananaScale
is_a: CO_325:1000015
relationship: scale_of CO_325:0010097 ! pseudostem colour - estimation
relationship: scale_of CO_325:0010103 ! petiole margin colour - estimation
relationship: scale_of CO_325:0010105 ! pigmentation of outer surface of cigar leaf - estimation
relationship: scale_of CO_325:0010118 ! colour of bract external face - estimation
relationship: scale_of CO_325:0010119 ! colour of bract internal face - estimation

[Term]
id: CO_325:0100043:1
name: Cream
namespace: BananaScale
synonym: "1" EXACT []
is_a: CO_325:0100043 ! bd colour chart a - 2016

[Term]
id: CO_325:0100043:10
name: Orange red
namespace: BananaScale
synonym: "10" EXACT []
is_a: CO_325:0100043 ! bd colour chart a - 2016

[Term]
id: CO_325:0100043:11
name: Red
namespace: BananaScale
synonym: "11" EXACT []
is_a: CO_325:0100043 ! bd colour chart a - 2016

[Term]
id: CO_325:0100043:12
name: Pink-purple
namespace: BananaScale
synonym: "12" EXACT []
is_a: CO_325:0100043 ! bd colour chart a - 2016

[Term]
id: CO_325:0100043:13
name: Purple-brown
namespace: BananaScale
synonym: "13" EXACT []
is_a: CO_325:0100043 ! bd colour chart a - 2016

[Term]
id: CO_325:0100043:14
name: Red-purple
namespace: BananaScale
synonym: "14" EXACT []
is_a: CO_325:0100043 ! bd colour chart a - 2016

[Term]
id: CO_325:0100043:15
name: Purple
namespace: BananaScale
synonym: "15" EXACT []
is_a: CO_325:0100043 ! bd colour chart a - 2016

[Term]
id: CO_325:0100043:2
name: Yellow
namespace: BananaScale
synonym: "2" EXACT []
is_a: CO_325:0100043 ! bd colour chart a - 2016

[Term]
id: CO_325:0100043:3
name: Watery green
namespace: BananaScale
synonym: "3" EXACT []
is_a: CO_325:0100043 ! bd colour chart a - 2016

[Term]
id: CO_325:0100043:4
name: Green yellow
namespace: BananaScale
synonym: "4" EXACT []
is_a: CO_325:0100043 ! bd colour chart a - 2016

[Term]
id: CO_325:0100043:5
name: Light green
namespace: BananaScale
synonym: "5" EXACT []
is_a: CO_325:0100043 ! bd colour chart a - 2016

[Term]
id: CO_325:0100043:6
name: Medium green
namespace: BananaScale
synonym: "6" EXACT []
is_a: CO_325:0100043 ! bd colour chart a - 2016

[Term]
id: CO_325:0100043:7
name: Green
namespace: BananaScale
synonym: "7" EXACT []
is_a: CO_325:0100043 ! bd colour chart a - 2016

[Term]
id: CO_325:0100043:8
name: Dark green
namespace: BananaScale
synonym: "8" EXACT []
is_a: CO_325:0100043 ! bd colour chart a - 2016

[Term]
id: CO_325:0100043:9
name: Whitish
namespace: BananaScale
synonym: "9" EXACT []
is_a: CO_325:0100043 ! bd colour chart a - 2016

[Term]
id: CO_325:0100044
name: blotch pigmentation scale (1 to 4)
namespace: BananaScale
is_a: CO_325:1000012
relationship: scale_of CO_325:0010098 ! blotches area - estimation

[Term]
id: CO_325:0100044:1
name: No pigmentation
namespace: BananaScale
synonym: "1" EXACT []
is_a: CO_325:0100044 ! blotch pigmentation scale (1 to 4)

[Term]
id: CO_325:0100044:2
name: Sparse blotching (<20%)
namespace: BananaScale
synonym: "2" EXACT []
is_a: CO_325:0100044 ! blotch pigmentation scale (1 to 4)

[Term]
id: CO_325:0100044:3
name: Moderate blotching (20-50%)
namespace: BananaScale
synonym: "3" EXACT []
is_a: CO_325:0100044 ! blotch pigmentation scale (1 to 4)

[Term]
id: CO_325:0100044:4
name: Extensive pigmentation (>50%)
namespace: BananaScale
synonym: "4" EXACT []
is_a: CO_325:0100044 ! blotch pigmentation scale (1 to 4)

[Term]
id: CO_325:0100045
name: blotch pigmentation scale (1 to 5)
namespace: BananaScale
is_a: CO_325:1000012
relationship: scale_of CO_325:0010098 ! blotches area - estimation

[Term]
id: CO_325:0100045:1
name: Sparse blotching
namespace: BananaScale
synonym: "1" EXACT []
is_a: CO_325:0100045 ! blotch pigmentation scale (1 to 5)

[Term]
id: CO_325:0100045:2
name: Small blotches
namespace: BananaScale
synonym: "2" EXACT []
is_a: CO_325:0100045 ! blotch pigmentation scale (1 to 5)

[Term]
id: CO_325:0100045:3
name: Large blotches
namespace: BananaScale
synonym: "3" EXACT []
is_a: CO_325:0100045 ! blotch pigmentation scale (1 to 5)

[Term]
id: CO_325:0100045:4
name: Extensive pigmentation
namespace: BananaScale
synonym: "4" EXACT []
is_a: CO_325:0100045 ! blotch pigmentation scale (1 to 5)

[Term]
id: CO_325:0100045:5
name: Without pigmentation
namespace: BananaScale
synonym: "5" EXACT []
is_a: CO_325:0100045 ! blotch pigmentation scale (1 to 5)

[Term]
id: CO_325:0100046
name: blotch color scale (1 to 4)
namespace: BananaScale
is_a: CO_325:1000015
relationship: scale_of CO_325:0010099 ! blotches colour - estimation

[Term]
id: CO_325:0100046:1
name: Orange-brown (mahogany, like in Pisang Mas)
namespace: BananaScale
synonym: "1" EXACT []
is_a: CO_325:0100046 ! blotch color scale (1 to 4)

[Term]
id: CO_325:0100046:2
name: Brown
namespace: BananaScale
synonym: "2" EXACT []
is_a: CO_325:0100046 ! blotch color scale (1 to 4)

[Term]
id: CO_325:0100046:3
name: Black-purple
namespace: BananaScale
synonym: "3" EXACT []
is_a: CO_325:0100046 ! blotch color scale (1 to 4)

[Term]
id: CO_325:0100046:4
name: Other
namespace: BananaScale
synonym: "4" EXACT []
is_a: CO_325:0100046 ! blotch color scale (1 to 4)

[Term]
id: CO_325:0100047
name: blotch color scale (1 to 5)
namespace: BananaScale
is_a: CO_325:1000015
relationship: scale_of CO_325:0010099 ! blotches colour - estimation

[Term]
id: CO_325:0100047:1
name: Brown
namespace: BananaScale
synonym: "1" EXACT []
is_a: CO_325:0100047 ! blotch color scale (1 to 5)

[Term]
id: CO_325:0100047:2
name: Dark brown
namespace: BananaScale
synonym: "2" EXACT []
is_a: CO_325:0100047 ! blotch color scale (1 to 5)

[Term]
id: CO_325:0100047:3
name: Brown-black
namespace: BananaScale
synonym: "3" EXACT []
is_a: CO_325:0100047 ! blotch color scale (1 to 5)

[Term]
id: CO_325:0100047:4
name: Black-purple
namespace: BananaScale
synonym: "4" EXACT []
is_a: CO_325:0100047 ! blotch color scale (1 to 5)

[Term]
id: CO_325:0100047:5
name: Other
namespace: BananaScale
synonym: "5" EXACT []
is_a: CO_325:0100047 ! blotch color scale (1 to 5)

[Term]
id: CO_325:0100048
name: margin behaviour scale (1 to 4)
namespace: BananaScale
is_a: CO_325:1000015
relationship: scale_of CO_325:0010100 ! margin behaviour on petiole canal of third leaf  - estimation

[Term]
id: CO_325:0100048:1
name: Margins spreading
namespace: BananaScale
synonym: "1" EXACT []
is_a: CO_325:0100048 ! margin behaviour scale (1 to 4)

[Term]
id: CO_325:0100048:2
name: Margins erect
namespace: BananaScale
synonym: "2" EXACT []
is_a: CO_325:0100048 ! margin behaviour scale (1 to 4)

[Term]
id: CO_325:0100048:3
name: Margins curved inward
namespace: BananaScale
synonym: "3" EXACT []
is_a: CO_325:0100048 ! margin behaviour scale (1 to 4)

[Term]
id: CO_325:0100048:4
name: Margins overlapping
namespace: BananaScale
synonym: "4" EXACT []
is_a: CO_325:0100048 ! margin behaviour scale (1 to 4)

[Term]
id: CO_325:0100049
name: margin behaviour scale (1 to 5)
namespace: BananaScale
is_a: CO_325:1000015
relationship: scale_of CO_325:0010100 ! margin behaviour on petiole canal of third leaf  - estimation

[Term]
id: CO_325:0100049:1
name: Open with margins spreading
namespace: BananaScale
synonym: "1" EXACT []
is_a: CO_325:0100049 ! margin behaviour scale (1 to 5)

[Term]
id: CO_325:0100049:2
name: Wide with erect margins
namespace: BananaScale
synonym: "2" EXACT []
is_a: CO_325:0100049 ! margin behaviour scale (1 to 5)

[Term]
id: CO_325:0100049:3
name: Straight with erect margins
namespace: BananaScale
synonym: "3" EXACT []
is_a: CO_325:0100049 ! margin behaviour scale (1 to 5)

[Term]
id: CO_325:0100049:4
name: Margins curved inward
namespace: BananaScale
synonym: "4" EXACT []
is_a: CO_325:0100049 ! margin behaviour scale (1 to 5)

[Term]
id: CO_325:0100049:5
name: Margins overlapping
namespace: BananaScale
synonym: "5" EXACT []
is_a: CO_325:0100049 ! margin behaviour scale (1 to 5)

[Term]
id: CO_325:0100050
name: wing presence/absence
namespace: BananaScale
is_a: CO_325:1000015
relationship: scale_of CO_325:0010101 ! winged petiole margin - estimation

[Term]
id: CO_325:0100050:1
name: Winged
namespace: BananaScale
synonym: "1" EXACT []
is_a: CO_325:0100050 ! wing presence/absence

[Term]
id: CO_325:0100050:2
name: Not winged
namespace: BananaScale
synonym: "2" EXACT []
is_a: CO_325:0100050 ! wing presence/absence

[Term]
id: CO_325:0100051
name: wing presence/absence and clasping presence/absence scale 1 to 5
namespace: BananaScale
is_a: CO_325:1000015
relationship: scale_of CO_325:0010101 ! winged petiole margin - estimation

[Term]
id: CO_325:0100051:1
name: Winged and undulating
namespace: BananaScale
synonym: "1" EXACT []
is_a: CO_325:0100051 ! wing presence/absence and clasping presence/absence scale 1 to 5

[Term]
id: CO_325:0100051:2
name: Winged and not clasping the pseudostem
namespace: BananaScale
synonym: "2" EXACT []
is_a: CO_325:0100051 ! wing presence/absence and clasping presence/absence scale 1 to 5

[Term]
id: CO_325:0100051:3
name: Winged and clasping the pseudostem
namespace: BananaScale
synonym: "3" EXACT []
is_a: CO_325:0100051 ! wing presence/absence and clasping presence/absence scale 1 to 5

[Term]
id: CO_325:0100051:4
name: Not winged and clasping the pseudostem
namespace: BananaScale
synonym: "4" EXACT []
is_a: CO_325:0100051 ! wing presence/absence and clasping presence/absence scale 1 to 5

[Term]
id: CO_325:0100051:5
name: Not winged and not clasping the pseudostem
namespace: BananaScale
synonym: "5" EXACT []
is_a: CO_325:0100051 ! wing presence/absence and clasping presence/absence scale 1 to 5

[Term]
id: CO_325:0100052
name: clasping or not clasping
namespace: BananaScale
is_a: CO_325:1000015
relationship: scale_of CO_325:0010102 ! petiole margin clasping - estimation

[Term]
id: CO_325:0100052:1
name: Clasping
namespace: BananaScale
synonym: "1" EXACT []
is_a: CO_325:0100052 ! clasping or not clasping

[Term]
id: CO_325:0100052:2
name: Not clasping
namespace: BananaScale
synonym: "2" EXACT []
is_a: CO_325:0100052 ! clasping or not clasping

[Term]
id: CO_325:0100053
name: bd colour chart a - 1996
namespace: BananaScale
is_a: CO_325:1000015
relationship: scale_of CO_325:0010103 ! petiole margin colour - estimation
relationship: scale_of CO_325:0010118 ! colour of bract external face - estimation
relationship: scale_of CO_325:0010119 ! colour of bract internal face - estimation

[Term]
id: CO_325:0100053:1
name: Green
namespace: BananaScale
synonym: "1" EXACT []
is_a: CO_325:0100053 ! bd colour chart a - 1996

[Term]
id: CO_325:0100053:2
name: Pink-purple to red
namespace: BananaScale
synonym: "2" EXACT []
is_a: CO_325:0100053 ! bd colour chart a - 1996

[Term]
id: CO_325:0100053:3
name: Purple to blue
namespace: BananaScale
synonym: "3" EXACT []
is_a: CO_325:0100053 ! bd colour chart a - 1996

[Term]
id: CO_325:0100053:4
name: Other
namespace: BananaScale
synonym: "4" EXACT []
is_a: CO_325:0100053 ! bd colour chart a - 1996

[Term]
id: CO_325:0100054
name: petiole-margin contrast
namespace: BananaScale
is_a: CO_325:1000015
relationship: scale_of CO_325:0010104 ! colour line along edge of petiole margin - estimation

[Term]
id: CO_325:0100054:1
name: No contrast between margin and petiole (without a colour line along)
namespace: BananaScale
synonym: "1" EXACT []
is_a: CO_325:0100054 ! petiole-margin contrast

[Term]
id: CO_325:0100054:2
name: Contrast between margin and petiole (with a contrasting colour line along)
namespace: BananaScale
synonym: "2" EXACT []
is_a: CO_325:0100054 ! petiole-margin contrast

[Term]
id: CO_325:0100055
name: bunch position scale(1 to 5)
namespace: BananaScale
is_a: CO_325:1000012
relationship: scale_of CO_325:0010106 ! bunch position - estimation

[Term]
id: CO_325:0100055:1
name: Hanging vertically
namespace: BananaScale
synonym: "1" EXACT []
is_a: CO_325:0100055 ! bunch position scale(1 to 5)

[Term]
id: CO_325:0100055:2
name: Slightly angled
namespace: BananaScale
synonym: "2" EXACT []
is_a: CO_325:0100055 ! bunch position scale(1 to 5)

[Term]
id: CO_325:0100055:3
name: Hanging at a 45 degree angle
namespace: BananaScale
synonym: "3" EXACT []
is_a: CO_325:0100055 ! bunch position scale(1 to 5)

[Term]
id: CO_325:0100055:4
name: Horizontal
namespace: BananaScale
synonym: "4" EXACT []
is_a: CO_325:0100055 ! bunch position scale(1 to 5)

[Term]
id: CO_325:0100055:5
name: Erect
namespace: BananaScale
synonym: "5" EXACT []
is_a: CO_325:0100055 ! bunch position scale(1 to 5)

[Term]
id: CO_325:0100056
name: bunch shape scale (1 to 5)
namespace: BananaScale
is_a: CO_325:1000015
relationship: scale_of CO_325:0010107 ! bunch shape - estimation

[Term]
id: CO_325:0100056:1
name: Cylindrical
namespace: BananaScale
synonym: "1" EXACT []
is_a: CO_325:0100056 ! bunch shape scale (1 to 5)

[Term]
id: CO_325:0100056:2
name: cone shaped)
namespace: BananaScale
synonym: "2" EXACT []
synonym: "Truncate (" EXACT []
is_a: CO_325:0100056 ! bunch shape scale (1 to 5)

[Term]
id: CO_325:0100056:3
name: Asymmetrical
namespace: BananaScale
synonym: "3" EXACT []
is_a: CO_325:0100056 ! bunch shape scale (1 to 5)

[Term]
id: CO_325:0100056:4
name: Spiral (all fruit are attached to a unique crown coiled around the stalk)
namespace: BananaScale
synonym: "4" EXACT []
is_a: CO_325:0100056 ! bunch shape scale (1 to 5)

[Term]
id: CO_325:0100056:5
name: Other
namespace: BananaScale
synonym: "5" EXACT []
is_a: CO_325:0100056 ! bunch shape scale (1 to 5)

[Term]
id: CO_325:0100057
name: rachis type scale (1 to 2)
namespace: BananaScale
is_a: CO_325:1000015
relationship: scale_of CO_325:0010108 ! male rachis type - estimation

[Term]
id: CO_325:0100057:1
name: Truncated
namespace: BananaScale
synonym: "1" EXACT []
is_a: CO_325:0100057 ! rachis type scale (1 to 2)

[Term]
id: CO_325:0100057:2
name: Present
namespace: BananaScale
synonym: "2" EXACT []
is_a: CO_325:0100057 ! rachis type scale (1 to 2)

[Term]
id: CO_325:0100058
name: rachis angle scale (1 to 2)
namespace: BananaScale
is_a: CO_325:1000015
relationship: scale_of CO_325:0010109 ! male rachis position - estimation

[Term]
id: CO_325:0100058:1
name: Falling vertically
namespace: BananaScale
synonym: "1" EXACT []
is_a: CO_325:0100058 ! rachis angle scale (1 to 2)

[Term]
id: CO_325:0100058:2
name: At an angle
namespace: BananaScale
synonym: "2" EXACT []
is_a: CO_325:0100058 ! rachis angle scale (1 to 2)

[Term]
id: CO_325:0100058:3
name: With a curve
namespace: BananaScale
synonym: "3" EXACT []
is_a: CO_325:0100058 ! rachis angle scale (1 to 2)

[Term]
id: CO_325:0100058:4
name: Horizontal or supra-horizontal
namespace: BananaScale
synonym: "4" EXACT []
is_a: CO_325:0100058 ! rachis angle scale (1 to 2)

[Term]
id: CO_325:0100058:5
name: Erect
namespace: BananaScale
synonym: "5" EXACT []
is_a: CO_325:0100058 ! rachis angle scale (1 to 2)

[Term]
id: CO_325:0100059
name: rachis appearance scale (1 to 5)
namespace: BananaScale
is_a: CO_325:1000015
relationship: scale_of CO_325:0010110 ! male rachis appearance - estimation

[Term]
id: CO_325:0100059:1
name: Bare
namespace: BananaScale
synonym: "1" EXACT []
is_a: CO_325:0100059 ! rachis appearance scale (1 to 5)

[Term]
id: CO_325:0100059:2
name: Neutral flowers on one to few hands only near the bunch (rest of stalk is bare)
namespace: BananaScale
synonym: "2" EXACT []
is_a: CO_325:0100059 ! rachis appearance scale (1 to 5)

[Term]
id: CO_325:0100059:3
name: Male flowers/bracts above the male bud (rest of stalk is bare)
namespace: BananaScale
synonym: "3" EXACT []
is_a: CO_325:0100059 ! rachis appearance scale (1 to 5)

[Term]
id: CO_325:0100059:4
name: Neutral/male flowers and presence of withered bracts on the entire stalk
namespace: BananaScale
synonym: "4" EXACT []
is_a: CO_325:0100059 ! rachis appearance scale (1 to 5)

[Term]
id: CO_325:0100059:5
name: Neutral/male flowers on the whole stalk without persistent bracts (still firmly attached to the rachis)
namespace: BananaScale
synonym: "5" EXACT []
is_a: CO_325:0100059 ! rachis appearance scale (1 to 5)

[Term]
id: CO_325:0100059:6
name: Small bunch from neutral/hermaphrodite flowers just above the male bud
namespace: BananaScale
synonym: "6" EXACT []
is_a: CO_325:0100059 ! rachis appearance scale (1 to 5)

[Term]
id: CO_325:0100059:7
name: Other
namespace: BananaScale
synonym: "7" EXACT []
is_a: CO_325:0100059 ! rachis appearance scale (1 to 5)

[Term]
id: CO_325:0100060
name: bud shape scale (1 to 3)
namespace: BananaScale
is_a: CO_325:1000012
relationship: scale_of CO_325:0010111 ! male bud shape - computation

[Term]
id: CO_325:0100060:1
name: Skinny (w/y less than or equal to 0.45)
namespace: BananaScale
synonym: "1" EXACT []
is_a: CO_325:0100060 ! bud shape scale (1 to 3)

[Term]
id: CO_325:0100060:2
name: Medium (0.45 < w/y < 0.55)
namespace: BananaScale
synonym: "2" EXACT []
is_a: CO_325:0100060 ! bud shape scale (1 to 3)

[Term]
id: CO_325:0100060:3
name: Fat (w/y equal to or more than 0.55)
namespace: BananaScale
synonym: "3" EXACT []
is_a: CO_325:0100060 ! bud shape scale (1 to 3)

[Term]
id: CO_325:0100061
name: bud shape scale (1 to 5)
namespace: BananaScale
is_a: CO_325:1000012
relationship: scale_of CO_325:0010111 ! male bud shape - computation

[Term]
id: CO_325:0100061:1
name: Like a top
namespace: BananaScale
synonym: "1" EXACT []
is_a: CO_325:0100061 ! bud shape scale (1 to 5)

[Term]
id: CO_325:0100061:2
name: Lanceolate
namespace: BananaScale
synonym: "2" EXACT []
is_a: CO_325:0100061 ! bud shape scale (1 to 5)

[Term]
id: CO_325:0100061:3
name: Intermediate
namespace: BananaScale
synonym: "3" EXACT []
is_a: CO_325:0100061 ! bud shape scale (1 to 5)

[Term]
id: CO_325:0100061:4
name: Ovoid
namespace: BananaScale
synonym: "4" EXACT []
is_a: CO_325:0100061 ! bud shape scale (1 to 5)

[Term]
id: CO_325:0100061:5
name: Rounded
namespace: BananaScale
synonym: "5" EXACT []
is_a: CO_325:0100061 ! bud shape scale (1 to 5)

[Term]
id: CO_325:0100062
name: bud length scale (1 to 3)
namespace: BananaScale
is_a: CO_325:1000012
relationship: scale_of CO_325:0010112 ! male bud length - measurement

[Term]
id: CO_325:0100062:1
name: Short (y less than or equal to 20 cm)
namespace: BananaScale
synonym: "1" EXACT []
is_a: CO_325:0100062 ! bud length scale (1 to 3)

[Term]
id: CO_325:0100062:2
name: Medium (20 cm < y < 30 cm)
namespace: BananaScale
synonym: "2" EXACT []
is_a: CO_325:0100062 ! bud length scale (1 to 3)

[Term]
id: CO_325:0100062:3
name: Long (equal to or more than 30 cm)
namespace: BananaScale
synonym: "3" EXACT []
is_a: CO_325:0100062 ! bud length scale (1 to 3)

[Term]
id: CO_325:0100063
name: bud size scale (1 to 3)
namespace: BananaScale
is_a: CO_325:1000012
relationship: scale_of CO_325:0010113 ! male bud size - measurement

[Term]
id: CO_325:0100063:1
name: Less than or equal to 20 cm
namespace: BananaScale
synonym: "1" EXACT []
is_a: CO_325:0100063 ! bud size scale (1 to 3)

[Term]
id: CO_325:0100063:2
name: 21-30 cm
namespace: BananaScale
synonym: "2" EXACT []
is_a: CO_325:0100063 ! bud size scale (1 to 3)

[Term]
id: CO_325:0100063:3
name: Equal to or more than 31 cm
namespace: BananaScale
synonym: "3" EXACT []
is_a: CO_325:0100063 ! bud size scale (1 to 3)

[Term]
id: CO_325:0100064
name: bud shoulder scale (1 to 3)
namespace: BananaScale
is_a: CO_325:1000012
relationship: scale_of CO_325:0010114 ! male bud shoulder - computation

[Term]
id: CO_325:0100064:1
name: High shouldered (x/y less than or equal to 0.28)
namespace: BananaScale
synonym: "1" EXACT []
is_a: CO_325:0100064 ! bud shoulder scale (1 to 3)

[Term]
id: CO_325:0100064:2
name: Medium shouldered (0.28 < x/y < 0.30)
namespace: BananaScale
synonym: "2" EXACT []
is_a: CO_325:0100064 ! bud shoulder scale (1 to 3)

[Term]
id: CO_325:0100064:3
name: Low shouldered (x/y more than or equal to 0.30)
namespace: BananaScale
synonym: "3" EXACT []
is_a: CO_325:0100064 ! bud shoulder scale (1 to 3)

[Term]
id: CO_325:0100065
name: bract apex scale (1 to 4)
namespace: BananaScale
is_a: CO_325:1000015
relationship: scale_of CO_325:0010115 ! bract apex shape - estimation

[Term]
id: CO_325:0100065:1
name: Pointed
namespace: BananaScale
synonym: "1" EXACT []
is_a: CO_325:0100065 ! bract apex scale (1 to 4)

[Term]
id: CO_325:0100065:2
name: Intermeditae
namespace: BananaScale
synonym: "2" EXACT []
is_a: CO_325:0100065 ! bract apex scale (1 to 4)

[Term]
id: CO_325:0100065:3
name: Obtuse
namespace: BananaScale
synonym: "3" EXACT []
is_a: CO_325:0100065 ! bract apex scale (1 to 4)

[Term]
id: CO_325:0100065:4
name: Obtuse and split
namespace: BananaScale
synonym: "4" EXACT []
is_a: CO_325:0100065 ! bract apex scale (1 to 4)

[Term]
id: CO_325:0100066
name: bract apex scale (1 to 5)
namespace: BananaScale
is_a: CO_325:1000015
relationship: scale_of CO_325:0010115 ! bract apex shape - estimation

[Term]
id: CO_325:0100066:1
name: Pointed
namespace: BananaScale
synonym: "1" EXACT []
is_a: CO_325:0100066 ! bract apex scale (1 to 5)

[Term]
id: CO_325:0100066:2
name: Slightly pointed
namespace: BananaScale
synonym: "2" EXACT []
is_a: CO_325:0100066 ! bract apex scale (1 to 5)

[Term]
id: CO_325:0100066:3
name: Intermediate
namespace: BananaScale
synonym: "3" EXACT []
is_a: CO_325:0100066 ! bract apex scale (1 to 5)

[Term]
id: CO_325:0100066:4
name: Obtuse
namespace: BananaScale
synonym: "4" EXACT []
is_a: CO_325:0100066 ! bract apex scale (1 to 5)

[Term]
id: CO_325:0100066:5
name: Obtuse and split
namespace: BananaScale
synonym: "5" EXACT []
is_a: CO_325:0100066 ! bract apex scale (1 to 5)

[Term]
id: CO_325:0100067
name: bract imbrication scale (1 to 3)
namespace: BananaScale
is_a: CO_325:1000015
relationship: scale_of CO_325:0010116 ! bract imbrication at apex of male bud - estimation

[Term]
id: CO_325:0100067:1
name: Convolute
namespace: BananaScale
synonym: "1" EXACT []
is_a: CO_325:0100067 ! bract imbrication scale (1 to 3)

[Term]
id: CO_325:0100067:2
name: Moderately imbricate
namespace: BananaScale
synonym: "2" EXACT []
is_a: CO_325:0100067 ! bract imbrication scale (1 to 3)

[Term]
id: CO_325:0100067:3
name: Highly imbricate
namespace: BananaScale
synonym: "3" EXACT []
is_a: CO_325:0100067 ! bract imbrication scale (1 to 3)

[Term]
id: CO_325:0100068
name: bract behaviour scale (1 to 2)
namespace: BananaScale
is_a: CO_325:1000015
relationship: scale_of CO_325:0010117 ! bract behaviour before falling - estimation

[Term]
id: CO_325:0100068:1
name: Revolute (rolling)
namespace: BananaScale
synonym: "1" EXACT []
is_a: CO_325:0100068 ! bract behaviour scale (1 to 2)

[Term]
id: CO_325:0100068:2
name: Not revolute (not rolling)
namespace: BananaScale
synonym: "2" EXACT []
is_a: CO_325:0100068 ! bract behaviour scale (1 to 2)

[Term]
id: CO_325:0100069
name: bd colour chart b - 2016
namespace: BananaScale
is_a: CO_325:1000015
relationship: scale_of CO_325:0010120 ! compound tepal main colour - estimation
relationship: scale_of CO_325:0010121 ! lobe colour of tip of compound tepal - estimation
relationship: scale_of CO_325:0010122 ! anther colour - estimation

[Term]
id: CO_325:0100069:1
name: White
namespace: BananaScale
synonym: "1" EXACT []
is_a: CO_325:0100069 ! bd colour chart b - 2016

[Term]
id: CO_325:0100069:10
name: Pink/pink-purple
namespace: BananaScale
synonym: "10" EXACT []
is_a: CO_325:0100069 ! bd colour chart b - 2016

[Term]
id: CO_325:0100069:11
name: Brown/Rusty-brown
namespace: BananaScale
synonym: "11" EXACT []
is_a: CO_325:0100069 ! bd colour chart b - 2016

[Term]
id: CO_325:0100069:12
name: Beige-pink
namespace: BananaScale
synonym: "12" EXACT []
is_a: CO_325:0100069 ! bd colour chart b - 2016

[Term]
id: CO_325:0100069:13
name: Silvery
namespace: BananaScale
synonym: "13" EXACT []
is_a: CO_325:0100069 ! bd colour chart b - 2016

[Term]
id: CO_325:0100069:14
name: Light green
namespace: BananaScale
synonym: "14" EXACT []
is_a: CO_325:0100069 ! bd colour chart b - 2016

[Term]
id: CO_325:0100069:15
name: Green
namespace: BananaScale
synonym: "15" EXACT []
is_a: CO_325:0100069 ! bd colour chart b - 2016

[Term]
id: CO_325:0100069:2
name: Cream
namespace: BananaScale
synonym: "2" EXACT []
is_a: CO_325:0100069 ! bd colour chart b - 2016

[Term]
id: CO_325:0100069:3
name: Ivory
namespace: BananaScale
synonym: "3" EXACT []
is_a: CO_325:0100069 ! bd colour chart b - 2016

[Term]
id: CO_325:0100069:4
name: Yellow
namespace: BananaScale
synonym: "4" EXACT []
is_a: CO_325:0100069 ! bd colour chart b - 2016

[Term]
id: CO_325:0100069:5
name: Bright yellow
namespace: BananaScale
synonym: "5" EXACT []
is_a: CO_325:0100069 ! bd colour chart b - 2016

[Term]
id: CO_325:0100069:6
name: Orange
namespace: BananaScale
synonym: "6" EXACT []
is_a: CO_325:0100069 ! bd colour chart b - 2016

[Term]
id: CO_325:0100069:7
name: Orange red
namespace: BananaScale
synonym: "7" EXACT []
is_a: CO_325:0100069 ! bd colour chart b - 2016

[Term]
id: CO_325:0100069:8
name: Red
namespace: BananaScale
synonym: "8" EXACT []
is_a: CO_325:0100069 ! bd colour chart b - 2016

[Term]
id: CO_325:0100069:9
name: Red-purple
namespace: BananaScale
synonym: "9" EXACT []
is_a: CO_325:0100069 ! bd colour chart b - 2016

[Term]
id: CO_325:0100070
name: bd colour chart b - 1996
namespace: BananaScale
is_a: CO_325:1000015
relationship: scale_of CO_325:0010120 ! compound tepal main colour - estimation
relationship: scale_of CO_325:0010121 ! lobe colour of tip of compound tepal - estimation
relationship: scale_of CO_325:0010122 ! anther colour - estimation

[Term]
id: CO_325:0100070:1
name: White
namespace: BananaScale
synonym: "1" EXACT []
is_a: CO_325:0100070 ! bd colour chart b - 1996

[Term]
id: CO_325:0100070:2
name: Cream
namespace: BananaScale
synonym: "2" EXACT []
is_a: CO_325:0100070 ! bd colour chart b - 1996

[Term]
id: CO_325:0100070:3
name: Yellow
namespace: BananaScale
synonym: "3" EXACT []
is_a: CO_325:0100070 ! bd colour chart b - 1996

[Term]
id: CO_325:0100070:4
name: Orange
namespace: BananaScale
synonym: "4" EXACT []
is_a: CO_325:0100070 ! bd colour chart b - 1996

[Term]
id: CO_325:0100070:5
name: Pink/pink-purple
namespace: BananaScale
synonym: "5" EXACT []
is_a: CO_325:0100070 ! bd colour chart b - 1996

[Term]
id: CO_325:0100070:6
name: Other
namespace: BananaScale
synonym: "6" EXACT []
is_a: CO_325:0100070 ! bd colour chart b - 1996

[Term]
id: CO_325:0100071
name: hands
namespace: BananaScale
is_a: CO_325:1000013
relationship: scale_of CO_325:0010123 ! number of hands on whole bunch - counting

[Term]
id: CO_325:0100072
name: fruit length scale (1 to 5)
namespace: BananaScale
is_a: CO_325:1000012
relationship: scale_of CO_325:0010126 ! fruit length - range - measurement

[Term]
id: CO_325:0100072:1
name: Less than or equal to 15 cm
namespace: BananaScale
synonym: "1" EXACT []
is_a: CO_325:0100072 ! fruit length scale (1 to 5)

[Term]
id: CO_325:0100072:2
name: 16-20 cm
namespace: BananaScale
synonym: "2" EXACT []
is_a: CO_325:0100072 ! fruit length scale (1 to 5)

[Term]
id: CO_325:0100072:3
name: 21-25 cm
namespace: BananaScale
synonym: "3" EXACT []
is_a: CO_325:0100072 ! fruit length scale (1 to 5)

[Term]
id: CO_325:0100072:4
name: 26-30 cm
namespace: BananaScale
synonym: "4" EXACT []
is_a: CO_325:0100072 ! fruit length scale (1 to 5)

[Term]
id: CO_325:0100072:5
name: Equal to or more than 31 cm
namespace: BananaScale
synonym: "5" EXACT []
is_a: CO_325:0100072 ! fruit length scale (1 to 5)

[Term]
id: CO_325:0100073
name: fruit curve shape (scale 1 to 6)
namespace: BananaScale
is_a: CO_325:1000015
relationship: scale_of CO_325:0010127 ! fruit shape of curve - estimation

[Term]
id: CO_325:0100073:1
name: Straight
namespace: BananaScale
synonym: "1" EXACT []
is_a: CO_325:0100073 ! fruit curve shape (scale 1 to 6)

[Term]
id: CO_325:0100073:2
name: Slightly curved
namespace: BananaScale
synonym: "2" EXACT []
is_a: CO_325:0100073 ! fruit curve shape (scale 1 to 6)

[Term]
id: CO_325:0100073:3
name: Straight in the distal part
namespace: BananaScale
synonym: "3" EXACT []
is_a: CO_325:0100073 ! fruit curve shape (scale 1 to 6)

[Term]
id: CO_325:0100073:4
name: Curved (sharp curve)
namespace: BananaScale
synonym: "4" EXACT []
is_a: CO_325:0100073 ! fruit curve shape (scale 1 to 6)

[Term]
id: CO_325:0100073:5
name: Curved in slight 'S' shape (double curvature)
namespace: BananaScale
synonym: "5" EXACT []
is_a: CO_325:0100073 ! fruit curve shape (scale 1 to 6)

[Term]
id: CO_325:0100073:6
name: Other
namespace: BananaScale
synonym: "6" EXACT []
is_a: CO_325:0100073 ! fruit curve shape (scale 1 to 6)

[Term]
id: CO_325:0100074
name: fruit curve shape (scale 1 to 5)
namespace: BananaScale
is_a: CO_325:1000015
relationship: scale_of CO_325:0010127 ! fruit shape of curve - estimation

[Term]
id: CO_325:0100074:1
name: Straight (or slightly curved)
namespace: BananaScale
synonym: "1" EXACT []
is_a: CO_325:0100074 ! fruit curve shape (scale 1 to 5)

[Term]
id: CO_325:0100074:2
name: Straight in the distal part
namespace: BananaScale
synonym: "2" EXACT []
is_a: CO_325:0100074 ! fruit curve shape (scale 1 to 5)

[Term]
id: CO_325:0100074:3
name: Curved (sharp curve)
namespace: BananaScale
synonym: "3" EXACT []
is_a: CO_325:0100074 ! fruit curve shape (scale 1 to 5)

[Term]
id: CO_325:0100074:4
name: Curved in 'S' shape (double curvature)
namespace: BananaScale
synonym: "4" EXACT []
is_a: CO_325:0100074 ! fruit curve shape (scale 1 to 5)

[Term]
id: CO_325:0100074:5
name: Other
namespace: BananaScale
synonym: "5" EXACT []
is_a: CO_325:0100074 ! fruit curve shape (scale 1 to 5)

[Term]
id: CO_325:0100075
name: fruit apex scale (1 to 5)
namespace: BananaScale
is_a: CO_325:1000015
relationship: scale_of CO_325:0010128 ! fruit apex point - estimation

[Term]
id: CO_325:0100075:1
name: Pointed
namespace: BananaScale
synonym: "1" EXACT []
is_a: CO_325:0100075 ! fruit apex scale (1 to 5)

[Term]
id: CO_325:0100075:2
name: Lengthily pointed (like plantain)
namespace: BananaScale
synonym: "2" EXACT []
is_a: CO_325:0100075 ! fruit apex scale (1 to 5)

[Term]
id: CO_325:0100075:3
name: Blunt-tipped (plateau at tip)
namespace: BananaScale
synonym: "3" EXACT []
is_a: CO_325:0100075 ! fruit apex scale (1 to 5)

[Term]
id: CO_325:0100075:4
name: Strongly bottle-necked (wider under tip than number 2)
namespace: BananaScale
synonym: "4" EXACT []
is_a: CO_325:0100075 ! fruit apex scale (1 to 5)

[Term]
id: CO_325:0100075:5
name: Rounded
namespace: BananaScale
synonym: "5" EXACT []
is_a: CO_325:0100075 ! fruit apex scale (1 to 5)

[Term]
id: CO_325:0100076
name: fruit relicts scale (1 to 4)
namespace: BananaScale
is_a: CO_325:1000015
relationship: scale_of CO_325:0010129 ! remains of flower relicts at fruit apex - estimation

[Term]
id: CO_325:0100076:1
name: Without flower relicts
namespace: BananaScale
synonym: "1" EXACT []
is_a: CO_325:0100076 ! fruit relicts scale (1 to 4)

[Term]
id: CO_325:0100076:2
name: Few flower relicts (< 20% of the fruits with relicts)
namespace: BananaScale
synonym: "2" EXACT []
is_a: CO_325:0100076 ! fruit relicts scale (1 to 4)

[Term]
id: CO_325:0100076:3
name: Persistent flower relicts (> 20% of the fruits with relicts)
namespace: BananaScale
synonym: "3" EXACT []
is_a: CO_325:0100076 ! fruit relicts scale (1 to 4)

[Term]
id: CO_325:0100076:4
name: Only base of the style persists
namespace: BananaScale
synonym: "4" EXACT []
is_a: CO_325:0100076 ! fruit relicts scale (1 to 4)

[Term]
id: CO_325:0100077
name: fruit relicts scale (1 to 3)
namespace: BananaScale
is_a: CO_325:1000015
relationship: scale_of CO_325:0010129 ! remains of flower relicts at fruit apex - estimation

[Term]
id: CO_325:0100077:1
name: Without any floral relicts
namespace: BananaScale
synonym: "1" EXACT []
is_a: CO_325:0100077 ! fruit relicts scale (1 to 3)

[Term]
id: CO_325:0100077:2
name: Persistent style
namespace: BananaScale
synonym: "2" EXACT []
is_a: CO_325:0100077 ! fruit relicts scale (1 to 3)

[Term]
id: CO_325:0100077:3
name: Base of the style prominent
namespace: BananaScale
synonym: "3" EXACT []
is_a: CO_325:0100077 ! fruit relicts scale (1 to 3)

[Term]
id: CO_325:0100078
name: fruit pedicel scale (1 to 3)
namespace: BananaScale
is_a: CO_325:1000012
relationship: scale_of CO_325:0010131 ! fruit pedical length - range - measurement

[Term]
id: CO_325:0100078:1
name: Less than or equal to 10 mm
namespace: BananaScale
synonym: "1" EXACT []
is_a: CO_325:0100078 ! fruit pedicel scale (1 to 3)

[Term]
id: CO_325:0100078:2
name: 11-20 mm
namespace: BananaScale
synonym: "2" EXACT []
is_a: CO_325:0100078 ! fruit pedicel scale (1 to 3)

[Term]
id: CO_325:0100078:3
name: Equal to or more than 21 mm
namespace: BananaScale
synonym: "3" EXACT []
is_a: CO_325:0100078 ! fruit pedicel scale (1 to 3)

[Term]
id: CO_325:0100079
name: fusion of pedicel scale (1 to 2)
namespace: BananaScale
is_a: CO_325:1000015
relationship: scale_of CO_325:0010132 ! fusion of pedicels - estimation

[Term]
id: CO_325:0100079:1
name: No visible sign of fusion
namespace: BananaScale
synonym: "1" EXACT []
is_a: CO_325:0100079 ! fusion of pedicel scale (1 to 2)

[Term]
id: CO_325:0100079:2
name: Partially fused 9up to 50% of the length of the pedicel)
namespace: BananaScale
synonym: "2" EXACT []
is_a: CO_325:0100079 ! fusion of pedicel scale (1 to 2)

[Term]
id: CO_325:0100080
name: 1 to 5 acceptability score
namespace: BananaScale
is_a: CO_325:1000012
relationship: scale_of CO_325:0010133 ! visual appearance  - estimation
relationship: scale_of CO_325:0010133 ! visual appearance  - estimation
relationship: scale_of CO_325:0010134 ! taste  - estimation
relationship: scale_of CO_325:0010134 ! taste  - estimation
relationship: scale_of CO_325:0010135 ! finger feel  - estimation
relationship: scale_of CO_325:0010135 ! finger feel  - estimation
relationship: scale_of CO_325:0010136 ! smoothness-mouth feel - estimation
relationship: scale_of CO_325:0010136 ! smoothness-mouth feel - estimation
relationship: scale_of CO_325:0010137 ! nosal smell  - estimation

[Term]
id: CO_325:0100080:1 
name: Dislike very much
namespace: BananaScale
synonym: "1" EXACT []
is_a: CO_325:0100080 ! 1 to 5 acceptability score

[Term]
id: CO_325:0100080:2
name: Dislike
namespace: BananaScale
synonym: "2" EXACT []
is_a: CO_325:0100080 ! 1 to 5 acceptability score

[Term]
id: CO_325:0100080:3
name: Like fairly
namespace: BananaScale
synonym: "3" EXACT []
is_a: CO_325:0100080 ! 1 to 5 acceptability score

[Term]
id: CO_325:0100080:4
name: Like very much
namespace: BananaScale
synonym: "4" EXACT []
is_a: CO_325:0100080 ! 1 to 5 acceptability score

[Term]
id: CO_325:0100080:5 
name: Like extremely
namespace: BananaScale
synonym: "5" EXACT []
is_a: CO_325:0100080 ! 1 to 5 acceptability score

[Term]
id: CO_325:0100081
name: %
namespace: BananaScale
is_a: CO_325:1000013
relationship: scale_of CO_325:0010138 ! peripheral damage - measurement
relationship: scale_of CO_325:0010140 ! percentage of root necrosis - method
relationship: scale_of CO_325:0010181 ! black sigatoka disease severity - estimation
relationship: scale_of CO_325:0010194 ! percentage of plants with yellowing leaves caused by fusarium wilt - computation
relationship: scale_of CO_325:0010195 ! percentage of plants with a splitting pseudostem base caused by fusarium wilt - computation
relationship: scale_of CO_325:0010196 ! percentage of plants with changes in new leaves caused by fusarium wilt - computation
relationship: scale_of CO_325:0010197 ! percentage of plants with petiole collapse caused by fusarium wilt - computation
relationship: scale_of CO_325:0010198 ! percentage of plants with external disease symptoms caused by fusarium wilt - computation
relationship: scale_of CO_325:0010199 ! percentage of plants with internal disease symptoms caused by fusarium wilt - computation
relationship: scale_of CO_325:0010210 ! damage index-x-inner - measurement
relationship: scale_of CO_325:0010211 ! damage index-x-outer - measurement

[Term]
id: CO_325:0100082
name: multiplication factor
namespace: BananaScale
is_a: CO_325:1000013
relationship: scale_of CO_325:0010139 ! nematode multiplication from single root inoculation - computation

[Term]
id: CO_325:0100083
name: Number
namespace: BananaScale
is_a: CO_325:1000013
relationship: scale_of CO_325:0010141 ! number of functional roots - method
relationship: scale_of CO_325:0010142 ! number of dead roots - method

[Term]
id: CO_325:0100084
name: No. per 100ml
namespace: BananaScale
is_a: CO_325:1000013
relationship: scale_of CO_325:0010143 ! number of nematodes (unclassified spp.) per unit fresh root weight - method

[Term]
id: CO_325:0100085
name: No. per 10g
namespace: BananaScale
is_a: CO_325:1000013
relationship: scale_of CO_325:0010144 ! number of nematodes (radopholus similis ) per  unit fresh root weight - method
relationship: scale_of CO_325:0010145 ! number of nematodes (helicotylenchus multicinctus) per  unit fresh root weight - method
relationship: scale_of CO_325:0010146 ! number of nematodes (rotylenchulus spp.) per  unit fresh root weight - method
relationship: scale_of CO_325:0010147 ! number of nematodes (meloidogyne spp.) per  unit fresh root weight - method
relationship: scale_of CO_325:0010148 ! number of nematodes (pratylenchus spp.) per  unit fresh root weight - method
relationship: scale_of CO_325:0010149 ! number of nematodes (hoplolaimus spp.) per  unit fresh root weight - method
relationship: scale_of CO_325:0010150 ! number of nematodes (pratylenchus goodeyi) per  unit fresh root weight - method
relationship: scale_of CO_325:0010151 ! number of nematodes (pratylenchus coffeae) per  unit fresh root weight - method
relationship: scale_of CO_325:0010152 ! number of nematodes per  unit fresh root weight
relationship: scale_of CO_325:0010153 ! number of nematodes (radopholus similis ) per  unit fresh root weight -method
relationship: scale_of CO_325:0010154 ! number of nematodes (meloidogyne spp.)  per  unit fresh root weight -method
relationship: scale_of CO_325:0010155 ! number of nematodes (pratylenchus spp.)  per  unit fresh root weight -method
relationship: scale_of CO_325:0010156 ! number of nematodes (hoplolaimus spp.)  per  unit fresh root weight -method
relationship: scale_of CO_325:0010157 ! number of nematodes (pratylenchus goodeyi)  per  unit fresh root weight -method
relationship: scale_of CO_325:0010158 ! number of nematodes (pratylenchus coffeae)  per  unit fresh root weight -method

[Term]
id: CO_325:0100086
name: leaf rank
namespace: BananaScale
is_a: CO_325:1000013
relationship: scale_of CO_325:0010159 ! youngest leaf spotted - counting
relationship: scale_of CO_325:0010161 ! rank of oldest standing leaf - counting
relationship: scale_of CO_325:0010173 ! rank of youngest leaf - counting
relationship: scale_of CO_325:0010174 ! rank of previously marked leaf - counting

[Term]
id: CO_325:0100087
name: Index
namespace: BananaScale
is_a: CO_325:1000013
relationship: scale_of CO_325:0010162 ! black sigatoka disease infection index - computation
relationship: scale_of CO_325:0010180 ! index of non-spotted leaves - computation

[Term]
id: CO_325:0100088
name: 5 pt corm discolouration scale
namespace: BananaScale
is_a: CO_325:1000015
relationship: scale_of CO_325:0010168 ! extent of internal discolouration in corm of plant caused by fusarium wilt - estimation
relationship: scale_of CO_325:0010170 ! extent of internal discolouration in corm of tallest sucker caused by fusarium wilt - estimation

[Term]
id: CO_325:0100088:1
name: Corm completely clean, no vascular discolouration
namespace: BananaScale
synonym: "1" EXACT []
is_a: CO_325:0100088 ! 5 pt corm discolouration scale

[Term]
id: CO_325:0100088:2
name: Isolated points of discolouration in vascular tissue
namespace: BananaScale
synonym: "2" EXACT []
is_a: CO_325:0100088 ! 5 pt corm discolouration scale

[Term]
id: CO_325:0100088:3
name: Discolouration of up to one-third of vascular tissue
namespace: BananaScale
synonym: "3" EXACT []
is_a: CO_325:0100088 ! 5 pt corm discolouration scale

[Term]
id: CO_325:0100088:4
name: Discolouration of between one-third and two-thirds of vascular tissue
namespace: BananaScale
synonym: "4" EXACT []
is_a: CO_325:0100088 ! 5 pt corm discolouration scale

[Term]
id: CO_325:0100088:5
name: Discolouration greater than two-thirds of vascular tissue
namespace: BananaScale
synonym: "5" EXACT []
is_a: CO_325:0100088 ! 5 pt corm discolouration scale

[Term]
id: CO_325:0100088:6
name: Total discolouration of vascular tissue
namespace: BananaScale
synonym: "6" EXACT []
is_a: CO_325:0100088 ! 5 pt corm discolouration scale

[Term]
id: CO_325:0100089
name: presence/absence scale
namespace: BananaScale
is_a: CO_325:1000012
relationship: scale_of CO_325:0010171 ! presence of petiole collapse caused by fusarium wilt - estimation
relationship: scale_of CO_325:0010171 ! presence of petiole collapse caused by fusarium wilt - estimation
relationship: scale_of CO_325:0010190 ! presence of yellowing leaves caused by fusarium wilt - estimation
relationship: scale_of CO_325:0010190 ! presence of yellowing leaves caused by fusarium wilt - estimation
relationship: scale_of CO_325:0010191 ! presence of splitting pseudostem base caused by fusarium wilt - estimation
relationship: scale_of CO_325:0010191 ! presence of splitting pseudostem base caused by fusarium wilt - estimation
relationship: scale_of CO_325:0010192 ! presence of changes in new leaves caused by fusarium wilt - estimation
relationship: scale_of CO_325:0010192 ! presence of changes in new leaves caused by fusarium wilt - estimation

[Term]
id: CO_325:0100089:1
name: Absent
namespace: BananaScale
synonym: "1" EXACT []
is_a: CO_325:0100089 ! presence/absence scale

[Term]
id: CO_325:0100089:2
name: Present
namespace: BananaScale
synonym: "2" EXACT []
is_a: CO_325:0100089 ! presence/absence scale

[Term]
id: CO_325:0100090
name: leaves/month
namespace: BananaScale
is_a: CO_325:1000013
relationship: scale_of CO_325:0010175 ! leaf emission rate - computation

[Term]
id: CO_325:0100091
name: leaves/week
namespace: BananaScale
is_a: CO_325:1000013
relationship: scale_of CO_325:0010175 ! leaf emission rate - computation

[Term]
id: CO_325:0100092
name: leaf
namespace: BananaScale
is_a: CO_325:1000013
relationship: scale_of CO_325:0010176 ! number of functional leaves - counting
relationship: scale_of CO_325:0010178 ! number of spotted leaves - counting
relationship: scale_of CO_325:0010179 ! number of standing leaves - counting
relationship: scale_of CO_325:0010182 ! number of leaves with black sigatoka disease severity grade 0 - computation
relationship: scale_of CO_325:0010183 ! number of leaves with black sigatoka disease severity grade 1 - computation
relationship: scale_of CO_325:0010184 ! number of leaves with black sigatoka disease severity grade 2 - computation
relationship: scale_of CO_325:0010185 ! number of leaves with black sigatoka disease severity grade 3 - computation
relationship: scale_of CO_325:0010186 ! number of leaves with black sigatoka disease severity grade 4 - computation
relationship: scale_of CO_325:0010187 ! number of leaves with black sigatoka disease severity grade 5 - computation
relationship: scale_of CO_325:0010188 ! number of leaves with black sigatoka disease severity grade 6 - computation

[Term]
id: CO_325:0100093
name: gauhl's modification of stover's severity scoring system (yyyy)
namespace: BananaScale
is_a: CO_325:1000015
relationship: scale_of CO_325:0010181 ! black sigatoka disease severity - estimation

[Term]
id: CO_325:0100093:0
name: No symptoms
namespace: BananaScale
synonym: "0" EXACT []
is_a: CO_325:0100093 ! gauhl's modification of stover's severity scoring system (yyyy)

[Term]
id: CO_325:0100093:1
name: Less than 1% of lamina with symptoms, only streaks and/or up to 10 spots
namespace: BananaScale
synonym: "1" EXACT []
is_a: CO_325:0100093 ! gauhl's modification of stover's severity scoring system (yyyy)

[Term]
id: CO_325:0100093:2
name: 1-5% of lamina with symptoms
namespace: BananaScale
synonym: "2" EXACT []
is_a: CO_325:0100093 ! gauhl's modification of stover's severity scoring system (yyyy)

[Term]
id: CO_325:0100093:3
name: 6-15% of lamina with symptoms
namespace: BananaScale
synonym: "3" EXACT []
is_a: CO_325:0100093 ! gauhl's modification of stover's severity scoring system (yyyy)

[Term]
id: CO_325:0100093:4
name: 16-33% of lamina with symptoms
namespace: BananaScale
synonym: "4" EXACT []
is_a: CO_325:0100093 ! gauhl's modification of stover's severity scoring system (yyyy)

[Term]
id: CO_325:0100093:5
name: 34-50% of lamina with symptoms
namespace: BananaScale
synonym: "5" EXACT []
is_a: CO_325:0100093 ! gauhl's modification of stover's severity scoring system (yyyy)

[Term]
id: CO_325:0100093:6
name: 51-100% of lamina with symptoms
namespace: BananaScale
synonym: "6" EXACT []
is_a: CO_325:0100093 ! gauhl's modification of stover's severity scoring system (yyyy)

[Term]
id: CO_325:0100094
name: faure's stages of development of bls disease scale (1987)
namespace: BananaScale
is_a: CO_325:1000015
relationship: scale_of CO_325:0010181 ! black sigatoka disease severity - estimation

[Term]
id: CO_325:0100094:1
name: Stage 1 appears as a small depigmentation spot whose whitish or yellow colour resembles stage 1 of Yellow Sigatoka disease. These symptoms are not visible in transmitted light and can be observed only on the underside of the leaf.
namespace: BananaScale
synonym: "1" EXACT []
is_a: CO_325:0100094 ! faure's stages of development of bls disease scale (1987)

[Term]
id: CO_325:0100094:2
name: Stage 2 appears as a stripe, generally brown in colour and visible on the underside of the leaf; later the symptom also appears on the upper part of the limb as a stripe, the yellow colour of which resembles the stripe at stage 1 of Yellow Sigatoka. The colour of this stripe will change progressively from brown and later to black on the upper side of the limb, but will retain the brown colour on the underside.
namespace: BananaScale
synonym: "2" EXACT []
is_a: CO_325:0100094 ! faure's stages of development of bls disease scale (1987)

[Term]
id: CO_325:0100094:3
name: Stage 3 differs from the previous one by its dimensions. The stripe becomes longer, is enlarged and in certain conditions (weak inoculum and unfavourable climatic conditions) can reach 2 or 3 cm.
namespace: BananaScale
synonym: "3" EXACT []
is_a: CO_325:0100094 ! faure's stages of development of bls disease scale (1987)

[Term]
id: CO_325:0100094:4
name: Stage 4 appears on the underside as a brown spot and on the upper side as a black spot.
namespace: BananaScale
synonym: "4" EXACT []
is_a: CO_325:0100094 ! faure's stages of development of bls disease scale (1987)

[Term]
id: CO_325:0100094:5
name: Stage 5 is when the elliptical spot is totally black and has spread to the underside of the limb. It is surrounded by a yellow halo with the centre beginning to flatten out.
namespace: BananaScale
synonym: "5" EXACT []
is_a: CO_325:0100094 ! faure's stages of development of bls disease scale (1987)

[Term]
id: CO_325:0100094:6
name: Stage 6 is when the centre of the spot dries out, turns clear gray and is surrounded by a well-defined black ring, which is, in turn, surrounded by a bright yellow halo. These spots remain visible after the leaf has dried out because the ring persists.
namespace: BananaScale
synonym: "6" EXACT []
is_a: CO_325:0100094 ! faure's stages of development of bls disease scale (1987)

[Term]
id: CO_325:0100095
name: meredith & lawrence (1969) - complete
namespace: BananaScale
is_a: CO_325:1000015
relationship: scale_of CO_325:0010181 ! black sigatoka disease severity - estimation

[Term]
id: CO_325:0100095:1
name: Initial speck stage: symptoms are first visible to the naked eye as faint, minute (less than 0.25 mm diam), reddish brown specks on the lower surface of the leaf. Specks are often most abundant near the margin of the left side of the leaf, particularly towards the tip. Where leaf spot is severe, specks have been observed on the second leaf of plants that have not yet produced a bunch. Elsewhere they usually appear on the third, fourth, or older leaves.
namespace: BananaScale
synonym: "1" EXACT []
is_a: CO_325:0100095 ! meredith & lawrence (1969) - complete

[Term]
id: CO_325:0100095:2
name: First streak stage: the initial speck elongates, becoming slightly wider, to form a characteristic narrow, reddish brown streak up to 20 mm long and 2.0 mm wide, with the long axis parallel to the leaf venation. At this stage, streaks are more clearly visible on the lower surface of the leaf than on the upper one. The distribution of streaks is variable. Sometimes they are most numerous near the edge of the left side of the leaf. At other times they are equally numerous on both sides of the leaf, and more or less evenly distributed. Frequently they are densely aggregated in a band several cm wide on one side or both sides of the mid-rib, becoming less numerous towards the edge of the leaf. Streaks may be so numerous that every cm2 of leaf surface bears one or more. There is considerable variation in the length of individual streaks on a given leaf, and they frequently overlap to form larger, compound streaks.
namespace: BananaScale
synonym: "2" EXACT []
is_a: CO_325:0100095 ! meredith & lawrence (1969) - complete

[Term]
id: CO_325:0100095:3
name: Second-streak stage: the streaks may elongate slightly, but the most notable change is that in colour from reddish brown to dark brown or almost black, sometimes with a purplish tinge. The streak is now clearly visible on the upper surface of the leaf. The distribution of streaks at this stage of development varies in the same way as mentioned above. When streaks are very numerous, and more or less evenly distributed, the entire leaf blackens.
namespace: BananaScale
synonym: "3" EXACT []
is_a: CO_325:0100095 ! meredith & lawrence (1969) - complete

[Term]
id: CO_325:0100095:4
name: First-spot stage: the streak broadens and becomes more or less fusiform and elliptical in outline and similar to the 'first-spot stage' of Sigatoka (Leach 1946). The transition from streak to spot is further characterised by the development of a light brown, water-soaked border around the spot. This water-soaked effect is especially clear in the early morning, when dew is still present on the leaf, or after rain.
namespace: BananaScale
synonym: "4" EXACT []
is_a: CO_325:0100095 ! meredith & lawrence (1969) - complete

[Term]
id: CO_325:0100095:5
name: Second-spot stage: the dark brown or black central area of the spot becomes slightly depressed and the water-soaked border becomes more pronounced due to darkening. At this stage, a slight yellowing of the leaf tissue immediately surrounding the water-soaked border may occur.
namespace: BananaScale
synonym: "5" EXACT []
is_a: CO_325:0100095 ! meredith & lawrence (1969) - complete

[Term]
id: CO_325:0100095:6
name: Third or mature spot stage: the centre of the spot dries out, becoming light grey or buff-coloured, and further depressed. The spot is surrounded by a narrow, well-defined, dark brown or black border. between the latter and the normal green colour of the leaf, there is often a bright yellow transitional zone. After the leaf has collapsed and withered, spots remain clearly visible because of the light-coloured centre and dark border.
namespace: BananaScale
synonym: "6" EXACT []
is_a: CO_325:0100095 ! meredith & lawrence (1969) - complete

[Term]
id: CO_325:0100096
name: meredith & lawrence (1969) - condensed
namespace: BananaScale
is_a: CO_325:1000015
relationship: scale_of CO_325:0010181 ! black sigatoka disease severity - estimation

[Term]
id: CO_325:0100096:1
name: Initial speck stage: faint, minute, reddish-brown specks on the lower surface of the leaf.
namespace: BananaScale
synonym: "1" EXACT []
is_a: CO_325:0100096 ! meredith & lawrence (1969) - condensed

[Term]
id: CO_325:0100096:2
name: First streak stage: specks elongate, becoming slightly wider to form narrow reddish-brown streaks.
namespace: BananaScale
synonym: "2" EXACT []
is_a: CO_325:0100096 ! meredith & lawrence (1969) - condensed

[Term]
id: CO_325:0100096:3
name: Second-streak stage: streaks change colour from reddish brown to dark brown or black, sometimes with a purplish tinge, clearly visible at the upper surface of the leaf.
namespace: BananaScale
synonym: "3" EXACT []
is_a: CO_325:0100096 ! meredith & lawrence (1969) - condensed

[Term]
id: CO_325:0100096:4
name: First-spot stage: the streaks broaden and become more or less fusiform or elliptical in outline and a water soaked border appears around each lesion.
namespace: BananaScale
synonym: "4" EXACT []
is_a: CO_325:0100096 ! meredith & lawrence (1969) - condensed

[Term]
id: CO_325:0100096:5
name: Second-spot stage: the dark brown or black centre of each lesion becomes slightly depressed and water soaked border becomes more pronounced.
namespace: BananaScale
synonym: "5" EXACT []
is_a: CO_325:0100096 ! meredith & lawrence (1969) - condensed

[Term]
id: CO_325:0100096:6
name: Third or mature spot stage: the centres of the lesions dry out becoming light grey or buff coloured and a bright yellow transitional zone appears between them and the normal green colour of the leaf. The lesions remain clearly visible after the leaf has collapsed or withered because of their light coloured centre and dark border.
namespace: BananaScale
synonym: "6" EXACT []
is_a: CO_325:0100096 ! meredith & lawrence (1969) - condensed

[Term]
id: CO_325:0100097
name: Ex: g/100 mL juice????
namespace: BananaScale
is_a: CO_325:1000013
relationship: scale_of CO_325:0010200 ! vitamin c - measurement

[Term]
id: CO_325:0100098
name: weevil
namespace: BananaScale
is_a: CO_325:1000013
relationship: scale_of CO_325:0010201 ! number of adult weevils - counting
relationship: scale_of CO_325:0010201 ! number of adult weevils - counting
relationship: scale_of CO_325:0010202 ! number of adult weevil trap - counting
relationship: scale_of CO_325:0010203 ! number of weevil larvae - counting
relationship: scale_of CO_325:0010203 ! number of weevil larvae - counting
relationship: scale_of CO_325:0010203 ! number of weevil larvae - counting
relationship: scale_of CO_325:0010204 ! number of adult larvae - counting

[Term]
id: CO_325:0100099
name: ?M
namespace: BananaScale
is_a: CO_325:1000013
relationship: scale_of CO_325:0010205 ! adult weevil head capsule - measurement
relationship: scale_of CO_325:0010205 ! adult weevil head capsule - measurement
relationship: scale_of CO_325:0010206 ! adult weevil body - measurement
relationship: scale_of CO_325:0010206 ! adult weevil body - measurement
relationship: scale_of CO_325:0010207 ! weevil larvae head capsule - measurement
relationship: scale_of CO_325:0010207 ! weevil larvae head capsule - measurement
relationship: scale_of CO_325:0010208 ! weevil larvae body length - measurement
relationship: scale_of CO_325:0010208 ! weevil larvae body length - measurement

[Term]
id: CO_325:0100100
name: mg
namespace: BananaScale
is_a: CO_325:1000013
relationship: scale_of CO_325:0010206 ! adult weevil body - measurement
relationship: scale_of CO_325:0010206 ! adult weevil body - measurement
relationship: scale_of CO_325:0010209 ! weevil larvae body weight - measurement
relationship: scale_of CO_325:0010209 ! weevil larvae body weight - measurement

[Term]
id: CO_325:1000000
name: Physiological
namespace: BananaTrait
is_a: CO_325:1000023 ! Banana Ontology

[Term]
id: CO_325:1000001
name: Biotic_stress
namespace: BananaTrait
is_a: CO_325:1000023 ! Banana Ontology

[Term]
id: CO_325:1000002
name: Phenological
namespace: BananaTrait
is_a: CO_325:1000023 ! Banana Ontology

[Term]
id: CO_325:1000003
name: Quality_traits
namespace: BananaTrait
is_a: CO_325:1000023 ! Banana Ontology

[Term]
id: CO_325:1000004
name: ??
namespace: BananaTrait
is_a: CO_325:1000023 ! Banana Ontology

[Term]
id: CO_325:1000005
name: Agronomical
namespace: BananaTrait
is_a: CO_325:1000023 ! Banana Ontology

[Term]
id: CO_325:1000006
name: Biochemical
namespace: BananaTrait
is_a: CO_325:1000023 ! Banana Ontology

[Term]
id: CO_325:1000007
name: Morphological
namespace: BananaTrait
is_a: CO_325:1000023 ! Banana Ontology

[Term]
id: CO_325:1000008
name: Measurement
namespace: BananaMethod
is_a: CO_325:1000021 ! Method

[Term]
id: CO_325:1000009
name: Counting
namespace: BananaMethod
is_a: CO_325:1000021 ! Method

[Term]
id: CO_325:1000010
name: Computation
namespace: BananaMethod
is_a: CO_325:1000021 ! Method

[Term]
id: CO_325:1000011
name: Estimation
namespace: BananaMethod
is_a: CO_325:1000021 ! Method

[Term]
id: CO_325:1000012
name: Ordinal
namespace: BananaScale
is_a: CO_325:1000022 ! Scale

[Term]
id: CO_325:1000013
name: numerical
namespace: BananaScale
is_a: CO_325:1000022 ! Scale

[Term]
id: CO_325:1000014
name: Text
namespace: BananaScale
is_a: CO_325:1000022 ! Scale

[Term]
id: CO_325:1000015
name: Nominal
namespace: BananaScale
is_a: CO_325:1000022 ! Scale

[Term]
id: CO_325:1000016
name: Duration
namespace: BananaScale
is_a: CO_325:1000022 ! Scale

[Term]
id: CO_325:1000017
name: Numerical
namespace: BananaScale
is_a: CO_325:1000022 ! Scale

[Term]
id: CO_325:1000018
name: Time
namespace: BananaScale
is_a: CO_325:1000022 ! Scale

[Term]
id: CO_325:1000019
name: supplementary_variable
namespace: Banana
is_a: CO_325:1000024 ! Variable

[Term]
id: CO_325:1000020
name: breeding_variable
namespace: Banana
is_a: CO_325:1000024 ! Variable

[Term]
id: CO_325:1000021
name: Method
namespace: BananaMethod

[Term]
id: CO_325:1000022
name: Scale
namespace: BananaScale

[Term]
id: CO_325:1000023
name: Banana Ontology
namespace: BananaTrait

[Term]
id: CO_325:1000024
name: Variable
namespace: Banana

[Typedef]
id: method_of
name: method_of

[Typedef]
id: scale_of
name: scale_of

[Typedef]
id: variable_of
name: variable_of

