format-version: 1.2
date: 11:04:2018 16:34
saved-by: guillaume
auto-generated-by: OBO-Edit 2.3.1
default-namespace: banana_trait_ontology
namespace-id-rule: * CO_325:$sequence(7,0000000,0009999)$
ontology: CO_325

[Term]
id: CO_325:0000000
name: CGIAR banana trait ontology
namespace: BananaTrait

[Term]
id: CO_325:0000001
name: flowering
namespace: BananaTrait
def: "Developmental stage where bloom or blossom on a banana plant." []
synonym: "FLW" RELATED []
is_a: CO_325:1000005 ! Physiological
created_by: guillaume
creation_date: 2018-04-11T01:02:17Z

[Term]
id: CO_325:0000002
name: fruit maturity-harvest
namespace: BananaTrait
def: "Physiological stage at which the fruit is mature and can be  harvested." []
synonym: "HVST" RELATED []
is_a: CO_325:1000005 ! Physiological
created_by: guillaume
creation_date: 2018-04-11T01:11:15Z

[Term]
id: CO_325:0000003
name: time from shooting to harvest
namespace: BananaTrait
def: "The time elapsed from shooting (when the inflorescence emerges from the pseudostem and is still in an erect position) to the harvest of the bunch." []
synonym: "shoot2harvest" EXACT []
synonym: "Time of fruit-filling, Fruit-filling period, Bunch maturity period, Length of reproductive stage, Bunch maturation period" EXACT []
is_a: CO_325:1000004 ! Phenological

[Term]
id: CO_325:0000004
name: Flowering of the plant
namespace: BananaTrait
is_a: CO_325:1000024 ! Variable
relationship: variable_of CO_325:0000001 ! flowering
created_by: guillaume
creation_date: 2018-04-11T11:01:27Z

[Term]
id: CO_325:0000005
name: fruit maturity of the plant
namespace: BananaTrait
is_a: CO_325:1000024 ! Variable
relationship: variable_of CO_325:0000002 ! fruit maturity-harvest
created_by: guillaume
creation_date: 2018-04-11T11:32:48Z

[Term]
id: CO_325:0000006
name: plant crop cycle
namespace: BananaTrait
def: "The time elapsed from planting to the harvest of the bunch." []
synonym: "Crop cycle, Mother plant crop cycle, Time from planting to harvest" EXACT []
synonym: "plant2harvest" EXACT []
is_a: CO_325:1000004 ! Phenological

[Term]
id: CO_325:0000009
name: plant height
namespace: BananaTrait
def: "The height of the pseudostem of the plant, from the collar to the intersection of the petioles of the two youngest leaves." []
synonym: "plantheightpetioles" EXACT []
synonym: "Pseudostem height" EXACT []
is_a: CO_325:1000001 ! Agronomical

[Term]
id: CO_325:0000012
name: plant circumference from the collar
namespace: BananaTrait
def: "The circumference of the pseudostem of the plant at 100 cm from the collar." []
synonym: "plantcircumf100cm" EXACT []
synonym: "Pseudostem girth, Plant circumference, Pseudostem circumference, Plant girth" EXACT []
is_a: CO_325:1000001 ! Agronomical

[Term]
id: CO_325:0000021
name: monthly leaf emission rate
namespace: BananaTrait
def: "A rate that expresses the number of leaves that have emerged from the pseudostem in a month." []
synonym: "LER" EXACT []
is_a: CO_325:1000005 ! Physiological

[Term]
id: CO_325:0000024
name: number of suckers
namespace: BananaTrait
def: "The number of all types of suckers in the mat." []
synonym: "numsuckers" EXACT []
is_a: CO_325:1000001 ! Agronomical

[Term]
id: CO_325:0000027
name: tallest sucker height
namespace: BananaTrait
def: "The height of the pseudostem of the tallest sucker within the same mat as the plant (the sucker that will become the next plant with a bunch, once the bunch from the current plant is harvested)" []
synonym: "Height of tallest sucker, Following sucker height, Height of following sucker" EXACT []
synonym: "suckerheight" EXACT []
is_a: CO_325:1000001 ! Agronomical

[Term]
id: CO_325:0000033
name: bunch weight
namespace: BananaTrait
def: "The weight of the bunch, including the rachis." []
synonym: "bunchweight" EXACT []
is_a: CO_325:1000001 ! Agronomical

[Term]
id: CO_325:0000036
name: number of hands in bunch
namespace: BananaTrait
def: "The number of hands in the bunch." []
synonym: "numhands" EXACT []
is_a: CO_325:1000001 ! Agronomical

[Term]
id: CO_325:0000039
name: number of fingers in bunch
namespace: BananaTrait
def: "The number of fingers in the bunch." []
synonym: "numfingersbunch" EXACT []
is_a: CO_325:1000001 ! Agronomical

[Term]
id: CO_325:0000042
name: number of fingers in hand: count
namespace: BananaTrait
def: "The number of fingers in a third hand." []
synonym: "numfingershand" EXACT []
is_a: CO_325:1000001 ! Agronomical

[Term]
id: CO_325:0000045
name: hand weight
namespace: BananaTrait
def: "The weight of a hand." []
synonym: "handweight" EXACT []
is_a: CO_325:1000001 ! Agronomical

[Term]
id: CO_325:0000048
name: finger weight
namespace: BananaTrait
def: "The weight of a finger." []
synonym: "fingerweight" EXACT []
is_a: CO_325:1000001 ! Agronomical

[Term]
id: CO_325:0000051
name: finger external length
namespace: BananaTrait
def: "The length of a finger measured along the external (dorsal) arc, excluding the pedicel and the fruit tip." []
synonym: "Finger dorsal length" EXACT []
synonym: "fingerextlength" EXACT []
is_a: CO_325:1000001 ! Agronomical

[Term]
id: CO_325:0000054
name: finger circumference
namespace: BananaTrait
def: "The circumference of a finger." []
synonym: "Finger girth" EXACT []
synonym: "fingercircumf" EXACT []
is_a: CO_325:1000001 ! Agronomical

[Term]
id: CO_325:0000057
name: black leaf streak disease incubation time
namespace: BananaTrait
def: "The time elapsed between a tagged cigar leaf at Brun's stage B of unrolling and the development of black leaf streak disease symptoms at Foure's black leaf streak disease severity grade 1." []
synonym: "Black Sigatoka disease incubation time" EXACT []
synonym: "DIT" EXACT []
is_a: CO_325:1000002 ! Biotic_stress

[Term]
id: CO_325:0000060
name: black leaf streak disease evolution time
namespace: BananaTrait
def: "The time elapsed between the development of black leaf streak disease symptoms at Foure's black leaf streak disease severity grade 1, to 6." []
synonym: "Black Sigatoka disease evolution time" EXACT []
synonym: "DET" EXACT []
is_a: CO_325:1000002 ! Biotic_stress

[Term]
id: CO_325:0000066
name: number of functional leaves
namespace: BananaTrait
def: "The number of leaves on the plant that have 50% or more of the leaf surface area as green, healthy, photosynthetic tissue." []
synonym: "functleaves" EXACT []
is_a: CO_325:1000001 ! Agronomical

[Term]
id: CO_325:0000069
name: number of standing leaves
namespace: BananaTrait
def: "The number of leaves attached to the plant that have an erect petiole (not bent or broken)." []
is_a: CO_325:1000002 ! Biotic_stress

[Term]
id: CO_325:0000072
name: extent of internal discolouration in corm of tallest sucker caused by fusarium wilt
namespace: BananaTrait
def: "The extent of discolouration in the corm of the tallest sucker, caused by Fusarium wilt." []
is_a: CO_325:1000002 ! Biotic_stress

[Term]
id: CO_325:0000075
name: distance of internal discolouration in pseudostem of plant caused by fusarium wilt
namespace: BananaTrait
def: "The distance of discolouration in the pseudostem of the plant, caused by Fusarium wilt." []
is_a: CO_325:1000002 ! Biotic_stress

[Term]
id: CO_325:0000078
name: percentage of plants with external disease symptoms caused by fusarium wilt
namespace: BananaTrait
def: "The percentage of plants with any or multiple of the external disease symptoms - yellowing leaves, splitting of pseudostem base, changes in new leaves, petiole collapse, caused by Fusarium wilt." []
is_a: CO_325:1000002 ! Biotic_stress

[Term]
id: CO_325:0000081
name: percentage of plants with internal disease symptoms caused by fusarium wilt
namespace: BananaTrait
def: "The percentage of plants with any or multiple of the internal disease symptoms - discolouration in the corm, and/or discolouration in the pseudostem, caused by Fusarium wilt." []
is_a: CO_325:1000002 ! Biotic_stress

[Term]
id: CO_325:0000084
name: time from start of crop cycle to first external disease symptoms caused by fusarium wilt
namespace: BananaTrait
def: "The time elapsed from the start of the crop cycle to the appearance on the plant of any of the external disease symptoms - - yellowing leaves, splitting pseudostem base, changes in new leaves, petiole collapse, caused by Fusarium wilt." []
is_a: CO_325:1000002 ! Biotic_stress

[Term]
id: CO_325:0000087
name: presence of yellowing leaves caused by fusarium wilt
namespace: BananaTrait
def: "The presence/absence of yellowing leaves, caused by Fusarium wilt." []
synonym: "YL" EXACT []
is_a: CO_325:1000002 ! Biotic_stress

[Term]
id: CO_325:0000090
name: presence of splitting pseudostem base caused by fusarium wilt
namespace: BananaTrait
def: "The presence/absence of a splitting pseudostem base, caused by Fusarium wilt." []
synonym: "SP" EXACT []
is_a: CO_325:1000002 ! Biotic_stress

[Term]
id: CO_325:0000093
name: presence of changes in new leaves caused by fusarium wilt
namespace: BananaTrait
def: "The presence/absence of changes in new leaves - irregular pale margins, narrowing of lamina, burning plus ripping of lamina, lamina becoming more erect, caused by Fusarium wilt." []
synonym: "CNL" EXACT []
is_a: CO_325:1000002 ! Biotic_stress

[Term]
id: CO_325:0000096
name: presence of petiole collapse caused by fusarium wilt
namespace: BananaTrait
def: "The presence/absence of petiole collapse, caused by Fusarium wilt." []
synonym: "PC" EXACT []
is_a: CO_325:1000002 ! Biotic_stress

[Term]
id: CO_325:0000099
name: youngest leaf spotted
namespace: BananaTrait
def: "The rank (order) of the first fully unfurled leaf with at least 10 discrete, mature, necrotic lesions or one large necrotic area with 10 leaf spot light-coloued dry centres, caused by black leaf streak disease." []
synonym: "YLS" EXACT []
is_a: CO_325:1000002 ! Biotic_stress

[Term]
id: CO_325:0000102
name: index of non-spotted leaves
namespace: BananaTrait
def: "An index to express the proportion of standing leaves without the typical late-stage symptoms of black leaf streak disease, i.e. a black spot with a necrotic centre. This index provides an estimation of available photosynthetic leaf area prior to fruit filling and is a measure of resistance. It also corrects for the difference in the number of leaves produced by different types of bananas." []
synonym: "INSL" EXACT []
is_a: CO_325:1000002 ! Biotic_stress

[Term]
id: CO_325:0000105
name: black leaf streak disease severity index
namespace: BananaTrait
def: "An index to express the degree of leaf area of all standing leaves on the plant affected by black leaf streak disease." []
synonym: "Black Sigatoka disease infection index" EXACT []
is_a: CO_325:1000002 ! Biotic_stress

[Term]
id: CO_325:0000108
name: number of dead roots
namespace: BananaTrait
def: "The number of dead roots in a standard-size excavation of 20 x 20 x 20 cm extending outwards from the corm of the plant." []
is_a: CO_325:1000002 ! Biotic_stress

[Term]
id: CO_325:0000111
name: number of functional roots
namespace: BananaTrait
def: "The number of functional roots in a standard-size excavation of 20 x 20 x 20 cm extending outwards from the corm of the plant." []
is_a: CO_325:1000002 ! Biotic_stress

[Term]
id: CO_325:0000123
name: root necrosis caused by nematodes
namespace: BananaTrait
def: "The percentage of the root cortex of five functional roots approximately 10 cm long that is necrotic due to nematode damage." []
is_a: CO_325:1000002 ! Biotic_stress

[Term]
id: CO_325:0000156
name: Days from planting to shooting in days
namespace: BananaTrait
def: "Calculate as: the time elapsed between the Date of planting and the Date of shooting, e.g. 24/09/2014 - 24/01/2014 = 243 days." []
synonym: "PlntShtTime_Comp_d, plant2shoot" EXACT []
is_a: CO_325:1000024 ! Variable
relationship: variable_of CO_325:0000958 ! time from planting to shooting
relationship: variable_of CO_325:0010011 ! time from planting to shooting - computation
relationship: variable_of CO_325:0100003 ! day

[Term]
id: CO_325:0000157
name: Days from shooting to harvest
namespace: BananaTrait
def: "Calculate as: the time elapsed between the Date of shooting to the Date of harvest, e.g. 24/12/2014 - 24/09/2014 = 91 days." []
synonym: "ShtHvstTime_Comp_d, DAYMAT" EXACT []
is_a: CO_325:1000024 ! Variable
relationship: variable_of CO_325:0000003 ! time from shooting to harvest
relationship: variable_of CO_325:0010013 ! time from shooting to harvest - computation
relationship: variable_of CO_325:0100003 ! day

[Term]
id: CO_325:0000158
name: Plant crop cycle in days
namespace: BananaTrait
def: "Calculate as: the time elapsed between the Date of planting to the Date of harvest, e.g. 24/12/2014 - 24/01/2014 = 334 days." []
synonym: "CropCyc_Comp_d, FLWHAV" EXACT []
is_a: CO_325:1000024 ! Variable
relationship: variable_of CO_325:0000006 ! plant crop cycle
relationship: variable_of CO_325:0010012 ! plant crop cycle - computation
relationship: variable_of CO_325:0100003 ! day

[Term]
id: CO_325:0000159
name: Plant height in cm
namespace: BananaTrait
def: "Measure the distance from the collar, or from the pseudostem base at the ground if the collar is not visible, to the intersection of the petioles of the two youngest leaves (leaf ranks 1 and 2), using a measuring pole or sliding ruler. In cm" []
synonym: "PStmHt_M1_cm, PHTSHT, plantheightpetioles" EXACT []
is_a: CO_325:1000024 ! Variable
relationship: variable_of CO_325:0000009 ! plant height
relationship: variable_of CO_325:0010023 ! plant height - petiole of two youngest leaves - measurement
relationship: variable_of CO_325:0100008 ! cm

[Term]
id: CO_325:0000160
name: Plant circumference at 100 cm from the collar
namespace: BananaTrait
def: "Measure the circumference of the pseudostem of the plant at 1 m from the collar, or from the pseudostem base at the ground if the collar is not visible, using a tape measure. In cm" []
synonym: "PStmGrth_M_cm, PGFL, plantcircumf100cm" EXACT []
is_a: CO_325:1000024 ! Variable
relationship: variable_of CO_325:0010248 ! plant circumference at 100 cm - measurement
relationship: variable_of CO_325:0100008 ! cm

[Term]
id: CO_325:0000165
name: Weekly Leaf emission rate in leaves/week
namespace: BananaTrait
def: "Calculate as: the Rank of previously marked leaf at one point in time, minus 1 (equivalent to the Rank of marked youngest leaf), divided by the time elapsed between the two Date of data collection events when the marked leaf was recorded as 1) the Rank of marked youngest leaf and 2) the Rank of previously marked leaf, e.g. (2 - 1) / 1 week = LER of 1 leaves/week during a particular time period." []
synonym: "LfEmRate_Comp_LfWk, LER_week" EXACT []
is_a: CO_325:1000024 ! Variable
relationship: variable_of CO_325:0000726 ! weekly leaf emission rate
relationship: variable_of CO_325:0010021 ! weekly leaf emission rate - computation
relationship: variable_of CO_325:0100006 ! leaves/week

[Term]
id: CO_325:0000166
name: Number of suckers: count
namespace: BananaTrait
def: "Count how many of all types of suckers are in the mat." []
synonym: "SuckNum_Ct_Suck, NUMSUC, numsuckers" EXACT []
is_a: CO_325:1000024 ! Variable
relationship: variable_of CO_325:0000024 ! number of suckers
relationship: variable_of CO_325:0010031 ! number of suckers - counting
relationship: variable_of CO_325:0100013 ! sucker

[Term]
id: CO_325:0000167
name: Tallest sucker height in cm
namespace: BananaTrait
def: "On the tallest sucker, measure the distance from the pseudostem base at the ground to the intersection of the petioles of the two youngest leaves (leaf ranks 1 and 2), using a measuring pole or sliding ruler. In cm" []
synonym: "SuckHtShtStg_M_cm, HTSF, suckerheight" EXACT []
is_a: CO_325:1000024 ! Variable
relationship: variable_of CO_325:0000027 ! tallest sucker height
relationship: variable_of CO_325:0010026 ! tallest sucker height - measurement
relationship: variable_of CO_325:0100008 ! cm

[Term]
id: CO_325:0000169
name: Bunch weight in kg
namespace: BananaTrait
def: "Harvest the bunch by cutting the peduncle 10 cm above the first ridge above the most proximal, hand and immediately below the most distal hand and weigh the bunch (including the rachis), using scales. In kg" []
synonym: "BnchWt_M_kg, BWT, bunchweight" EXACT []
is_a: CO_325:1000024 ! Variable
relationship: variable_of CO_325:0000033 ! bunch weight
relationship: variable_of CO_325:0010033 ! bunch weight - measurement
relationship: variable_of CO_325:0100015 ! kg

[Term]
id: CO_325:0000170
name: Number of hands in bunch: count
namespace: BananaTrait
def: "Count how many hands are in the bunch." []
synonym: "BnchHndNum_Ct_Hnd, numhands" EXACT []
is_a: CO_325:1000024 ! Variable
relationship: variable_of CO_325:0000036 ! number of hands in bunch
relationship: variable_of CO_325:0010038 ! number of hands in bunch - counting
relationship: variable_of CO_325:0100016 ! hand

[Term]
id: CO_325:0000171
name: Number of fingers in bunch: count
namespace: BananaTrait
def: "Count how many fingers are in the bunch." []
synonym: "BnchFrtNum_Ct_Frt, NUMFING, numfingersbunch" EXACT []
is_a: CO_325:1000024 ! Variable
relationship: variable_of CO_325:0000039 ! number of fingers in bunch
relationship: variable_of CO_325:0010039 ! number of fingers in bunch - counting
relationship: variable_of CO_325:0100017 ! finger

[Term]
id: CO_325:0000172
name: Number of fingers in hand: count
namespace: BananaTrait
def: "Count how many fingers are in a hand. Associate the data with the Hand rank. The recommendation is to collect this data from the second and second-most distal hands." []
synonym: "HndFrtNum_Ct_Frt, NUMFIN3, numfingershand" EXACT []
is_a: CO_325:1000024 ! Variable
relationship: variable_of CO_325:0000042 ! number of fingers in hand: count
relationship: variable_of CO_325:0010046 ! number of fingers in third hand - counting
relationship: variable_of CO_325:0100017 ! finger

[Term]
id: CO_325:0000173
name: Hand weight in kg
namespace: BananaTrait
def: "Cut a hand from the rachis and weigh the hand, using scales. Associate the data with the Hand rank. In kg" []
synonym: "HandWt_M_kgPlnt, handweight" EXACT []
is_a: CO_325:1000024 ! Variable
relationship: variable_of CO_325:0000045 ! hand weight
relationship: variable_of CO_325:0010042 ! hand weight - measurement
relationship: variable_of CO_325:0100015 ! kg

[Term]
id: CO_325:0000174
name: Finger weight in g
namespace: BananaTrait
def: "Weigh a finger, using scales. Associate the data with the Hand rank. The recommendation is to collect this data from six fingers in total - three fingers in the middle of the outer whorl from the second hand and from the second-most distal hand. In g" []
synonym: "FrtWt_M_gFruit, fingerweight" EXACT []
is_a: CO_325:1000024 ! Variable
relationship: variable_of CO_325:0000048 ! finger weight
relationship: variable_of CO_325:0010052 ! finger weight - measurement
relationship: variable_of CO_325:0100019 ! g

[Term]
id: CO_325:0000175
name: Finger external length in mm
namespace: BananaTrait
def: "Measure the length of a finger that is at the 'ready to eat' stage, along the external (dorsal) arc, excluding the pedicel and the fruit tip, using a tape measure. Associate the data with the Hand rank and the Number of fingers measured. The recommendation is to collect this data from six fingers in total - three fingers in the middle of the outer whorl from the second hand and from the second-most distal hand. In mm" []
synonym: "FrtExtLng_M_mm, FINCUM, fingerextlength" EXACT []
is_a: CO_325:1000024 ! Variable
relationship: variable_of CO_325:0000051 ! finger external length
relationship: variable_of CO_325:0010056 ! finger external length - measurement
relationship: variable_of CO_325:0100020 ! mm

[Term]
id: CO_325:0000176
name: Finger circumference in cm
namespace: BananaTrait
def: "Measure the circumference of a finger at its widest point, using a tape measure. Associate the data with the Hand rank. The recommendation is to collect this data from six fingers in total - three fingers in the middle of the outer whorl from the second hand and from the second-most distal hand. In cm" []
synonym: "FrtGrth_M_cm, fingercircumf_cm" EXACT []
is_a: CO_325:1000024 ! Variable
relationship: variable_of CO_325:0000054 ! finger circumference
relationship: variable_of CO_325:0010060 ! finger circumference - measurement
relationship: variable_of CO_325:0100008 ! cm

[Term]
id: CO_325:0000177
name: Black Sigatoka incubation time
namespace: BananaTrait
def: "Calculate as: the time elapsed between the Date of tagged leaf presenting black leaf streak disease symptoms at Foure's stage 1 and the Date of tagged cigar leaf unrolling at stage B, e.g. 24/04/2014 - 24/03/2014 = 31 days." []
synonym: "DIT_Comp_d, DIT" EXACT []
is_a: CO_325:1000024 ! Variable
relationship: variable_of CO_325:0000057 ! black leaf streak disease incubation time
relationship: variable_of CO_325:0010122 ! black leaf streak disease incubation time - computation
relationship: variable_of CO_325:0100003 ! day

[Term]
id: CO_325:0000178
name: Black Sigatoka disease evolution time
namespace: BananaTrait
def: "Calculate as: the time elapsed between the Date of tagged leaf presenting black leaf streak disease symptoms at Foure's stage 6 and the Date of tagged leaf presenting black leaf streak disease symptoms at Foure's stage 1, e.g. 24/06/2014 - 24/04/2014 = 61 days." []
synonym: "DET_Comp_d, DET" EXACT []
is_a: CO_325:1000024 ! Variable
relationship: variable_of CO_325:0000060 ! black leaf streak disease evolution time
relationship: variable_of CO_325:0010123 ! black leaf streak disease evolution time - computation
relationship: variable_of CO_325:0100003 ! day

[Term]
id: CO_325:0000181
name: Number of standing leaves: count
namespace: BananaTrait
def: "Count how many of the leaves are standing leaves (without a bent or broken petiole)" []
synonym: "StdLf_Ct_leaf, NSLF" EXACT []
is_a: CO_325:1000024 ! Variable
relationship: variable_of CO_325:0000069 ! number of standing leaves
relationship: variable_of CO_325:0010106 ! number of standing leaves - counting
relationship: variable_of CO_325:0100007 ! leaf

[Term]
id: CO_325:0000182
name: Extent of internal discolouration in corm of tallest sucker caused by Fusarium wilt in cm
namespace: BananaTrait
def: "The extent to which vascular discolouration extends up the pseudostem of the tallest sucker should be determined by making cross-section cuts, from the base of the pseudostem upwards, and examining the internal tissues following each cut. The point at which discolouration is no longer visible should be noted and the distance from this point to the pseudostem base recorded. In cm" []
synonym: "CormDiscol_Est_1to6," EXACT []
is_a: CO_325:1000024 ! Variable
relationship: variable_of CO_325:0000072 ! extent of internal discolouration in corm of tallest sucker caused by fusarium wilt
relationship: variable_of CO_325:0010126 ! extent of internal discolouration in corm of tallest sucker caused by fusarium wilt - estimation
relationship: variable_of CO_325:0100008 ! cm

[Term]
id: CO_325:0000183
name: Fusarium wilt internal discolouration of pseudostem 1-6
namespace: BananaTrait
def: "For the plant, the complete corm should be removed from the soil, the roots cut off and excess soil removed. Cross-sections of the corm should be cut (using a guillotine or other suitable device) to obtain five slices of equal thickness. The upper surface of each cut section should be examined and visually evaluate the extent of the vascular discolouration., 1 = corm completely clean, no vascular discolouration; 2 = isolated points of discolouration in vascular tissue; 3 = discolouration of up to one-third of vascular tissue; 4 = discolouration of between one-third and two-thirds of vascular tissue; 5 = discolouration greater than two-thirds of vascular tissue; 6 = total discolouration of vascular tissue" []
synonym: "PStmDiscol_Est_cm," EXACT []
is_a: CO_325:1000024 ! Variable
relationship: variable_of CO_325:0000075 ! distance of internal discolouration in pseudostem of plant caused by fusarium wilt
relationship: variable_of CO_325:0010125 ! distance of internal discolouration in pseudostem of plant caused by fusarium wilt
relationship: variable_of CO_325:0100052 ! 5 pt corm discolouration scale

[Term]
id: CO_325:0000184
name: Percentage of plants with external disease symptoms caused by Fusarium wilt: calculation
namespace: BananaTrait
def: "Calculate as: the sum of the number of plants with any or multiple of the external disease symptoms caused by Fusarium wilt - yellowing leaves, splitting of pseudostem base, changes in new leaves, petiole collapse - divided by the Number of plants planted * 100, e.g. 112 / 300 * 100 = 37%. In %" []
synonym: "ExtDisProp_Comp_pct," EXACT []
is_a: CO_325:1000024 ! Variable
relationship: variable_of CO_325:0000078 ! percentage of plants with external disease symptoms caused by fusarium wilt
relationship: variable_of CO_325:0010138 ! percentage of plants with external disease symptoms caused by fusarium wilt - computation
relationship: variable_of CO_325:0100046 ! %

[Term]
id: CO_325:0000185
name: Percentage of plants with internal disease symptoms caused by Fusarium wilt: calculation
namespace: BananaTrait
def: "Calculate as: the sum of the number of plants with any or multiple of the internal disease symptoms caused by Fusarium wilt - discolouration in the corm, and/or discolouration in the pseudostem - divided by the Number of plants planted * 100, e.g. 108 / 300 * 100 = 36%. In %" []
synonym: "IntDisProp_Comp_pct," EXACT []
is_a: CO_325:1000024 ! Variable
relationship: variable_of CO_325:0000081 ! percentage of plants with internal disease symptoms caused by fusarium wilt
relationship: variable_of CO_325:0010139 ! percentage of plants with internal disease symptoms caused by fusarium wilt - computation
relationship: variable_of CO_325:0100046 ! %

[Term]
id: CO_325:0000186
name: Days from crop cycle start to first external Fusarium wilt symptoms
namespace: BananaTrait
def: "Calculate as: the time elapsed between the Date of planting or the Date of harvest of the bunch from the plant of the previous crop cycle and the Date of first external disease symptoms caused by Fusarium wilt. In day" []
synonym: "PlntgDisTim_Comp_d," EXACT []
is_a: CO_325:1000024 ! Variable
relationship: variable_of CO_325:0000084 ! time from start of crop cycle to first external disease symptoms caused by fusarium wilt
relationship: variable_of CO_325:0010133 ! time from start of crop cycle to first external disease symptoms caused by fusarium wilt - computation
relationship: variable_of CO_325:0100003 ! day

[Term]
id: CO_325:0000187
name: Presence of yellowing leaves caused by Fusarium wilt 1-2
namespace: BananaTrait
def: "Visual assessment., 1 = absent; 2 = present" []
synonym: "YellowPres_Est_1or2, YL_1-2" EXACT []
is_a: CO_325:1000024 ! Variable
relationship: variable_of CO_325:0000087 ! presence of yellowing leaves caused by fusarium wilt
relationship: variable_of CO_325:0010128 ! presence of yellowing leaves caused by fusarium wilt - estimation
relationship: variable_of CO_325:0100054 ! presence absence 1

[Term]
id: CO_325:0000188
name: Presence of splitting pseudostem base caused by Fusarium wilt 1-2
namespace: BananaTrait
def: "Visual assessment., 1 = absent; 2 = present" []
synonym: "PStmSplitPres_Est_1or2, SP_1-2" EXACT []
is_a: CO_325:1000024 ! Variable
relationship: variable_of CO_325:0000090 ! presence of splitting pseudostem base caused by fusarium wilt
relationship: variable_of CO_325:0010129 ! presence of splitting pseudostem base caused by fusarium wilt - estimation
relationship: variable_of CO_325:0100054 ! presence absence 1

[Term]
id: CO_325:0000189
name: Presence of changes in new leaves caused by Fusarium wilt 1-2
namespace: BananaTrait
def: "Visual assessment., 1 = absent; 2 = present" []
synonym: "LfChgPres_Est_1or2, CNL_1-2" EXACT []
is_a: CO_325:1000024 ! Variable
relationship: variable_of CO_325:0000093 ! presence of changes in new leaves caused by fusarium wilt
relationship: variable_of CO_325:0010130 ! presence of changes in new leaves caused by fusarium wilt - estimation
relationship: variable_of CO_325:0100054 ! presence absence 1

[Term]
id: CO_325:0000190
name: Presence of petiole collapse caused by Fusarium wilt 1-2
namespace: BananaTrait
def: "Visual assessment., 1 = absent; 2 = present" []
synonym: "PetColpPres_Est_1or2, PC_1-2" EXACT []
is_a: CO_325:1000024 ! Variable
relationship: variable_of CO_325:0000096 ! presence of petiole collapse caused by fusarium wilt
relationship: variable_of CO_325:0010131 ! presence of petiole collapse caused by fusarium wilt - estimation
relationship: variable_of CO_325:0100054 ! presence absence 1

[Term]
id: CO_325:0000191
name: Youngest leaf spotted rank
namespace: BananaTrait
def: "Record the rank (order) of the youngest leaf spotted (the first fully unfurled leaf (or 50 pc unfurled for pathology trials) with at least 10 discrete, mature, necrotic lesions or one large necrotic area with 10 light-coloured dry centres), counting the rank by starting with the youngest completely unrolled leaf as 1 and moving downwards, associating the data with the Date of data collection." []
synonym: "SpotLfNum_Ct_Lf, YLSF" EXACT []
is_a: CO_325:1000024 ! Variable
relationship: variable_of CO_325:0000099 ! youngest leaf spotted
relationship: variable_of CO_325:0010102 ! youngest leaf spotted - counting
relationship: variable_of CO_325:0100004 ! leaf rank

[Term]
id: CO_325:0000192
name: Index of non-spotted leaves: calculation
namespace: BananaTrait
def: "Calculate as: 100 multiplied by (Youngest leaf spotted, minus 1), divided by Number of standing leaves, e.g. 100 * (6 - 1) / 12 = 42." []
synonym: "NSpotLfProp_Comp_idx, INSL" EXACT []
is_a: CO_325:1000024 ! Variable
relationship: variable_of CO_325:0000102 ! index of non-spotted leaves
relationship: variable_of CO_325:0010109 ! index of non-spotted leaves - computation
relationship: variable_of CO_325:0100045 ! index of non-spotted leaves

[Term]
id: CO_325:0000193
name: Black Sigatoka disease infection index
namespace: BananaTrait
def: "Calculate as: ((((Number of leaves with black leaf streak disease severity grade 0, multiplied by 0), plus (Number of leaves with black leaf streak disease severity grade 1, multiplied by 1), plus (Number of leaves with black leaf streak disease severity grade 2, multiplied by 2), plus (Number of leaves with black leaf streak disease severity grade 3, multiplied by 3), plus (Number of leaves with black leaf streak disease severity grade 4, multiplied by 4), plus (Number of leaves with black leaf streak disease severity grade 5, multiplied by 5), plus (Number of leaves with black leaf streak disease severity grade 6, multiplied by 6)), divided by the number of grades in the scale minus 1 (i.e. 7-1)), divided by the Number of standing leaves), multiplied by 100. For example, ((((3 * 0) + (1 * 1) + (1 * 2) + (3 * 3) + (5 * 4) + (0 * 5) + (0 * 6)) / 6) / 13) * 100 = ((32 / 6) / 13) * 100 = 41." []
synonym: "BlkLfStrkInfIndex_Comp_Idx," EXACT []
is_a: CO_325:1000024 ! Variable
relationship: variable_of CO_325:0000105 ! black leaf streak disease severity index
relationship: variable_of CO_325:0010118 ! black leaf streak disease severity index - computation
relationship: variable_of CO_325:0100051 ! index of black leaf streak disease severity

[Term]
id: CO_325:0000194
name: Number of dead roots: count
namespace: BananaTrait
def: "Collect all roots from a standard-size excavation of 20 x 20 x 20 cm extending outwards from the corm of the plant. Take only roots from the selected plant. Divide the collected roots into two categories: dead roots, functional roots. Dead roots are completely rotten or shrivelled whereas functional roots show at least some healthy tissue. Count the number of dead roots." []
synonym: "DeadRtNum2_Ct_Rt," EXACT []
is_a: CO_325:1000024 ! Variable
relationship: variable_of CO_325:0000108 ! number of dead roots
relationship: variable_of CO_325:0010156 ! number of dead roots - counting
relationship: variable_of CO_325:0100059 ! dead roots

[Term]
id: CO_325:0000195
name: Number of functional roots: count
namespace: BananaTrait
def: "Collect all roots from a standard-size excavation of 20 x 20 x 20 cm extending outwards from the corm of the plant. Take only roots from the selected plant. Divide the collected roots into two categories: dead roots, functional roots. Dead roots are completely rotten or shrivelled whereas functional roots show at least some healthy tissue. Count the number of functional roots." []
synonym: "FuncRtNum2_Ct_Rt," EXACT []
is_a: CO_325:1000024 ! Variable
relationship: variable_of CO_325:0000111 ! number of functional roots
relationship: variable_of CO_325:0010157 ! number of functional roots - counting
relationship: variable_of CO_325:0100060 ! functional roots

[Term]
id: CO_325:0000199
name: Root necrosis caused by nematodes in percent
namespace: BananaTrait
def: "Select at random five functional primary roots, at least 10 cm long. Reduce the length of the five selected roots to 10 cm and slice through the roots length-wise. Evaluate one half of each of the five roots for the percentage of root cortex showing necrosis. The maximum root necrosis per root half can be 20%, giving a maximum root necrosis of 100% for the five halves together. Mentally determine the necrosis of the individual roots (1 to 5) and sum these together to get the total root necrosis of the sample. In %" []
synonym: "rtNcr_M_%, RTNCRS" EXACT []
is_a: CO_325:1000024 ! Variable
relationship: variable_of CO_325:0000123 ! root necrosis caused by nematodes
relationship: variable_of CO_325:0010219 ! root necrosis caused by nematodes - estimation
relationship: variable_of CO_325:0100046 ! %

[Term]
id: CO_325:0000202
name: Number of Radopholus similis per soil sample per 100 ml: count
namespace: BananaTrait
def: "Count from 100 ml of soil sample" []
synonym: "RadoNumSlWt_Comp_Nema" EXACT []
is_a: CO_325:1000024 ! Variable
relationship: variable_of CO_325:0000522 ! number of radopholus similis per soil sample
relationship: variable_of CO_325:0010222 ! number of nematodes (radopholus similis ) per unit of soil sample - method
relationship: variable_of CO_325:0100109 ! no. per 100 ml

[Term]
id: CO_325:0000203
name: Number of Helicotylenchus multicinctus per soil sample per 100 ml: count
namespace: BananaTrait
def: "Count from 100 ml of soil sample" []
synonym: "HelicoNumSlWt_Comp_Nema" EXACT []
is_a: CO_325:1000024 ! Variable
relationship: variable_of CO_325:0000523 ! number of helicotylenchus multicinctus per soil sample
relationship: variable_of CO_325:0010223 ! number of nematodes (helicotylenchus multicinctus) per unit of soil sample - method
relationship: variable_of CO_325:0100109 ! no. per 100 ml

[Term]
id: CO_325:0000204
name: Number of Meloidogyne spp. per soil sample per 100 ml: count
namespace: BananaTrait
def: "Count from 100 ml of soil sample" []
synonym: "MeloiNumSlWt_Comp_Nema" EXACT []
is_a: CO_325:1000024 ! Variable
relationship: variable_of CO_325:0000526 ! number of meloidogyne spp. per soil sample
relationship: variable_of CO_325:0010225 ! number of nematodes (meloidogyne spp.) per unit of soil sample - method
relationship: variable_of CO_325:0100109 ! no. per 100 ml

[Term]
id: CO_325:0000205
name: Number of Pratylenchus spp. per soil sample per 100 ml: count
namespace: BananaTrait
def: "Count from 100 ml of soil sample" []
synonym: "PratyNumSlWt_Comp_Nema" EXACT []
is_a: CO_325:1000024 ! Variable
relationship: variable_of CO_325:0000527 ! number of pratylenchus spp. per soil sample
relationship: variable_of CO_325:0010226 ! number of nematodes (pratylenchus spp.) per unit of soil sample - method
relationship: variable_of CO_325:0100109 ! no. per 100 ml

[Term]
id: CO_325:0000206
name: Number of Hoplolaimus spp. per soil sample per 100 ml: count
namespace: BananaTrait
def: "Count from 100 ml of soil sample" []
synonym: "HoploNumSlWt_Comp_Nema" EXACT []
is_a: CO_325:1000024 ! Variable
relationship: variable_of CO_325:0000528 ! number of hoplolaimus spp. per soil sample
relationship: variable_of CO_325:0010227 ! number of nematodes (hoplolaimus spp.) per unit of soil sample - method
relationship: variable_of CO_325:0100109 ! no. per 100 ml

[Term]
id: CO_325:0000207
name: Number of Pratylenchus goodeyi per soil sample per 100 ml: count
namespace: BananaTrait
def: "Count from 100 ml of soil sample" []
synonym: "PratyGooNumSlWt_Comp_Nema" EXACT []
is_a: CO_325:1000024 ! Variable
relationship: variable_of CO_325:0000529 ! number of pratylenchus goodeyi per soil sample
relationship: variable_of CO_325:0010228 ! number of nematodes (pratylenchus goodeyi) per unit of soil sample - method
relationship: variable_of CO_325:0100109 ! no. per 100 ml

[Term]
id: CO_325:0000208
name: Number of Pratylenchus coffeae per soil sample per 100 ml: count
namespace: BananaTrait
def: "Count from 100 ml of soil sample" []
synonym: "PratyCofNumSlWt_Comp_Nema" EXACT []
is_a: CO_325:1000024 ! Variable
relationship: variable_of CO_325:0000530 ! number of pratylenchus coffeae per soil sample
relationship: variable_of CO_325:0010229 ! number of nematodes (pratylenchus coffeae) per unit of soil sample - method
relationship: variable_of CO_325:0100109 ! no. per 100 ml

[Term]
id: CO_325:0000220
name: Number of maiden suckers: count
namespace: BananaTrait
def: "Count how many maiden suckers are in the mat." []
synonym: "MSuckN_Ct_MSuck, MAIDSUC, nummaidensuckers" EXACT []
is_a: CO_325:1000024 ! Variable
relationship: variable_of CO_325:0000221 ! number of maiden suckers
relationship: variable_of CO_325:0010027 ! number of maiden suckers - counting
relationship: variable_of CO_325:0100009 ! maiden sucker

[Term]
id: CO_325:0000221
name: number of maiden suckers
namespace: BananaTrait
def: "The number of maiden suckers (fully grown suckers with foliage leaves) in the mat." []
synonym: "nummaidensuckers" EXACT []
is_a: CO_325:1000001 ! Agronomical

[Term]
id: CO_325:0000224
name: Number of sword suckers: count
namespace: BananaTrait
def: "Count how many sword suckers are in the mat." []
synonym: "SSuckN_Ct_SSuck, SWDSUC, numswordsuckers" EXACT []
is_a: CO_325:1000024 ! Variable
relationship: variable_of CO_325:0000225 ! Number of sword suckers
relationship: variable_of CO_325:0010028 ! number of sword suckers - counting
relationship: variable_of CO_325:0100010 ! sword sucker

[Term]
id: CO_325:0000225
name: Number of sword suckers
namespace: BananaTrait
def: "The number of sword suckers (suckers with narrow leaves and a large rhizome) in the mat." []
synonym: "numswordsuckers" EXACT []
is_a: CO_325:1000001 ! Agronomical

[Term]
id: CO_325:0000228
name: Number of peeper suckers: count
namespace: BananaTrait
def: "Count how many peeper suckers are in the mat." []
synonym: "PSuckN_Ct_PSuck, PEPSUC, numpeepersuckers" EXACT []
is_a: CO_325:1000024 ! Variable
relationship: variable_of CO_325:0000229 ! number of peeper suckers
relationship: variable_of CO_325:0010029 ! number of peeper suckers - counting
relationship: variable_of CO_325:0100011 ! peeper sucker

[Term]
id: CO_325:0000229
name: number of peeper suckers
namespace: BananaTrait
def: "The number of peeper suckers (suckers < 15 cm tall) in the mat." []
synonym: "numpeepersuckers" EXACT []
is_a: CO_325:1000001 ! Agronomical

[Term]
id: CO_325:0000232
name: Finger lateral diameter in cm
namespace: BananaTrait
def: "Measure the lateral diameter of a finger from the left to the right side (not from the ventral to the dorsal side), at the widest point, using calipers. Associate the data with the Hand rank. The recommendation is to collect this data from six fingers in total - three fingers in the middle of the outer whorl from the second hand and from the second-most distal hand. In cm" []
synonym: "FrtDiam_M_cm, FLDIA, fingerlatdiam" EXACT []
is_a: CO_325:1000024 ! Variable
relationship: variable_of CO_325:0000233 ! finger lateral diameter
relationship: variable_of CO_325:0010062 ! finger lateral diameter - measurement
relationship: variable_of CO_325:0100008 ! cm

[Term]
id: CO_325:0000233
name: finger lateral diameter
namespace: BananaTrait
def: "The lateral (side to side) diameter of a finger." []
synonym: "Finger grade, Fruit diameter, Fruit grade" EXACT []
synonym: "fingerlatdiam" EXACT []
is_a: CO_325:1000001 ! Agronomical

[Term]
id: CO_325:0000235
name: Finger peel thickness in mm
namespace: BananaTrait
def: "Cut a finger in half, crosswise at its widest point, and on the cross-section measure the width of the peel, using calipers. Associate the data with the Hand rank. The recommendation is to collect this data from six fingers in total - three fingers in the middle of the outer whorl from the second hand and from the second-most distal hand. In mm" []
synonym: "PeelThck_M_mm, FPEELT, peelthickness" EXACT []
is_a: CO_325:1000024 ! Variable
relationship: variable_of CO_325:0000236 ! finger peel thickness
relationship: variable_of CO_325:0010066 ! finger peel thickness - measurement
relationship: variable_of CO_325:0100020 ! mm

[Term]
id: CO_325:0000236
name: finger peel thickness
namespace: BananaTrait
def: "The thickness of the peel of a finger." []
synonym: "peelthickness" EXACT []
synonym: "Width of the peel, Width of the skin, Width of the exocarp, Finger peel thickness" EXACT []
is_a: CO_325:1000001 ! Agronomical

[Term]
id: CO_325:0000239
name: Fruit pulp lateral diameter in cm
namespace: BananaTrait
def: "Cut a finger in half, crosswise at its widest point, and on the cross-section measure the lateral diameter of the fruit pulp, from the left to the right side (not from the ventral to the dorsal side), using calipers. Associate the data with the Hand rank. The recommendation is to collect this data from six fingers in total - three fingers in the middle of the outer whorl from the second hand and from the second-most distal hand. In cm" []
synonym: "PulpDiam_M_cm, FPULPD" EXACT []
is_a: CO_325:1000024 ! Variable
relationship: variable_of CO_325:0000240 ! fruit pulp lateral diameter
relationship: variable_of CO_325:0010064 ! fruit pulp lateral diameter - measurement
relationship: variable_of CO_325:0100008 ! cm

[Term]
id: CO_325:0000240
name: fruit pulp lateral diameter
namespace: BananaTrait
def: "The lateral (side to side) diameter of the pulp of a fruit." []
synonym: "Finger pulp diameter" EXACT []
synonym: "pulpdiam" EXACT []
is_a: CO_325:1000001 ! Agronomical

[Term]
id: CO_325:0000242
name: Pseudostem main color 1-16
namespace: BananaTrait
def: "Detach the outermost sheath from the pseudostem (the sheath should not be too dry). Record the overall impression of colour of the exposed surface of the underlying pseudostem. Note that this 'main colour' should cover more than 75% of the underlying pseudostem surface. Use colour chart A and observe out of direct sunlight., 1 = cream; 2 = yellow; 3 = watery green; 4 = green yellow; 5 = light green; 6 = medium green; 7 = green; 8 = dark green; 9 = whitish; 10 = orange red; 11 = red; 12 = pink-purple; 13 = purple-brown; 14 = red-purple; 15 = purple; 16 = blue" []
synonym: "PStmCol_Est_1to16, COLSTE" EXACT []
is_a: CO_325:1000024 ! Variable
relationship: variable_of CO_325:0000243 ! main underlying colour of pseudostem
relationship: variable_of CO_325:0010160 ! pseudostem colour - estimation
relationship: variable_of CO_325:0100063 ! bd colour chart a - 2016

[Term]
id: CO_325:0000243
name: main underlying colour of pseudostem
namespace: BananaTrait
def: "Main colour of the pseudostem under the outermost sheath." []
synonym: "Predominant underlying colour of the pseudostem" EXACT []
is_a: CO_325:1000003 ! Morphological

[Term]
id: CO_325:0000247
name: Edge of petiole margin color 1-2
namespace: BananaTrait
def: "Observations on the margins and petiole wings should be made where the petiole and pseudostem meet at shooting. Record on the last developed leaf at [x flowering stage] [shooting]., 1 = no contrast between margin and petiole (without a colour line along); 2 = contrast between margin and petiole (with a contrasting colour line along)" []
synonym: "PMargColL_Est_1or2, PETMG" EXACT []
is_a: CO_325:1000024 ! Variable
relationship: variable_of CO_325:0000248 ! colour line along edge of petiole margin
relationship: variable_of CO_325:0010167 ! colour line along edge of petiole margin - estimation
relationship: variable_of CO_325:0100074 ! petiole-margin contrast

[Term]
id: CO_325:0000248
name: colour line along edge of petiole margin
namespace: BananaTrait
def: "Presence or absence of colour line along edge of petiole margin" []
synonym: "Edge of petiole margin" EXACT []
is_a: CO_325:1000003 ! Morphological

[Term]
id: CO_325:0000251
name: Pigmentation of outer surface of cigar leaf on sucker 1-3
namespace: BananaTrait
def: "Visually observe the pigmentation of the outer surface of the cigar leaf of a developed sucker or on another plant of the same accession. [x Observation should be made before shooting, on a developed sucker or on another plant of the same accession.], 1 = green; 2 = red-purple; 3 = other (specify on answer sheet)" []
synonym: "CigLfPigm_Est_1to3, CGLFCO" EXACT []
is_a: CO_325:1000024 ! Variable
relationship: variable_of CO_325:0000252 ! pigmentation of outer surface of cigar leaf on sucker
relationship: variable_of CO_325:0010168 ! pigmentation of outer surface of cigar leaf - estimation
relationship: variable_of CO_325:0100063 ! bd colour chart a - 2016

[Term]
id: CO_325:0000252
name: pigmentation of outer surface of cigar leaf on sucker
namespace: BananaTrait
def: "Colour of pigmentation on outer surface of cigar leaf on a developed sucker" []
synonym: "Colour of cigar leaf dorsal surface" EXACT []
is_a: CO_325:1000003 ! Morphological

[Term]
id: CO_325:0000255
name: Petiole margins winged 1-2
namespace: BananaTrait
def: "Observations on the margins and petiole wings should be made where the petiole and pseudostem meet at shooting. Margin is the part of the petiole that can be bent outwards/inwards. [x Observe at flowering time.], 1 = winged; 2 = not winged" []
synonym: "PMargWing_Est_1or2," EXACT []
is_a: CO_325:1000024 ! Variable
relationship: variable_of CO_325:0000256 ! petiole margins winged
relationship: variable_of CO_325:0010164 ! winged petiole margin - estimation
relationship: variable_of CO_325:0100070 ! wing presence/absence

[Term]
id: CO_325:0000256
name: petiole margins winged
namespace: BananaTrait
def: "Behaviour of the petiole margins - winged or not winged. The petiole and pseudostem meet at shooting. Margin is the part of the petiole that can be bent outwards/inwards." []
synonym: "Petiole margins" EXACT []
is_a: CO_325:1000003 ! Morphological

[Term]
id: CO_325:0000259
name: Petiole margins clasping 1-2
namespace: BananaTrait
def: "Observations on the margins and petiole wings should be made where the petiole and pseudostem meet at shooting. Observation should be made at shooting on the neck, where the petiole and pseudostem meet. Margin is the part of the petiole that can be bent outwards/inwards. [x Observe at flowering time.], 1 = clasping; 2 = not clasping" []
synonym: "PMargClasp_Est_1or2," EXACT []
is_a: CO_325:1000024 ! Variable
relationship: variable_of CO_325:0000260 ! petiole margins clasping
relationship: variable_of CO_325:0010165 ! petiole margin clasping - estimation
relationship: variable_of CO_325:0100072 ! clasping or not clasping

[Term]
id: CO_325:0000260
name: petiole margins clasping
namespace: BananaTrait
def: "Behaviour of the petiole margins - winged or not winged. the petiole and pseudostem meet at shooting. Margin is the part of the petiole that can be bent outwards/inwards" []
synonym: "Petiole margins" EXACT []
is_a: CO_325:1000003 ! Morphological

[Term]
id: CO_325:0000263
name: Petiole margin colour 1-16
namespace: BananaTrait
def: "Observations on the margins and petiole wings should be made where the petiole and pseudostem meet at shooting. Use colour chart A and observe out of direct sunlight. Record the colour of the margin (general colour is below the rim). [x Observe at flowering time.], 1 = cream; 2 = yellow; 3 = watery green; 4 = green yellow; 5 = light green; 6 = medium green; 7 = green; 8 = dark green; 9 = whitish; 10 = orange red; 11 = red; 12 = pink-purple; 13 = purple-brown; 14 = red-purple; 15 = purple; 16 = blue" []
synonym: "PMargCol_Esr_1to16, PETMCO_1-16" EXACT []
is_a: CO_325:1000024 ! Variable
relationship: variable_of CO_325:0000264 ! petiole margin colour
relationship: variable_of CO_325:0010166 ! petiole margin colour - estimation
relationship: variable_of CO_325:0100063 ! bd colour chart a - 2016

[Term]
id: CO_325:0000264
name: petiole margin colour
namespace: BananaTrait
def: "Main colour of the petiole margin. Where the petiole and pseudostem meet at shooting. Margin is the part of the petiole that can be bent outwards/inwards" []
is_a: CO_325:1000003 ! Morphological

[Term]
id: CO_325:0000292
name: time from flowering to harvest
namespace: BananaTrait
def: "The time elapsed from flowering (when the last bracts fall from the most distal hand to display the female flowers) to the harvest of the bunch." []
synonym: "flower2harvest" EXACT []
is_a: CO_325:1000004 ! Phenological

[Term]
id: CO_325:0000293
name: Days from flowering to harvest
namespace: BananaTrait
def: "Calculate as: the time elapsed between the Date of flowering to the Date of harvest, e.g. 24/12/2014 - 24/10/2014 = 61 days. In day format" []
synonym: "FlwHvstTime_Comp_d, flower2harvest" EXACT []
is_a: CO_325:1000024 ! Variable
relationship: variable_of CO_325:0000292 ! time from flowering to harvest
relationship: variable_of CO_325:0010014 ! time from flowering to harvest - computation
relationship: variable_of CO_325:0100003 ! day

[Term]
id: CO_325:0000294
name: time from planting to death
namespace: BananaTrait
def: "The time elapsed from planting to the death of the plant." []
synonym: "plant2death" EXACT []
synonym: "Time to death" EXACT []
is_a: CO_325:1000001 ! Agronomical

[Term]
id: CO_325:0000295
name: Time from planting to death in days
namespace: BananaTrait
def: "Calculate as: the time elapsed between the Date of planting and the Date of death, e.g. 24/05/2014 - 24/01/2014 = 120 days." []
synonym: "PltDth_Comp_d, plant2death" EXACT []
is_a: CO_325:1000024 ! Variable
relationship: variable_of CO_325:0000294 ! time from planting to death
relationship: variable_of CO_325:0010015 ! time from planting to death - computation
relationship: variable_of CO_325:0100003 ! day

[Term]
id: CO_325:0000296
name: time from harvest to death
namespace: BananaTrait
def: "The time elapsed from the harvest of the bunch of the plant from the preceding crop cycle to the death of the plant from the current crop cycle." []
synonym: "harvest2death" EXACT []
synonym: "Time to death of the ratoon plant" EXACT []
is_a: CO_325:1000001 ! Agronomical

[Term]
id: CO_325:0000297
name: Time from harvest to death in days
namespace: BananaTrait
def: "Calculate as: the time elapsed between the Date of harvest of the bunch of the plant from the preceeding crop cycle and the Date of death of the current plant, e.g. 24/03/2015 - 24/12/2014 = 90 days." []
synonym: "HvstDth_Comp_d, harvest2death" EXACT []
is_a: CO_325:1000024 ! Variable
relationship: variable_of CO_325:0000296 ! time from harvest to death
relationship: variable_of CO_325:0010016 ! time from harvest to death - computation
relationship: variable_of CO_325:0100003 ! day

[Term]
id: CO_325:0000298
name: ratoon crop cycle
namespace: BananaTrait
def: "The time elapsed from the harvest of the bunch of the plant from the preceding crop cycle to the harvest of the bunch of the plant from the current crop cycle." []
synonym: "harvest2harvest" EXACT []
synonym: "Time from harvest to harvest" EXACT []
is_a: CO_325:1000004 ! Phenological

[Term]
id: CO_325:0000299
name: Ratoon crop cycle in days
namespace: BananaTrait
def: "Calculate as: the time elapsed between the Date of harvest of the bunch of the plant from the preceeding crop cycle and the Date of harvest of the bunch of the plant from the current crop cycle, e.g. 24/11/2015 - 24/12/2014 = 335 days." []
synonym: "RtnCrpCyc_Comp_d, harvest2harvest" EXACT []
is_a: CO_325:1000024 ! Variable
relationship: variable_of CO_325:0000298 ! ratoon crop cycle
relationship: variable_of CO_325:0010017 ! ratoon crop cycle - computation
relationship: variable_of CO_325:0100003 ! day

[Term]
id: CO_325:0000307
name: plant height to neck of peduncle
namespace: BananaTrait
def: "The height of the pseudostem of the plant from the collar to the curved neck of the peduncle." []
synonym: "plantheightneck" EXACT []
synonym: "Pseudostem height" EXACT []
is_a: CO_325:1000001 ! Agronomical

[Term]
id: CO_325:0000308
name: Plant height to peduncle neck
namespace: BananaTrait
def: "Measure the distance from the collar, or from the pseudostem base at the ground if the collar is not visible, to under the 'neck' of the curved peduncle, using a measuring pole or sliding ruler. In cm" []
synonym: "PStmHt_M2_cm, plantheightneck" EXACT []
is_a: CO_325:1000024 ! Variable
relationship: variable_of CO_325:0000307 ! plant height to neck of peduncle
relationship: variable_of CO_325:0010024 ! plant height - neck of peduncle - measurement
relationship: variable_of CO_325:0100008 ! cm

[Term]
id: CO_325:0000310
name: number of water suckers
namespace: BananaTrait
def: "The number of water suckers (suckers with broad leaves, a small rhizome, and a weak connection to the plant) in the mat." []
synonym: "numwatersuckers" EXACT []
is_a: CO_325:1000001 ! Agronomical

[Term]
id: CO_325:0000311
name: Number of water suckers
namespace: BananaTrait
def: "Count how many water suckers are in the mat." []
synonym: "WSuckN_Ct_WSuck, numwatersuckers" EXACT []
is_a: CO_325:1000024 ! Variable
relationship: variable_of CO_325:0000310 ! number of water suckers
relationship: variable_of CO_325:0010030 ! number of water suckers - counting
relationship: variable_of CO_325:0100012 ! water suckers

[Term]
id: CO_325:0000312
name: bunch maturity stage at harvest
namespace: BananaTrait
def: "The stage of maturity of the bunch at harvest." []
synonym: "bunchmaturity" EXACT []
synonym: "Stage of harvesting" EXACT []
is_a: CO_325:1000001 ! Agronomical

[Term]
id: CO_325:0000313
name: Bunch maturity stage
namespace: BananaTrait
def: "Estimate maturity stage of the bunch., 1 = fully green; 2 = one yellow finger;" []
synonym: "BnchMatStg_Est_1to2, bunchmaturity" EXACT []
is_a: CO_325:1000024 ! Variable
relationship: variable_of CO_325:0000312 ! bunch maturity stage at harvest
relationship: variable_of CO_325:0010032 ! bunch maturity stage - estimation
relationship: variable_of CO_325:0100014 ! bunch maturity

[Term]
id: CO_325:0000314
name: rachis weight
namespace: BananaTrait
def: "The weight of the rachis." []
synonym: "rachisweight" EXACT []
is_a: CO_325:1000001 ! Agronomical

[Term]
id: CO_325:0000315
name: Rachis weight
namespace: BananaTrait
def: "Cut the hands off the rachis and weigh the rachis, using scales. In kg" []
synonym: "RchsWt_M_kg, rachisweight" EXACT []
is_a: CO_325:1000024 ! Variable
relationship: variable_of CO_325:0000314 ! rachis weight
relationship: variable_of CO_325:0010036 ! rachis weight - measurement
relationship: variable_of CO_325:0100015 ! kg

[Term]
id: CO_325:0000316
name: total finger weight
namespace: BananaTrait
def: "The weight of all the hands of the bunch, excluding the rachis." []
synonym: "Total fruit weight, Total hand weight" EXACT []
synonym: "totalfingerweight" EXACT []
is_a: CO_325:1000001 ! Agronomical

[Term]
id: CO_325:0000317
name: Total finger weight
namespace: BananaTrait
def: "Calculate as: the Bunch weight, minus the Rachis weight, e.g. 50 - 10 = 40. In kg" []
synonym: "FngWtTtl_Comp_kg, totalfingerweight" EXACT []
is_a: CO_325:1000024 ! Variable
relationship: variable_of CO_325:0000316 ! total finger weight
relationship: variable_of CO_325:0010037 ! total finger weight - computation
relationship: variable_of CO_325:0100015 ! kg

[Term]
id: CO_325:0000318
name: hand rank
namespace: BananaTrait
def: "The rank (order) of a hand in the bunch." []
synonym: "handid" EXACT []
is_a: CO_325:1000001 ! Agronomical

[Term]
id: CO_325:0000319
name: Hand rank 1 to 3
namespace: BananaTrait
def: "Record the rank (order) of a hand in the bunch, starting with the hand at the proximal end (closest to the pseudostem) of the bunch as 1 and continuing to the hand at the most distal end (closest to the male bud)." []
synonym: "HndRnk_Ct_HndRnk, handid" EXACT []
is_a: CO_325:1000024 ! Variable
relationship: variable_of CO_325:0000318 ! hand rank
relationship: variable_of CO_325:0010041 ! hand rank - counting
relationship: variable_of CO_325:0100018 ! hand rank

[Term]
id: CO_325:0000320
name: multiple number of fingers in hand
namespace: BananaTrait
def: "The number of fingers in multiple hands." []
synonym: "multnumfingshand" EXACT []
is_a: CO_325:1000001 ! Agronomical

[Term]
id: CO_325:0000321
name: Multiple number of fingers in hand: count
namespace: BananaTrait
def: "Count how many fingers are in multiple hands. Associate the data with the Hand rank and the Number of hands measured. The recommendation is to collect this data from the second and second-most distal hands." []
synonym: "HndMltpFrtNum_Ct_Frt, multnumfingshand" EXACT []
is_a: CO_325:1000024 ! Variable
relationship: variable_of CO_325:0000320 ! multiple number of fingers in hand
relationship: variable_of CO_325:0010047 ! multiple number of fingers in hand - counting
relationship: variable_of CO_325:0100017 ! finger

[Term]
id: CO_325:0000322
name: number of hands measured
namespace: BananaTrait
def: "The number of hands used to obtain a measurement." []
synonym: "numhandsmeas" EXACT []
is_a: CO_325:1000001 ! Agronomical

[Term]
id: CO_325:0000323
name: Number of hands measured: count
namespace: BananaTrait
def: "Count how many hands are used to obtain a measurement." []
synonym: "HndNumMsrd_Ct_Hnd, numhandsmeas" EXACT []
is_a: CO_325:1000024 ! Variable
relationship: variable_of CO_325:0000322 ! number of hands measured
relationship: variable_of CO_325:0010048 ! number of hands measured - counting
relationship: variable_of CO_325:0100016 ! hand

[Term]
id: CO_325:0000324
name: average number of fingers in hand
namespace: BananaTrait
def: "The average number of fingers in a hand." []
synonym: "avenumfingshand_rltv" EXACT []
is_a: CO_325:1000001 ! Agronomical

[Term]
id: CO_325:0000325
name: Average number of fingers in hand: calculation
namespace: BananaTrait
def: "Calculate as: the Multiple number of fingers in hand, divided by the Number of hands measured, e.g. 40 / 2 = 20." []
synonym: "HndFrtAvgNum_Ct_Frt, avenumfingshand_rltv" EXACT []
is_a: CO_325:1000024 ! Variable
relationship: variable_of CO_325:0000324 ! average number of fingers in hand
relationship: variable_of CO_325:0010049 ! average number of fingers in hand - computation
relationship: variable_of CO_325:0100017 ! finger

[Term]
id: CO_325:0000326
name: Estimated number of fingers in bunch
namespace: BananaTrait
def: "Calculate as: the sum of the Number of fingers in 3rd hand and the Number of fingers in 2nd-most distal hand, divided by 2, and multiplied by the Number of hands in bunch, e.g. (16 + 12) / 2 * 8 = 112." []
synonym: "BnchFrtNum_Comp_Frt, estnumfingers" EXACT []
is_a: CO_325:1000024 ! Variable
relationship: variable_of CO_325:0000039 ! number of fingers in bunch
relationship: variable_of CO_325:0010040 ! number of fingers in bunch - estimation
relationship: variable_of CO_325:0100017 ! finger

[Term]
id: CO_325:0000327
name: multiple hand weight
namespace: BananaTrait
def: "The weight of multiple hands." []
synonym: "multhandweight" EXACT []
is_a: CO_325:1000001 ! Agronomical

[Term]
id: CO_325:0000328
name: Multiple hand weight in kg
namespace: BananaTrait
def: "Cut multiple hands from the rachis and weigh them together, using scales. Associate the data with the Hank rank and the Number of hands measured. In kg" []
synonym: "MltHandWt_M_kgPlnt, multhandweight" EXACT []
is_a: CO_325:1000024 ! Variable
relationship: variable_of CO_325:0000327 ! multiple hand weight
relationship: variable_of CO_325:0010043 ! multiple hand weight - measurement
relationship: variable_of CO_325:0100015 ! kg

[Term]
id: CO_325:0000329
name: average hand weight
namespace: BananaTrait
def: "The average weight of the hands." []
synonym: "avehandweight" EXACT []
is_a: CO_325:1000001 ! Agronomical

[Term]
id: CO_325:0000330
name: Average hand weight in kg
namespace: BananaTrait
def: "Calculate as: the Multiple hand weight, divided by the Number of hands measured, e.g. 5.6 / 2 = 2.8. In kg" []
synonym: "HandAvgWt_M_kgPlnt, avehandweight" EXACT []
is_a: CO_325:1000024 ! Variable
relationship: variable_of CO_325:0000329 ! average hand weight
relationship: variable_of CO_325:0010044 ! average hand weight - computation
relationship: variable_of CO_325:0100015 ! kg

[Term]
id: CO_325:0000331
name: multiple finger weight
namespace: BananaTrait
def: "The weight of multiple fingers." []
synonym: "multfingerweight" EXACT []
is_a: CO_325:1000001 ! Agronomical

[Term]
id: CO_325:0000332
name: Multiple finger weight in g
namespace: BananaTrait
def: "Weigh multiple fingers together, using scales. Associate the data with the Hank rank and the Number of fingers measured. The recommendation is to collect this data from six fingers in total - three fingers in the middle of the outer whorl from the second hand and from the second-most distal hand. In g" []
synonym: "MltFrtWt_M_gFruit, multfingerweight" EXACT []
is_a: CO_325:1000024 ! Variable
relationship: variable_of CO_325:0000331 ! multiple finger weight
relationship: variable_of CO_325:0010053 ! multiple finger weight - measurement
relationship: variable_of CO_325:0100019 ! g

[Term]
id: CO_325:0000333
name: number of fingers measured
namespace: BananaTrait
def: "The number of fingers used to obtain a measurement." []
synonym: "numfingersmeas" EXACT []
is_a: CO_325:1000001 ! Agronomical

[Term]
id: CO_325:0000334
name: Number of fingers measured
namespace: BananaTrait
def: "Count how many fingers are used to obtain a measurement." []
synonym: "FrtNb_Ct_gFruit, numfingersmeas" EXACT []
is_a: CO_325:1000024 ! Variable
relationship: variable_of CO_325:0000333 ! number of fingers measured
relationship: variable_of CO_325:0010054 ! number of fingers measured - counting
relationship: variable_of CO_325:0100017 ! finger

[Term]
id: CO_325:0000335
name: average finger weight
namespace: BananaTrait
def: "The average weight of the fingers." []
synonym: "avefingerweight" EXACT []
is_a: CO_325:1000001 ! Agronomical

[Term]
id: CO_325:0000336
name: Average finger weight in g
namespace: BananaTrait
def: "Calculate as: the sum of the the Finger weight measurements, divided by the number of those measurements, e.g. (150 + 146 + 147 + 152 + 140 + 146) / 6 = 147. In g" []
synonym: "FrtWtAvg_M_g, WGTFRU, avefingerweight" EXACT []
is_a: CO_325:1000024 ! Variable
relationship: variable_of CO_325:0000335 ! average finger weight
relationship: variable_of CO_325:0010055 ! average finger weight - computation
relationship: variable_of CO_325:0100019 ! g

[Term]
id: CO_325:0000337
name: average finger external length
namespace: BananaTrait
def: "The average length of the fingers measured along the external (dorsal) arc, excluding the pedicel and the fruit tip." []
synonym: "avefingerextlength" EXACT []
synonym: "Average finger dorsal length" EXACT []
is_a: CO_325:1000001 ! Agronomical

[Term]
id: CO_325:0000338
name: Average finger external length in cm
namespace: BananaTrait
def: "Calculate as: the sum of the Finger external length measurements, divided by the number of those measurements, e.g. (30 + 34 + 32 + 33 + 33 + 31) / 6 = 32.1. In cm" []
synonym: "AvgFrtExtLng_M_cm, avefingerextlength" EXACT []
is_a: CO_325:1000024 ! Variable
relationship: variable_of CO_325:0000337 ! average finger external length
relationship: variable_of CO_325:0010057 ! average finger external length - computation
relationship: variable_of CO_325:0100008 ! cm

[Term]
id: CO_325:0000339
name: finger internal length
namespace: BananaTrait
def: "The length of a finger measured along the internal (ventral) arc, excluding the pedicel and the fruit tip." []
synonym: "Finger ventral length" EXACT []
synonym: "fingerintlength" EXACT []
is_a: CO_325:1000001 ! Agronomical

[Term]
id: CO_325:0000340
name: Finger internal length in mm
namespace: BananaTrait
def: "Measure the length of a finger, along the internal (ventral) arc, excluding the pedicel and the fruit tip, using a tape measure. Associate the data with the Hand rank and the Number of fingers measured. The recommendation is to collect this data from six fingers in total - three fingers in the middle of the outer whorl from the second hand and from the second-most distal hand. In mm" []
synonym: "FrtIntLng_M_cm, fingerintlength_cm" EXACT []
is_a: CO_325:1000024 ! Variable
relationship: variable_of CO_325:0000339 ! finger internal length
relationship: variable_of CO_325:0010058 ! finger internal length - measurement
relationship: variable_of CO_325:0100020 ! mm

[Term]
id: CO_325:0000341
name: average finger internal length
namespace: BananaTrait
def: "The average length of the fingers measured along the internal (ventral) arc, excluding the pedicel and the fruit tip." []
synonym: "avefingerintlength" EXACT []
synonym: "Average finger ventral length" EXACT []
is_a: CO_325:1000001 ! Agronomical

[Term]
id: CO_325:0000342
name: Average finger internal length in cm
namespace: BananaTrait
def: "Calculate as: the sum of the Finger internal length measurements, divided by the number of those measurements, e.g. (27 + 31 + 29 + 30 + 30 + 28) / 6 = 29.2. In cm" []
synonym: "AvgFrtIntLng_M_cm, avefingerintlength" EXACT []
is_a: CO_325:1000024 ! Variable
relationship: variable_of CO_325:0000341 ! average finger internal length
relationship: variable_of CO_325:0010059 ! average finger internal length - computation
relationship: variable_of CO_325:0100008 ! cm

[Term]
id: CO_325:0000343
name: Finger circumference in mm
namespace: BananaTrait
def: "Measure the circumference of a finger at its widest point, using a tape measure. Associate the data with the Hand rank. The recommendation is to collect this data from six fingers in total - three fingers in the middle of the outer whorl from the second hand and from the second-most distal hand. In mm" []
synonym: "FrtGrth_M_mm, fingercircumf_mm" EXACT []
is_a: CO_325:1000024 ! Variable
relationship: variable_of CO_325:0000054 ! finger circumference
relationship: variable_of CO_325:0010060 ! finger circumference - measurement
relationship: variable_of CO_325:0100020 ! mm

[Term]
id: CO_325:0000344
name: average finger circumference
namespace: BananaTrait
def: "The average circumference of the fingers." []
synonym: "avefingercircumf" EXACT []
synonym: "Average finger girth" EXACT []
is_a: CO_325:1000001 ! Agronomical

[Term]
id: CO_325:0000345
name: Average finger circumference in mm
namespace: BananaTrait
def: "Calculate as: the sum of the Finger circumference measurements, divided by the number of those measurements, e.g. (7.0 + 8.0 + 9.0 + 10.0 + 7.0 + 9.5) / 6 = 8.4. In cm" []
synonym: "AvgFrtGrth_M_mm, avefingercircumf" EXACT []
is_a: CO_325:1000024 ! Variable
relationship: variable_of CO_325:0000344 ! average finger circumference
relationship: variable_of CO_325:0010061 ! average finger circumference - computation
relationship: variable_of CO_325:0100008 ! cm

[Term]
id: CO_325:0000347
name: Finger lateral diameter in mm
namespace: BananaTrait
def: "Measure the lateral diameter of a finger from the left to the right side (not from the ventral to the dorsal side), at the widest point, using calipers. Associate the data with the Hand rank. The recommendation is to collect this data from six fingers in total - three fingers in the middle of the outer whorl from the second hand and from the second-most distal hand. In mm" []
synonym: "FrtDiam_M_mm, fingerlatdiam" EXACT []
is_a: CO_325:1000024 ! Variable
relationship: variable_of CO_325:0000233 ! finger lateral diameter
relationship: variable_of CO_325:0010062 ! finger lateral diameter - measurement
relationship: variable_of CO_325:0100020 ! mm

[Term]
id: CO_325:0000348
name: average finger lateral diameter
namespace: BananaTrait
def: "The average lateral (side to side) diameter of a finger." []
synonym: "avefingerlatdiam" EXACT []
synonym: "Finger grade, Fruit diameter, Fruit grade" EXACT []
is_a: CO_325:1000001 ! Agronomical

[Term]
id: CO_325:0000349
name: Average finger lateral diameter in mm
namespace: BananaTrait
def: "Calculate as: the sum of the Finger lateral diameter measurements, divided by the number of those measurements, e.g. (3.5 + 5.2 + 4.1 + 5 + 6 + 6.8) / 6 = 5.1. In cm" []
synonym: "AvgFrtDiam_M_mm, avefingerlatdiam" EXACT []
is_a: CO_325:1000024 ! Variable
relationship: variable_of CO_325:0000348 ! average finger lateral diameter
relationship: variable_of CO_325:0010063 ! average finger lateral diameter - computation
relationship: variable_of CO_325:0100008 ! cm

[Term]
id: CO_325:0000351
name: Fruit pulp lateral diameter in mm
namespace: BananaTrait
def: "Cut a finger in half, crosswise at its widest point, and on the cross-section measure the lateral diameter of the fruit pulp, from the left to the right side (not from the ventral to the dorsal side), using calipers. Associate the data with the Hand rank. The recommendation is to collect this data from six fingers in total - three fingers in the middle of the outer whorl from the second hand and from the second-most distal hand. In mm" []
synonym: "PulpDiam_M_mm, pulpdiam" EXACT []
is_a: CO_325:1000024 ! Variable
relationship: variable_of CO_325:0000240 ! fruit pulp lateral diameter
relationship: variable_of CO_325:0010064 ! fruit pulp lateral diameter - measurement
relationship: variable_of CO_325:0100020 ! mm

[Term]
id: CO_325:0000352
name: average fruit pulp lateral diameter
namespace: BananaTrait
def: "The average lateral (side to side) diameter of the pulp of a fruit." []
synonym: "avepulpdiam" EXACT []
synonym: "Finger pulp diameter" EXACT []
is_a: CO_325:1000001 ! Agronomical

[Term]
id: CO_325:0000353
name: Average fruit pulp lateral diameter in cm
namespace: BananaTrait
def: "Calculate as: the sum of the Fruit pulp lateral diameter measurements, divided by the number of those measurements, e.g. (3.1 + 4.8 + 3.7 + 4.6 + 5.6 + 6.4) / 6 = 4.7. In cm" []
synonym: "AvgPulpDiam_M_mm, avepulpdiam" EXACT []
is_a: CO_325:1000024 ! Variable
relationship: variable_of CO_325:0000352 ! average fruit pulp lateral diameter
relationship: variable_of CO_325:0010065 ! average fruit pulp lateral diameter - computation
relationship: variable_of CO_325:0100008 ! cm

[Term]
id: CO_325:0000355
name: average finger peel thickness
namespace: BananaTrait
def: "The average thickness of the peel of a finger." []
synonym: "avepeelthickness" EXACT []
synonym: "Width of the peel, Width of the skin, Width of the exocarp, Finger peel thickness" EXACT []
is_a: CO_325:1000001 ! Agronomical

[Term]
id: CO_325:0000356
name: Average finger peel thickness in mm
namespace: BananaTrait
def: "Calculate as: the sum of the Finger peel thickness measurements, divided by the number of those measurements, e.g. (2 + 2 + 2 + 3 + 2 + 3 + 3) / 6 = 2. In mm" []
synonym: "AvgPeelThck_M_mm, avepeelthickness" EXACT []
is_a: CO_325:1000024 ! Variable
relationship: variable_of CO_325:0000355 ! average finger peel thickness
relationship: variable_of CO_325:0010067 ! average finger peel thickness - computation
relationship: variable_of CO_325:0100020 ! mm

[Term]
id: CO_325:0000357
name: number of plants planted
namespace: BananaTrait
def: "The number of plants that are planted." []
synonym: "numplanted" EXACT []
is_a: CO_325:1000001 ! Agronomical

[Term]
id: CO_325:0000358
name: Number of plants planted: count
namespace: BananaTrait
def: "Calculate as: the sum of the number of values for Date of planting." []
synonym: "PltPltd_Ct_Plnt, numplanted" EXACT []
is_a: CO_325:1000024 ! Variable
relationship: variable_of CO_325:0000357 ! number of plants planted
relationship: variable_of CO_325:0010068 ! number of plants planted - computation
relationship: variable_of CO_325:0100021 ! plant

[Term]
id: CO_325:0000359
name: plant spacing
namespace: BananaTrait
def: "The area allocated to one plant." []
synonym: "plantspacing" EXACT []
is_a: CO_325:1000001 ! Agronomical

[Term]
id: CO_325:0000360
name: Plant spacing in m2
namespace: BananaTrait
def: "Calculate as: multiply the distance of the spacing between the plants, both latitudinally and longitudinally, e.g. 2 m x 3 m = 6 m2. In m2" []
synonym: "PltSpcg_Comp_m2, plantspacing" EXACT []
is_a: CO_325:1000024 ! Variable
relationship: variable_of CO_325:0000359 ! plant spacing
relationship: variable_of CO_325:0010069 ! plant spacing - computation
relationship: variable_of CO_325:0100022 ! m2

[Term]
id: CO_325:0000361
name: plant density
namespace: BananaTrait
def: "The number of plants that are planted, in a defined area." []
synonym: "plantdens" EXACT []
is_a: CO_325:1000001 ! Agronomical

[Term]
id: CO_325:0000362
name: Plant density: calculation
namespace: BananaTrait
def: "Calculate as: number of square metres in the area unit of choice, divided by the Plant spacing, e.g. 10,000 square metres in 1 hectare / 6 = 1,667 plants/ha." []
synonym: "PltDnsty_Comp_PlntHa, plantdens" EXACT []
is_a: CO_325:1000024 ! Variable
relationship: variable_of CO_325:0000361 ! plant density
relationship: variable_of CO_325:0010070 ! plant density - computation
relationship: variable_of CO_325:0100023 ! plants/unit of area

[Term]
id: CO_325:0000363
name: number of plants dead
namespace: BananaTrait
def: "The number of plants that are dead." []
synonym: "numdead" EXACT []
is_a: CO_325:1000001 ! Agronomical

[Term]
id: CO_325:0000364
name: Number of plants dead: count
namespace: BananaTrait
def: "Calculate as: the sum of the number of values for Date of death." []
synonym: "PltDead_Ct_Plnt, numdead" EXACT []
is_a: CO_325:1000024 ! Variable
relationship: variable_of CO_325:0000363 ! number of plants dead
relationship: variable_of CO_325:0010071 ! number of plants dead - computation
relationship: variable_of CO_325:0100021 ! plant

[Term]
id: CO_325:0000365
name: number of plants harvested
namespace: BananaTrait
def: "The number of plants that are harvested." []
synonym: "numharv" EXACT []
is_a: CO_325:1000001 ! Agronomical

[Term]
id: CO_325:0000366
name: Number of plants harvested: count
namespace: BananaTrait
def: "Calculate as: the sum of the number of values for Date of harvest." []
synonym: "PltHvstd_Ct_Plnt, numharv" EXACT []
is_a: CO_325:1000024 ! Variable
relationship: variable_of CO_325:0000365 ! number of plants harvested
relationship: variable_of CO_325:0010072 ! number of plants harvested - computation
relationship: variable_of CO_325:0100021 ! plant

[Term]
id: CO_325:0000367
name: number of plants not harvested
namespace: BananaTrait
def: "The number of plants that are alive but not harvested (e.g. due to slow or poor development)." []
synonym: "numnotharv" EXACT []
is_a: CO_325:1000001 ! Agronomical

[Term]
id: CO_325:0000368
name: Number of plants not harvested: count
namespace: BananaTrait
def: "Calculate as: the Number of plants planted, minus the Number of plants dead, minus the Number of plants harvested, e.g. 24 - 4 - 18 = 2." []
synonym: "PltNtHvstd_Ct_Plnt, numnotharv" EXACT []
is_a: CO_325:1000024 ! Variable
relationship: variable_of CO_325:0000367 ! number of plants not harvested
relationship: variable_of CO_325:0010073 ! number of plants not harvested - computation
relationship: variable_of CO_325:0100021 ! plant

[Term]
id: CO_325:0000369
name: death proportion
namespace: BananaTrait
def: "The proportion of plants that are dead, from the number of plants planted." []
synonym: "deathprop" EXACT []
is_a: CO_325:1000001 ! Agronomical

[Term]
id: CO_325:0000370
name: Death proportion: calculation
namespace: BananaTrait
def: "Calculate as: the Number of plants dead, divided by the Number of plants planted, e.g. 4 / 24 = 0.17. In plants dead/plants planted" []
synonym: "DthPrp_Comp_DdPltRt, deathprop" EXACT []
is_a: CO_325:1000024 ! Variable
relationship: variable_of CO_325:0000369 ! death proportion
relationship: variable_of CO_325:0010074 ! death proportion - computation
relationship: variable_of CO_325:0100024 ! plants dead/plants planted

[Term]
id: CO_325:0000371
name: death density
namespace: BananaTrait
def: "The number of plants that are dead, in a defined area." []
synonym: "deathdens" EXACT []
is_a: CO_325:1000001 ! Agronomical

[Term]
id: CO_325:0000372
name: Death density
namespace: BananaTrait
def: "Calculate as: the Plant density multiplied by the Death proportion, e.g. 1,667 * 0.17 = 283. In plants/unit of area" []
synonym: "DthDnst_Comp_PlntHa, deathdens" EXACT []
is_a: CO_325:1000024 ! Variable
relationship: variable_of CO_325:0000371 ! death density
relationship: variable_of CO_325:0010075 ! death density - computation
relationship: variable_of CO_325:0100023 ! plants/unit of area

[Term]
id: CO_325:0000373
name: harvest proportion
namespace: BananaTrait
def: "The proportion of plants that are harvested, from the number of plants planted." []
synonym: "harvprop" EXACT []
is_a: CO_325:1000001 ! Agronomical

[Term]
id: CO_325:0000374
name: Harvest proportion: calculation
namespace: BananaTrait
def: "Calculate as: the Number of plants harvested, divided by the Number of plants planted, e.g. 18 / 24 = 0.75. In plants harvested/plants planted" []
synonym: "HvstPrp_Comp_PlntNb, harvprop" EXACT []
is_a: CO_325:1000024 ! Variable
relationship: variable_of CO_325:0000373 ! harvest proportion
relationship: variable_of CO_325:0010076 ! harvest proportion - computation
relationship: variable_of CO_325:0100025 ! plants harvested/plants planted

[Term]
id: CO_325:0000375
name: harvest density
namespace: BananaTrait
def: "The number of plants that are harvested, in a defined area." []
synonym: "harvdens" EXACT []
is_a: CO_325:1000001 ! Agronomical

[Term]
id: CO_325:0000376
name: Harvest density: calculation
namespace: BananaTrait
def: "Calculate as: the Plant density multiplied by the Harvest proportion, e.g. 1,667 * 0.75 = 1,250. In plants/unit of area" []
synonym: "HvstDst_Comp_PlntHa, harvdens" EXACT []
is_a: CO_325:1000024 ! Variable
relationship: variable_of CO_325:0000375 ! harvest density
relationship: variable_of CO_325:0010077 ! harvest density - computation
relationship: variable_of CO_325:0100023 ! plants/unit of area

[Term]
id: CO_325:0000377
name: non-harvest proportion
namespace: BananaTrait
def: "The proportion of plants that are alive but not harvested (e.g. due to slow or poor development), from the number of plants planted." []
synonym: "nonharvprop" EXACT []
is_a: CO_325:1000001 ! Agronomical

[Term]
id: CO_325:0000378
name: Non-harvest proportion: calculation
namespace: BananaTrait
def: "Calculate as: the Number of plants not harvested, divided by the Number of plants planted, e.g. 2 / 24 = 0.08. In plants not harvested/plants planted" []
synonym: "NtHvstPrp_Comp_PlntNb, nonharvprop" EXACT []
is_a: CO_325:1000024 ! Variable
relationship: variable_of CO_325:0000377 ! non-harvest proportion
relationship: variable_of CO_325:0010078 ! non-harvest proportion - computation
relationship: variable_of CO_325:0100026 ! plants not harvested/plants planted

[Term]
id: CO_325:0000379
name: non-harvest density
namespace: BananaTrait
def: "The number of plants that are alive but not harvested (e.g. due to slow or poor development), in a defined area." []
synonym: "nonharvdens" EXACT []
is_a: CO_325:1000001 ! Agronomical

[Term]
id: CO_325:0000380
name: Non-harvest density: calculation
namespace: BananaTrait
def: "Calculate as: the Plant density multiplied by the Non-harvest proportion, e.g. 1,667 * 0.08 = 133. In plants/unit of area" []
synonym: "NtHvstDst_Comp_PlntHa, nonharvdens" EXACT []
is_a: CO_325:1000024 ! Variable
relationship: variable_of CO_325:0000379 ! non-harvest density
relationship: variable_of CO_325:0010079 ! non-harvest density - computation
relationship: variable_of CO_325:0100023 ! plants/unit of area

[Term]
id: CO_325:0000381
name: annual crop cycle proportion
namespace: BananaTrait
def: "The proportion of the crop cycle that takes place in one year." []
synonym: "anncropcycprop" EXACT []
is_a: CO_325:1000001 ! Agronomical

[Term]
id: CO_325:0000382
name: Annual crop cycle proportion: calculation
namespace: BananaTrait
def: "Calculate as: the length of a year (e.g. 365 days) divided by the Plant crop cycle or the Ratoon crop cycle, e.g. 365 / 334 = 1.09. In crop cycle duration/year." []
synonym: "AnCrpCyclPrp_Comp_CrpCclY, anncropcycprop" EXACT []
is_a: CO_325:1000024 ! Variable
relationship: variable_of CO_325:0000381 ! annual crop cycle proportion
relationship: variable_of CO_325:0010080 ! annual crop cycle proportion - computation
relationship: variable_of CO_325:0100027 ! crop cycle duration/year

[Term]
id: CO_325:0000383
name: plant annual yield
namespace: BananaTrait
def: "The bunch weight produced by the plant over the course of the crop cycle, averaged across one year." []
synonym: "plantannyield" EXACT []
is_a: CO_325:1000001 ! Agronomical

[Term]
id: CO_325:0000384
name: Plant annual yield in kg/plant/y
namespace: BananaTrait
def: "Calculate as: the Bunch weight multiplied by the Annual crop cycle proportion, e.g. 48 * 1.09 = 52.32. In kg/plant/y" []
synonym: "AnPltPrp_Comp_KgHaY, plantannyield" EXACT []
is_a: CO_325:1000024 ! Variable
relationship: variable_of CO_325:0000383 ! plant annual yield
relationship: variable_of CO_325:0010081 ! annual plant productivity - computation
relationship: variable_of CO_325:0100028 ! kg/plant/y

[Term]
id: CO_325:0000385
name: average actual annual yield
namespace: BananaTrait
def: "The average actual annual yield, taking into account the proportion of plants harvested, from the number of plants planted" []
synonym: "actualannyield" EXACT []
synonym: "Yield" EXACT []
is_a: CO_325:1000001 ! Agronomical

[Term]
id: CO_325:0000386
name: Average actual annual yield in t/unit of area/y
namespace: BananaTrait
def: "Calculate as: the Bunch weight divided by 1,000, multiplied by the Annual crop cycle proportion, multiplied by the Harvest density, e.g. (50 / 1,000) * 1.09 * 1,250 = 68.13. In t/unit of area/y" []
synonym: "AcAnYd_Comp_TnHaY, actualannyield" EXACT []
is_a: CO_325:1000024 ! Variable
relationship: variable_of CO_325:0000385 ! average actual annual yield
relationship: variable_of CO_325:0010082 ! actual annual yield - computation
relationship: variable_of CO_325:0100029 ! t/unit of area/y

[Term]
id: CO_325:0000387
name: average potential annual yield
namespace: BananaTrait
def: "The average potential annual yield, assuming that all plants are harvested, from the number of plants planted." []
synonym: "potannyield" EXACT []
synonym: "Yield" EXACT []
is_a: CO_325:1000001 ! Agronomical

[Term]
id: CO_325:0000388
name: Average potential annual yield in t/unit of area/y
namespace: BananaTrait
def: "Calculate as: the Bunch weight divided by 1,000, multiplied by the Annual crop cycle proportion, multiplied by the Plant density, e.g. (50 / 1,000) * 1.09 * 1,667 = 90.85. In t/unit of area/y" []
synonym: "PtYd_Comp_TnHaY, potannyield" EXACT []
is_a: CO_325:1000024 ! Variable
relationship: variable_of CO_325:0000387 ! average potential annual yield
relationship: variable_of CO_325:0010083 ! potential annual yield - computation
relationship: variable_of CO_325:0100029 ! t/unit of area/y

[Term]
id: CO_325:0000389
name: overall fruit pendulance quality
namespace: BananaTrait
def: "The overall estimation fruit pendulance on a bunch" []
synonym: "pendulantfruit" EXACT []
is_a: CO_325:1000001 ! Agronomical

[Term]
id: CO_325:0000390
name: Overall fruit pendulance 1-2
namespace: BananaTrait
def: "Visual estimation of fruit pendulance on a bunch, for Early Evaluation Trial stage only., 1 = bad; 2 = good" []
synonym: "PdltFrt_Est_1to2, pendulantfruit" EXACT []
is_a: CO_325:1000024 ! Variable
relationship: variable_of CO_325:0000389 ! overall fruit pendulance quality
relationship: variable_of CO_325:0010084 ! fruit pendulance - estimation
relationship: variable_of CO_325:0100030 ! bad good

[Term]
id: CO_325:0000391
name: overall bunch quality
namespace: BananaTrait
def: "The overall estimation of the bunch quality on a mat" []
synonym: "goodbunch" EXACT []
is_a: CO_325:1000001 ! Agronomical

[Term]
id: CO_325:0000392
name: Overall bunch quality 1-2
namespace: BananaTrait
def: "Visual estimation of bunch quality, for Early Evaluation Trial stage only., 1 = bad; 2 = good" []
synonym: "GdBnch_Est_1to2, goodbunch" EXACT []
is_a: CO_325:1000024 ! Variable
relationship: variable_of CO_325:0000391 ! overall bunch quality
relationship: variable_of CO_325:0010085 ! bunch quality - estimation
relationship: variable_of CO_325:0100030 ! bad good

[Term]
id: CO_325:0000393
name: fruitfill
namespace: BananaTrait
def: "The overall estimation of fruitfilling level on a bunch" []
synonym: "goodfruitfill" EXACT []
is_a: CO_325:1000001 ! Agronomical

[Term]
id: CO_325:0000394
name: Fruitfill 1-2
namespace: BananaTrait
def: "Visual estimation of a fruit filling for Early Evaluation Trial stage only., 1 = filled; 2 = not filled" []
synonym: "GdFrtFll_Est_1to2, goodfruitfill" EXACT []
is_a: CO_325:1000024 ! Variable
relationship: variable_of CO_325:0000393 ! fruitfill
relationship: variable_of CO_325:0010086 ! fruitfill - estimation
relationship: variable_of CO_325:0100031 ! fruitfill

[Term]
id: CO_325:0000395
name: overall suckering quality
namespace: BananaTrait
def: "The overall estimation of sucker quality on a mat" []
synonym: "suckering" EXACT []
is_a: CO_325:1000001 ! Agronomical

[Term]
id: CO_325:0000396
name: Overall suckering quality 1-2
namespace: BananaTrait
def: "Visual estimation of suckering, for Early Evaluation Trial stage only., 1 = bad; 2 = good" []
synonym: "Sckr_Est_1to2, suckering" EXACT []
is_a: CO_325:1000024 ! Variable
relationship: variable_of CO_325:0000395 ! overall suckering quality
relationship: variable_of CO_325:0010087 ! sucker quality - estimation
relationship: variable_of CO_325:0100030 ! bad good

[Term]
id: CO_325:0000397
name: dwarfism
namespace: BananaTrait
def: "The presence or absence of dwarfism on a mat" []
synonym: "dwarfism" EXACT []
is_a: CO_325:1000001 ! Agronomical

[Term]
id: CO_325:0000398
name: Dwarfism 1-2
namespace: BananaTrait
def: "Visual estimation of dwarfism, for Early Evaluation Trial stage only., 1 = dwarf; 2 = not dwarf" []
synonym: "Dwfsm_Est_1to2, dwarfism" EXACT []
is_a: CO_325:1000024 ! Variable
relationship: variable_of CO_325:0000397 ! dwarfism
relationship: variable_of CO_325:0010088 ! dwarfism - estimation
relationship: variable_of CO_325:0100032 ! dwarfism

[Term]
id: CO_325:0000425
name: pseudostem height
namespace: BananaTrait
def: "Distance from the base of the pseudostem to the emerging point of the peduncle." []
synonym: "Plant height" EXACT []
is_a: CO_325:1000003 ! Morphological

[Term]
id: CO_325:0000426
name: Pseudostem height 1-3
namespace: BananaTrait
def: "Recorded from the base of the pseudostem to the emerging point of the peduncle., 1 = yes; 2 = no; 3 = equal to or more than 3 m" []
synonym: "PsdHght_E, PSEHT" EXACT []
is_a: CO_325:1000024 ! Variable
relationship: variable_of CO_325:0000425 ! pseudostem height
relationship: variable_of CO_325:0010159 ! pseudostem height - estimation
relationship: variable_of CO_325:0100062 ! height score (1 to 3)

[Term]
id: CO_325:0000427
name: blotches relative area at petiole base
namespace: BananaTrait
def: "Percentage coverage of petiole base by blotches." []
synonym: "Blotches at the petiole base" EXACT []
is_a: CO_325:1000003 ! Morphological

[Term]
id: CO_325:0000428
name: Blotches relative area at petiole base 1-4
namespace: BananaTrait
def: "Record the relative surface area coverage by blotches. [x Look at several plants if possible to get an overall idea. Observe at flowering time]., 1 = no pigmentation; 2 = sparse blotching (<20%); 3 = moderate blotching (20-50%); 4 = extensive pigmentation (>50%)" []
synonym: "BlotchA_Est_1to4," EXACT []
is_a: CO_325:1000024 ! Variable
relationship: variable_of CO_325:0000427 ! blotches relative area at petiole base
relationship: variable_of CO_325:0010161 ! blotches area - estimation
relationship: variable_of CO_325:0100064 ! blotch pigmentation scale (1 to 4)

[Term]
id: CO_325:0000429
name: Blotches relative area at petiole base 1-5
namespace: BananaTrait
def: "Record the relative surface area coverage by blotches. [x Look at several plants if possible to get an overall idea. Observe at flowering time]., 1 = sparse blotching; 2 = small blotches; 3 = large blotches; 4 = extensive pigmentation; 5 = without pigmentation" []
synonym: "BlotchA_Est_1to5," EXACT []
is_a: CO_325:1000024 ! Variable
relationship: variable_of CO_325:0000427 ! blotches relative area at petiole base
relationship: variable_of CO_325:0010161 ! blotches area - estimation
relationship: variable_of CO_325:0100065 ! blotch pigmentation scale (1 to 5)

[Term]
id: CO_325:0000430
name: blotches colour at the petiole base
namespace: BananaTrait
def: "Colour of the blotches on the upper leaf sheath of the petiole base." []
synonym: "Blotches colour" EXACT []
is_a: CO_325:1000003 ! Morphological

[Term]
id: CO_325:0000431
name: Blotches colour at the petiole base 1-4
namespace: BananaTrait
def: "Observe visually the colour of the blotches on the upper leaf sheath., 1 = orange-brown (mahogany, like in Pisang Mas); 2 = brown; 3 = black-purple; 4 = other" []
synonym: "BlotchCol_Est_1to4," EXACT []
is_a: CO_325:1000024 ! Variable
relationship: variable_of CO_325:0000430 ! blotches colour at the petiole base
relationship: variable_of CO_325:0010162 ! blotches colour - estimation
relationship: variable_of CO_325:0100066 ! blotch color scale (1 to 4)

[Term]
id: CO_325:0000432
name: Blotches colour at the petiole base 1-5
namespace: BananaTrait
def: "Observe visually the colour of the blotches on the upper leaf sheath., 1 = brown; 2 = dark brown; 3 = brown-black; 4 = black-purple; 5 = other" []
synonym: "BlotchCol_Est_1to5, BLOPB" EXACT []
is_a: CO_325:1000024 ! Variable
relationship: variable_of CO_325:0000430 ! blotches colour at the petiole base
relationship: variable_of CO_325:0010162 ! blotches colour - estimation
relationship: variable_of CO_325:0100067 ! blotch color scale (1 to 5)

[Term]
id: CO_325:0000433
name: margin behaviour on petiole canal of third leaf
namespace: BananaTrait
def: "Margin behaviour of the petiole canal of the third leaf before bunch." []
synonym: "Petiole canal of the third leaf, Petiole canal leaf III" EXACT []
is_a: CO_325:1000003 ! Morphological

[Term]
id: CO_325:0000434
name: Margin behaviour on petiole canal of third leaf 1-4
namespace: BananaTrait
def: "The third leaf (Leaf III) is counted from the last leaf produced before [x bunch emergence] [shooting]. Cut the petiole halfway between the pseudostem and the leaf blade and examine the cross section. [x Observe at flowering time]., 1 = margins spreading; 2 = margins erect; 3 = margins curved inward; 4 = margins overlapping" []
synonym: "MgnBhvPtCnlThrdLf_Est_1to4, PENCL4" EXACT []
is_a: CO_325:1000024 ! Variable
relationship: variable_of CO_325:0000433 ! margin behaviour on petiole canal of third leaf
relationship: variable_of CO_325:0010163 ! margin behaviour on petiole canal of third leaf - estimation
relationship: variable_of CO_325:0100068 ! margin behaviour scale (1 to 4)

[Term]
id: CO_325:0000435
name: Margin behaviour on petiole canal of third leaf 1-5
namespace: BananaTrait
def: "The third leaf (Leaf III) is counted from the last leaf produced before [x bunch emergence] [shooting]. Cut the petiole halfway between the pseudostem and the leaf blade and examine the cross section. [x Observe at flowering time]., 1 = open with margins spreading; 2 = wide with erect margins; 3 = straight with erect margins; 4 = margins curved inward; 5 = margins overlapping" []
synonym: "MgnBhvPtCnlThrdLf_Est_1to5, PENCL5" EXACT []
is_a: CO_325:1000024 ! Variable
relationship: variable_of CO_325:0000433 ! margin behaviour on petiole canal of third leaf
relationship: variable_of CO_325:0010163 ! margin behaviour on petiole canal of third leaf - estimation
relationship: variable_of CO_325:0100069 ! margin behaviour scale (1 to 5)

[Term]
id: CO_325:0000436
name: Petiole margins winged 1-5
namespace: BananaTrait
def: "Observations on the margins and petiole wings should be made where the petiole and pseudostem meet at shooting. Margin is the part of the petiole that can be bent outwards/inwards. [x Observe at flowering time.], 1 = winged and undulating; 2 = winged and not clasping the pseudostem; 3 = winged and clasping the pseudostem; 4 = not winged and clasping the pseudostem; 5 = not winged and not clasping the pseudostem" []
synonym: "PMargWing_Est_1or5, PETMWG" EXACT []
is_a: CO_325:1000024 ! Variable
relationship: variable_of CO_325:0000256 ! petiole margins winged
relationship: variable_of CO_325:0010164 ! winged petiole margin - estimation
relationship: variable_of CO_325:0100071 ! wing presence/absence and clasping presence/absence scale 1 to 5

[Term]
id: CO_325:0000437
name: Petiole margin colour 1-4
namespace: BananaTrait
def: "Observations on the margins and petiole wings should be made where the petiole and pseudostem meet at shooting. Use colour chart A and observe out of direct sunlight. Record the colour of the margin (general colour is below the rim). [x Observe at flowering time.], 1 = green; 2 = pink-purple to red; 3 = purple to blue; 4 = other" []
synonym: "PMargCol_Esr_1to4, PETMCO_1-4" EXACT []
is_a: CO_325:1000024 ! Variable
relationship: variable_of CO_325:0000264 ! petiole margin colour
relationship: variable_of CO_325:0010166 ! petiole margin colour - estimation
relationship: variable_of CO_325:0100073 ! bd colour chart a - 1996

[Term]
id: CO_325:0000438
name: bunch position
namespace: BananaTrait
def: "Angle between the axis of the bunch and the vertical" []
is_a: CO_325:1000003 ! Morphological

[Term]
id: CO_325:0000439
name: Bunch position 1-5
namespace: BananaTrait
def: "Visually observe the angle of the bunch and choose the option that is most similar, from the 5 schematic drawings of descriptor 6.4.6 in the reference material., 1 = hanging vertically; 2 = slightly angled; 3 = hanging at a 45 degree angle; 4 = horizontal; 5 = erect" []
synonym: "BnchPst_Estm_1to5, BNCPOS" EXACT []
is_a: CO_325:1000024 ! Variable
relationship: variable_of CO_325:0000438 ! bunch position
relationship: variable_of CO_325:0010169 ! bunch position - estimation
relationship: variable_of CO_325:0100075 ! bunch position scale(1 to 5)

[Term]
id: CO_325:0000440
name: bunch shape
namespace: BananaTrait
def: "Shape of the fully developed bunch on a plant" []
is_a: CO_325:1000003 ! Morphological

[Term]
id: CO_325:0000441
name: Bunch shape 1-5
namespace: BananaTrait
def: "Visually observe the shape of the mature bunch on a fully developed plant that is not experiencing environmental stress and choose the option that is most similar, from the 4 photos of descriptor 6.4.7. in the reference material. 1 = cylindrical; 2 = truncate =cone shaped; 3 = asymmetrical; 4 = spiral (all fruit are attached to a unique crown coiled around the stalk); 5 = other" []
synonym: "BnchShp_Estm_1to5, BNSHP" EXACT []
is_a: CO_325:1000024 ! Variable
relationship: variable_of CO_325:0000440 ! bunch shape
relationship: variable_of CO_325:0010170 ! bunch shape - estimation
relationship: variable_of CO_325:0100076 ! bunch shape scale (1 to 5)

[Term]
id: CO_325:0000442
name: male rachis type
namespace: BananaTrait
def: "Behaviour of male rachis - truncated or present. Truncated means there is no bract scar below the last hand. Present means there is a degenerated or persistent male bud" []
is_a: CO_325:1000003 ! Morphological

[Term]
id: CO_325:0000443
name: Male rachis type 1-2
namespace: BananaTrait
def: "Visually observe the part of the rachis between the last hand and the male bud. Truncated means there is no bract scar below the last hand. Present means there is a degenerated or persistent male bud, 1 = truncated; 2 = present" []
synonym: "MlRchsTp_Estm_1to2," EXACT []
is_a: CO_325:1000024 ! Variable
relationship: variable_of CO_325:0000442 ! male rachis type
relationship: variable_of CO_325:0010171 ! male rachis type - estimation
relationship: variable_of CO_325:0100077 ! rachis type scale (1 to 2)

[Term]
id: CO_325:0000444
name: male rachis position
namespace: BananaTrait
def: "Angle of the rachis between last hand and male bud" []
synonym: "Rachis angle" EXACT []
is_a: CO_325:1000003 ! Morphological

[Term]
id: CO_325:0000445
name: Male rachis position 1-2
namespace: BananaTrait
def: "Visually observe the male rachis position (the part between the last hand and the male bud) and choose the option that is most similar, from the 5 schematic drawings of descriptor 6.4.12 in the reference material., 1 = falling vertically; 2 = at an angle; 3 = with a curve; 4 = horizontal or supra-horizontal; 5 = erect" []
synonym: "MlRchsPst_Estm_1to5, RACPOS" EXACT []
is_a: CO_325:1000024 ! Variable
relationship: variable_of CO_325:0000444 ! male rachis position
relationship: variable_of CO_325:0010172 ! male rachis position - estimation
relationship: variable_of CO_325:0100078 ! rachis angle scale (1 to 2)

[Term]
id: CO_325:0000446
name: male rachis appearance
namespace: BananaTrait
def: "Appearance of flowers/bracts on the male rachis" []
synonym: "Rachis appearance" EXACT []
is_a: CO_325:1000003 ! Morphological

[Term]
id: CO_325:0000447
name: Male rachis appearance 1-5
namespace: BananaTrait
def: "Visually observe the male rachis appearance and choose the option that is most similar., 1 = bare; 2 = neutral flowers on one to few hands only near the bunch (rest of stalk is bare); 3 = male flowers/bracts above the male bud (rest of stalk is bare); 4 = neutral/male flowers and presence of withered bracts on the entire stalk; 5 = neutral/male flowers on the whole stalk without persistent bracts (still firmly attached to the rachis)" []
synonym: "MlRchsApp_Estm_1to7, RACHAP" EXACT []
is_a: CO_325:1000024 ! Variable
relationship: variable_of CO_325:0000446 ! male rachis appearance
relationship: variable_of CO_325:0010173 ! male rachis appearance - estimation
relationship: variable_of CO_325:0100079 ! rachis appearance scale (1 to 5)

[Term]
id: CO_325:0000448
name: male bud shape
namespace: BananaTrait
def: "Shape of the male bud defined as the ratio of male bud broadest width to total male bud length" []
is_a: CO_325:1000003 ! Morphological

[Term]
id: CO_325:0000449
name: Male bud shape 1-3
namespace: BananaTrait
def: "Calculate the ratio w/y, i.e. the broadest width of the male bud to the total length of the male bud. Do not measure the dimensions along the bud but rather on a projection/outline of the bud (e.g. trace the outline of the bud on paper) and use ruler or measuring tape., 1 = skinny (w/y less than or equal to 0.45); 2 = medium (0.45 < w/y < 0.55); 3 = fat (w/y equal to or more than 0.55)" []
synonym: "MlBdShp_Comp_1to3, BUDSHP" EXACT []
is_a: CO_325:1000024 ! Variable
relationship: variable_of CO_325:0000448 ! male bud shape
relationship: variable_of CO_325:0010174 ! male bud shape - computation
relationship: variable_of CO_325:0100080 ! bud shape scale (1 to 3)

[Term]
id: CO_325:0000450
name: Male bud shape 1-5
namespace: BananaTrait
def: "Calculate the ratio w/y, i.e. the broadest width of the male bud to the total length of the male bud. Do not measure the dimensions along the bud but rather on a projection/outline of the bud (e.g. trace the outline of the bud on paper) and use ruler or measuring tape., 1 = like a top; 2 = lanceolate; 3 = intermediate; 4 = ovoid; 5 = rounded" []
synonym: "MlBdShp_Comp_1to5, BUDSH5" EXACT []
is_a: CO_325:1000024 ! Variable
relationship: variable_of CO_325:0000448 ! male bud shape
relationship: variable_of CO_325:0010174 ! male bud shape - computation
relationship: variable_of CO_325:0100081 ! bud shape scale (1 to 5)

[Term]
id: CO_325:0000451
name: male bud length
namespace: BananaTrait
def: "Length of male bud from end of rachis to apex of the bud" []
synonym: "Male bud size" EXACT []
is_a: CO_325:1000003 ! Morphological

[Term]
id: CO_325:0000452
name: Male bud length 1-3
namespace: BananaTrait
def: "Measure the length (y) of a projection/outline of the male bud on paper, with a measuring tape or ruler., 1 = short (y less than or equal to 20 cm); 2 = medium (20 cm < y < 30 cm); 3 = long (equal to or more than 30 cm)" []
synonym: "MlBdLngth_M_1to3, BUDSZE" EXACT []
is_a: CO_325:1000024 ! Variable
relationship: variable_of CO_325:0000451 ! male bud length
relationship: variable_of CO_325:0010175 ! male bud length - measurement
relationship: variable_of CO_325:0100082 ! bud length scale (1 to 3)

[Term]
id: CO_325:0000453
name: Male bud size ratio 1-3
namespace: BananaTrait
def: "Length and maximum diameter of male bud at harvest. 1 = less than or equal to 20 cm; 2 = 21-30 cm; 3 = equal to or more than 31 cm" []
synonym: "MlBdLngthRt_M_1to3," EXACT []
is_a: CO_325:1000024 ! Variable
relationship: variable_of CO_325:0000451 ! male bud length
relationship: variable_of CO_325:0010176 ! male bud size - measurement
relationship: variable_of CO_325:0100083 ! bud size scale (1 to 3)

[Term]
id: CO_325:0000454
name: male bud shoulder
namespace: BananaTrait
def: "Male bud shoulder description" []
synonym: "Male bud size" EXACT []
is_a: CO_325:1000003 ! Morphological

[Term]
id: CO_325:0000455
name: Male bud shoulder 1-3
namespace: BananaTrait
def: "Calculate the ratio w/y, i.e. the broadest width of the male bud to the total length of the male bud. Do not measure the dimensions along the bud but rather on a projection/outline of the bud (e.g. trace the outline of the bud on paper) and use ruler or measuring tape, 1 = High shouldered (x/y less than or equal to 0.28); 2 = medium shouldered (0.28 < x/y < 0.30); 3 = low shouldered (x/y more than or equal to 0.30)" []
synonym: "MlBdShd_Comp_1to3," EXACT []
is_a: CO_325:1000024 ! Variable
relationship: variable_of CO_325:0000454 ! male bud shoulder
relationship: variable_of CO_325:0010179 ! male bud shoulder - computation
relationship: variable_of CO_325:0100084 ! bud shoulder scale (1 to 3)

[Term]
id: CO_325:0000456
name: bract apex shape
namespace: BananaTrait
def: "Appearance of flowers/bracts on the male rachis" []
is_a: CO_325:1000003 ! Morphological

[Term]
id: CO_325:0000457
name: Bract apex shape 1-4
namespace: BananaTrait
def: "Refers to the first external unlifted bract. Visually observe the apex shape of flattened bracts to determine shape and choose the option that is most similar, from the 4 photos of descriptor 6.5.2. in the reference material., 1 = pointed; 2 = intermeditae; 3 = obtuse; 4 = obtuse and split" []
synonym: "FstBrctApxShp_Est_1to4," EXACT []
is_a: CO_325:1000024 ! Variable
relationship: variable_of CO_325:0000456 ! bract apex shape
relationship: variable_of CO_325:0010180 ! bract apex shape - estimation
relationship: variable_of CO_325:0100085 ! bract apex scale (1 to 4)

[Term]
id: CO_325:0000458
name: Bract apex shape 1-5
namespace: BananaTrait
def: "Refers to the first external unlifted bract. Visually observe the apex shape of flattened bracts to determine shape and choose the option that is most similar, from the 4 photos of descriptor 6.5.2. in the reference material., 1 = pointed; 2 = slightly pointed; 3 = intermediate; 4 = obtuse; 5 = obtuse and split" []
synonym: "BrctApxShp_Est_1to5, BTAPXS" EXACT []
is_a: CO_325:1000024 ! Variable
relationship: variable_of CO_325:0000456 ! bract apex shape
relationship: variable_of CO_325:0010180 ! bract apex shape - estimation
relationship: variable_of CO_325:0100086 ! bract apex scale (1 to 5)

[Term]
id: CO_325:0000459
name: bract imbrication at apex of male bud
namespace: BananaTrait
def: "Alignment of bracts at the apex of the male bud" []
synonym: "Bract imbrication" EXACT []
is_a: CO_325:1000003 ! Morphological

[Term]
id: CO_325:0000460
name: Bract imbrication at apex of male bud 1-3
namespace: BananaTrait
def: "Visually observe the bract imbrication of the apex of the male bud and choose the option that is most similar, from the 3 photos of descriptor 6.5.3 in the reference material., 1 = convolute; 2 = moderately imbricate; 3 = highly imbricate" []
synonym: "BrctImbrcApxMlBd_Est_1to3, BTIMBR" EXACT []
is_a: CO_325:1000024 ! Variable
relationship: variable_of CO_325:0000459 ! bract imbrication at apex of male bud
relationship: variable_of CO_325:0010181 ! bract imbrication at apex of male bud - estimation
relationship: variable_of CO_325:0100087 ! bract imbrication scale (1 to 3)

[Term]
id: CO_325:0000461
name: bract behaviour before falling
namespace: BananaTrait
def: "Behaviour of the last lifted bract - revolute or not revolute" []
is_a: CO_325:1000003 ! Morphological

[Term]
id: CO_325:0000462
name: Bract behaviour before falling 1-2
namespace: BananaTrait
def: "Visually observe the last bract to lift from the hands, ideally when the bract has lifted to a horizontal position, and choose the option that is most similar, from the 2 photos of descriptpr 6.5.12 in the reference material., 1 = revolute (rolling); 2 = not revolute (not rolling)" []
synonym: "BrctBhvBfFll_Est_1to2, BBBF" EXACT []
is_a: CO_325:1000024 ! Variable
relationship: variable_of CO_325:0000461 ! bract behaviour before falling
relationship: variable_of CO_325:0010182 ! bract behaviour before falling - estimation
relationship: variable_of CO_325:0100088 ! bract behaviour scale (1 to 2)

[Term]
id: CO_325:0000463
name: colour of bract external face
namespace: BananaTrait
def: "Main colour of the first external unlifted bract external face" []
synonym: "Colour of the bract external face" EXACT []
is_a: CO_325:1000003 ! Morphological

[Term]
id: CO_325:0000464
name: Colour of bract external face 1-16
namespace: BananaTrait
def: "Visually observe the colour of the external face of the first unlifted bract. Use colour chart A and observe out of direct sunlight., 1 = cream; 2 = yellow; 3 = watery green; 4 = green yellow; 5 = light green; 6 = medium green; 7 = green; 8 = dark green; 9 = whitish; 10 = orange red; 11 = red; 12 = pink-purple; 13 = purple-brown; 14 = red-purple; 15 = purple; 16 = blue" []
synonym: "BrctClExtFc_Est_1to16, CBXF16" EXACT []
is_a: CO_325:1000024 ! Variable
relationship: variable_of CO_325:0000463 ! colour of bract external face
relationship: variable_of CO_325:0010183 ! colour of bract external face - estimation
relationship: variable_of CO_325:0100063 ! bd colour chart a - 2016

[Term]
id: CO_325:0000465
name: Colour of bract external face 1-10
namespace: BananaTrait
def: "Visually observe the colour of the external face of the first unlifted bract. Use colour chart A and observe out of direct sunlight., 1 = yellow; 2 = green; 3 = red; 4 = red-purple; 5 = purple-brown; 6 = purple; 7 = blue; 8 = pink-purple; 9 = orange-red; 10 = other" []
synonym: "BrctClExtFc_Est_1to10, CBXF10" EXACT []
is_a: CO_325:1000024 ! Variable
relationship: variable_of CO_325:0000463 ! colour of bract external face
relationship: variable_of CO_325:0010183 ! colour of bract external face - estimation
relationship: variable_of CO_325:0100073 ! bd colour chart a - 1996

[Term]
id: CO_325:0000466
name: colour of bract internal face
namespace: BananaTrait
def: "Main colour of the first external unlifted bract internal face" []
synonym: "Colour of the bract internal face" EXACT []
is_a: CO_325:1000003 ! Morphological

[Term]
id: CO_325:0000467
name: Colour of bract internal face 1-16
namespace: BananaTrait
def: "Visually observe the colour of the internal face of the first unlifted bract. Use colour chart A and observe out of direct sunlight., 1 = cream; 2 = yellow; 3 = watery green; 4 = green yellow; 5 = light green; 6 = medium green; 7 = green; 8 = dark green; 9 = whitish; 10 = orange red; 11 = red; 12 = pink-purple; 13 = purple-brown; 14 = red-purple; 15 = purple; 16 = blue" []
synonym: "BrctClExtFc_Int_1to16, CBIF16" EXACT []
is_a: CO_325:1000024 ! Variable
relationship: variable_of CO_325:0000466 ! colour of bract internal face
relationship: variable_of CO_325:0010184 ! colour of bract internal face - estimation
relationship: variable_of CO_325:0100063 ! bd colour chart a - 2016

[Term]
id: CO_325:0000468
name: Colour of bract internal face 1-10
namespace: BananaTrait
def: "Visually observe the colour of the internal face of the first unlifted bract. Use colour chart A and observe out of direct sunlight., 1 = whitish; 2 = yellow or green; 3 = orange red; 4 = red; 5 = purple; 6 = purple-brown; 7 = pink-purple; 8 = other" []
synonym: "BrctClExtFc_Int_1to8, CBIF8" EXACT []
is_a: CO_325:1000024 ! Variable
relationship: variable_of CO_325:0000466 ! colour of bract internal face
relationship: variable_of CO_325:0010184 ! colour of bract internal face - estimation
relationship: variable_of CO_325:0100073 ! bd colour chart a - 1996

[Term]
id: CO_325:0000469
name: compound tepal main colour
namespace: BananaTrait
def: "Main colour of the backside of the compound tepal" []
synonym: "Tepal colour, Compound tepal basic colour" EXACT []
is_a: CO_325:1000003 ! Morphological

[Term]
id: CO_325:0000470
name: Compound tepal main colour 1-16
namespace: BananaTrait
def: "The following flower descriptors refer to the flowers at the axil of the first external unlifted bract. Fresh material must be used (make the observation as soon as you detach the bract/flower from the rachis). Visually observe the colour of the backside middle of tepal. Use colour chart B and observe out of direct sunlight., 1 = white; 2 = cream; 3 = ivory; 4 = yellow; 5 = bright yellow; 6 = orange; 7 = orange red; 8 = red; 9 = red-purple; 10 = pink/pink-purple; 11 = brown/rusty-brown; 12 = beige-pink; 13 = silvery; 14 = light green; 15 = green; 16 = dark green" []
synonym: "CmpdTplMnCl_Est_1to16, CTBC16" EXACT []
is_a: CO_325:1000024 ! Variable
relationship: variable_of CO_325:0000469 ! compound tepal main colour
relationship: variable_of CO_325:0010185 ! compound tepal main colour - estimation
relationship: variable_of CO_325:0100089 ! bd colour chart b - 2016

[Term]
id: CO_325:0000471
name: Compound tepal main colour 1-6
namespace: BananaTrait
def: "The following flower descriptors refer to the flowers at the axil of the first external unlifted bract. Fresh material must be used (make the observation as soon as you detach the bract/flower from the rachis). Visually observe the colour of the backside middle of tepal. Use colour chart B and observe out of direct sunlight., 1 =white; 2 = cream; 3 = yellow; 4 = orange; 5 = pink/pink-purple; 6 = other" []
synonym: "CmpdTplMnCl_Est_1to6, CTBC6" EXACT []
is_a: CO_325:1000024 ! Variable
relationship: variable_of CO_325:0000469 ! compound tepal main colour
relationship: variable_of CO_325:0010185 ! compound tepal main colour - estimation
relationship: variable_of CO_325:0100090 ! bd colour chart b - 1996

[Term]
id: CO_325:0000472
name: lobe colour of tip of compound tepal
namespace: BananaTrait
def: "Main colour of the tip of the compound tepal (lobe)" []
synonym: "Lobe colour, Lobe colour of compound tepal" EXACT []
is_a: CO_325:1000003 ! Morphological

[Term]
id: CO_325:0000473
name: Lobe colour of tip of compound tepal 1-16
namespace: BananaTrait
def: "The following flower descriptors refer to the flowers at the axil of the first external unlifted bract. Fresh material must be used (make the observation as soon as you detach the bract/flower from the rachis). Visually observe the colour of the lobe at the tip of the tepal. Use colour chart B and observe out of direct sunlight., 1 = white; 2 = cream; 3 = ivory; 4 = yellow; 5 = bright yellow; 6 = orange; 7 = orange red; 8 = red; 9 = red-purple; 10 = pink/pink-purple; 11 = brown/rusty-brown; 12 = beige-pink; 13 = silvery; 14 = light green; 15 = green; 16 = dark green" []
synonym: "CmpdTplLbCl_Est_1to16, LBCT16" EXACT []
is_a: CO_325:1000024 ! Variable
relationship: variable_of CO_325:0000472 ! lobe colour of tip of compound tepal
relationship: variable_of CO_325:0010186 ! lobe colour of tip of compound tepal - estimation
relationship: variable_of CO_325:0100089 ! bd colour chart b - 2016

[Term]
id: CO_325:0000474
name: Lobe colour of tip of compound tepal 1-5
namespace: BananaTrait
def: "The following flower descriptors refer to the flowers at the axil of the first external unlifted bract. Fresh material must be used (make the observation as soon as you detach the bract/flower from the rachis). Visually observe the colour of the lobe at the tip of the tepal. Use colour chart B and observe out of direct sunlight., 1 = cream; 2 = yellow; 3 = orange; 4 = green; 5 = other" []
synonym: "CmpdTplLbCl_Est_1to5, LBCOT5" EXACT []
is_a: CO_325:1000024 ! Variable
relationship: variable_of CO_325:0000472 ! lobe colour of tip of compound tepal
relationship: variable_of CO_325:0010186 ! lobe colour of tip of compound tepal - estimation
relationship: variable_of CO_325:0100090 ! bd colour chart b - 1996

[Term]
id: CO_325:0000475
name: anther colour
namespace: BananaTrait
def: "Main colour of the face of anther opposite to dehiscence" []
is_a: CO_325:1000003 ! Morphological

[Term]
id: CO_325:0000476
name: Anther colour 1-16
namespace: BananaTrait
def: "The following flower descriptors refer to the flowers at the axil of the first external unlifted bract. Fresh material must be used (make the observation as soon as you detach the bract/flower from the rachis). Visually observe the anther colour on the face opposite to the dehiscence split of the anther. Use colour chart B and observe out of direct sunlight., 1 = white; 2 = cream; 3 = ivory; 4 = yellow; 5 = bright yellow; 6 = orange; 7 = orange red; 8 = red; 9 = red-purple; 10 = pink/pink-purple; 11 = brown/rusty-brown; 12 = beige-pink; 13 = silvery; 14 = light green; 15 = green; 16 = dark green" []
synonym: "AnthrCl_Est_1to16, ANTC16" EXACT []
is_a: CO_325:1000024 ! Variable
relationship: variable_of CO_325:0000475 ! anther colour
relationship: variable_of CO_325:0010187 ! anther colour - estimation
relationship: variable_of CO_325:0100089 ! bd colour chart b - 2016

[Term]
id: CO_325:0000477
name: Anther colour 1-8
namespace: BananaTrait
def: "The following flower descriptors refer to the flowers at the axil of the first external unlifted bract. Fresh material must be used (make the observation as soon as you detach the bract/flower from the rachis). Visually observe the anther colour on the face opposite to the dehiscence split of the anther. Use colour chart B and observe out of direct sunlight., 1 = white; 2 = cream; 3 = yellow; 4 = grey; 5 = brown/rusty-brown; 6 = pink/pink-purple; 7 = black (anthers aborted); 8=other" []
synonym: "AnthrCl_Est_1to8, ANTC8" EXACT []
is_a: CO_325:1000024 ! Variable
relationship: variable_of CO_325:0000475 ! anther colour
relationship: variable_of CO_325:0010187 ! anther colour - estimation
relationship: variable_of CO_325:0100090 ! bd colour chart b - 1996

[Term]
id: CO_325:0000478
name: number of hands on whole bunch
namespace: BananaTrait
def: "Number of hands on bunch **subsume" []
synonym: "Number of hands" EXACT []
is_a: CO_325:1000003 ! Morphological

[Term]
id: CO_325:0000479
name: Number of hands on whole bunch: count
namespace: BananaTrait
def: "On a bunch with mostly hands of > 10 fingers, a possible ultimate hand with 1-5 (rather smaller) fingers should not be counted." []
synonym: "HndNbWhlBnch_Ct_hands, NUMHND" EXACT []
is_a: CO_325:1000024 ! Variable
relationship: variable_of CO_325:0000478 ! number of hands on whole bunch
relationship: variable_of CO_325:0010188 ! number of hands on whole bunch - counting
relationship: variable_of CO_325:0100091 ! hands

[Term]
id: CO_325:0000480
name: number of fruits on mid-hand of the bunch
namespace: BananaTrait
def: "Number of fruits on the mid-hand of the bunch **subsume" []
synonym: "Number of fruits" EXACT []
is_a: CO_325:1000003 ! Morphological

[Term]
id: CO_325:0000481
name: Number of fruits on mid-hand of the bunch: count
namespace: BananaTrait
def: "Count only fully developed fruit. If there is an even number of hands, there will be two middle hands. Count the middle hand that developed first., 1 = less than or equal to 12; 2 = 13-16; 3 = equal to or more than 17" []
synonym: "FrtNbMdHndBnch_Ct_ft, NUMFMH" EXACT []
is_a: CO_325:1000024 ! Variable
relationship: variable_of CO_325:0000480 ! number of fruits on mid-hand of the bunch
relationship: variable_of CO_325:0010189 ! number of fruits on mid-hand of the bunch - counting
relationship: variable_of CO_325:0100017 ! finger

[Term]
id: CO_325:0000482
name: fruit length
namespace: BananaTrait
def: "Length of the internal arc of a finger ** subsume" []
synonym: "Fruit length" EXACT []
is_a: CO_325:1000003 ! Morphological

[Term]
id: CO_325:0000483
name: Fruit length in cm
namespace: BananaTrait
def: "Measure the length of the internal arc of a fruit, without pedicel. Record on the inner fruit in the middle of the mid-hand of the bunch. If there is an even number of hands, there will be two middle hands so use the upper hand that developed first. Record the exact value. In cm" []
synonym: "FrtLngth_M_cm, FRULGT" EXACT []
is_a: CO_325:1000024 ! Variable
relationship: variable_of CO_325:0000482 ! fruit length
relationship: variable_of CO_325:0010190 ! fruit length - exact value - measurement
relationship: variable_of CO_325:0100008 ! cm

[Term]
id: CO_325:0000484
name: Fruit length 1-5
namespace: BananaTrait
def: "Measure the length of the internal arc of a fruit, without pedicel. Record on the inner fruit in the middle of the mid-hand of the bunch. If there is an even number of hands, there will be two middle hands so use the upper hand that developed first. Record the range., 1 = less than or equal to 15 cm; 2 = 16-20 cm; 3 = 21-25 cm; 4 = 26-30 cm; 5 = equal to or more than 31 cm" []
synonym: "FrtLngth_M_1to5," EXACT []
is_a: CO_325:1000024 ! Variable
relationship: variable_of CO_325:0000482 ! fruit length
relationship: variable_of CO_325:0010191 ! fruit length - range - measurement
relationship: variable_of CO_325:0100092 ! fruit length scale (1 to 5)

[Term]
id: CO_325:0000485
name: fruit shape of curve
namespace: BananaTrait
def: "Shape of a fruit (finger) in the middle of the bunch **subsume" []
synonym: "Fruit shape (longitudinal curve)" EXACT []
is_a: CO_325:1000003 ! Morphological

[Term]
id: CO_325:0000486
name: Fruit shape of curve 1-6
namespace: BananaTrait
def: "Visually observe the shape of the curve of the fruit and choose the option that is most similar, from the 5 photos of descriptor 6.7.4. in the reference material. Observe the inner fruit in the middle of the mid-hand of the bunch. In case of an asymmetric bunch that has straight and curved fruits, please indicate it in the note section and score only the fruit on the upper side of the bunch., 1 = straight; 2 = slightly curved; 3 = straight in the distal part; 4 = curved (sharp curve); 5 = curved in slight 'S' shape (double curvature)" []
synonym: "FrtCvShp_Est_1to6," EXACT []
is_a: CO_325:1000024 ! Variable
relationship: variable_of CO_325:0000485 ! fruit shape of curve
relationship: variable_of CO_325:0010192 ! fruit shape of curve - estimation
relationship: variable_of CO_325:0100093 ! fruit curve shape (scale 1 to 6)

[Term]
id: CO_325:0000487
name: Fruit shape of curve 1-5
namespace: BananaTrait
def: "Visually observe the shape of the curve of the fruit and choose the option that is most similar, from the 5 photos of descriptor 6.7.4. in the reference material. Observe the inner fruit in the middle of the mid-hand of the bunch. In case of an asymmetric bunch that has straight and curved fruits, please indicate it in the note section and score only the fruit on the upper side of the bunch., 1 = straight (or slightly curved); 2 = straight in the distal part; 3 = curved (sharp curve); 4 = curved in 'S' shape (double curvature); 5 = other" []
synonym: "FrtCvShp_Est_1to5, FRUSHP" EXACT []
is_a: CO_325:1000024 ! Variable
relationship: variable_of CO_325:0000485 ! fruit shape of curve
relationship: variable_of CO_325:0010192 ! fruit shape of curve - estimation
relationship: variable_of CO_325:0100094 ! fruit curve shape (scale 1 to 5)

[Term]
id: CO_325:0000488
name: fruit apex point
namespace: BananaTrait
def: "Description of fruit apex" []
synonym: "Fruit apex" EXACT []
is_a: CO_325:1000003 ! Morphological

[Term]
id: CO_325:0000489
name: Fruit apex point 1-5
namespace: BananaTrait
def: "Visually observe the fruit apex point and choose the option that is most similar, from the 5 photos of descriptor 6.7.6 in the reference material., 1 = pointed; 2 = lengthily pointed (like plantain); 3 = blunt-tipped (plateau at tip); 4 = strongly bottle-necked (wider under tip than number 2); 5 = rounded" []
synonym: "FrtApxPt_Est_1to5, FRAPX" EXACT []
is_a: CO_325:1000024 ! Variable
relationship: variable_of CO_325:0000488 ! fruit apex point
relationship: variable_of CO_325:0010193 ! fruit apex point - estimation
relationship: variable_of CO_325:0100095 ! fruit apex scale (1 to 5)

[Term]
id: CO_325:0000490
name: remains of flower relicts at fruit apex
namespace: BananaTrait
def: "Percentage of flower relicts at fruit apex" []
is_a: CO_325:1000003 ! Morphological

[Term]
id: CO_325:0000491
name: Remains of flower relicts at fruit apex 1-4
namespace: BananaTrait
def: "Visually observe the remains, or not, of flower relicts at the finger apex, and choose the option that is most similar, from the 4 photos of descriptor 6.7.7 in the reference materials., 1 = without flower relicts; 2 = few flower relicts (< 20% of the fruits with relicts); 3 = persistent flower relicts (> 20% of the fruits with relicts); 4 = only base of the style persists" []
synonym: "FrtApxFlwRlt_Est_1to4," EXACT []
is_a: CO_325:1000024 ! Variable
relationship: variable_of CO_325:0000490 ! remains of flower relicts at fruit apex
relationship: variable_of CO_325:0010194 ! remains of flower relicts at fruit apex - estimation
relationship: variable_of CO_325:0100096 ! fruit relicts scale (1 to 4)

[Term]
id: CO_325:0000492
name: Remains of flower relicts at fruit apex 1-3
namespace: BananaTrait
def: "Visually observe the remains, or not, of flower relicts at the finger apex, and choose the option that is most similar, from the 4 photos of descriptor 6.7.7 in the reference materials., 1 = without any floral relicts; 2 = persistent style; 3 = base of the style prominent" []
synonym: "FrtApxFlwRlt_Est_1to3, FLRCTS" EXACT []
is_a: CO_325:1000024 ! Variable
relationship: variable_of CO_325:0000490 ! remains of flower relicts at fruit apex
relationship: variable_of CO_325:0010194 ! remains of flower relicts at fruit apex - estimation
relationship: variable_of CO_325:0100097 ! fruit relicts scale (1 to 3)

[Term]
id: CO_325:0000493
name: fruit pedicel length
namespace: BananaTrait
def: "Length of the fruit pedicel from rachis to the beginning of the pulp" []
is_a: CO_325:1000003 ! Morphological

[Term]
id: CO_325:0000494
name: Fruit pedicel length in mm
namespace: BananaTrait
def: "Measure from the scar on the rachis until the beginning of the fruit. Record on the inner fruit in the middle of the mid-hand of the bunch. Tip: use string to measure or trace outline of fruit on paper. Record the exact value. In mm" []
synonym: "FrtftPdclLgth_M_mm," EXACT []
is_a: CO_325:1000024 ! Variable
relationship: variable_of CO_325:0000493 ! fruit pedicel length
relationship: variable_of CO_325:0010195 ! fruit pedicel length - exact value - measurement
relationship: variable_of CO_325:0100020 ! mm

[Term]
id: CO_325:0000495
name: Fruit pedicel length 1-3
namespace: BananaTrait
def: "Measure from the scar on the rachis until the beginning of the fruit. Record on the inner fruit in the middle of the mid-hand of the bunch. Tip: use string to measure or trace outline of fruit on paper. Record the range., 1 = less than or equal to 10 mm; 2 = 11-20 mm; 3 = equal to or more than 21 mm" []
synonym: "FrtftPdclLgth_Est_1to3, PEDLGT" EXACT []
is_a: CO_325:1000024 ! Variable
relationship: variable_of CO_325:0000493 ! fruit pedicel length
relationship: variable_of CO_325:0010196 ! fruit pedical length - range - measurement
relationship: variable_of CO_325:0100098 ! fruit pedicel scale (1 to 3)

[Term]
id: CO_325:0000496
name: fusion of pedicels
namespace: BananaTrait
def: "Degree of fusion of the pedicels before they join the rachis" []
is_a: CO_325:1000003 ! Morphological

[Term]
id: CO_325:0000497
name: Fusion of pedicels 1-2
namespace: BananaTrait
def: "Visually observe the fusion of pedicels and choose the option that is most similar, from the 3 photos of descriptor 6.7.11. in the reference materials. Observe before they join the rachis at the bract scar. Look upwards from the bottom of the bunch., 1 = no visible sign of fusion; 2 = partially fused (up to 50% of the length of the pedicel); 3 = totally fused (more than 50% of the length of the pedicel)" []
synonym: "PdcFsn_Est_1to2, FUSHPD" EXACT []
is_a: CO_325:1000024 ! Variable
relationship: variable_of CO_325:0000496 ! fusion of pedicels
relationship: variable_of CO_325:0010197 ! fusion of pedicels - estimation
relationship: variable_of CO_325:0100099 ! fusion of pedicel scale (1 to 2)

[Term]
id: CO_325:0000498
name: fruit smashed pulp colour
namespace: BananaTrait
def: "The color of the smashed pulp of a mature fruit" []
is_a: CO_325:1000006 ! Quality_traits

[Term]
id: CO_325:0000499
name: Fruit smashed pulp colour 1-5
namespace: BananaTrait
def: "Subjective visual assessment of smashed and unsmashed fruit pulp, 1 = dislike very much; 2 = dislike; 3 = like fairly; 4 = like very much; 5 = like extremely" []
synonym: "FngSmshdPlpCl_Est_1to5," EXACT []
is_a: CO_325:1000024 ! Variable
relationship: variable_of CO_325:0000498 ! fruit smashed pulp colour
relationship: variable_of CO_325:0010198 ! visual appearance - estimation
relationship: variable_of CO_325:0100100 ! 1 to 5 acceptability score

[Term]
id: CO_325:0000500
name: fruit unsmashed pulp colour
namespace: BananaTrait
def: "The color of the unsmashed pulp of a mature fruit" []
is_a: CO_325:1000006 ! Quality_traits

[Term]
id: CO_325:0000501
name: Fruit unsmashed pulp colour 1-5
namespace: BananaTrait
def: "Subjective visual assessment of smashed and unsmashed fruit pulp, 1 = dislike very much; 2 = dislike; 3 = like fairly; 4 = like very much; 5 = like extremely" []
synonym: "FngUnSmshdPlpCl_Est_1to5," EXACT []
is_a: CO_325:1000024 ! Variable
relationship: variable_of CO_325:0000500 ! fruit unsmashed pulp colour
relationship: variable_of CO_325:0010198 ! visual appearance - estimation
relationship: variable_of CO_325:0100100 ! 1 to 5 acceptability score

[Term]
id: CO_325:0000502
name: fruit smashed pulp taste
namespace: BananaTrait
def: "The taste of the smashed pulp of a mature fruit" []
is_a: CO_325:1000006 ! Quality_traits

[Term]
id: CO_325:0000503
name: Fruit smashed pulp taste 1-5
namespace: BananaTrait
def: "Subjective taste assessment of smashed and unsmashed fruit pulp, 1 = dislike very much; 2 = dislike; 3 = like fairly; 4 = like very much; 5 = like extremely" []
synonym: "FngSmshdPlpTst_Est_1to5," EXACT []
is_a: CO_325:1000024 ! Variable
relationship: variable_of CO_325:0000502 ! fruit smashed pulp taste
relationship: variable_of CO_325:0010199 ! taste - estimation
relationship: variable_of CO_325:0100100 ! 1 to 5 acceptability score

[Term]
id: CO_325:0000504
name: fruit unsmashed pulp taste
namespace: BananaTrait
def: "The taste of the unsmashed pulp of a mature fruit" []
is_a: CO_325:1000006 ! Quality_traits

[Term]
id: CO_325:0000505
name: Fruit unsmashed pulp taste 1-5
namespace: BananaTrait
def: "Subjective taste assessment of smashed and unsmashed fruit pulp, 1 = dislike very much; 2 = dislike; 3 = like fairly; 4 = like very much; 5 = like extremely" []
synonym: "FngUnSmshdPlpTst_Est_1to5," EXACT []
is_a: CO_325:1000024 ! Variable
relationship: variable_of CO_325:0000504 ! fruit unsmashed pulp taste
relationship: variable_of CO_325:0010199 ! taste - estimation
relationship: variable_of CO_325:0100100 ! 1 to 5 acceptability score

[Term]
id: CO_325:0000506
name: fruit smashed pulp texture
namespace: BananaTrait
def: "The texture of the smashed pulp of a mature fruit" []
is_a: CO_325:1000006 ! Quality_traits

[Term]
id: CO_325:0000507
name: Fruit smashed pulp texture 1-5
namespace: BananaTrait
def: "Finger feel assessment of smashed and unsmashed fruit pulp, 1 = dislike very much; 2 = dislike; 3 = like fairly; 4 = like very much; 5 = like extremely" []
synonym: "FngSmshdPlpTxt_Est_1to5," EXACT []
is_a: CO_325:1000024 ! Variable
relationship: variable_of CO_325:0000506 ! fruit smashed pulp texture
relationship: variable_of CO_325:0010200 ! finger feel - estimation
relationship: variable_of CO_325:0100100 ! 1 to 5 acceptability score

[Term]
id: CO_325:0000508
name: fruit unsmashed pulp texture
namespace: BananaTrait
def: "The texture of the unsmashed pulp of a mature fruit" []
is_a: CO_325:1000006 ! Quality_traits

[Term]
id: CO_325:0000509
name: Fruit unsmashed pulp texture 1-5
namespace: BananaTrait
def: "Finger feel assessment of smashed and unsmashed fruit pulp, 1 = dislike very much; 2 = dislike; 3 = like fairly; 4 = like very much; 5 = like extremely" []
synonym: "FngUnSmshdPlpTxt_Est_1to5," EXACT []
is_a: CO_325:1000024 ! Variable
relationship: variable_of CO_325:0000508 ! fruit unsmashed pulp texture
relationship: variable_of CO_325:0010200 ! finger feel - estimation
relationship: variable_of CO_325:0100100 ! 1 to 5 acceptability score

[Term]
id: CO_325:0000510
name: fruit smashed pulp smoothness-mouth feel
namespace: BananaTrait
def: "The smoothness-mouth feel of the smashed pulp of a mature fruit" []
is_a: CO_325:1000006 ! Quality_traits

[Term]
id: CO_325:0000511
name: Fruit smashed pulp smoothness-mouth feel 1-5
namespace: BananaTrait
def: "Mouth feel assessment of smashed and unsmashed fruit pulp, 1 = dislike very much; 2 = dislike; 3 = like fairly; 4 = like very much; 5 = like extremely" []
synonym: "FngSmshdPlpSmth_Est_1to5," EXACT []
is_a: CO_325:1000024 ! Variable
relationship: variable_of CO_325:0000510 ! fruit smashed pulp smoothness-mouth feel
relationship: variable_of CO_325:0010201 ! smoothness-mouth feel - estimation
relationship: variable_of CO_325:0100100 ! 1 to 5 acceptability score

[Term]
id: CO_325:0000512
name: fruit unsmashed pulp smoothness-mouth feel
namespace: BananaTrait
def: "The smoothness-mouth feel of the unsmashed pulp of a mature fruit" []
is_a: CO_325:1000006 ! Quality_traits

[Term]
id: CO_325:0000513
name: Fruit unsmashed pulp smoothness-mouth feel 1-5
namespace: BananaTrait
def: "Mouth feel assessment of smashed and unsmashed fruit pulp, 1 = dislike very much; 2 = dislike; 3 = like fairly; 4 = like very much; 5 = like extremely" []
synonym: "FngUnSmshdPlpSmth_Est_1to5," EXACT []
is_a: CO_325:1000024 ! Variable
relationship: variable_of CO_325:0000512 ! fruit unsmashed pulp smoothness-mouth feel
relationship: variable_of CO_325:0010201 ! smoothness-mouth feel - estimation
relationship: variable_of CO_325:0100100 ! 1 to 5 acceptability score

[Term]
id: CO_325:0000514
name: fruit smashed pulp aroma/smell
namespace: BananaTrait
def: "The pulp aroma of the smashed pulp of a mature fruit" []
is_a: CO_325:1000006 ! Quality_traits

[Term]
id: CO_325:0000515
name: Fruit smashed pulp aroma/smell 1-5
namespace: BananaTrait
def: "Nosal smell assessment of smashed and unsmashed fruit pulp aromas, 1 = dislike very much; 2 = dislike; 3 = like fairly; 4 = like very much; 5 = like extremely" []
synonym: "FngSmshdPlpArm_Est_1to5," EXACT []
is_a: CO_325:1000024 ! Variable
relationship: variable_of CO_325:0000514 ! fruit smashed pulp aroma/smell
relationship: variable_of CO_325:0010202 ! nosal smell - estimation
relationship: variable_of CO_325:0100100 ! 1 to 5 acceptability score

[Term]
id: CO_325:0000516
name: damage to periphery of peeled corm caused by weevils
namespace: BananaTrait
def: "The amount of damage to the periphery of the peeled corm, assessed by tunnels caused by weevils" []
synonym: "peripheral damage" EXACT []
is_a: CO_325:1000002 ! Biotic_stress

[Term]
id: CO_325:0000517
name: Weevils damage to periphery of peeled corm %
namespace: BananaTrait
def: "Visual observation In %" []
synonym: "DmgPrphl_M_%," EXACT []
is_a: CO_325:1000024 ! Variable
relationship: variable_of CO_325:0000516 ! damage to periphery of peeled corm caused by weevils
relationship: variable_of CO_325:0010153 ! peripheral damage - measurement
relationship: variable_of CO_325:0100046 ! %

[Term]
id: CO_325:0000518
name: nematode reproduction factor (microplot screening)
namespace: BananaTrait
def: "Nematode multiplication from single root inoculation of 50 nematodes per 8 cm length after 12 weeks" []
is_a: CO_325:1000002 ! Biotic_stress

[Term]
id: CO_325:0000519
name: Nematode reproduction factor (microplot screening) multiplication factor Numerical
namespace: BananaTrait
def: "Count from 100 ml of soil sample" []
synonym: "NmRpFctr_Ct_Nema" EXACT []
is_a: CO_325:1000024 ! Variable
relationship: variable_of CO_325:0000518 ! nematode reproduction factor (microplot screening)
relationship: variable_of CO_325:0010221 ! nematode multiplication from single root inoculation - computation
relationship: variable_of CO_325:0100108 ! multiplication factor

[Term]
id: CO_325:0000520
name: nematode population density per soil sample
namespace: BananaTrait
def: "Number of nematodes in soil" []
is_a: CO_325:1000002 ! Biotic_stress

[Term]
id: CO_325:0000521
name: Nematode population density by species in soil No. per 100ml
namespace: BananaTrait
def: "Count from 100 ml of soil sample" []
synonym: "NmNumSlWt" EXACT []
is_a: CO_325:1000024 ! Variable
relationship: variable_of CO_325:0000520 ! nematode population density per soil sample
relationship: variable_of CO_325:0010220 ! number of nematodes (unclassified spp.) per unit fresh root weight - method
relationship: variable_of CO_325:0100107 ! no. per 100ml

[Term]
id: CO_325:0000522
name: number of radopholus similis per soil sample
namespace: BananaTrait
def: "Number of Radopholus similis in soil" []
is_a: CO_325:1000002 ! Biotic_stress

[Term]
id: CO_325:0000523
name: number of helicotylenchus multicinctus per soil sample
namespace: BananaTrait
def: "Number of Helicotylenchus multicinctus in soil" []
is_a: CO_325:1000002 ! Biotic_stress

[Term]
id: CO_325:0000524
name: number of rotylenchulus spp.per soil sample
namespace: BananaTrait
def: "Number of Rotylenchulus spp.in soil" []
is_a: CO_325:1000002 ! Biotic_stress

[Term]
id: CO_325:0000525
name: Number of Rotylenchulus spp.per soil sample per 100 ml
namespace: BananaTrait
def: "Count from 100 ml of soil sample" []
synonym: "RotyNumSlWt_CompNema" EXACT []
is_a: CO_325:1000024 ! Variable
relationship: variable_of CO_325:0000524 ! number of rotylenchulus spp.per soil sample
relationship: variable_of CO_325:0010224 ! number of nematodes (rotylenchulus spp.) per unit of soil sample - method
relationship: variable_of CO_325:0100109 ! no. per 100 ml

[Term]
id: CO_325:0000526
name: number of meloidogyne spp. per soil sample
namespace: BananaTrait
def: "Number of Meloidogyne spp. in soil" []
is_a: CO_325:1000002 ! Biotic_stress

[Term]
id: CO_325:0000527
name: number of pratylenchus spp. per soil sample
namespace: BananaTrait
def: "Number of Pratylenchus spp. in soil" []
is_a: CO_325:1000002 ! Biotic_stress

[Term]
id: CO_325:0000528
name: number of hoplolaimus spp. per soil sample
namespace: BananaTrait
def: "Number of Hoplolaimus spp. in soil" []
is_a: CO_325:1000002 ! Biotic_stress

[Term]
id: CO_325:0000529
name: number of pratylenchus goodeyi per soil sample
namespace: BananaTrait
def: "Number of Pratylenchus goodeyi in soil" []
is_a: CO_325:1000002 ! Biotic_stress

[Term]
id: CO_325:0000530
name: number of pratylenchus coffeae per soil sample
namespace: BananaTrait
def: "Number of Pratylenchus coffeae in soil" []
is_a: CO_325:1000002 ! Biotic_stress

[Term]
id: CO_325:0000531
name: root nematode density
namespace: BananaTrait
def: "The number of nematode individuals per unit of fresh root weight." []
is_a: CO_325:1000002 ! Biotic_stress

[Term]
id: CO_325:0000532
name: Number of nematode per root weight
namespace: BananaTrait
def: "Collect all roots from a standard-size excavation of 20 x 20 x 20 cm extending outwards from the corm of the plant. Take only roots from the selected plant; do not include roots from adjacent plants. Carefully wash the soil from the roots with tap water. Cut the roots into 10 cm long pieces and dry with paper tissue. Take a subsample of 15 g, add 100 ml distilled water and store the roots at 4 degrees Celsius. Put the roots in 100 ml of distilled water in a kitchen blender. Macerate the roots 3 times for 10 secs (separated by 5 sec intervals). Pour the macerated suspension through 250, 106 and 40 micro-metre sieves and rinse the sieves with tap water. Using distilled water, collect in a beaker the nematodes from the 40 micro-metre sieve. Using distilled water, dilute to 200 ml the nematode suspension in a graduated cylinder. Blow air through the nematode suspension with a pipette (to homogenise the suspension). Take a subsample of 6 ml (counting dish) or 2 ml (counting slide). Count the nematodes in the counting dish (stereo microscope) or in the counting slide (light microscope). Calculate the final nematode population per unit of fresh root weight." []
synonym: "NmNumRtWt," EXACT []
is_a: CO_325:1000024 ! Variable
relationship: variable_of CO_325:0000531 ! root nematode density
relationship: variable_of CO_325:0010158 ! root nematode density - computation
relationship: variable_of CO_325:0100061 ! nematodes/unit of fresh root weight

[Term]
id: CO_325:0000533
name: number of radopholus similis per fresh root weight
namespace: BananaTrait
def: "Number of Radopholus similis in roots" []
is_a: CO_325:1000002 ! Biotic_stress

[Term]
id: CO_325:0000534
name: Number of Radopholus similis per fresh root weight per 10 g: count
namespace: BananaTrait
def: "Count from 10 g of chopped roots from the tested banana plant sample" []
synonym: "RadoNumRtWt2_Comp_Nema" EXACT []
is_a: CO_325:1000024 ! Variable
relationship: variable_of CO_325:0000533 ! number of radopholus similis per fresh root weight
relationship: variable_of CO_325:0010230 ! number of nematodes (radopholus similis ) per unit fresh root weight -method
relationship: variable_of CO_325:0100110 ! no. per 10g

[Term]
id: CO_325:0000535
name: number of meloidogyne spp. per fresh root weight
namespace: BananaTrait
def: "Number of Meloidogyne spp. in roots" []
is_a: CO_325:1000002 ! Biotic_stress

[Term]
id: CO_325:0000536
name: Number of Meloidogyne spp. per fresh root weight per 10 g: count
namespace: BananaTrait
def: "Count from 10 g of chopped roots from the tested banana plant sample" []
synonym: "MeloiNumRtWt2_Comp_Nema" EXACT []
is_a: CO_325:1000024 ! Variable
relationship: variable_of CO_325:0000535 ! number of meloidogyne spp. per fresh root weight
relationship: variable_of CO_325:0010231 ! number of nematodes (meloidogyne spp.) per unit fresh root weight -method
relationship: variable_of CO_325:0100110 ! no. per 10g

[Term]
id: CO_325:0000537
name: number of pratylenchus spp. per fresh root weight
namespace: BananaTrait
def: "Number of Pratylenchus spp. in roots" []
is_a: CO_325:1000002 ! Biotic_stress

[Term]
id: CO_325:0000538
name: Number of Pratylenchus spp. per fresh root weight per 10 g: count
namespace: BananaTrait
def: "Count from 10 g of chopped roots from the tested banana plant sample" []
synonym: "PratyNumRtWt2_Comp_Nema" EXACT []
is_a: CO_325:1000024 ! Variable
relationship: variable_of CO_325:0000537 ! number of pratylenchus spp. per fresh root weight
relationship: variable_of CO_325:0010232 ! number of nematodes (pratylenchus spp.) per unit fresh root weight -method
relationship: variable_of CO_325:0100110 ! no. per 10g

[Term]
id: CO_325:0000539
name: number of hoplolaimus spp. per fresh root weight
namespace: BananaTrait
def: "Number of Hoplolaimus spp. in roots" []
is_a: CO_325:1000002 ! Biotic_stress

[Term]
id: CO_325:0000540
name: Number of Hoplolaimus spp. per fresh root weight per 10 g: count
namespace: BananaTrait
def: "Count from 10 g of chopped roots from the tested banana plant sample" []
synonym: "HoploNumRtWt2_Comp_Nema" EXACT []
is_a: CO_325:1000024 ! Variable
relationship: variable_of CO_325:0000539 ! number of hoplolaimus spp. per fresh root weight
relationship: variable_of CO_325:0010233 ! number of nematodes (hoplolaimus spp.) per unit fresh root weight -method
relationship: variable_of CO_325:0100110 ! no. per 10g

[Term]
id: CO_325:0000541
name: number of pratylenchus goodeyi per fresh root weight
namespace: BananaTrait
def: "Number of Pratylenchus goodeyi in roots" []
is_a: CO_325:1000002 ! Biotic_stress

[Term]
id: CO_325:0000542
name: Number of Pratylenchus goodeyi per fresh root weight per 10 g: count
namespace: BananaTrait
def: "Count from 10 g of chopped roots from the tested banana plant sample" []
synonym: "PratyGooNumRtWt2_Comp_Nema" EXACT []
is_a: CO_325:1000024 ! Variable
relationship: variable_of CO_325:0000541 ! number of pratylenchus goodeyi per fresh root weight
relationship: variable_of CO_325:0010234 ! number of nematodes (pratylenchus goodeyi) per unit fresh root weight -method
relationship: variable_of CO_325:0100110 ! no. per 10g

[Term]
id: CO_325:0000543
name: number of pratylenchus coffeae per fresh root weight
namespace: BananaTrait
def: "Number of Pratylenchus coffeae in roots" []
is_a: CO_325:1000002 ! Biotic_stress

[Term]
id: CO_325:0000544
name: Number of Pratylenchus coffeae per fresh root weight per 10 g: count
namespace: BananaTrait
def: "Count from 10 g of chopped roots from the tested banana plant sample" []
synonym: "PratyCofNumRtWt2_Comp_Nema" EXACT []
is_a: CO_325:1000024 ! Variable
relationship: variable_of CO_325:0000543 ! number of pratylenchus coffeae per fresh root weight
relationship: variable_of CO_325:0010235 ! number of nematodes (pratylenchus coffeae) per unit fresh root weight -method
relationship: variable_of CO_325:0100110 ! no. per 10g

[Term]
id: CO_325:0000548
name: rank of oldest standing leaf
namespace: BananaTrait
def: "The rank (order) of the oldest (most-distal) standing leaf (with an erect petiole)." []
is_a: CO_325:1000002 ! Biotic_stress

[Term]
id: CO_325:0000549
name: Rank of oldest standing leaf: count
namespace: BananaTrait
def: "Record the rank (order) of the oldest standing leaf (with an erect petiole), counting the rank by starting with the youngest completely unrolled leaf as 1 and moving downwards, associating the data with the Date of data collection." []
synonym: "OdStdLfRk_Ct_leaf," EXACT []
is_a: CO_325:1000024 ! Variable
relationship: variable_of CO_325:0000548 ! rank of oldest standing leaf
relationship: variable_of CO_325:0010108 ! rank of oldest standing leaf - counting
relationship: variable_of CO_325:0100004 ! leaf rank

[Term]
id: CO_325:0000559
name: extent of internal discolouration in corm of plant caused by fusarium wilt
namespace: BananaTrait
def: "The extent of discolouration in the corm of the plant, caused by Fusarium wilt." []
is_a: CO_325:1000002 ! Biotic_stress

[Term]
id: CO_325:0000560
name: Extent of internal discolouration in corm of plant caused by Fusarium wilt in cm
namespace: BananaTrait
def: "The extent to which vascular discolouration extends up the pseudostem should be determined by making cross-section cuts, from the base of the pseudostem upwards, and examining the internal tissues following each cut. The point at which discolouration is no longer visible should be noted and the distance from this point to the pseudostem base recorded. In cm" []
synonym: "CrmIntDiscFW_Est_1to5," EXACT []
is_a: CO_325:1000024 ! Variable
relationship: variable_of CO_325:0000559 ! extent of internal discolouration in corm of plant caused by fusarium wilt
relationship: variable_of CO_325:0010124 ! extent of internal discolouration in corm of plant caused by fusarium wilt - estimation
relationship: variable_of CO_325:0100008 ! cm

[Term]
id: CO_325:0000564
name: rank of marked youngest leaf
namespace: BananaTrait
def: "The rank (position) of the youngest completely unrolled leaf." []
synonym: "rankyoungleaf" EXACT []
is_a: CO_325:1000001 ! Agronomical

[Term]
id: CO_325:0000565
name: Rank of marked youngest leaf (value1)
namespace: BananaTrait
def: "Mark the youngest completely unrolled leaf and record its rank, which is always 1. Associate the data with the Date of data collection. In leaf rank format" []
synonym: "RkYgstLf_Comp_leafrank, rankyoungleaf" EXACT []
is_a: CO_325:1000024 ! Variable
relationship: variable_of CO_325:0000564 ! rank of marked youngest leaf
relationship: variable_of CO_325:0010018 ! rank of marked youngest leaf - counting
relationship: variable_of CO_325:0100004 ! leaf rank

[Term]
id: CO_325:0000566
name: Rank of previously marked leaf
namespace: BananaTrait
def: "The current rank (position) of the leaf that was previously marked as the youngest leaf at the time of the last data collection event." []
synonym: "rankprevleaf" EXACT []
is_a: CO_325:1000001 ! Agronomical

[Term]
id: CO_325:0000567
name: Rank of previously marked leaf 1 to 30
namespace: BananaTrait
def: "Record the rank of the previously marked leaf (the leaf that was marked in the Rank of marked youngest leaf during the last data collection), counting the leaf rank by starting with the newest completely unrolled leaf as 1 and moving downwards. Associate the data with the Date of data collection." []
synonym: "RkPvsMktLf_Comp_leafrank, rankprevleaf" EXACT []
is_a: CO_325:1000024 ! Variable
relationship: variable_of CO_325:0000566 ! Rank of previously marked leaf
relationship: variable_of CO_325:0010019 ! rank of previously marked leaf - counting
relationship: variable_of CO_325:0100004 ! leaf rank

[Term]
id: CO_325:0000568
name: Monthly Leaf emission rate in leaves/month
namespace: BananaTrait
def: "Calculate as: the Rank of previously marked leaf at one point in time, minus 1 (equivalent to the Rank of marked youngest leaf), divided by the time elapsed between the two Date of data collection events when the marked leaf was recorded as 1) the Rank of marked youngest leaf and 2) the Rank of previously marked leaf, e.g. (4 - 1) / 1 month = LER of 3 leaves/month during a particular time period." []
synonym: "LfEmRate_Comp_LfMth, LER_month" EXACT []
is_a: CO_325:1000024 ! Variable
relationship: variable_of CO_325:0000021 ! monthly leaf emission rate
relationship: variable_of CO_325:0010020 ! monthly leaf emission rate - computation
relationship: variable_of CO_325:0100005 ! leaves/month

[Term]
id: CO_325:0000569
name: Number of functional leaves: count
namespace: BananaTrait
def: "Count how many functional leaves (leaves that have 50% or more of their surface as green, healthy, photosynthetic tissue) are on the plant." []
synonym: "FnctLeav_Ct_Leaf, NUMFFH, functleaves" EXACT []
is_a: CO_325:1000024 ! Variable
relationship: variable_of CO_325:0000066 ! number of functional leaves
relationship: variable_of CO_325:0010022 ! number of functional leaves - counting
relationship: variable_of CO_325:0100007 ! leaf

[Term]
id: CO_325:0000570
name: time from planting to first youngest leaf spotted
namespace: BananaTrait
def: "Time elapsed between planting and the appearance of the first youngest leaf spotted." []
is_a: CO_325:1000002 ! Biotic_stress

[Term]
id: CO_325:0000571
name: Time from planting to first youngest leaf spotted in days
namespace: BananaTrait
def: "Calculate as: the time elapsed between the Date of planting and the Date of first youngest leaf spotted, e.g. 24/06/2014 - 24/01/2014 = 151 days." []
synonym: "PltFstLfSptd_Ct_leaf," EXACT []
is_a: CO_325:1000024 ! Variable
relationship: variable_of CO_325:0000570 ! time from planting to first youngest leaf spotted
relationship: variable_of CO_325:0010104 ! time from planting to first youngest spotted leaf - computation
relationship: variable_of CO_325:0100003 ! day

[Term]
id: CO_325:0000572
name: number of spotted leaves
namespace: BananaTrait
def: "The number of leaves with at least 10 discrete, mature, necrotic lesions or one large necrotic area with 10 light-coloured dry centres, caused by black leaf streak disease." []
synonym: "Number and severity of spotted leaves" EXACT []
is_a: CO_325:1000002 ! Biotic_stress

[Term]
id: CO_325:0000573
name: Number of spotted leaves: count
namespace: BananaTrait
def: "Count how many of the standing leaves are spotted (with at least 10 discrete, mature, necrotic lesions or one large necrotic area with 10 light-coloured dry centres), considering all leaves in between and inclusive of, the youngest leaf and the oldest standing leaf." []
synonym: "SptLfNb_Ct_leaf," EXACT []
is_a: CO_325:1000024 ! Variable
relationship: variable_of CO_325:0000572 ! number of spotted leaves
relationship: variable_of CO_325:0010105 ! number of spotted leaves - counting
relationship: variable_of CO_325:0100007 ! leaf

[Term]
id: CO_325:0000574
name: black leaf streak disease severity and stage
namespace: BananaTrait
def: "An indication of the extent of damage on an individual leaf caused by black leaf streak disease." []
synonym: "Black Sigatoka disease severity; Percentage area necrotic" EXACT []
synonym: "BLS" EXACT []
is_a: CO_325:1000002 ! Biotic_stress

[Term]
id: CO_325:0000575
name: Black Sigatoka disease severity Pct
namespace: BananaTrait
def: "Visually observe and record the amount of the surface area of a standing leaf (if measured in the field) or a leaf sample (if measured in the lab) that is affected by black leaf streak disease. In %" []
synonym: "BlkLfStrkSvrt_Est_pct, BLS_pct" EXACT []
is_a: CO_325:1000024 ! Variable
relationship: variable_of CO_325:0000574 ! black leaf streak disease severity and stage
relationship: variable_of CO_325:0010110 ! black leaf streak disease severity - estimation
relationship: variable_of CO_325:0100046 ! %

[Term]
id: CO_325:0000576
name: Black Sigatoka disease severity Gauhl
namespace: BananaTrait
def: "Visually observe and record the amount of the surface area of a standing leaf that is affected by black leaf streak disease., 0 = no symptoms; 1 = less than 1% of lamina with symptoms, only streaks and/or up to 10 spots; 2 = 1-5% of lamina with symptoms; 3 = 6-15% of lamina with symptoms; 4 = 16-33% of lamina with symptoms; 5 = 34-50% of lamina with symptoms; 6 = 51-100% of lamina with symptoms" []
synonym: "BlkLfStrkStg_Est_Gauhl, BLS_Gaulh" EXACT []
is_a: CO_325:1000024 ! Variable
relationship: variable_of CO_325:0000574 ! black leaf streak disease severity and stage
relationship: variable_of CO_325:0010110 ! black leaf streak disease severity - estimation
relationship: variable_of CO_325:0100047 ! gauhl's modification of stover's severity scoring system (yyyy)

[Term]
id: CO_325:0000577
name: Black Sigatoka disease stage Foure
namespace: BananaTrait
def: "Visually observe and record the amount of the surface area of a standing leaf that is affected by black leaf streak disease., 1 = Stage 1 appears as a small depigmentation spot whose whitish or yellow colour resembles stage 1 of Yellow Sigatoka disease. These symptoms are not visible in transmitted light and can be observed only on the underside of the leaf.; 2 = Stage 2 appears as a stripe, generally brown in colour and visible on the underside of the leaf; later the symptom also appears on the upper part of the limb as a stripe, the yellow colour of which resembles the stripe at stage 1 of Yellow Sigatoka. The colour of this stripe will change progressively from brown and later to black on the upper side of the limb, but will retain the brown colour on the underside.; 3 = Stage 3 differs from the previous one by its dimensions. The stripe becomes longer, is enlarged and in certain conditions (weak inoculum and unfavourable climatic conditions) can reach 2 or 3 cm.; 4 = Stage 4 appears on the underside as a brown spot and on the upper side as a black spot.; 5 = Stage 5 is when the elliptical spot is totally black and has spread to the underside of the limb. It is surrounded by a yellow halo with the centre beginning to flatten out.; 6 = Stage 6 is when the centre of the spot dries out, turns clear gray and is surrounded by a well-defined black ring, which is, in turn, surrounded by a bright yellow halo. These spots remain visible after the leaf has dried out because the ring persists." []
synonym: "BlkLfStrkStg_Est_Foure, BLS_Foure" EXACT []
is_a: CO_325:1000024 ! Variable
relationship: variable_of CO_325:0000574 ! black leaf streak disease severity and stage
relationship: variable_of CO_325:0010110 ! black leaf streak disease severity - estimation
relationship: variable_of CO_325:0100048 ! Foure's stages of development of bls disease scale (1987)

[Term]
id: CO_325:0000578
name: Black Sigatoka disease stage MedLaw cpl
namespace: BananaTrait
def: "Visually observe and record the amount of the surface area of a standing leaf that is affected by black leaf streak disease., 1 = Initial speck stage: symptoms are first visible to the naked eye as faint, minute (less than 0.25 mm diam), reddish brown specks on the lower surface of the leaf. Specks are often most abundant near the margin of the left side of the leaf, particularly towards the tip. Where leaf spot is severe, specks have been observed on the second leaf of plants that have not yet produced a bunch. Elsewhere they usually appear on the third, fourth, or older leaves.; 2 = First streak stage: the initial speck elongates, becoming slightly wider, to form a characteristic narrow, reddish brown streak up to 20 mm long and 2.0 mm wide, with the long axis parallel to the leaf venation. At this stage, streaks are more clearly visible on the lower surface of the leaf than on the upper one. The distribution of streaks is variable. Sometimes they are most numerous near the edge of the left side of the leaf. At other times they are equally numerous on both sides of the leaf, and more or less evenly distributed. Frequently they are densely aggregated in a band several cm wide on one side or both sides of the mid-rib, becoming less numerous towards the edge of the leaf. Streaks may be so numerous that every cm2 of leaf surface bears one or more. There is considerable variation in the length of individual streaks on a given leaf, and they frequently overlap to form larger, compound streaks.; 3 = Second-streak stage: the streaks may elongate slightly, but the most notable change is that in colour from reddish brown to dark brown or almost black, sometimes with a purplish tinge. The streak is now clearly visible on the upper surface of the leaf. The distribution of streaks at this stage of development varies in the same way as mentioned above. When streaks are very numerous, and more or less evenly distributed, the entire leaf blackens.; 4 = First-spot stage: the streak broadens and becomes more or less fusiform and elliptical in outline and similar to the 'first-spot stage' of Sigatoka (Leach 1946). The transition from streak to spot is further characterised by the development of a light brown, water-soaked border around the spot. This water-soaked effect is especially clear in the early morning, when dew is still present on the leaf, or after rain.; 5 = Second-spot stage: the dark brown or black central area of the spot becomes slightly depressed and the water-soaked border becomes more pronounced due to darkening. At this stage, a slight yellowing of the leaf tissue immediately surrounding the water-soaked border may occur.; 6 = Third or mature spot stage: the centre of the spot dries out, becoming light grey or buff-coloured, and further depressed. The spot is surrounded by a narrow, well-defined, dark brown or black border. between the latter and the normal green colour of the leaf, there is often a bright yellow transitional zone. After the leaf has collapsed and withered, spots remain clearly visible because of the light-coloured centre and dark border." []
synonym: "BlkLfStrkSvrt_Est_MedLawCpt, BLS_MedLaw_cpt" EXACT []
is_a: CO_325:1000024 ! Variable
relationship: variable_of CO_325:0000574 ! black leaf streak disease severity and stage
relationship: variable_of CO_325:0010110 ! black leaf streak disease severity - estimation
relationship: variable_of CO_325:0100049 ! meredith & lawrence (1969) - complete

[Term]
id: CO_325:0000579
name: Black Sigatoka disease stage MedLaw cnd
namespace: BananaTrait
def: "Visually observe and record the amount of the surface area of a standing leaf that is affected by black leaf streak disease., 1 = Initial speck stage: faint, minute, reddish-brown specks on the lower surface of the leaf.; 2 = First streak stage: specks elongate, becoming slightly wider to form narrow reddish-brown streaks.; 3 = Second-streak stage: streaks change colour from reddish brown to dark brown or black, sometimes with a purplish tinge, clearly visible at the upper surface of the leaf.; 4 = First-spot stage: the streaks broaden and become more or less fusiform or elliptical in outline and a water soaked border appears around each lesion.; 5 = Second-spot stage: the dark brown or black centre of each lesion becomes slightly depressed and water soaked border becomes more pronounced.; 6 = Third or mature spot stage: the centres of the lesions dry out becoming light grey or buff coloured and a bright yellow transitional zone appears between them and the normal green colour of the leaf. The lesions remain clearly visible after the leaf has collapsed or withered because of their light coloured centre and dark border." []
synonym: "BlkLfStrkStg_Est_MedLawCdsd, BLS_MedLaw_cds" EXACT []
is_a: CO_325:1000024 ! Variable
relationship: variable_of CO_325:0000574 ! black leaf streak disease severity and stage
relationship: variable_of CO_325:0010110 ! black leaf streak disease severity - estimation
relationship: variable_of CO_325:0100050 ! meredith & lawrence (1969) - condensed

[Term]
id: CO_325:0000580
name: number of leaves with black leaf streak disease severity grade 0
namespace: BananaTrait
def: "The number of leaves on a plant with a black leaf streak disease severity grade of 0." []
synonym: "Number of leaves with black Sigatoka disease severity grade 0" EXACT []
is_a: CO_325:1000002 ! Biotic_stress

[Term]
id: CO_325:0000581
name: Number of leaves with black Sigatoka disease severity grade 0
namespace: BananaTrait
def: "Calculate as: the sum of values with a Black leaf streak disease severity grade of 0." []
synonym: "BlkLfStrkSvrtLfNb_Ct_grd0," EXACT []
is_a: CO_325:1000024 ! Variable
relationship: variable_of CO_325:0000580 ! number of leaves with black leaf streak disease severity grade 0
relationship: variable_of CO_325:0010111 ! number of leaves with black leaf streak disease severity grade 0 - computation
relationship: variable_of CO_325:0100007 ! leaf

[Term]
id: CO_325:0000582
name: number of leaves with black leaf streak disease severity grade 1
namespace: BananaTrait
def: "The number of leaves on a plant with a black leaf streak disease severity grade of 1." []
synonym: "Number of leaves with black Sigatoka disease severity grade 1" EXACT []
is_a: CO_325:1000002 ! Biotic_stress

[Term]
id: CO_325:0000583
name: Number of leaves with black Sigatoka disease severity grade 1
namespace: BananaTrait
def: "Calculate as: the sum of values with a Black leaf streak disease severity grade of 1." []
synonym: "BlkLfStrkSvrtLfNb_Ct_grd1," EXACT []
is_a: CO_325:1000024 ! Variable
relationship: variable_of CO_325:0000582 ! number of leaves with black leaf streak disease severity grade 1
relationship: variable_of CO_325:0010112 ! number of leaves with black leaf streak disease severity grade 1 - computation
relationship: variable_of CO_325:0100007 ! leaf

[Term]
id: CO_325:0000584
name: number of leaves with black leaf streak disease severity grade 2
namespace: BananaTrait
def: "The number of leaves on a plant with a black leaf streak disease severity grade of 2." []
synonym: "Number of leaves with black Sigatoka disease severity grade 2" EXACT []
is_a: CO_325:1000002 ! Biotic_stress

[Term]
id: CO_325:0000585
name: Number of leaves with black Sigatoka disease severity grade 2
namespace: BananaTrait
def: "Calculate as: the sum of values with a Black leaf streak disease severity grade of 2." []
synonym: "BlkLfStrkSvrtLfNb_Ct_grd2," EXACT []
is_a: CO_325:1000024 ! Variable
relationship: variable_of CO_325:0000584 ! number of leaves with black leaf streak disease severity grade 2
relationship: variable_of CO_325:0010113 ! number of leaves with black leaf streak disease severity grade 2 - computation
relationship: variable_of CO_325:0100007 ! leaf

[Term]
id: CO_325:0000586
name: number of leaves with black leaf streak disease severity grade 3
namespace: BananaTrait
def: "The number of leaves on a plant with a black leaf streak disease severity grade of 3." []
synonym: "Number of leaves with black Sigatoka disease severity grade 3" EXACT []
is_a: CO_325:1000002 ! Biotic_stress

[Term]
id: CO_325:0000587
name: Number of leaves with black Sigatoka disease severity grade 3
namespace: BananaTrait
def: "Calculate as: the sum of values with a Black leaf streak disease severity grade of 3." []
synonym: "BlkLfStrkSvrtLfNb_Ct_grd3," EXACT []
is_a: CO_325:1000024 ! Variable
relationship: variable_of CO_325:0000586 ! number of leaves with black leaf streak disease severity grade 3
relationship: variable_of CO_325:0010114 ! number of leaves with black leaf streak disease severity grade 3 - computation
relationship: variable_of CO_325:0100007 ! leaf

[Term]
id: CO_325:0000588
name: number of leaves with black leaf streak disease severity grade 4
namespace: BananaTrait
def: "The number of leaves on a plant with a black leaf streak disease severity grade of 4." []
synonym: "Number of leaves with black Sigatoka disease severity grade 4" EXACT []
is_a: CO_325:1000002 ! Biotic_stress

[Term]
id: CO_325:0000589
name: Number of leaves with black Sigatoka disease severity grade 4
namespace: BananaTrait
def: "Calculate as: the sum of values with a Black leaf streak disease severity grade of 4." []
synonym: "BlkLfStrkSvrtLfNb_Ct_grd4," EXACT []
is_a: CO_325:1000024 ! Variable
relationship: variable_of CO_325:0000588 ! number of leaves with black leaf streak disease severity grade 4
relationship: variable_of CO_325:0010115 ! number of leaves with black leaf streak disease severity grade 4 - computation
relationship: variable_of CO_325:0100007 ! leaf

[Term]
id: CO_325:0000590
name: number of leaves with black leaf streak disease severity grade 5
namespace: BananaTrait
def: "The number of leaves on a plant with a black leaf streak disease severity grade of 5." []
synonym: "Number of leaves with black Sigatoka disease severity grade 5" EXACT []
is_a: CO_325:1000002 ! Biotic_stress

[Term]
id: CO_325:0000591
name: Number of leaves with black Sigatoka disease severity grade 5
namespace: BananaTrait
def: "Calculate as: the sum of values with a Black leaf streak disease severity grade of 5." []
synonym: "BlkLfStrkSvrtLfNb_Ct_grd5," EXACT []
is_a: CO_325:1000024 ! Variable
relationship: variable_of CO_325:0000590 ! number of leaves with black leaf streak disease severity grade 5
relationship: variable_of CO_325:0010116 ! number of leaves with black leaf streak disease severity grade 5 - computation
relationship: variable_of CO_325:0100007 ! leaf

[Term]
id: CO_325:0000592
name: number of leaves with black leaf streak disease severity grade 6
namespace: BananaTrait
def: "The number of leaves on a plant with a black leaf streak disease severity grade of 6." []
synonym: "Number of leaves with black Sigatoka disease severity grade 6" EXACT []
is_a: CO_325:1000002 ! Biotic_stress

[Term]
id: CO_325:0000593
name: Number of leaves with black Sigatoka disease severity grade 6
namespace: BananaTrait
def: "Calculate as: the sum of values with a Black leaf streak disease severity grade of 6." []
synonym: "BlkLfStrkSvrtLfNb_Ct_grd6," EXACT []
is_a: CO_325:1000024 ! Variable
relationship: variable_of CO_325:0000592 ! number of leaves with black leaf streak disease severity grade 6
relationship: variable_of CO_325:0010117 ! number of leaves with black leaf streak disease severity grade 6 - computation
relationship: variable_of CO_325:0100007 ! leaf

[Term]
id: CO_325:0000594
name: distance of internal discolouration in pseudostem of tallest sucker caused by fusarium wilt
namespace: BananaTrait
def: "The distance of discolouration in the pseudostem of the tallest sucker, caused by Fusarium wilt." []
is_a: CO_325:1000002 ! Biotic_stress

[Term]
id: CO_325:0000595
name: Fusarium wilt internal discolouration of pseudostem tallest sucker 1-6
namespace: BananaTrait
def: "For the tallest sucker, the complete corm should be removed from the soil, the roots cut off and excess soil removed. Cross-sections of the corm should be cut (using a guillotine or other suitable device) to obtain five slices of equal thickness. The upper surface of each cut section should be examined and visually evaluate the extent of the vascular discolouration., 1 = corm completely clean, no vascular discolouration; 2 = isolated points of discolouration in vascular tissue; 3 = discolouration of up to one-third of vascular tissue; 4 = discolouration of between one-third and two-thirds of vascular tissue; 5 = discolouration greater than two-thirds of vascular tissue; 6 = total discolouration of vascular tissue" []
synonym: "CrmDiscDistTlstSckFW_M_cm," EXACT []
is_a: CO_325:1000024 ! Variable
relationship: variable_of CO_325:0000594 ! distance of internal discolouration in pseudostem of tallest sucker caused by fusarium wilt
relationship: variable_of CO_325:0010127 ! distance of internal discolouration in pseudostem of tallest sucker caused by fusarium wilt
relationship: variable_of CO_325:0100052 ! 5 pt corm discolouration scale

[Term]
id: CO_325:0000596
name: Fusarium wilt yellowing leaves 0-1
namespace: BananaTrait
def: "Visual assessment., 0 = absent; 1 = present" []
synonym: "YellowPres_Est_0or1, YL_0-1" EXACT []
is_a: CO_325:1000024 ! Variable
relationship: variable_of CO_325:0000087 ! presence of yellowing leaves caused by fusarium wilt
relationship: variable_of CO_325:0010128 ! presence of yellowing leaves caused by fusarium wilt - estimation
relationship: variable_of CO_325:0100053 ! presence absence 0

[Term]
id: CO_325:0000597
name: Fusarium wilt splitting pseudostem 0-1
namespace: BananaTrait
def: "Visual assessment., 0 = absent; 1 = present" []
synonym: "PStmSplitPres_Est_0or1, SP_0-1" EXACT []
is_a: CO_325:1000024 ! Variable
relationship: variable_of CO_325:0000090 ! presence of splitting pseudostem base caused by fusarium wilt
relationship: variable_of CO_325:0010129 ! presence of splitting pseudostem base caused by fusarium wilt - estimation
relationship: variable_of CO_325:0100053 ! presence absence 0

[Term]
id: CO_325:0000598
name: Presence of changes in new leaves caused by Fusarium wilt 0-1
namespace: BananaTrait
def: "Visual assessment., 0 = absent; 1 = present" []
synonym: "LfChgPres_Est_0or1, CNL_0-1" EXACT []
is_a: CO_325:1000024 ! Variable
relationship: variable_of CO_325:0000093 ! presence of changes in new leaves caused by fusarium wilt
relationship: variable_of CO_325:0010130 ! presence of changes in new leaves caused by fusarium wilt - estimation
relationship: variable_of CO_325:0100053 ! presence absence 0

[Term]
id: CO_325:0000599
name: Presence of petiole collapse caused by Fusarium wilt 0-1
namespace: BananaTrait
def: "Visual assessment., 0 = absent; 1 = present" []
synonym: "PetColpPres_Est_0or1, PC_0-1" EXACT []
is_a: CO_325:1000024 ! Variable
relationship: variable_of CO_325:0000096 ! presence of petiole collapse caused by fusarium wilt
relationship: variable_of CO_325:0010131 ! presence of petiole collapse caused by fusarium wilt - estimation
relationship: variable_of CO_325:0100053 ! presence absence 0

[Term]
id: CO_325:0000600
name: percentage of plants with yellowing leaves caused by fusarium wilt
namespace: BananaTrait
def: "Percentage of plants with yellowing leaves, caused by Fusarium wilt." []
is_a: CO_325:1000002 ! Biotic_stress

[Term]
id: CO_325:0000601
name: Percentage of plants with yellowing leaves caused by Fusarium wilt: calculation
namespace: BananaTrait
def: "Calculate as: the sum of the number of values for Presence of yellowing leaves caused by Fusarium wilt scored as Present, divided by the Number of plants planted, multiplied by 100, e.g. 78 / 300 * 100 = 26%. In %" []
synonym: "YlLfPercFW_Comp_pct," EXACT []
is_a: CO_325:1000024 ! Variable
relationship: variable_of CO_325:0000600 ! percentage of plants with yellowing leaves caused by fusarium wilt
relationship: variable_of CO_325:0010134 ! percentage of plants with yellowing leaves caused by fusarium wilt - computation
relationship: variable_of CO_325:0100046 ! %

[Term]
id: CO_325:0000602
name: percentage of plants with a splitting pseudostem base caused by fusarium wilt
namespace: BananaTrait
def: "Percentage of plants with a splitting pseudostem base, caused by Fusarium wilt." []
is_a: CO_325:1000002 ! Biotic_stress

[Term]
id: CO_325:0000603
name: Percentage of plants with a splitting pseudostem base caused by Fusarium wilt: calculation
namespace: BananaTrait
def: "Calculate as: the sum of the number of values for Presence of splitting pseudostem base caused by Fusarium wilt scored as Present, divided by the Number of plants planted, multiplied by 100, e.g. 24 / 300 * 100 = 8%. In %" []
synonym: "SptPsdStmPercFW_Comp_pct," EXACT []
is_a: CO_325:1000024 ! Variable
relationship: variable_of CO_325:0000602 ! percentage of plants with a splitting pseudostem base caused by fusarium wilt
relationship: variable_of CO_325:0010135 ! percentage of plants with a splitting pseudostem base caused by fusarium wilt - computation
relationship: variable_of CO_325:0100046 ! %

[Term]
id: CO_325:0000604
name: percentage of plants with changes in new leaves caused by fusarium wilt
namespace: BananaTrait
def: "Percentage of plants with changes in new leaves, caused by Fusarium wilt." []
is_a: CO_325:1000002 ! Biotic_stress

[Term]
id: CO_325:0000605
name: Percentage of plants with changes in new leaves caused by Fusarium wilt: calculation
namespace: BananaTrait
def: "Calculate as: the sum of the number of values for Presence of changes in new leaves caused by Fusarium wilt scored as Present, divided by the Number of plants planted, multiplied by 100, e.g. 67 / 300 * 100 = 22%. In %" []
synonym: "ChgNwLfPercFW_Comp_pct," EXACT []
is_a: CO_325:1000024 ! Variable
relationship: variable_of CO_325:0000604 ! percentage of plants with changes in new leaves caused by fusarium wilt
relationship: variable_of CO_325:0010136 ! percentage of plants with changes in new leaves caused by fusarium wilt - computation
relationship: variable_of CO_325:0100046 ! %

[Term]
id: CO_325:0000606
name: percentage of plants with petiole collapse caused by fusarium wilt
namespace: BananaTrait
def: "Percentage of plants with petiole collapse, caused by Fusarium wilt." []
is_a: CO_325:1000002 ! Biotic_stress

[Term]
id: CO_325:0000607
name: Percentage of plants with petiole collapse caused by Fusarium wilt: calculation
namespace: BananaTrait
def: "Calculate as: the sum of the number of values for Presence of petiole collapse caused by Fusarium wilt scored as Present, divided by the Number of plants planted, multiplied by 100, e.g. 84 / 300 * 100 = 28%. In %" []
synonym: "PtlClpFW_Comp_pct," EXACT []
is_a: CO_325:1000024 ! Variable
relationship: variable_of CO_325:0000606 ! percentage of plants with petiole collapse caused by fusarium wilt
relationship: variable_of CO_325:0010137 ! percentage of plants with petiole collapse caused by fusarium wilt - computation
relationship: variable_of CO_325:0100046 ! %

[Term]
id: CO_325:0000610
name: number of banana weevil adults per trap
namespace: BananaTrait
def: "How many banana weevil adults caught per trap." []
is_a: CO_325:1000002 ! Biotic_stress

[Term]
id: CO_325:0000611
name: Number of adult weevils per trap
namespace: BananaTrait
def: "Visual counting method of Weevils per trap (the trap should be minimum 30 cm long)" []
synonym: "WvlAdltPrTrp_Ct_weevil," EXACT []
is_a: CO_325:1000024 ! Variable
relationship: variable_of CO_325:0000610 ! number of banana weevil adults per trap
relationship: variable_of CO_325:0010145 ! number of adult weevils - counting
relationship: variable_of CO_325:0100055 ! weevil

[Term]
id: CO_325:0000612
name: number of banana weevil traps used
namespace: BananaTrait
def: "How many banana weevil traps used." []
is_a: CO_325:1000002 ! Biotic_stress

[Term]
id: CO_325:0000613
name: Number of weevils traps used
namespace: BananaTrait
def: "Visual counting method of Weevil traps (the trap should be minimum 30 cm long)." []
synonym: "TrpNum_Ct_weeviltrap," EXACT []
is_a: CO_325:1000024 ! Variable
relationship: variable_of CO_325:0000612 ! number of banana weevil traps used
relationship: variable_of CO_325:0010144 ! number of adult weevil trap - counting
relationship: variable_of CO_325:0100055 ! weevil

[Term]
id: CO_325:0000614
name: average number of banana weevil adults per trap
namespace: BananaTrait
def: "The average of how many adult banana weevils caught per trap." []
is_a: CO_325:1000002 ! Biotic_stress

[Term]
id: CO_325:0000615
name: Average number of adult weevils per trap per mat
namespace: BananaTrait
def: "Average visual counting method of Weevils per trap (the trap should be minimum 30 cm long) on the number of traps" []
synonym: "WvlAdlt_Ct_weevil," EXACT []
is_a: CO_325:1000024 ! Variable
relationship: variable_of CO_325:0000614 ! average number of banana weevil adults per trap
relationship: variable_of CO_325:0010145 ! number of adult weevils - counting
relationship: variable_of CO_325:0100055 ! weevil

[Term]
id: CO_325:0000616
name: number of banana weevil larvae per trap
namespace: BananaTrait
def: "How many banana weevil larvae caught per trap." []
is_a: CO_325:1000002 ! Biotic_stress

[Term]
id: CO_325:0000617
name: Number of weevil larvae per trap
namespace: BananaTrait
def: "Visual counting method" []
synonym: "WvlLvPrTrp_Ct_weevil," EXACT []
is_a: CO_325:1000024 ! Variable
relationship: variable_of CO_325:0000616 ! number of banana weevil larvae per trap
relationship: variable_of CO_325:0010146 ! number of weevil larvae - counting
relationship: variable_of CO_325:0100055 ! weevil

[Term]
id: CO_325:0000618
name: average number of banana weevil larvae per trap
namespace: BananaTrait
def: "The average of how many banana weevil larvae caught per trap." []
is_a: CO_325:1000002 ! Biotic_stress

[Term]
id: CO_325:0000619
name: Average number of weevil larvae per mat
namespace: BananaTrait
def: "Visual counting method" []
synonym: "WvlLv_Ct_weevil," EXACT []
is_a: CO_325:1000024 ! Variable
relationship: variable_of CO_325:0000618 ! average number of banana weevil larvae per trap
relationship: variable_of CO_325:0010146 ! number of weevil larvae - counting
relationship: variable_of CO_325:0100055 ! weevil

[Term]
id: CO_325:0000620
name: number of banana weevil adults measured
namespace: BananaTrait
def: "How many banana weevil adults used to obtain a measurement." []
is_a: CO_325:1000002 ! Biotic_stress

[Term]
id: CO_325:0000621
name: Number of adult weevils measured
namespace: BananaTrait
def: "Visual counting method" []
synonym: "WvlAdltMsrd_Ct_weevil," EXACT []
is_a: CO_325:1000024 ! Variable
relationship: variable_of CO_325:0000620 ! number of banana weevil adults measured
relationship: variable_of CO_325:0010147 ! number of adult larvae - counting
relationship: variable_of CO_325:0100055 ! weevil

[Term]
id: CO_325:0000622
name: number of banana weevil larvae measured
namespace: BananaTrait
def: "How many banana weevil larvae used to obtain a measurement." []
is_a: CO_325:1000002 ! Biotic_stress

[Term]
id: CO_325:0000623
name: Number of weevil larvae measured
namespace: BananaTrait
def: "Visual counting method" []
synonym: "WvlLvMsrd_Ct_weevil," EXACT []
is_a: CO_325:1000024 ! Variable
relationship: variable_of CO_325:0000622 ! number of banana weevil larvae measured
relationship: variable_of CO_325:0010146 ! number of weevil larvae - counting
relationship: variable_of CO_325:0100055 ! weevil

[Term]
id: CO_325:0000624
name: banana weevil adult head capsule width
namespace: BananaTrait
def: "The width of a banana weevil adult weevil head." []
is_a: CO_325:1000002 ! Biotic_stress

[Term]
id: CO_325:0000625
name: Adult weevil head capsule width
namespace: BananaTrait
def: "Measurement under microscope In ?M" []
synonym: "WvlAdltHdCps_M_?M," EXACT []
is_a: CO_325:1000024 ! Variable
relationship: variable_of CO_325:0000624 ! banana weevil adult head capsule width
relationship: variable_of CO_325:0010148 ! adult weevil head capsule - measurement
relationship: variable_of CO_325:0100056 ! m

[Term]
id: CO_325:0000626
name: banana weevil adult average head capsule width
namespace: BananaTrait
def: "The average width of a banana weevil adult head." []
is_a: CO_325:1000002 ! Biotic_stress

[Term]
id: CO_325:0000627
name: Average adult weevil head capsule width
namespace: BananaTrait
def: "Measurement under microscope In ?M" []
synonym: "AvgWvlAdltHdCps_M_?M," EXACT []
is_a: CO_325:1000024 ! Variable
relationship: variable_of CO_325:0000626 ! banana weevil adult average head capsule width
relationship: variable_of CO_325:0010148 ! adult weevil head capsule - measurement
relationship: variable_of CO_325:0100056 ! m

[Term]
id: CO_325:0000628
name: banana weevil adult body length
namespace: BananaTrait
def: "The length of a banana weevil adult body, from the head to the tip of the abdomen." []
is_a: CO_325:1000002 ! Biotic_stress

[Term]
id: CO_325:0000629
name: Adult weevil body length
namespace: BananaTrait
def: "Measurement under microscope In ?M" []
synonym: "WvlAdltBdLgt_M_?M," EXACT []
is_a: CO_325:1000024 ! Variable
relationship: variable_of CO_325:0000628 ! banana weevil adult body length
relationship: variable_of CO_325:0010149 ! adult weevil body - measurement
relationship: variable_of CO_325:0100056 ! m

[Term]
id: CO_325:0000630
name: banana weevil adult average body length
namespace: BananaTrait
def: "The average length of a banana weevil adult body, from the head to the tip of the abdomen." []
is_a: CO_325:1000002 ! Biotic_stress

[Term]
id: CO_325:0000631
name: Average adult weevil body length
namespace: BananaTrait
def: "Measurement under microscope In ?M" []
synonym: "AvgWvlAdltBdLgt_M_?M," EXACT []
is_a: CO_325:1000024 ! Variable
relationship: variable_of CO_325:0000630 ! banana weevil adult average body length
relationship: variable_of CO_325:0010149 ! adult weevil body - measurement
relationship: variable_of CO_325:0100056 ! m

[Term]
id: CO_325:0000632
name: banana weevil adult body weight
namespace: BananaTrait
def: "The weight of a banana weevil adult weevil body." []
is_a: CO_325:1000002 ! Biotic_stress

[Term]
id: CO_325:0000633
name: Adult weevil body weight
namespace: BananaTrait
def: "Electronic weighing method In mg" []
synonym: "WvlAdltBdWght_M_mg," EXACT []
is_a: CO_325:1000024 ! Variable
relationship: variable_of CO_325:0000632 ! banana weevil adult body weight
relationship: variable_of CO_325:0010149 ! adult weevil body - measurement
relationship: variable_of CO_325:0100057 ! mg

[Term]
id: CO_325:0000634
name: banana weevil adult average body weight
namespace: BananaTrait
def: "The average weight of a banana weevil adult body." []
is_a: CO_325:1000002 ! Biotic_stress

[Term]
id: CO_325:0000635
name: Average adult weevil body weight
namespace: BananaTrait
def: "Electronic weighing method In mg" []
synonym: "AvgWvlAdltBdWght_M_mg," EXACT []
is_a: CO_325:1000024 ! Variable
relationship: variable_of CO_325:0000634 ! banana weevil adult average body weight
relationship: variable_of CO_325:0010149 ! adult weevil body - measurement
relationship: variable_of CO_325:0100057 ! mg

[Term]
id: CO_325:0000636
name: banana weevil larvae head capsule width
namespace: BananaTrait
def: "The width of a weevil larvae head capsule." []
is_a: CO_325:1000002 ! Biotic_stress

[Term]
id: CO_325:0000637
name: Weevil larvae head capsule width
namespace: BananaTrait
def: "Measurement under microscope In ?M" []
synonym: "WvlLvHdCps_M_?M," EXACT []
is_a: CO_325:1000024 ! Variable
relationship: variable_of CO_325:0000636 ! banana weevil larvae head capsule width
relationship: variable_of CO_325:0010150 ! weevil larvae head capsule - measurement
relationship: variable_of CO_325:0100056 ! m

[Term]
id: CO_325:0000638
name: banana weevil larvae average head capsule width
namespace: BananaTrait
def: "The average width of a banana weevil larvae head capsule." []
is_a: CO_325:1000002 ! Biotic_stress

[Term]
id: CO_325:0000639
name: Average weevil larvae head capsule width
namespace: BananaTrait
def: "Measurement under microscope In ?M" []
synonym: "AvgWvlLvHdCps_M_?M," EXACT []
is_a: CO_325:1000024 ! Variable
relationship: variable_of CO_325:0000638 ! banana weevil larvae average head capsule width
relationship: variable_of CO_325:0010150 ! weevil larvae head capsule - measurement
relationship: variable_of CO_325:0100056 ! m

[Term]
id: CO_325:0000640
name: banana weevil larvae body length
namespace: BananaTrait
def: "The length of a weevil larvae body, from the weevil larvae head to the tip of the abdomen." []
is_a: CO_325:1000002 ! Biotic_stress

[Term]
id: CO_325:0000641
name: Weevil larvae body length
namespace: BananaTrait
def: "Measurement under microscope In ?M" []
synonym: "WvlLvBdLgt_M_?M," EXACT []
is_a: CO_325:1000024 ! Variable
relationship: variable_of CO_325:0000640 ! banana weevil larvae body length
relationship: variable_of CO_325:0010151 ! weevil larvae body length - measurement
relationship: variable_of CO_325:0100056 ! m

[Term]
id: CO_325:0000642
name: banana weevil larvae average body length
namespace: BananaTrait
def: "The average length of a weevil larvae body, from the head to the tip of the abdomen." []
is_a: CO_325:1000002 ! Biotic_stress

[Term]
id: CO_325:0000643
name: Average weevil larvae body length
namespace: BananaTrait
def: "Measurement under microscope In ?M" []
synonym: "AvgWvlLvBdLgt_M_?M," EXACT []
is_a: CO_325:1000024 ! Variable
relationship: variable_of CO_325:0000642 ! banana weevil larvae average body length
relationship: variable_of CO_325:0010151 ! weevil larvae body length - measurement
relationship: variable_of CO_325:0100056 ! m

[Term]
id: CO_325:0000644
name: banana weevil larvae body weight
namespace: BananaTrait
def: "The weight of a banana weevil larvae body." []
is_a: CO_325:1000002 ! Biotic_stress

[Term]
id: CO_325:0000645
name: Weevil larvae weight
namespace: BananaTrait
def: "Measurement under microscope In mg" []
synonym: "WvlLvBdWght_M_mg," EXACT []
is_a: CO_325:1000024 ! Variable
relationship: variable_of CO_325:0000644 ! banana weevil larvae body weight
relationship: variable_of CO_325:0010152 ! weevil larvae body weight - measurement
relationship: variable_of CO_325:0100057 ! mg

[Term]
id: CO_325:0000646
name: banana weevil larvae average body weight
namespace: BananaTrait
def: "The average weight of a banana weevil larvae body." []
is_a: CO_325:1000002 ! Biotic_stress

[Term]
id: CO_325:0000647
name: Average weevil larvae weight
namespace: BananaTrait
def: "Measurement under microscope In mg" []
synonym: "AvgWvlLvBdWght_M_mg," EXACT []
is_a: CO_325:1000024 ! Variable
relationship: variable_of CO_325:0000646 ! banana weevil larvae average body weight
relationship: variable_of CO_325:0010152 ! weevil larvae body weight - measurement
relationship: variable_of CO_325:0100057 ! mg

[Term]
id: CO_325:0000648
name: percentage damage to upper cross-section outer corm caused by weevils
namespace: BananaTrait
def: "The amount of damage to the outer corm (cortex) upper cross-section, assessed by percentage of tunnels caused by weevils." []
synonym: "Damage index-X-outer" EXACT []
is_a: CO_325:1000002 ! Biotic_stress

[Term]
id: CO_325:0000649
name: Weevils damage to corm cortex cross-section %
namespace: BananaTrait
def: "Cut a transverse cross section of the corm at the collar (upper cross-section). Score weevil damage (galleries) as percentage damage on the side of the cross-section that was facing the ground, downwards. In %" []
synonym: "DmgIdxInn_M_%, CORMDG" EXACT []
is_a: CO_325:1000024 ! Variable
relationship: variable_of CO_325:0000648 ! percentage damage to upper cross-section outer corm caused by weevils
relationship: variable_of CO_325:0010141 ! damage to upper outer corm weevils - measurement
relationship: variable_of CO_325:0100046 ! %

[Term]
id: CO_325:0000650
name: percentage damage to upper cross-section inner corm caused by weevils
namespace: BananaTrait
def: "The amount of damage to the inner corm (central cylinder) upper cross-section, assessed by the percentage of tunnels caused by weevils." []
synonym: "Damage index-X-inner" EXACT []
is_a: CO_325:1000002 ! Biotic_stress

[Term]
id: CO_325:0000651
name: Weevils damage to corm outer cylinder cross-section %
namespace: BananaTrait
def: "Cut a transverse cross section of the corm at the collar (upper cross-section). Score weevil damage (galleries) as percentage damage on the side of the cross-section that was facing the ground, downwards. In %" []
synonym: "DmgIdxOut_M_%," EXACT []
is_a: CO_325:1000024 ! Variable
relationship: variable_of CO_325:0000650 ! percentage damage to upper cross-section inner corm caused by weevils
relationship: variable_of CO_325:0010140 ! damage to upper inner corm weevils - measurement
relationship: variable_of CO_325:0100046 ! %

[Term]
id: CO_325:0000662
name: Finger external length in cm
namespace: BananaTrait
def: "Measure the length of a finger that is at the 'ready to eat' stage, along the external (dorsal) arc, excluding the pedicel and the fruit tip, using a tape measure. Associate the data with the Hand rank and the Number of fingers measured. The recommendation is to collect this data from six fingers in total - three fingers in the middle of the outer whorl from the second hand and from the second-most distal hand. In cm" []
synonym: "FrtExtLng_M_cm, fingerextlength" EXACT []
is_a: CO_325:1000024 ! Variable
relationship: variable_of CO_325:0000051 ! finger external length
relationship: variable_of CO_325:0010056 ! finger external length - measurement
relationship: variable_of CO_325:0100008 ! cm

[Term]
id: CO_325:0000677
name: percentage damage to lower cross-section inner corm caused by weevils
namespace: BananaTrait
def: "The amount of damage to the inner corm (central cylinder) lower cross-section, assessed by percentage of tunnels caused by weevils." []
synonym: "Damage index-X-inner" EXACT []
is_a: CO_325:1000002 ! Biotic_stress

[Term]
id: CO_325:0000678
name: Weevils damage to lower cross-section inner corm %
namespace: BananaTrait
def: "Cut a transverse cross section of the corm at 10 cm below the collar (lower cross-section). Score weevil damage (galleries) as percentage damage on the side of the cross-section that was facing the ground, downwards. In %" []
synonym: "InrCrmDmg_M_%," EXACT []
is_a: CO_325:1000024 ! Variable
relationship: variable_of CO_325:0000677 ! percentage damage to lower cross-section inner corm caused by weevils
relationship: variable_of CO_325:0010142 ! damage to lower inner corm weevils - measurement
relationship: variable_of CO_325:0100046 ! %

[Term]
id: CO_325:0000679
name: percentage damage to lower cross-section outer corm caused by weevils
namespace: BananaTrait
def: "The amount of damage to the outer corm (cortex) lower cross-section, assessed by percentage of tunnels caused by weevils." []
synonym: "Damage index-X-outer" EXACT []
is_a: CO_325:1000002 ! Biotic_stress

[Term]
id: CO_325:0000680
name: Weevils damage to lower cross-section outer corm %
namespace: BananaTrait
def: "Cut a transverse cross section of the corm at 10 cm below the collar (lower cross-section). Score weevil damage (galleries) as percentage damage on the side of the cross-section that was facing the ground, downwards. In %" []
synonym: "OutCrmDmg_M_%," EXACT []
is_a: CO_325:1000024 ! Variable
relationship: variable_of CO_325:0000679 ! percentage damage to lower cross-section outer corm caused by weevils
relationship: variable_of CO_325:0010143 ! damage to lower outer corm weevils - measurement
relationship: variable_of CO_325:0100046 ! %

[Term]
id: CO_325:0000726
name: weekly leaf emission rate
namespace: BananaTrait
def: "A rate that expresses the number of leaves that have emerged from the pseudostem in a week." []
synonym: "LER" EXACT []
is_a: CO_325:1000005 ! Physiological

[Term]
id: CO_325:0000755
name: Average hand weight in a bunch in kg
namespace: BananaTrait
def: "Calculate as: the Total finger weight, divided by the Number of hands in bunch, e.g. 46.8 / 16 = 2.9. In kg" []
synonym: "HandAvgWtBnch_M_kgPlnt, avehandweightpbunch" EXACT []
is_a: CO_325:1000024 ! Variable
relationship: variable_of CO_325:0000329 ! average hand weight
relationship: variable_of CO_325:0010045 ! average hand weight - all - computation
relationship: variable_of CO_325:0100015 ! kg

[Term]
id: CO_325:0000756
name: Average number of fingers in a bunch: calculation
namespace: BananaTrait
def: "Calculate as: the Number of fingers in bunch, divided by the Number of hands in bunch, e.g. 172 / 16 = 10.8." []
synonym: "AvgFrtInBch_Comp_Frt, avenumfingsbunch" EXACT []
is_a: CO_325:1000024 ! Variable
relationship: variable_of CO_325:0000324 ! average number of fingers in hand
relationship: variable_of CO_325:0010050 ! average number of fingers in bunch - bunch - computation
relationship: variable_of CO_325:0100017 ! finger

[Term]
id: CO_325:0000757
name: Average number of fingers in all hands of a bunch: calculation
namespace: BananaTrait
def: "Calculate as: the sum of the Number of fingers in hand, divided by the Number of hands in bunch, e.g. (10 + 10 + 11 + 10 + 10 + 10 + 12 + 12 + 12 + 11 +12 + 12 + 10 + 10 + 10 + 11) / 16 = 10.8." []
synonym: "AvgFrtInHd_Comp_Frt, avenumfingshand_abs" EXACT []
is_a: CO_325:1000024 ! Variable
relationship: variable_of CO_325:0000324 ! average number of fingers in hand
relationship: variable_of CO_325:0010051 ! average number of fingers in hand - hands - computation
relationship: variable_of CO_325:0100017 ! finger

[Term]
id: CO_325:0000758
name: Finger internal length in cm
namespace: BananaTrait
def: "Measure the length of a finger, along the internal (ventral) arc, excluding the pedicel and the fruit tip, using a tape measure. Associate the data with the Hand rank and the Number of fingers measured. The recommendation is to collect this data from six fingers in total - three fingers in the middle of the outer whorl from the second hand and from the second-most distal hand. In cm" []
synonym: "FrtIntLng_M_mm, fingerintlength_mm" EXACT []
is_a: CO_325:1000024 ! Variable
relationship: variable_of CO_325:0000339 ! finger internal length
relationship: variable_of CO_325:0010058 ! finger internal length - measurement
relationship: variable_of CO_325:0100008 ! cm

[Term]
id: CO_325:0000759
name: Number of standing leaves (grades)
namespace: BananaTrait
def: "Calculate as: the Number of leaves with black leaf streak disease severity grade 0 + Number of leaves with black leaf streak disease severity grade 1 + Number of leaves with black leaf streak disease severity grade 2 + Number of leaves with black leaf streak disease severity grade 3 + Number of leaves with black leaf streak disease severity grade 4 + Number of leaves with black leaf streak disease severity grade 5 + Number of leaves with black leaf streak disease severity grade 6." []
synonym: "StdLf_Comp_leaf," EXACT []
is_a: CO_325:1000024 ! Variable
relationship: variable_of CO_325:0000069 ! number of standing leaves
relationship: variable_of CO_325:0010107 ! number of standing leaves - computation
relationship: variable_of CO_325:0100007 ! leaf

[Term]
id: CO_325:0000792
name: Bunch height in cm
namespace: BananaTrait
def: "circumference taken as width of widest part, length taken from first hand attachment to peduncle upto last hand attachement to peduncle In cm" []
synonym: "BnchHght_M_cm, BHT, bunchheight" EXACT []
is_a: CO_325:1000024 ! Variable
relationship: variable_of CO_325:0000793 ! bunch height
relationship: variable_of CO_325:0010034 ! bunch height - measurement
relationship: variable_of CO_325:0100008 ! cm

[Term]
id: CO_325:0000793
name: bunch height
namespace: BananaTrait
def: "The height of the bunch" []
synonym: "bunchheight" EXACT []
is_a: CO_325:1000001 ! Agronomical

[Term]
id: CO_325:0000794
name: Bunch circumference in cm
namespace: BananaTrait
def: "circumference taken as width of widest part In cm" []
synonym: "BnchCirc_M_cm, BCI, bunchcircumference" EXACT []
is_a: CO_325:1000024 ! Variable
relationship: variable_of CO_325:0000795 ! bunch circumference
relationship: variable_of CO_325:0010035 ! bunch circumference - measurement
relationship: variable_of CO_325:0100008 ! cm

[Term]
id: CO_325:0000795
name: bunch circumference
namespace: BananaTrait
def: "The circumference of the bunch" []
synonym: "bunchcircumference" EXACT []
is_a: CO_325:1000001 ! Agronomical

[Term]
id: CO_325:0000838
name: Weevils damage to periphery of peeled corm 1-3
namespace: BananaTrait
def: "Visual observation (potted trials), 1=no weevil damage; 2=partial damage; 3=severe damage" []
synonym: "DmgPrphl_M_1-3, damageperiphcorm" EXACT []
is_a: CO_325:1000024 ! Variable
relationship: variable_of CO_325:0000516 ! damage to periphery of peeled corm caused by weevils
relationship: variable_of CO_325:0010154 ! weevil damage -estimation
relationship: variable_of CO_325:0100058 ! weevil damage

[Term]
id: CO_325:0000840
name: Weevil damage to corm of mother plant 1-3
namespace: BananaTrait
def: "weevil damage on the corm after cutting the pseudostem at harvest, score extend of weevil damages (field evaluation), 1=no weevil damage; 2=partial damage; 3=severe damage" []
synonym: "DmgCrmMthPlt_M_1-3, damagemothercorm" EXACT []
is_a: CO_325:1000024 ! Variable
relationship: variable_of CO_325:0000841 ! damage to the corm of the mother plant caused by weevils
relationship: variable_of CO_325:0010154 ! weevil damage -estimation
relationship: variable_of CO_325:0100058 ! weevil damage

[Term]
id: CO_325:0000841
name: damage to the corm of the mother plant caused by weevils
namespace: BananaTrait
def: "The score of damage to the mother plant corm, assessed by tunnels caused by weevils" []
synonym: "damagemothercorm" EXACT []
is_a: CO_325:1000002 ! Biotic_stress

[Term]
id: CO_325:0000842
name: Corm inner diameter after weevils introduction in cm
namespace: BananaTrait
def: "slice the corm measure the diameter using a tape (cm) 35 and 66 days after weevil introduction (experiement done in potted plant) In cm" []
synonym: "CrmInDiam_M_cm, sizeinnercorm" EXACT []
is_a: CO_325:1000024 ! Variable
relationship: variable_of CO_325:0000843 ! size of corm inner diameter after weevils introduction
relationship: variable_of CO_325:0010155 ! corm size - measurement
relationship: variable_of CO_325:0100008 ! cm

[Term]
id: CO_325:0000843
name: size of corm inner diameter after weevils introduction
namespace: BananaTrait
def: "The diameter of the inner corm after weevil introduction" []
synonym: "sizeinnercorm" EXACT []
is_a: CO_325:1000002 ! Biotic_stress

[Term]
id: CO_325:0000844
name: Corm outer diameter after weevils introduction in cm
namespace: BananaTrait
def: "slice the corm measure the diameter using a tape (cm) 35 and 66 days after weevil introduction (experiement done in potted plant) In cm" []
synonym: "CrmOutDiam_M_cm, sizeouttercorm" EXACT []
is_a: CO_325:1000024 ! Variable
relationship: variable_of CO_325:0000845 ! size of corm outter diameter after weevils introduction
relationship: variable_of CO_325:0010155 ! corm size - measurement
relationship: variable_of CO_325:0100008 ! cm

[Term]
id: CO_325:0000845
name: size of corm outter diameter after weevils introduction
namespace: BananaTrait
def: "The diameter of the outter corm after weevil introduction" []
synonym: "sizeouttercorm" EXACT []
is_a: CO_325:1000002 ! Biotic_stress

[Term]
id: CO_325:0000854
name: Male bud length in cm
namespace: BananaTrait
def: "Length of male bud at harvest. In cm" []
synonym: "MlBdLngth_M_cm," EXACT []
is_a: CO_325:1000024 ! Variable
relationship: variable_of CO_325:0000451 ! male bud length
relationship: variable_of CO_325:0010177 ! male bud metric length - measurement
relationship: variable_of CO_325:0100008 ! cm

[Term]
id: CO_325:0000856
name: Male bud width in cm
namespace: BananaTrait
def: "Width of male bud at harvest. In cm" []
synonym: "MlBdWidth_M_cm," EXACT []
is_a: CO_325:1000024 ! Variable
relationship: variable_of CO_325:0000857 ! male bud width
relationship: variable_of CO_325:0010178 ! male bud width - measurement
relationship: variable_of CO_325:0100008 ! cm

[Term]
id: CO_325:0000857
name: male bud width
namespace: BananaTrait
def: "Width of male bud at its largets point" []
synonym: "Male bud size" EXACT []
is_a: CO_325:1000003 ! Morphological

[Term]
id: CO_325:0000858
name: Fruit dry matter content in g
namespace: BananaTrait
def: "Take a standard fresh weigth in grams (i.e. 100 g.) of fruit pulp and oven dry it 24hrs at 50 centigrade (measured from the middle finger of second hand), calculate the ratio fresh weight (g.)/dry weight (g.)measured from the middle finger of second hand) In g" []
synonym: "FrtDryMtCt_M_mg, DMC, drymattercontent" EXACT []
is_a: CO_325:1000024 ! Variable
relationship: variable_of CO_325:0000859 ! fruit dry matter content
relationship: variable_of CO_325:0010203 ! dry matter content- calculation
relationship: variable_of CO_325:0100019 ! g

[Term]
id: CO_325:0000859
name: fruit dry matter content
namespace: BananaTrait
def: "The average dry matter content per unit of fruit fresh weight" []
synonym: "drymattercontent" EXACT []
is_a: CO_325:1000006 ! Quality_traits

[Term]
id: CO_325:0000882
name: Projected top area in cm2
namespace: BananaTrait
def: "Measure top view image in cm2" []
synonym: "topLeafArea_Meas_cm2, area_topView, areaPlantTop" EXACT []
is_a: CO_325:1000024 ! Variable
relationship: variable_of CO_325:0000921 ! projected top area
relationship: variable_of CO_325:0010204 ! leaf area - measurement
relationship: variable_of CO_325:0100101 ! cm2

[Term]
id: CO_325:0000883
name: All leaves area in cm2
namespace: BananaTrait
def: "Measure top view image of loose leaves in cm2" []
synonym: "totLeafArea_Meas_cm2, areaLeaves, areaTotLeaves" EXACT []
is_a: CO_325:1000024 ! Variable
relationship: variable_of CO_325:0000922 ! leaf area
relationship: variable_of CO_325:0010204 ! leaf area - measurement
relationship: variable_of CO_325:0100101 ! cm2

[Term]
id: CO_325:0000884
name: Leaf area in cm2
namespace: BananaTrait
def: "Measure top view image of a single leave in cm2" []
synonym: "singleLeafArea_Meas_cm2, areaPerLeaf, areaSingleLeaf" EXACT []
is_a: CO_325:1000024 ! Variable
relationship: variable_of CO_325:0000922 ! leaf area
relationship: variable_of CO_325:0010204 ! leaf area - measurement
relationship: variable_of CO_325:0100101 ! cm2

[Term]
id: CO_325:0000885
name: Leaf area to plant area ratio: calculation
namespace: BananaTrait
def: "computation of top leaf area with total (loose) leaf area as topLeafArea/totLeafArea ratio" []
synonym: "leafAreaRatio_Comp_unitless, areaRatio, areaPlant_per_areaTot" EXACT []
is_a: CO_325:1000024 ! Variable
relationship: variable_of CO_325:0000923 ! leaf area to plant area ratio
relationship: variable_of CO_325:0010205 ! leaf area ratio - computation
relationship: variable_of CO_325:0100102 ! unitless

[Term]
id: CO_325:0000886
name: Total length of all leaves in cm
namespace: BananaTrait
def: "Measure the longest diagonal of a fitted ellips in cm" []
synonym: "totLeafLength_Meas_cm, lengthSum" EXACT []
is_a: CO_325:1000024 ! Variable
relationship: variable_of CO_325:0000924 ! total length of all leaves
relationship: variable_of CO_325:0010206 ! leaf length - measurement
relationship: variable_of CO_325:0100008 ! cm

[Term]
id: CO_325:0000887
name: Single leaf length in cm
namespace: BananaTrait
def: "Measure the longest diagonal of a fitted ellips in cm" []
synonym: "singleLeafLength_Meas_cm, lengthPerLeaf, lengthSingleLeaf" EXACT []
is_a: CO_325:1000024 ! Variable
relationship: variable_of CO_325:0000925 ! single leaf length
relationship: variable_of CO_325:0010206 ! leaf length - measurement
relationship: variable_of CO_325:0100008 ! cm

[Term]
id: CO_325:0000888
name: Single leaf width in cm
namespace: BananaTrait
def: "Measure the shortest diagonal of a fitted ellips in cm" []
synonym: "singleLeafWidth_Meas_cm, widthPerLeaf, widthSingleLeaf" EXACT []
is_a: CO_325:1000024 ! Variable
relationship: variable_of CO_325:0000926 ! single leaf width
relationship: variable_of CO_325:0010207 ! leaf width - measurement
relationship: variable_of CO_325:0100008 ! cm

[Term]
id: CO_325:0000889
name: Leaf chlorosis: calculation
namespace: BananaTrait
def: "Compute ratio of non green to green plant pixels in unitless" []
synonym: "leafChlorosis_Comp_unitless, leafChlorosis" EXACT []
is_a: CO_325:1000024 ! Variable
relationship: variable_of CO_325:0000927 ! leaf chlorosis
relationship: variable_of CO_325:0010208 ! leaf chlorosis - computation
relationship: variable_of CO_325:0100102 ! unitless

[Term]
id: CO_325:0000890
name: Leaf dry weight in g
namespace: BananaTrait
def: "Measure 80?C, for 14 days, or longer untill dry in g" []
synonym: "leafDryMass_Meas_g, leaf_dry, massDryLeaf" EXACT []
is_a: CO_325:1000024 ! Variable
relationship: variable_of CO_325:0000928 ! leaf dry weight
relationship: variable_of CO_325:0010209 ! dry weight - measurement
relationship: variable_of CO_325:0100019 ! g

[Term]
id: CO_325:0000891
name: Pseudostem dry weight in g
namespace: BananaTrait
def: "Measure 80?C, for 14 days, or longer untill dry in g" []
synonym: "pseudostemDryMass_Meas_g, ps_dry, massDryPseudostem" EXACT []
is_a: CO_325:1000024 ! Variable
relationship: variable_of CO_325:0000929 ! pseudostem dry weight
relationship: variable_of CO_325:0010209 ! dry weight - measurement
relationship: variable_of CO_325:0100019 ! g

[Term]
id: CO_325:0000892
name: Root dry weight in g
namespace: BananaTrait
def: "Measure 80?C, for 14 days, or longer untill dry in g" []
synonym: "rootDryMass_Meas_g, root_dry, massDryRoot" EXACT []
is_a: CO_325:1000024 ! Variable
relationship: variable_of CO_325:0000930 ! root dry weight
relationship: variable_of CO_325:0010209 ! dry weight - measurement
relationship: variable_of CO_325:0100019 ! g

[Term]
id: CO_325:0000893
name: Plant dry weight in g
namespace: BananaTrait
def: "Measure 80?C, for 14 days, or longer untill dry in g" []
synonym: "plantDryMass_Meas_g, plant_dry, massDryPlant" EXACT []
is_a: CO_325:1000024 ! Variable
relationship: variable_of CO_325:0000931 ! plant dry weight
relationship: variable_of CO_325:0010209 ! dry weight - measurement
relationship: variable_of CO_325:0100019 ! g

[Term]
id: CO_325:0000894
name: Ratio root to shoot: calculation
namespace: BananaTrait
def: "Compute ratio of belowground (root) to aboveground (shoot) dry mass as rootDryMass / shootDryMass ratio" []
synonym: "rootShootDry_Comp_unitless, rootShootRatioDry, massDryRootShoot" EXACT []
is_a: CO_325:1000024 ! Variable
relationship: variable_of CO_325:0000932 ! ratio root to shoot
relationship: variable_of CO_325:0010210 ! ratio - computation
relationship: variable_of CO_325:0100102 ! unitless

[Term]
id: CO_325:0000895
name: Leaf relative water content: calculation
namespace: BananaTrait
def: "Compute leaf dry mass /leaf fresh mass as leaf dry mass /leaf fresh mass ratio" []
synonym: "rwcLeaf_Comp_unitless, leaf_rwc, rwcLeaf" EXACT []
is_a: CO_325:1000024 ! Variable
relationship: variable_of CO_325:0000933 ! leaf relative water content
relationship: variable_of CO_325:0010211 ! water content - computation
relationship: variable_of CO_325:0100102 ! unitless

[Term]
id: CO_325:0000896
name: Pseudostem relative water content: calculation
namespace: BananaTrait
def: "Compute pseudostem dry mass / pseudostem fresh mass as pseudostem dry mass / pseudostem fresh mass ratio" []
synonym: "rwcPseudostem_Comp_unitless, ps_rwc, rwcPseudostem" EXACT []
is_a: CO_325:1000024 ! Variable
relationship: variable_of CO_325:0000934 ! pseudostem relative water content
relationship: variable_of CO_325:0010211 ! water content - computation
relationship: variable_of CO_325:0100102 ! unitless

[Term]
id: CO_325:0000897
name: Root relative water content: calculation
namespace: BananaTrait
def: "Compute root dry mass / root fresh mass as root dry mass / root fresh mass ratio" []
synonym: "rwcRoot_Comp_unitless, root_rwc, rwcRoot" EXACT []
is_a: CO_325:1000024 ! Variable
relationship: variable_of CO_325:0000935 ! root relative water content
relationship: variable_of CO_325:0010211 ! water content - computation
relationship: variable_of CO_325:0100102 ! unitless

[Term]
id: CO_325:0000898
name: Plant relative water content: calculation
namespace: BananaTrait
def: "Compute plant dry mass / plantfresh mass as plant dry mass / plantfresh mass ratio" []
synonym: "rwcPlant_Comp_unitless, plant_rwc, rwcPlant" EXACT []
is_a: CO_325:1000024 ! Variable
relationship: variable_of CO_325:0000936 ! plant relative water content
relationship: variable_of CO_325:0010211 ! water content - computation
relationship: variable_of CO_325:0100102 ! unitless

[Term]
id: CO_325:0000899
name: Pseudostem length in cm
namespace: BananaTrait
def: "Measure manual height measurement in cm" []
synonym: "lengthPseudostem_Meas_cm, heightPS, heightPseudostem" EXACT []
is_a: CO_325:1000024 ! Variable
relationship: variable_of CO_325:0000937 ! pseudostem length
relationship: variable_of CO_325:0010212 ! length - measurement
relationship: variable_of CO_325:0100008 ! cm

[Term]
id: CO_325:0000900
name: Leaf number: count
namespace: BananaTrait
def: "Count the number of leaves, unitless" []
synonym: "numLeaves_Count_unitless, numLeaf, totalNumLeaves" EXACT []
is_a: CO_325:1000024 ! Variable
relationship: variable_of CO_325:0000938 ! leaf number
relationship: variable_of CO_325:0010213 ! leaf number - counting
relationship: variable_of CO_325:0100102 ! unitless

[Term]
id: CO_325:0000901
name: Functional leaf number: count
namespace: BananaTrait
def: "Count the number of leaves (functional only > 50% estimated green area) in unitless" []
synonym: "numFuncLeaves_Count_unitless, numFuncLeaf, totalNumFunctionalLeaves" EXACT []
is_a: CO_325:1000024 ! Variable
relationship: variable_of CO_325:0000939 ! functional leaf number
relationship: variable_of CO_325:0010213 ! leaf number - counting
relationship: variable_of CO_325:0100102 ! unitless

[Term]
id: CO_325:0000902
name: System water loss in mL
namespace: BananaTrait
def: "Measure weighing of water loss though system between timepoints (refer to experimental metadata) with measurements on 2 timepoints required (refer to experimental metadata) in mL" []
synonym: "waterLossSyst_Meas_ml, waterLossSystem, transpSyst" EXACT []
is_a: CO_325:1000024 ! Variable
relationship: variable_of CO_325:0000940 ! system water loss
relationship: variable_of CO_325:0010214 ! water loss - measurement
relationship: variable_of CO_325:0100103 ! ml

[Term]
id: CO_325:0000903
name: Plant water loss in mL
namespace: BananaTrait
def: "Measure weighing of water loss though plant between timepoints (refer to experimental metadata) with measurements on 2 timepoints required (refer to experimental metadata) in mL" []
synonym: "waterLossPlant_Meas_ml, waterLossPlant, transpPlant" EXACT []
is_a: CO_325:1000024 ! Variable
relationship: variable_of CO_325:0000941 ! plant water loss
relationship: variable_of CO_325:0010214 ! water loss - measurement
relationship: variable_of CO_325:0100103 ! ml

[Term]
id: CO_325:0000904
name: Transpiration efficiency in g/mL
namespace: BananaTrait
def: "Compute gram accumulated biomass per volume water transpired with growthDry / waterLossPlan ratio in g / mL" []
synonym: "transpirationEfficiency_Comp_gml, TE_dry, TEtotalDry" EXACT []
is_a: CO_325:1000024 ! Variable
relationship: variable_of CO_325:0000942 ! transpiration efficiency
relationship: variable_of CO_325:0010215 ! transpiration efficiency - computation
relationship: variable_of CO_325:0100104 ! g / ml

[Term]
id: CO_325:0000905
name: Leaf fresh weight in g
namespace: BananaTrait
def: "Measure leaf fresh weight in g" []
synonym: "leafFreshMass_Meas_g, leaf_fresh, massFreshLeaf" EXACT []
is_a: CO_325:1000024 ! Variable
relationship: variable_of CO_325:0000943 ! leaf fresh weight
relationship: variable_of CO_325:0010216 ! fresh weight - measurement
relationship: variable_of CO_325:0100019 ! g

[Term]
id: CO_325:0000906
name: Pseudostem fresh weight in g
namespace: BananaTrait
def: "Measure pseudostem fresh weight in g" []
synonym: "pseudostemFreshMass_Meas_g, pseudostem_fresh, massFreshPseudostem" EXACT []
is_a: CO_325:1000024 ! Variable
relationship: variable_of CO_325:0000944 ! pseudostem fresh weight
relationship: variable_of CO_325:0010216 ! fresh weight - measurement
relationship: variable_of CO_325:0100019 ! g

[Term]
id: CO_325:0000907
name: Root fresh weight in g
namespace: BananaTrait
def: "Measure root fresh weight in g" []
synonym: "rootFreshMass_Meas_g, root_fresh, massFreshRoot" EXACT []
is_a: CO_325:1000024 ! Variable
relationship: variable_of CO_325:0000945 ! root fresh weight
relationship: variable_of CO_325:0010216 ! fresh weight - measurement
relationship: variable_of CO_325:0100019 ! g

[Term]
id: CO_325:0000908
name: Plant fresh weight in g
namespace: BananaTrait
def: "Measure plant fresh weight in g" []
synonym: "plantFreshMass_Meas_g, plant_fresh, massFreshPlant" EXACT []
is_a: CO_325:1000024 ! Variable
relationship: variable_of CO_325:0000946 ! plant fresh weight
relationship: variable_of CO_325:0010216 ! fresh weight - measurement
relationship: variable_of CO_325:0100019 ! g

[Term]
id: CO_325:0000909
name: Leaf to whole plant mass ratio: calculation
namespace: BananaTrait
def: "Compute ratio of leaf dry mass versus plant dry mass as leafDryMass / plantDryMass ratio" []
synonym: "leafToPlantMassRatio_Comp_unitless, relativeLeaf_dry, massDryratioLeaf" EXACT []
is_a: CO_325:1000024 ! Variable
relationship: variable_of CO_325:0000947 ! leaf to whole plant mass ratio
relationship: variable_of CO_325:0010210 ! ratio - computation
relationship: variable_of CO_325:0100102 ! unitless

[Term]
id: CO_325:0000910
name: Pseudostem to whole plant mass ratio: calculation
namespace: BananaTrait
def: "Compute ratio of pseudostem dry mass versus plant dry mass as pseudostemDryMass / plantDryMass ratio" []
synonym: "pseudostemToPlantMassRatio_Comp_unitless, relativePS_dry, massDryratioPseudostem" EXACT []
is_a: CO_325:1000024 ! Variable
relationship: variable_of CO_325:0000948 ! pseudostem to whole plant mass ratio
relationship: variable_of CO_325:0010210 ! ratio - computation
relationship: variable_of CO_325:0100102 ! unitless

[Term]
id: CO_325:0000911
name: Root to whole plant mass ratio: calculation
namespace: BananaTrait
def: "Compute ratio of root dry mass versus plant dry mass as rootDryMass / plantDryMass ratio" []
synonym: "rootToPlantMassRatio_Comp_unitless, relativeRoot_dry, massDryratioRoot" EXACT []
is_a: CO_325:1000024 ! Variable
relationship: variable_of CO_325:0000949 ! root to whole plant mass ratio
relationship: variable_of CO_325:0010210 ! ratio - computation
relationship: variable_of CO_325:0100102 ! unitless

[Term]
id: CO_325:0000912
name: Daily rate of water loss in mL
namespace: BananaTrait
def: "Compute measurement of system water loss between two timepoints (refer to experimental metadata) in mL" []
synonym: "waterLossDay_Comp_ml, waterLossDaily, rateWaterLossPerDay" EXACT []
is_a: CO_325:1000024 ! Variable
relationship: variable_of CO_325:0000950 ! daily rate of water loss
relationship: variable_of CO_325:0010217 ! water loss rate - computation
relationship: variable_of CO_325:0100103 ! ml

[Term]
id: CO_325:0000913
name: System water loss per leaf area in mL/cm2
namespace: BananaTrait
def: "Measure weight of water loss though system normalized by leaf area in mL / cm2" []
synonym: "waterLossSystPerLeafArea_Meas_mlcm2, waterLossSystem_per_Area" EXACT []
is_a: CO_325:1000024 ! Variable
relationship: variable_of CO_325:0000951 ! system water loss per leaf area
relationship: variable_of CO_325:0010214 ! water loss - measurement
relationship: variable_of CO_325:0100105 ! ml / cm2

[Term]
id: CO_325:0000914
name: Dry plant growth in g
namespace: BananaTrait
def: "Compute dry weight difference between timepoints (refer to experimental metadata) with measurements on 2 timepoints required (refer to experimental metadata) ratio in g" []
synonym: "growthDry_Comp_g, plantGrowth_dry, growthDry" EXACT []
is_a: CO_325:1000024 ! Variable
relationship: variable_of CO_325:0000952 ! dry plant growth
relationship: variable_of CO_325:0010218 ! growth - computation
relationship: variable_of CO_325:0100019 ! g

[Term]
id: CO_325:0000915
name: Fresh plant growth in g
namespace: BananaTrait
def: "Compute fresh weight difference between timepoints (refer to experimental metadata) with measurements on 2 timepoints required (refer to experimental metadata) ratio in g" []
synonym: "growthFresh_Comp_g, plantGrowth_fresh, growthFresh" EXACT []
is_a: CO_325:1000024 ! Variable
relationship: variable_of CO_325:0000953 ! fresh plant growth
relationship: variable_of CO_325:0010218 ! growth - computation
relationship: variable_of CO_325:0100019 ! g

[Term]
id: CO_325:0000916
name: Increase of leaf area in cm2
namespace: BananaTrait
def: "Compute leaf area difference between timepoints (refer to experimental metadata) with measurements on 2 timepoints required (refer to experimental metadata) ratio in cm2" []
synonym: "leafAreaIncrease_Comp_cm2, leafAreaIncrease" EXACT []
is_a: CO_325:1000024 ! Variable
relationship: variable_of CO_325:0000954 ! increase of leaf area
relationship: variable_of CO_325:0010218 ! growth - computation
relationship: variable_of CO_325:0100101 ! cm2

[Term]
id: CO_325:0000917
name: Height increase of pseudostem in cm2
namespace: BananaTrait
def: "Compute pseudostem height difference between timepoints (refer to experimental metadata) with measurements on 2 timepoints required (refer to experimental metadata) ratio in cm2" []
synonym: "pseudostemHeightIncrease_Comp_cm2, pseudostemHeightIncrease" EXACT []
is_a: CO_325:1000024 ! Variable
relationship: variable_of CO_325:0000955 ! height increase of pseudostem
relationship: variable_of CO_325:0010218 ! growth - computation
relationship: variable_of CO_325:0100101 ! cm2

[Term]
id: CO_325:0000918
name: Pseudostem height increase per leaf formed in in cm
namespace: BananaTrait
def: "Compute pseudostem height difference between timepoints (refer to experimental metadata) per number of new leaves formed between timepoints (refer to experimental metadata) with measurements on 2 timepoints required (refer to experimental metadata) ratio in cm" []
synonym: "pseudostemHeightIncreasePerFormedLeaf_Comp_cm, growthPS_per_leafFormed" EXACT []
is_a: CO_325:1000024 ! Variable
relationship: variable_of CO_325:0000956 ! pseudostem height increase per leaf formed
relationship: variable_of CO_325:0010218 ! growth - computation
relationship: variable_of CO_325:0100008 ! cm

[Term]
id: CO_325:0000919
name: Leaves formed per pseudostem height increase in leaves/cm
namespace: BananaTrait
def: "Compute leaf area increase between timepoints (refer to experimental metadata) per number of new leaves formed between timepoints (refer to experimental metadata) with measurements on 2 timepoints required (refer to experimental metadata) ratio in []/cm" []
synonym: "leavesFormedPerPseudostemGrowth_Comp_percm, leaves_per_heightPS" EXACT []
is_a: CO_325:1000024 ! Variable
relationship: variable_of CO_325:0000957 ! leaves formed per pseudostem height increase
relationship: variable_of CO_325:0010218 ! growth - computation
relationship: variable_of CO_325:0100106 ! []/cm

[Term]
id: CO_325:0000921
name: projected top area
namespace: BananaTrait
def: "The projected leaf area of a plant (photosynthetic surface)" []
synonym: "topLeafArea" EXACT []
is_a: CO_325:1000004 ! Phenological

[Term]
id: CO_325:0000922
name: leaf area
namespace: BananaTrait
def: "The area of all leaves" []
synonym: "totLeafArea" EXACT []
is_a: CO_325:1000004 ! Phenological

[Term]
id: CO_325:0000923
name: leaf area to plant area ratio
namespace: BananaTrait
def: "Ratio of projected leaf area to the actual leaf area, measure for the compactness of the plant crown" []
synonym: "leafAreaRatio" EXACT []
is_a: CO_325:1000005 ! Physiological

[Term]
id: CO_325:0000924
name: total length of all leaves
namespace: BananaTrait
def: "The length of a leaf" []
synonym: "totLeafLength" EXACT []
is_a: CO_325:1000004 ! Phenological

[Term]
id: CO_325:0000925
name: single leaf length
namespace: BananaTrait
def: "The length of a leaf" []
synonym: "singleLeafLength" EXACT []
is_a: CO_325:1000004 ! Phenological

[Term]
id: CO_325:0000926
name: single leaf width
namespace: BananaTrait
def: "The width of a leaf" []
synonym: "singleLeafWidth" EXACT []
is_a: CO_325:1000004 ! Phenological

[Term]
id: CO_325:0000927
name: leaf chlorosis
namespace: BananaTrait
def: "leaf trait correlated to the health stage of the leaf" []
synonym: "leafChlorosis" EXACT []
is_a: CO_325:1000005 ! Physiological

[Term]
id: CO_325:0000928
name: leaf dry weight
namespace: BananaTrait
def: "The dry weight of a leaf" []
synonym: "leafDryMass" EXACT []
is_a: CO_325:1000004 ! Phenological

[Term]
id: CO_325:0000929
name: pseudostem dry weight
namespace: BananaTrait
def: "The dry weight of the pseudostem" []
synonym: "pseudostemDryMass" EXACT []
is_a: CO_325:1000004 ! Phenological

[Term]
id: CO_325:0000930
name: root dry weight
namespace: BananaTrait
def: "The dry weight of the root system" []
synonym: "rootDryMass" EXACT []
is_a: CO_325:1000004 ! Phenological

[Term]
id: CO_325:0000931
name: plant dry weight
namespace: BananaTrait
def: "The dry weight of the whole plant." []
synonym: "plantDryMass" EXACT []
is_a: CO_325:1000004 ! Phenological

[Term]
id: CO_325:0000932
name: ratio root to shoot
namespace: BananaTrait
def: "The ratio of dry mass of belowground (root) to abovegrund (shoot) biomass" []
synonym: "rootShootDry" EXACT []
is_a: CO_325:1000005 ! Physiological

[Term]
id: CO_325:0000933
name: leaf relative water content
namespace: BananaTrait
def: "The relative water content in a leaf" []
synonym: "rwcLeaf" EXACT []
is_a: CO_325:1000005 ! Physiological

[Term]
id: CO_325:0000934
name: pseudostem relative water content
namespace: BananaTrait
def: "The relative water content in a pseudostem" []
synonym: "rwcPseudostem" EXACT []
is_a: CO_325:1000005 ! Physiological

[Term]
id: CO_325:0000935
name: root relative water content
namespace: BananaTrait
def: "The relative water content in a root" []
synonym: "rwcRoot" EXACT []
is_a: CO_325:1000005 ! Physiological

[Term]
id: CO_325:0000936
name: plant relative water content
namespace: BananaTrait
def: "The relative water content in the whole plant" []
synonym: "rwcPlant" EXACT []
is_a: CO_325:1000005 ! Physiological

[Term]
id: CO_325:0000937
name: pseudostem length
namespace: BananaTrait
def: "The length of a pseudostem" []
synonym: "lengthPseudostem" EXACT []
is_a: CO_325:1000004 ! Phenological

[Term]
id: CO_325:0000938
name: leaf number
namespace: BananaTrait
def: "The number of all leaves (including dried/dead/wilted/yellow) in a shoot system" []
synonym: "numLeaves" EXACT []
is_a: CO_325:1000004 ! Phenological

[Term]
id: CO_325:0000939
name: functional leaf number
namespace: BananaTrait
def: "The number of functional leaves (greenness>50%) in a shoot system" []
synonym: "numFuncLeaves" EXACT []
is_a: CO_325:1000004 ! Phenological

[Term]
id: CO_325:0000940
name: system water loss
namespace: BananaTrait
def: "The amount of water loss in the system over time" []
synonym: "waterLossSyst" EXACT []
is_a: CO_325:1000005 ! Physiological

[Term]
id: CO_325:0000941
name: plant water loss
namespace: BananaTrait
def: "The amount of water loss through the plant over time" []
synonym: "waterLossPlant" EXACT []
is_a: CO_325:1000005 ! Physiological

[Term]
id: CO_325:0000942
name: transpiration efficiency
namespace: BananaTrait
def: "The growth (weight increase) per volume transpired water" []
synonym: "transpirationEfficiency" EXACT []
is_a: CO_325:1000005 ! Physiological

[Term]
id: CO_325:0000943
name: leaf fresh weight
namespace: BananaTrait
def: "A leaf weight trait which is the fresh weight of a leaf" []
synonym: "leafFreshMass" EXACT []
is_a: CO_325:1000004 ! Phenological

[Term]
id: CO_325:0000944
name: pseudostem fresh weight
namespace: BananaTrait
def: "A pseudostem weight trait which is the fresh weight of a pseudostem" []
synonym: "pseudostemFreshMass" EXACT []
is_a: CO_325:1000004 ! Phenological

[Term]
id: CO_325:0000945
name: root fresh weight
namespace: BananaTrait
def: "A root weight trait which is the fresh weight of a root" []
synonym: "rootFreshMass" EXACT []
is_a: CO_325:1000004 ! Phenological

[Term]
id: CO_325:0000946
name: plant fresh weight
namespace: BananaTrait
def: "A plant weight trait which is the fresh weight of a plant" []
synonym: "plantFreshMass" EXACT []
is_a: CO_325:1000004 ! Phenological

[Term]
id: CO_325:0000947
name: leaf to whole plant mass ratio
namespace: BananaTrait
def: "Measure for the biomass allocation: dry mass of leaves versus whole plant dry mass ratio" []
synonym: "leafToPlantMassRatio_dry" EXACT []
is_a: CO_325:1000005 ! Physiological

[Term]
id: CO_325:0000948
name: pseudostem to whole plant mass ratio
namespace: BananaTrait
def: "Measure for the biomass allocation: dry mass of pseudostem versus whole plant dry mass ratio" []
synonym: "pseudostemToPlantMassRatio_dry" EXACT []
is_a: CO_325:1000005 ! Physiological

[Term]
id: CO_325:0000949
name: root to whole plant mass ratio
namespace: BananaTrait
def: "Measure for the biomass allocation: dry mass of roots versus whole plant dry mass ratio" []
synonym: "rootToPlantMassRatio_dry" EXACT []
is_a: CO_325:1000005 ! Physiological

[Term]
id: CO_325:0000950
name: daily rate of water loss
namespace: BananaTrait
def: "The average daily water loss" []
synonym: "waterLossDay" EXACT []
is_a: CO_325:1000005 ! Physiological

[Term]
id: CO_325:0000951
name: system water loss per leaf area
namespace: BananaTrait
def: "The amount of water loss in the system normalized by the leaf area" []
synonym: "waterLossSystPerLeafArea" EXACT []
is_a: CO_325:1000005 ! Physiological

[Term]
id: CO_325:0000952
name: dry plant growth
namespace: BananaTrait
def: "Dry mass accumulation over time" []
synonym: "growthDry" EXACT []
is_a: CO_325:1000005 ! Physiological

[Term]
id: CO_325:0000953
name: fresh plant growth
namespace: BananaTrait
def: "Fresh mass accumulation over time" []
synonym: "growthFresh" EXACT []
is_a: CO_325:1000005 ! Physiological

[Term]
id: CO_325:0000954
name: increase of leaf area
namespace: BananaTrait
def: "Leaf area increase over time" []
synonym: "leafAreaIncrease" EXACT []
is_a: CO_325:1000005 ! Physiological

[Term]
id: CO_325:0000955
name: height increase of pseudostem
namespace: BananaTrait
def: "Pseudostem height increase over time" []
synonym: "pseudostemHeightIncrease" EXACT []
is_a: CO_325:1000005 ! Physiological

[Term]
id: CO_325:0000956
name: pseudostem height increase per leaf formed
namespace: BananaTrait
def: "Stunting expressed as height growth per new formed leaf" []
synonym: "pseudostemHeightIncreasePerFormedLeaf" EXACT []
is_a: CO_325:1000005 ! Physiological

[Term]
id: CO_325:0000957
name: leaves formed per pseudostem height increase
namespace: BananaTrait
def: "Stunting expressed as number of leaves per height growth" []
synonym: "leavesFormedPerPseudostemGrowth" EXACT []
is_a: CO_325:1000005 ! Physiological

[Term]
id: CO_325:0000958
name: time from planting to shooting
namespace: BananaTrait
def: "The time elapsed from planting to shooting (when the inflorescence emerges from the pseudostem and is still in an erect position)." []
synonym: "Length of vegetative stage" EXACT []
synonym: "plant2shoot" EXACT []
is_a: CO_325:1000004 ! Phenological

[Term]
id: CO_325:0000967
name: pollen germination
namespace: BananaTrait
def: "The rate of pollen grain germinating" []
synonym: "pollenGerm" EXACT []
is_a: CO_325:1000005 ! Physiological

[Term]
id: CO_325:0000968
name: Percentage of pollen viability
def: "Pollen viability percentage calculated as (number of viable pollen/total number of pollen)*100" []
is_a: CO_325:1000024 ! Variable
relationship: variable_of CO_325:0000970 ! pollen viability
relationship: variable_of CO_325:0010238 ! percentage of pollen grain viable- computation
relationship: variable_of CO_325:0100046 ! %

[Term]
id: CO_325:0000969
name: Percentage pollen germination
namespace: BananaTrait
def: "Under microscope, count germinated pollen grains. Calculate pollen germination percentage measured as number of pollen germinated divided by total number of pollen mulitplied by 100" []
synonym: "pollenGermProp" EXACT []
is_a: CO_325:1000024 ! Variable
relationship: variable_of CO_325:0000967 ! pollen germination
relationship: variable_of CO_325:0010237 ! percentage of pollen grain germinating - computation
relationship: variable_of CO_325:0100046 ! %

[Term]
id: CO_325:0000970
name: pollen viability
namespace: BananaTrait
def: "The amount of pollen grains which germinate and generate viable plantlets" []
synonym: "pollenVia" EXACT []
is_a: CO_325:1000005 ! Physiological

[Term]
id: CO_325:0000971
name: pollen per anther
namespace: BananaTrait
def: "pollen grains per one anther of a male flower" []
synonym: "pollenPerAnth" EXACT []
is_a: CO_325:1000005 ! Physiological

[Term]
id: CO_325:0000972
name: Number of pollen grain per anther: count
namespace: BananaTrait
def: "the Number of grain pollen counted from an anther" []
is_a: CO_325:1000024 ! Variable
relationship: variable_of CO_325:0000971 ! pollen per anther
relationship: variable_of CO_325:0010239 ! number of pollen grain per anther - counting
relationship: variable_of CO_325:0100102 ! unitless

[Term]
id: CO_325:0000973
name: black sigatoka leaf necrosis
namespace: BananaTrait
def: "Black sigatoka leaf symptoms evaluation" []
synonym: "BSLN" EXACT []
is_a: CO_325:1000002 ! Biotic_stress

[Term]
id: CO_325:0000974
name: yellow sigatoka leaf necrosis
namespace: BananaTrait
def: "Yellow sigatoka leaf symptoms evaluation" []
synonym: "YSLN" EXACT []
is_a: CO_325:1000002 ! Biotic_stress

[Term]
id: CO_325:0000975
name: emusacea leaf spot necrosis
namespace: BananaTrait
def: "Eumusacea leaf spot symptom evaluation" []
synonym: "ELSN" EXACT []
is_a: CO_325:1000002 ! Biotic_stress

[Term]
id: CO_325:0000979
name: Percentage of black sigatoka leaf necrosis
namespace: BananaTrait
def: "Evaluate resistance to black sigatoka, using leaf disk in a petri dish, on a weekly basis for 50-60 days, in percentage of necrosis observed" []
synonym: "BlksgtkLfNc_LfDsk_Est" EXACT []
is_a: CO_325:1000024 ! Variable
relationship: variable_of CO_325:0000973 ! black sigatoka leaf necrosis
relationship: variable_of CO_325:0010241 ! percentage of leaf necrosis - estimation
relationship: variable_of CO_325:0100046 ! %

[Term]
id: CO_325:0000980
name: Percentage of yellow sigatoka leaf necrosis
namespace: BananaTrait
def: "Evaluate resistance to yellow sigatoka, using leaf disk in a petri dish, on a weekly basis for 50-60 days, in percentage of necrosis observed" []
synonym: "YlsgtkLfNc_LfDsk_Est" EXACT []
is_a: CO_325:1000024 ! Variable
relationship: variable_of CO_325:0000974 ! yellow sigatoka leaf necrosis
relationship: variable_of CO_325:0010241 ! percentage of leaf necrosis - estimation
relationship: variable_of CO_325:0100046 ! %

[Term]
id: CO_325:0000981
name: Percentage of eumusae leaf necrosis
namespace: BananaTrait
def: "Evaluate resistance to eumusae leaf spot (Mycosphaerella eumusae), using leaf disk in a petri dish, on a weekly basis for 50-60 days, in percentage of necrosis observed" []
synonym: "EumuLfSpt_LfDisk_Est" EXACT []
is_a: CO_325:1000024 ! Variable
relationship: variable_of CO_325:0000975 ! emusacea leaf spot necrosis
relationship: variable_of CO_325:0010241 ! percentage of leaf necrosis - estimation
relationship: variable_of CO_325:0100046 ! %

[Term]
id: CO_325:0000983
name: Leaf chlorosis: estimation
namespace: BananaTrait
def: "Estimated, in percentage, of the amount of leaf chlorosis, on a weekly basis of a detached leaf disk (usually until 50-60 days) on a petri dish" []
synonym: "LfChlr_LfDisk_Est" EXACT []
is_a: CO_325:1000024 ! Variable
relationship: variable_of CO_325:0000927 ! leaf chlorosis
relationship: variable_of CO_325:0010240 ! percentage of leaf chlorosis - estimation
relationship: variable_of CO_325:0100046 ! %

[Term]
id: CO_325:0000984
name: youngest leaf with streak disease
namespace: BananaTrait
def: "first leaf with first streak disease development stage counted from the first 50% or more of unfurl leaf." []
is_a: CO_325:1000002 ! Biotic_stress

[Term]
id: CO_325:0000985
name: pollen grain per anther
namespace: BananaTrait
def: "number of pollen grains per anther" []
is_a: CO_325:1000005 ! Physiological

[Term]
id: CO_325:0000986
name: Youngest leaf black streak
namespace: BananaTrait
def: "Youngest leaf with streak is a leaf with first disease development stage counted from the first 50% or more of unfurl leaf.Visually observe and record the amount of the surface area of a standing leaf that is affected by black leaf streak disease.\nStage 1 appears as a small depigmentation spot whose whitish or yellow colour resembles stage 1 of Yellow Sigatoka disease. These symptoms are not visible in transmitted light and can be observed only on the underside of the leaf.;\nStage 2 appears as a stripe, generally brown in colour and visible on the underside of the leaf; later the symptom also appears on the upper part of the limb as a stripe, the yellow colour of which resembles the stripe at stage 1 of Yellow Sigatoka. The colour of this stripe will change progressively from brown and later to black on the upper side of the limb, but will retain the brown colour on the underside\nStage 3 differs from the previous one by its dimensions. The stripe becomes longer, is enlarged and in certain conditions (weak inoculum and unfavourable climatic conditions) can reach 2 or 3 cm.;" []
synonym: "YgStkLf_1-3_Est" EXACT []
is_a: CO_325:1000024 ! Variable
relationship: variable_of CO_325:0000984 ! youngest leaf with streak disease
relationship: variable_of CO_325:0010242 ! youngest leaf with black streak disease development stage  - estimation

[Term]
id: CO_325:0000994
name: Fruit parthenocarpy
namespace: BananaTrait
def: "Visual evaluation of parthenocarpy on mature fruit: absence (0) or presence (1) of seeds" []
is_a: CO_325:1000024 ! Variable
relationship: variable_of CO_325:0000995 ! fruit parthenocarpy
relationship: variable_of CO_325:0010245 ! fruit parthenocarpy - estimation
relationship: variable_of CO_325:0100053 ! presence absence 0

[Term]
id: CO_325:0000995
name: fruit parthenocarpy
namespace: BananaTrait
is_a: CO_325:1000005 ! Physiological

[Term]
id: CO_325:0000998
name: presence of fusarium wilt tropical race 4
namespace: BananaTrait
def: "The presence of symptoms of fusarium tropical race 4 (foc TR4) on a banana plant" []
is_a: CO_325:1000002 ! Biotic_stress

[Term]
id: CO_325:0000999
name: Presence of Fusarium Tropical Race 4 by PCR assay 0-1
namespace: BananaTrait
def: "Diagnose absence (0) or presence (1) of fusarium wilt tropical race 4 (foc TR4) by PCR assay on banana plant tissue sample" []
synonym: "focTR4_PCRassay_0-1" EXACT []
is_a: CO_325:1000024 ! Variable
relationship: variable_of CO_325:0000998 ! presence of fusarium wilt tropical race 4
relationship: variable_of CO_325:0010243 ! PCR assay
relationship: variable_of CO_325:0100053 ! presence absence 0

[Term]
id: CO_325:0001000
name: Plant height 1-3
namespace: BananaTrait
synonym: "PltHght_1-3" EXACT []
is_a: CO_325:1000024 ! Variable
relationship: variable_of CO_325:0000307 ! plant height to neck of peduncle
relationship: variable_of CO_325:0010024 ! plant height - neck of peduncle - measurement
relationship: variable_of CO_325:0100062 ! height score (1 to 3)

[Term]
id: CO_325:0001001
name: suckering behavior of the plant
namespace: BananaTrait
def: "Banana plant sucker apical dominance type" []
is_a: CO_325:1000001 ! Agronomical

[Term]
id: CO_325:0001002
name: Suckering behavior 1-3
namespace: BananaTrait
def: "Banana plant sucker apical dominance type: (1) High apical dominance; (2) Medium apical dominance; (3) Low apical dominance" []
synonym: "SuckerBhv1-3" EXACT []
is_a: CO_325:1000024 ! Variable

[Term]
id: CO_325:0001003
name: bunch size
namespace: BananaTrait
def: "The overall size of a banana bunch at mature green stage" []
synonym: "BSZ" EXACT []
is_a: CO_325:1000001 ! Agronomical

[Term]
id: CO_325:0001004
name: Plant circumference at 75 cm from the collar
namespace: BananaTrait
def: "Measure the circumference of the pseudostem of the plant at 75 cm from the collar, or from the pseudostem base at the ground if the collar is not visible, using a tape measure. In cm" []
synonym: "PStmGrth_M_cm, PGFL, plantcircumf100cm" EXACT []
is_a: CO_325:1000024 ! Variable
relationship: variable_of CO_325:0010249 ! plant circumference at 75 cm - measurement
relationship: variable_of CO_325:0100008 ! cm

[Term]
id: CO_325:0001005
name: Bunch size 1-3
def: "The overall size of a banana bunch at mature green stage: 1= small, 2 = medium, 3 = large" []
synonym: "BSZ" RELATED []
is_a: CO_325:1000024 ! Variable
relationship: variable_of CO_325:0001003 ! bunch size
relationship: variable_of CO_325:0010247 ! bunch size - estimation
relationship: variable_of CO_325:0100083 ! bud size scale (1 to 3)

[Term]
id: CO_325:0001007
name: Plant circumference at 20 cm from the collar
namespace: BananaTrait
def: "Measure the circumference of the pseudostem of the plant at 20 cm from the collar, or from the pseudostem base at the ground if the collar is not visible, using a tape measure. In cm" []
is_a: CO_325:1000024 ! Variable
relationship: variable_of CO_325:0010250 ! plant circumference at 20 cm - measurement
relationship: variable_of CO_325:0100008 ! cm

[Term]
id: CO_325:0010011
name: time from planting to shooting - computation
namespace: BananaMethod
def: "Calculate as: the time elapsed between the Date of planting and the Date of shooting, e.g. 24/09/2014 - 24/01/2014 = 243 days." []
is_a: CO_325:1000010 ! Computation
relationship: method_of CO_325:0000958 ! time from planting to shooting

[Term]
id: CO_325:0010012
name: plant crop cycle - computation
namespace: BananaMethod
def: "Calculate as: the time elapsed between the Date of planting to the Date of harvest, e.g. 24/12/2014 - 24/01/2014 = 334 days." []
is_a: CO_325:1000010 ! Computation
relationship: method_of CO_325:0000006 ! plant crop cycle

[Term]
id: CO_325:0010013
name: time from shooting to harvest - computation
namespace: BananaMethod
def: "Calculate as: the time elapsed between the Date of shooting to the Date of harvest, e.g. 24/12/2014 - 24/09/2014 = 91 days." []
is_a: CO_325:1000010 ! Computation
relationship: method_of CO_325:0000003 ! time from shooting to harvest

[Term]
id: CO_325:0010014
name: time from flowering to harvest - computation
namespace: BananaMethod
def: "Calculate as: the time elapsed between the Date of flowering to the Date of harvest, e.g. 24/12/2014 - 24/10/2014 = 61 days." []
is_a: CO_325:1000010 ! Computation
relationship: method_of CO_325:0000292 ! time from flowering to harvest

[Term]
id: CO_325:0010015
name: time from planting to death - computation
namespace: BananaMethod
def: "Calculate as: the time elapsed between the Date of planting and the Date of death, e.g. 24/05/2014 - 24/01/2014 = 120 days." []
is_a: CO_325:1000010 ! Computation
relationship: method_of CO_325:0000294 ! time from planting to death

[Term]
id: CO_325:0010016
name: time from harvest to death - computation
namespace: BananaMethod
def: "Calculate as: the time elapsed between the Date of harvest of the bunch of the plant from the preceeding crop cycle and the Date of death of the current plant, e.g. 24/03/2015 - 24/12/2014 = 90 days." []
is_a: CO_325:1000010 ! Computation
relationship: method_of CO_325:0000296 ! time from harvest to death

[Term]
id: CO_325:0010017
name: ratoon crop cycle - computation
namespace: BananaMethod
def: "Calculate as: the time elapsed between the Date of harvest of the bunch of the plant from the preceeding crop cycle and the Date of harvest of the bunch of the plant from the current crop cycle, e.g. 24/11/2015 - 24/12/2014 = 335 days." []
is_a: CO_325:1000010 ! Computation
relationship: method_of CO_325:0000298 ! ratoon crop cycle

[Term]
id: CO_325:0010018
name: rank of marked youngest leaf - counting
namespace: BananaMethod
def: "Mark the youngest completely unrolled leaf and record its rank, which is always 1. Associate the data with the Date of data collection." []
is_a: CO_325:1000009 ! Counting
relationship: method_of CO_325:0000564 ! rank of marked youngest leaf

[Term]
id: CO_325:0010019
name: rank of previously marked leaf - counting
namespace: BananaMethod
def: "Record the rank of the previously marked leaf (the leaf that was marked in the Rank of marked youngest leaf during the last data collection), counting the leaf rank by starting with the newest completely unrolled leaf as 1 and moving downwards. Associate the data with the Date of data collection." []
is_a: CO_325:1000009 ! Counting
relationship: method_of CO_325:0000566 ! Rank of previously marked leaf

[Term]
id: CO_325:0010020
name: monthly leaf emission rate - computation
namespace: BananaMethod
def: "Calculate as: the Rank of previously marked leaf at one point in time, minus 1 (equivalent to the Rank of marked youngest leaf), divided by the time elapsed between the two Date of data collection events when the marked leaf was recorded as 1) the Rank of marked youngest leaf and 2) the Rank of previously marked leaf, e.g. (4 - 1) / 1 month = LER of 3 leaves/month during a particular time period." []
is_a: CO_325:1000010 ! Computation
relationship: method_of CO_325:0000021 ! monthly leaf emission rate

[Term]
id: CO_325:0010021
name: weekly leaf emission rate - computation
namespace: BananaMethod
def: "Calculate as: the Rank of previously marked leaf at one point in time, minus 1 (equivalent to the Rank of marked youngest leaf), divided by the time elapsed between the two Date of data collection events when the marked leaf was recorded as 1) the Rank of marked youngest leaf and 2) the Rank of previously marked leaf, e.g. (2 - 1) / 1 week = LER of 1 leaves/week during a particular time period." []
is_a: CO_325:1000010 ! Computation
relationship: method_of CO_325:0000726 ! weekly leaf emission rate

[Term]
id: CO_325:0010022
name: number of functional leaves - counting
namespace: BananaMethod
def: "Count how many functional leaves (leaves that have 50% or more of their surface as green, healthy, photosynthetic tissue) are on the plant." []
is_a: CO_325:1000009 ! Counting
relationship: method_of CO_325:0000066 ! number of functional leaves

[Term]
id: CO_325:0010023
name: plant height - petiole of two youngest leaves - measurement
namespace: BananaMethod
def: "Measure the distance from the collar, or from the pseudostem base at the ground if the collar is not visible, to the intersection of the petioles of the two youngest leaves (leaf ranks 1 and 2), using a measuring pole or sliding ruler." []
is_a: CO_325:1000008 ! Measurement
relationship: method_of CO_325:0000009 ! plant height

[Term]
id: CO_325:0010024
name: plant height - neck of peduncle - measurement
namespace: BananaMethod
def: "Measure the distance from the collar, or from the pseudostem base at the ground if the collar is not visible, to under the 'neck' of the curved peduncle, using a measuring pole or sliding ruler." []
is_a: CO_325:1000008 ! Measurement
relationship: method_of CO_325:0000307 ! plant height to neck of peduncle

[Term]
id: CO_325:0010025
name: plant circumference - measurement
namespace: BananaMethod
def: "Measure the circumference of the pseudostem of the plant at selected distance from the collar, or from the pseudostem base at the ground if the collar is not visible, using a tape measure." []
is_a: CO_325:1000008 ! Measurement
relationship: method_of CO_325:0000012 ! plant circumference from the collar

[Term]
id: CO_325:0010026
name: tallest sucker height - measurement
namespace: BananaMethod
def: "On the tallest sucker, measure the distance from the pseudostem base at the ground to the intersection of the petioles of the two youngest leaves (leaf ranks 1 and 2), using a measuring pole or sliding ruler." []
is_a: CO_325:1000008 ! Measurement
relationship: method_of CO_325:0000027 ! tallest sucker height

[Term]
id: CO_325:0010027
name: number of maiden suckers - counting
namespace: BananaMethod
def: "Count how many maiden suckers are in the mat." []
is_a: CO_325:1000009 ! Counting
relationship: method_of CO_325:0000221 ! number of maiden suckers

[Term]
id: CO_325:0010028
name: number of sword suckers - counting
namespace: BananaMethod
def: "Count how many sword suckers are in the mat." []
is_a: CO_325:1000009 ! Counting
relationship: method_of CO_325:0000225 ! Number of sword suckers

[Term]
id: CO_325:0010029
name: number of peeper suckers - counting
namespace: BananaMethod
def: "Count how many peeper suckers are in the mat." []
is_a: CO_325:1000009 ! Counting
relationship: method_of CO_325:0000229 ! number of peeper suckers

[Term]
id: CO_325:0010030
name: number of water suckers - counting
namespace: BananaMethod
def: "Count how many water suckers are in the mat." []
is_a: CO_325:1000009 ! Counting
relationship: method_of CO_325:0000310 ! number of water suckers

[Term]
id: CO_325:0010031
name: number of suckers - counting
namespace: BananaMethod
def: "Count how many of all types of suckers are in the mat." []
is_a: CO_325:1000009 ! Counting
relationship: method_of CO_325:0000024 ! number of suckers

[Term]
id: CO_325:0010032
name: bunch maturity stage - estimation
namespace: BananaMethod
def: "Estimate maturity stage of the bunch." []
is_a: CO_325:1000011 ! Estimation
relationship: method_of CO_325:0000312 ! bunch maturity stage at harvest

[Term]
id: CO_325:0010033
name: bunch weight - measurement
namespace: BananaMethod
def: "Harvest the bunch by cutting the peduncle 10 cm above the first ridge above the most proximal, hand and immediately below the most distal hand and weigh the bunch (including the rachis), using scales." []
is_a: CO_325:1000008 ! Measurement
relationship: method_of CO_325:0000033 ! bunch weight

[Term]
id: CO_325:0010034
name: bunch height - measurement
namespace: BananaMethod
def: "Circumference taken as width of widest part, length taken from first hand attachment to peduncle upto last hand attachement to peduncle" []
is_a: CO_325:1000008 ! Measurement
relationship: method_of CO_325:0000793 ! bunch height

[Term]
id: CO_325:0010035
name: bunch circumference - measurement
namespace: BananaMethod
def: "Circumference taken as width of widest part" []
is_a: CO_325:1000008 ! Measurement
relationship: method_of CO_325:0000795 ! bunch circumference

[Term]
id: CO_325:0010036
name: rachis weight - measurement
namespace: BananaMethod
def: "Cut the hands off the rachis and weigh the rachis, using scales." []
is_a: CO_325:1000008 ! Measurement
relationship: method_of CO_325:0000314 ! rachis weight

[Term]
id: CO_325:0010037
name: total finger weight - computation
namespace: BananaMethod
def: "Calculate as: the Bunch weight, minus the Rachis weight, e.g. 50 - 10 = 40." []
is_a: CO_325:1000010 ! Computation
relationship: method_of CO_325:0000316 ! total finger weight

[Term]
id: CO_325:0010038
name: number of hands in bunch - counting
namespace: BananaMethod
def: "Count how many hands are in the bunch." []
is_a: CO_325:1000009 ! Counting
relationship: method_of CO_325:0000036 ! number of hands in bunch

[Term]
id: CO_325:0010039
name: number of fingers in bunch - counting
namespace: BananaMethod
def: "Count how many fingers are in the bunch." []
is_a: CO_325:1000009 ! Counting
relationship: method_of CO_325:0000039 ! number of fingers in bunch

[Term]
id: CO_325:0010040
name: number of fingers in bunch - estimation
namespace: BananaMethod
def: "Calculate as: the sum of the Number of fingers in 3rd hand and the Number of fingers in 2nd-most distal hand, divided by 2, and multiplied by the Number of hands in bunch, e.g. (16 + 12) / 2 * 8 = 112." []
is_a: CO_325:1000010 ! Computation
relationship: method_of CO_325:0000039 ! number of fingers in bunch

[Term]
id: CO_325:0010041
name: hand rank - counting
namespace: BananaMethod
def: "Record the rank (order) of a hand in the bunch, starting with the hand at the proximal end (closest to the pseudostem) of the bunch as 1 and continuing to the hand at the most distal end (closest to the male bud)." []
is_a: CO_325:1000009 ! Counting
relationship: method_of CO_325:0000318 ! hand rank

[Term]
id: CO_325:0010042
name: hand weight - measurement
namespace: BananaMethod
def: "Cut a hand from the rachis and weigh the hand, using scales. Associate the data with the Hand rank." []
is_a: CO_325:1000008 ! Measurement
relationship: method_of CO_325:0000045 ! hand weight

[Term]
id: CO_325:0010043
name: multiple hand weight - measurement
namespace: BananaMethod
def: "Cut multiple hands from the rachis and weigh them together, using scales. Associate the data with the Hank rank and the Number of hands measured." []
is_a: CO_325:1000008 ! Measurement
relationship: method_of CO_325:0000327 ! multiple hand weight

[Term]
id: CO_325:0010044
name: average hand weight - computation
namespace: BananaMethod
def: "Calculate as: the Multiple hand weight, divided by the Number of hands measured, e.g. 5.6 / 2 = 2.8." []
is_a: CO_325:1000010 ! Computation
relationship: method_of CO_325:0000329 ! average hand weight

[Term]
id: CO_325:0010045
name: average hand weight - all - computation
namespace: BananaMethod
def: "Calculate as: the Total finger weight, divided by the Number of hands in bunch, e.g. 46.8 / 16 = 2.9." []
is_a: CO_325:1000010 ! Computation
relationship: method_of CO_325:0000329 ! average hand weight

[Term]
id: CO_325:0010046
name: number of fingers in third hand - counting
namespace: BananaMethod
def: "Count how many fingers are in a hand. Associate the data with the Hand rank. The recommendation is to collect this data from the second and second-most distal hands." []
is_a: CO_325:1000009 ! Counting
relationship: method_of CO_325:0000042 ! number of fingers in hand: count

[Term]
id: CO_325:0010047
name: multiple number of fingers in hand - counting
namespace: BananaMethod
def: "Count how many fingers are in multiple hands. Associate the data with the Hand rank and the Number of hands measured. The recommendation is to collect this data from the second and second-most distal hands." []
is_a: CO_325:1000009 ! Counting
relationship: method_of CO_325:0000320 ! multiple number of fingers in hand

[Term]
id: CO_325:0010048
name: number of hands measured - counting
namespace: BananaMethod
def: "Count how many hands are used to obtain a measurement." []
is_a: CO_325:1000009 ! Counting
relationship: method_of CO_325:0000322 ! number of hands measured

[Term]
id: CO_325:0010049
name: average number of fingers in hand - computation
namespace: BananaMethod
def: "Calculate as: the Multiple number of fingers in hand, divided by the Number of hands measured, e.g. 40 / 2 = 20." []
is_a: CO_325:1000010 ! Computation
relationship: method_of CO_325:0000324 ! average number of fingers in hand

[Term]
id: CO_325:0010050
name: average number of fingers in bunch - bunch - computation
namespace: BananaMethod
def: "Calculate as: the Number of fingers in bunch, divided by the Number of hands in bunch, e.g. 172 / 16 = 10.8." []
is_a: CO_325:1000010 ! Computation
relationship: method_of CO_325:0000324 ! average number of fingers in hand

[Term]
id: CO_325:0010051
name: average number of fingers in hand - hands - computation
namespace: BananaMethod
def: "Calculate as: the sum of the Number of fingers in hand, divided by the Number of hands in bunch, e.g. (10 + 10 + 11 + 10 + 10 + 10 + 12 + 12 + 12 + 11 +12 + 12 + 10 + 10 + 10 + 11) / 16 = 10.8." []
is_a: CO_325:1000010 ! Computation
relationship: method_of CO_325:0000324 ! average number of fingers in hand

[Term]
id: CO_325:0010052
name: finger weight - measurement
namespace: BananaMethod
def: "Weigh a finger, using scales. Associate the data with the Hand rank. The recommendation is to collect this data from six fingers in total - three fingers in the middle of the outer whorl from the second hand and from the second-most distal hand." []
is_a: CO_325:1000008 ! Measurement
relationship: method_of CO_325:0000048 ! finger weight

[Term]
id: CO_325:0010053
name: multiple finger weight - measurement
namespace: BananaMethod
def: "Weigh multiple fingers together, using scales. Associate the data with the Hank rank and the Number of fingers measured. The recommendation is to collect this data from six fingers in total - three fingers in the middle of the outer whorl from the second hand and from the second-most distal hand." []
is_a: CO_325:1000008 ! Measurement
relationship: method_of CO_325:0000331 ! multiple finger weight

[Term]
id: CO_325:0010054
name: number of fingers measured - counting
namespace: BananaMethod
def: "Count how many fingers are used to obtain a measurement." []
is_a: CO_325:1000009 ! Counting
relationship: method_of CO_325:0000333 ! number of fingers measured

[Term]
id: CO_325:0010055
name: average finger weight - computation
namespace: BananaMethod
def: "Calculate as: the sum of the the Finger weight measurements, divided by the number of those measurements, e.g. (150 + 146 + 147 + 152 + 140 + 146) / 6 = 147." []
is_a: CO_325:1000010 ! Computation
relationship: method_of CO_325:0000335 ! average finger weight

[Term]
id: CO_325:0010056
name: finger external length - measurement
namespace: BananaMethod
def: "Measure the length of a finger that is at the 'ready to eat' stage, along the external (dorsal) arc, excluding the pedicel and the fruit tip, using a tape measure. Associate the data with the Hand rank and the Number of fingers measured. The recommendation is to collect this data from six fingers in total - three fingers in the middle of the outer whorl from the second hand and from the second-most distal hand." []
is_a: CO_325:1000008 ! Measurement
relationship: method_of CO_325:0000051 ! finger external length

[Term]
id: CO_325:0010057
name: average finger external length - computation
namespace: BananaMethod
def: "Calculate as: the sum of the Finger external length measurements, divided by the number of those measurements, e.g. (30 + 34 + 32 + 33 + 33 + 31) / 6 = 32.1." []
is_a: CO_325:1000010 ! Computation
relationship: method_of CO_325:0000337 ! average finger external length

[Term]
id: CO_325:0010058
name: finger internal length - measurement
namespace: BananaMethod
def: "Measure the length of a finger, along the internal (ventral) arc, excluding the pedicel and the fruit tip, using a tape measure. Associate the data with the Hand rank and the Number of fingers measured. The recommendation is to collect this data from six fingers in total - three fingers in the middle of the outer whorl from the second hand and from the second-most distal hand." []
is_a: CO_325:1000008 ! Measurement
relationship: method_of CO_325:0000339 ! finger internal length

[Term]
id: CO_325:0010059
name: average finger internal length - computation
namespace: BananaMethod
def: "Calculate as: the sum of the Finger internal length measurements, divided by the number of those measurements, e.g. (27 + 31 + 29 + 30 + 30 + 28) / 6 = 29.2." []
is_a: CO_325:1000010 ! Computation
relationship: method_of CO_325:0000341 ! average finger internal length

[Term]
id: CO_325:0010060
name: finger circumference - measurement
namespace: BananaMethod
def: "Measure the circumference of a finger at its widest point, using a tape measure. Associate the data with the Hand rank. The recommendation is to collect this data from six fingers in total - three fingers in the middle of the outer whorl from the second hand and from the second-most distal hand." []
is_a: CO_325:1000008 ! Measurement
relationship: method_of CO_325:0000054 ! finger circumference

[Term]
id: CO_325:0010061
name: average finger circumference - computation
namespace: BananaMethod
def: "Calculate as: the sum of the Finger circumference measurements, divided by the number of those measurements, e.g. (7.0 + 8.0 + 9.0 + 10.0 + 7.0 + 9.5) / 6 = 8.4." []
is_a: CO_325:1000010 ! Computation
relationship: method_of CO_325:0000344 ! average finger circumference

[Term]
id: CO_325:0010062
name: finger lateral diameter - measurement
namespace: BananaMethod
def: "Measure the lateral diameter of a finger from the left to the right side (not from the ventral to the dorsal side), at the widest point, using calipers. Associate the data with the Hand rank. The recommendation is to collect this data from six fingers in total - three fingers in the middle of the outer whorl from the second hand and from the second-most distal hand." []
is_a: CO_325:1000008 ! Measurement
relationship: method_of CO_325:0000233 ! finger lateral diameter

[Term]
id: CO_325:0010063
name: average finger lateral diameter - computation
namespace: BananaMethod
def: "Calculate as: the sum of the Finger lateral diameter measurements, divided by the number of those measurements, e.g. (3.5 + 5.2 + 4.1 + 5 + 6 + 6.8) / 6 = 5.1." []
is_a: CO_325:1000010 ! Computation
relationship: method_of CO_325:0000348 ! average finger lateral diameter

[Term]
id: CO_325:0010064
name: fruit pulp lateral diameter - measurement
namespace: BananaMethod
def: "Cut a finger in half, crosswise at its widest point, and on the cross-section measure the lateral diameter of the fruit pulp, from the left to the right side (not from the ventral to the dorsal side), using calipers. Associate the data with the Hand rank. The recommendation is to collect this data from six fingers in total - three fingers in the middle of the outer whorl from the second hand and from the second-most distal hand." []
is_a: CO_325:1000008 ! Measurement
relationship: method_of CO_325:0000240 ! fruit pulp lateral diameter

[Term]
id: CO_325:0010065
name: average fruit pulp lateral diameter - computation
namespace: BananaMethod
def: "Calculate as: the sum of the Fruit pulp lateral diameter measurements, divided by the number of those measurements, e.g. (3.1 + 4.8 + 3.7 + 4.6 + 5.6 + 6.4) / 6 = 4.7." []
is_a: CO_325:1000010 ! Computation
relationship: method_of CO_325:0000352 ! average fruit pulp lateral diameter

[Term]
id: CO_325:0010066
name: finger peel thickness - measurement
namespace: BananaMethod
def: "Cut a finger in half, crosswise at its widest point, and on the cross-section measure the width of the peel, using calipers. Associate the data with the Hand rank. The recommendation is to collect this data from six fingers in total - three fingers in the middle of the outer whorl from the second hand and from the second-most distal hand." []
is_a: CO_325:1000008 ! Measurement
relationship: method_of CO_325:0000236 ! finger peel thickness

[Term]
id: CO_325:0010067
name: average finger peel thickness - computation
namespace: BananaMethod
def: "Calculate as: the sum of the Finger peel thickness measurements, divided by the number of those measurements, e.g. (2 + 2 + 2 + 3 + 2 + 3 + 3) / 6 = 2." []
is_a: CO_325:1000010 ! Computation
relationship: method_of CO_325:0000355 ! average finger peel thickness

[Term]
id: CO_325:0010068
name: number of plants planted - computation
namespace: BananaMethod
def: "Calculate as: the sum of the number of values for Date of planting." []
is_a: CO_325:1000010 ! Computation
relationship: method_of CO_325:0000357 ! number of plants planted

[Term]
id: CO_325:0010069
name: plant spacing - computation
namespace: BananaMethod
def: "Calculate as: multiply the distance of the spacing between the plants, both latitudinally and longitudinally, e.g. 2 m x 3 m = 6 m2." []
is_a: CO_325:1000010 ! Computation
relationship: method_of CO_325:0000359 ! plant spacing

[Term]
id: CO_325:0010070
name: plant density - computation
namespace: BananaMethod
def: "Calculate as: number of square metres in the area unit of choice, divided by the Plant spacing, e.g. 10,000 square metres in 1 hectare / 6 = 1,667 plants/ha." []
is_a: CO_325:1000010 ! Computation
relationship: method_of CO_325:0000361 ! plant density

[Term]
id: CO_325:0010071
name: number of plants dead - computation
namespace: BananaMethod
def: "Calculate as: the sum of the number of values for Date of death." []
is_a: CO_325:1000010 ! Computation
relationship: method_of CO_325:0000363 ! number of plants dead

[Term]
id: CO_325:0010072
name: number of plants harvested - computation
namespace: BananaMethod
def: "Calculate as: the sum of the number of values for Date of harvest." []
is_a: CO_325:1000010 ! Computation
relationship: method_of CO_325:0000365 ! number of plants harvested

[Term]
id: CO_325:0010073
name: number of plants not harvested - computation
namespace: BananaMethod
def: "Calculate as: the Number of plants planted, minus the Number of plants dead, minus the Number of plants harvested, e.g. 24 - 4 - 18 = 2." []
is_a: CO_325:1000010 ! Computation
relationship: method_of CO_325:0000367 ! number of plants not harvested

[Term]
id: CO_325:0010074
name: death proportion - computation
namespace: BananaMethod
def: "Calculate as: the Number of plants dead, divided by the Number of plants planted, e.g. 4 / 24 = 0.17." []
is_a: CO_325:1000010 ! Computation
relationship: method_of CO_325:0000369 ! death proportion

[Term]
id: CO_325:0010075
name: death density - computation
namespace: BananaMethod
def: "Calculate as: the Plant density multiplied by the Death proportion, e.g. 1,667 * 0.17 = 283." []
is_a: CO_325:1000010 ! Computation
relationship: method_of CO_325:0000371 ! death density

[Term]
id: CO_325:0010076
name: harvest proportion - computation
namespace: BananaMethod
def: "Calculate as: the Number of plants harvested, divided by the Number of plants planted, e.g. 18 / 24 = 0.75." []
is_a: CO_325:1000010 ! Computation
relationship: method_of CO_325:0000373 ! harvest proportion

[Term]
id: CO_325:0010077
name: harvest density - computation
namespace: BananaMethod
def: "Calculate as: the Plant density multiplied by the Harvest proportion, e.g. 1,667 * 0.75 = 1,250." []
is_a: CO_325:1000010 ! Computation
relationship: method_of CO_325:0000375 ! harvest density

[Term]
id: CO_325:0010078
name: non-harvest proportion - computation
namespace: BananaMethod
def: "Calculate as: the Number of plants not harvested, divided by the Number of plants planted, e.g. 2 / 24 = 0.08." []
is_a: CO_325:1000010 ! Computation
relationship: method_of CO_325:0000377 ! non-harvest proportion

[Term]
id: CO_325:0010079
name: non-harvest density - computation
namespace: BananaMethod
def: "Calculate as: the Plant density multiplied by the Non-harvest proportion, e.g. 1,667 * 0.08 = 133." []
is_a: CO_325:1000010 ! Computation
relationship: method_of CO_325:0000379 ! non-harvest density

[Term]
id: CO_325:0010080
name: annual crop cycle proportion - computation
namespace: BananaMethod
def: "Calculate as: the length of a year (e.g. 365 days) divided by the Plant crop cycle or the Ratoon crop cycle, e.g. 365 / 334 = 1.09." []
is_a: CO_325:1000010 ! Computation
relationship: method_of CO_325:0000381 ! annual crop cycle proportion

[Term]
id: CO_325:0010081
name: annual plant productivity - computation
namespace: BananaMethod
def: "Calculate as: the Bunch weight multiplied by the Annual crop cycle proportion, e.g. 48 * 1.09 = 52.32." []
is_a: CO_325:1000010 ! Computation
relationship: method_of CO_325:0000383 ! plant annual yield

[Term]
id: CO_325:0010082
name: actual annual yield - computation
namespace: BananaMethod
def: "Calculate as: the Bunch weight divided by 1,000, multiplied by the Annual crop cycle proportion, multiplied by the Harvest density, e.g. (50 / 1,000) * 1.09 * 1,250 = 68.13." []
is_a: CO_325:1000010 ! Computation
relationship: method_of CO_325:0000385 ! average actual annual yield

[Term]
id: CO_325:0010083
name: potential annual yield - computation
namespace: BananaMethod
def: "Calculate as: the Bunch weight divided by 1,000, multiplied by the Annual crop cycle proportion, multiplied by the Plant density, e.g. (50 / 1,000) * 1.09 * 1,667 = 90.85." []
is_a: CO_325:1000010 ! Computation
relationship: method_of CO_325:0000387 ! average potential annual yield

[Term]
id: CO_325:0010084
name: fruit pendulance - estimation
namespace: BananaMethod
def: "Visual estimation of fruit pendulance on a bunch, for Early Evaluation Trial stage only." []
is_a: CO_325:1000011 ! Estimation
relationship: method_of CO_325:0000389 ! overall fruit pendulance quality

[Term]
id: CO_325:0010085
name: bunch quality - estimation
namespace: BananaMethod
def: "Visual estimation of bunch quality, for Early Evaluation Trial stage only." []
is_a: CO_325:1000011 ! Estimation
relationship: method_of CO_325:0000391 ! overall bunch quality

[Term]
id: CO_325:0010086
name: fruitfill - estimation
namespace: BananaMethod
def: "Visual estimation of a fruit filling for Early Evaluation Trial stage only." []
is_a: CO_325:1000011 ! Estimation
relationship: method_of CO_325:0000393 ! fruitfill

[Term]
id: CO_325:0010087
name: sucker quality - estimation
namespace: BananaMethod
def: "Visual estimation of suckering, for Early Evaluation Trial stage only." []
is_a: CO_325:1000011 ! Estimation
relationship: method_of CO_325:0000395 ! overall suckering quality

[Term]
id: CO_325:0010088
name: dwarfism - estimation
namespace: BananaMethod
def: "Visual estimation of dwarfism, for Early Evaluation Trial stage only." []
is_a: CO_325:1000011 ! Estimation
relationship: method_of CO_325:0000397 ! dwarfism

[Term]
id: CO_325:0010102
name: youngest leaf spotted - counting
namespace: BananaMethod
def: "Record the rank (order) of the youngest leaf spotted (the first fully unfurled leaf with at least 10 discrete, mature, necrotic lesions or one large necrotic area with 10 light-coloured dry centres), counting the rank by starting with the youngest completely unrolled leaf as 1 and moving downwards, associating the data with the Date of data collection." []
is_a: CO_325:1000009 ! Counting
relationship: method_of CO_325:0000099 ! youngest leaf spotted

[Term]
id: CO_325:0010104
name: time from planting to first youngest spotted leaf - computation
namespace: BananaMethod
def: "Calculate as: the time elapsed between the Date of planting and the Date of first youngest leaf spotted, e.g. 24/06/2014 - 24/01/2014 = 151 days." []
is_a: CO_325:1000010 ! Computation
relationship: method_of CO_325:0000570 ! time from planting to first youngest leaf spotted

[Term]
id: CO_325:0010105
name: number of spotted leaves - counting
namespace: BananaMethod
def: "Count how many of the standing leaves are spotted (with at least 10 discrete, mature, necrotic lesions or one large necrotic area with 10 light-coloured dry centres), considering all leaves in between and inclusive of, the youngest leaf and the oldest standing leaf." []
is_a: CO_325:1000009 ! Counting
relationship: method_of CO_325:0000572 ! number of spotted leaves

[Term]
id: CO_325:0010106
name: number of standing leaves - counting
namespace: BananaMethod
def: "Count how many of the leaves are standing leaves (without a bent or broken petiole)" []
is_a: CO_325:1000009 ! Counting
relationship: method_of CO_325:0000069 ! number of standing leaves

[Term]
id: CO_325:0010107
name: number of standing leaves - computation
namespace: BananaMethod
def: "Calculate as: the Number of leaves with black leaf streak disease severity grade 0 + Number of leaves with black leaf streak disease severity grade 1 + Number of leaves with black leaf streak disease severity grade 2 + Number of leaves with black leaf streak disease severity grade 3 + Number of leaves with black leaf streak disease severity grade 4 + Number of leaves with black leaf streak disease severity grade 5 + Number of leaves with black leaf streak disease severity grade 6." []
is_a: CO_325:1000010 ! Computation
relationship: method_of CO_325:0000069 ! number of standing leaves

[Term]
id: CO_325:0010108
name: rank of oldest standing leaf - counting
namespace: BananaMethod
def: "Record the rank (order) of the oldest standing leaf (with an erect petiole), counting the rank by starting with the youngest completely unrolled leaf as 1 and moving downwards, associating the data with the Date of data collection." []
is_a: CO_325:1000009 ! Counting
relationship: method_of CO_325:0000548 ! rank of oldest standing leaf

[Term]
id: CO_325:0010109
name: index of non-spotted leaves - computation
namespace: BananaMethod
def: "Calculate as: 100 multiplied by (Youngest leaf spotted, minus 1), divided by Number of standing leaves, e.g. 100 * (6 - 1) / 12 = 42." []
is_a: CO_325:1000010 ! Computation
relationship: method_of CO_325:0000102 ! index of non-spotted leaves

[Term]
id: CO_325:0010110
name: black leaf streak disease severity - estimation
namespace: BananaMethod
def: "Visually observe and record the amount of the surface area of a standing leaf that is affected by black leaf streak disease." []
is_a: CO_325:1000011 ! Estimation
relationship: method_of CO_325:0000574 ! black leaf streak disease severity and stage

[Term]
id: CO_325:0010111
name: number of leaves with black leaf streak disease severity grade 0 - computation
namespace: BananaMethod
def: "Calculate as: the sum of values with a Black leaf streak disease severity grade of 0." []
is_a: CO_325:1000010 ! Computation
relationship: method_of CO_325:0000580 ! number of leaves with black leaf streak disease severity grade 0

[Term]
id: CO_325:0010112
name: number of leaves with black leaf streak disease severity grade 1 - computation
namespace: BananaMethod
def: "Calculate as: the sum of values with a Black leaf streak disease severity grade of 1." []
is_a: CO_325:1000010 ! Computation
relationship: method_of CO_325:0000582 ! number of leaves with black leaf streak disease severity grade 1

[Term]
id: CO_325:0010113
name: number of leaves with black leaf streak disease severity grade 2 - computation
namespace: BananaMethod
def: "Calculate as: the sum of values with a Black leaf streak disease severity grade of 2." []
is_a: CO_325:1000010 ! Computation
relationship: method_of CO_325:0000584 ! number of leaves with black leaf streak disease severity grade 2

[Term]
id: CO_325:0010114
name: number of leaves with black leaf streak disease severity grade 3 - computation
namespace: BananaMethod
def: "Calculate as: the sum of values with a Black leaf streak disease severity grade of 3." []
is_a: CO_325:1000010 ! Computation
relationship: method_of CO_325:0000586 ! number of leaves with black leaf streak disease severity grade 3

[Term]
id: CO_325:0010115
name: number of leaves with black leaf streak disease severity grade 4 - computation
namespace: BananaMethod
def: "Calculate as: the sum of values with a Black leaf streak disease severity grade of 4." []
is_a: CO_325:1000010 ! Computation
relationship: method_of CO_325:0000588 ! number of leaves with black leaf streak disease severity grade 4

[Term]
id: CO_325:0010116
name: number of leaves with black leaf streak disease severity grade 5 - computation
namespace: BananaMethod
def: "Calculate as: the sum of values with a Black leaf streak disease severity grade of 5." []
is_a: CO_325:1000010 ! Computation
relationship: method_of CO_325:0000590 ! number of leaves with black leaf streak disease severity grade 5

[Term]
id: CO_325:0010117
name: number of leaves with black leaf streak disease severity grade 6 - computation
namespace: BananaMethod
def: "Calculate as: the sum of values with a Black leaf streak disease severity grade of 6." []
is_a: CO_325:1000010 ! Computation
relationship: method_of CO_325:0000592 ! number of leaves with black leaf streak disease severity grade 6

[Term]
id: CO_325:0010118
name: black leaf streak disease severity index - computation
namespace: BananaMethod
def: "Calculate as: ((((Number of leaves with black leaf streak disease severity grade 0, multiplied by 0), plus (Number of leaves with black leaf streak disease severity grade 1, multiplied by 1), plus (Number of leaves with black leaf streak disease severity grade 2, multiplied by 2), plus (Number of leaves with black leaf streak disease severity grade 3, multiplied by 3), plus (Number of leaves with black leaf streak disease severity grade 4, multiplied by 4), plus (Number of leaves with black leaf streak disease severity grade 5, multiplied by 5), plus (Number of leaves with black leaf streak disease severity grade 6, multiplied by 6)), divided by the number of grades in the scale minus 1 (i.e. 7-1)), divided by the Number of standing leaves), multiplied by 100. For example, ((((3 * 0) + (1 * 1) + (1 * 2) + (3 * 3) + (5 * 4) + (0 * 5) + (0 * 6)) / 6) / 13) * 100 = ((32 / 6) / 13) * 100 = 41." []
is_a: CO_325:1000010 ! Computation
relationship: method_of CO_325:0000105 ! black leaf streak disease severity index

[Term]
id: CO_325:0010122
name: black leaf streak disease incubation time - computation
namespace: BananaMethod
def: "Calculate as: the time elapsed between the Date of tagged leaf presenting black leaf streak disease symptoms at Foure's stage 1 and the Date of tagged cigar leaf unrolling at stage B, e.g. 24/04/2014 - 24/03/2014 = 31 days." []
is_a: CO_325:1000010 ! Computation
relationship: method_of CO_325:0000057 ! black leaf streak disease incubation time

[Term]
id: CO_325:0010123
name: black leaf streak disease evolution time - computation
namespace: BananaMethod
def: "Calculate as: the time elapsed between the Date of tagged leaf presenting black leaf streak disease symptoms at Foure's stage 6 and the Date of tagged leaf presenting black leaf streak disease symptoms at Foure's stage 1, e.g. 24/06/2014 - 24/04/2014 = 61 days." []
is_a: CO_325:1000010 ! Computation
relationship: method_of CO_325:0000060 ! black leaf streak disease evolution time

[Term]
id: CO_325:0010124
name: extent of internal discolouration in corm of plant caused by fusarium wilt - estimation
namespace: BananaMethod
def: "The extent to which vascular discolouration extends up the pseudostem should be determined by making cross-section cuts, from the base of the pseudostem upwards, and examining the internal tissues following each cut. The point at which discolouration is no longer visible should be noted and the distance from this point to the pseudostem base recorded." []
is_a: CO_325:1000011 ! Estimation
relationship: method_of CO_325:0000559 ! extent of internal discolouration in corm of plant caused by fusarium wilt

[Term]
id: CO_325:0010125
name: distance of internal discolouration in pseudostem of plant caused by fusarium wilt
namespace: BananaMethod
def: "For the plant, the complete corm should be removed from the soil, the roots cut off and excess soil removed. Cross-sections of the corm should be cut (using a guillotine or other suitable device) to obtain five slices of equal thickness. The upper surface of each cut section should be examined and visually evaluate the extent of the vascular discolouration." []
is_a: CO_325:1000008 ! Measurement
relationship: method_of CO_325:0000075 ! distance of internal discolouration in pseudostem of plant caused by fusarium wilt

[Term]
id: CO_325:0010126
name: extent of internal discolouration in corm of tallest sucker caused by fusarium wilt - estimation
namespace: BananaMethod
def: "The extent to which vascular discolouration extends up the pseudostem of the tallest sucker should be determined by making cross-section cuts, from the base of the pseudostem upwards, and examining the internal tissues following each cut. The point at which discolouration is no longer visible should be noted and the distance from this point to the pseudostem base recorded." []
is_a: CO_325:1000011 ! Estimation
relationship: method_of CO_325:0000072 ! extent of internal discolouration in corm of tallest sucker caused by fusarium wilt

[Term]
id: CO_325:0010127
name: distance of internal discolouration in pseudostem of tallest sucker caused by fusarium wilt
namespace: BananaMethod
def: "For the tallest sucker, the complete corm should be removed from the soil, the roots cut off and excess soil removed. Cross-sections of the corm should be cut (using a guillotine or other suitable device) to obtain five slices of equal thickness. The upper surface of each cut section should be examined and visually evaluate the extent of the vascular discolouration." []
is_a: CO_325:1000008 ! Measurement
relationship: method_of CO_325:0000594 ! distance of internal discolouration in pseudostem of tallest sucker caused by fusarium wilt

[Term]
id: CO_325:0010128
name: presence of yellowing leaves caused by fusarium wilt - estimation
namespace: BananaMethod
def: "Visual assessment." []
is_a: CO_325:1000011 ! Estimation
relationship: method_of CO_325:0000087 ! presence of yellowing leaves caused by fusarium wilt

[Term]
id: CO_325:0010129
name: presence of splitting pseudostem base caused by fusarium wilt - estimation
namespace: BananaMethod
def: "Visual assessment." []
is_a: CO_325:1000011 ! Estimation
relationship: method_of CO_325:0000090 ! presence of splitting pseudostem base caused by fusarium wilt

[Term]
id: CO_325:0010130
name: presence of changes in new leaves caused by fusarium wilt - estimation
namespace: BananaMethod
def: "Visual assessment." []
is_a: CO_325:1000011 ! Estimation
relationship: method_of CO_325:0000093 ! presence of changes in new leaves caused by fusarium wilt

[Term]
id: CO_325:0010131
name: presence of petiole collapse caused by fusarium wilt - estimation
namespace: BananaMethod
def: "Visual assessment." []
is_a: CO_325:1000011 ! Estimation
relationship: method_of CO_325:0000096 ! presence of petiole collapse caused by fusarium wilt

[Term]
id: CO_325:0010133
name: time from start of crop cycle to first external disease symptoms caused by fusarium wilt - computation
namespace: BananaMethod
def: "Calculate as: the time elapsed between the Date of planting or the Date of harvest of the bunch from the plant of the previous crop cycle and the Date of first external disease symptoms caused by Fusarium wilt." []
is_a: CO_325:1000010 ! Computation
relationship: method_of CO_325:0000084 ! time from start of crop cycle to first external disease symptoms caused by fusarium wilt

[Term]
id: CO_325:0010134
name: percentage of plants with yellowing leaves caused by fusarium wilt - computation
namespace: BananaMethod
def: "Calculate as: the sum of the number of values for Presence of yellowing leaves caused by Fusarium wilt scored as Present, divided by the Number of plants planted, multiplied by 100, e.g. 78 / 300 * 100 = 26%." []
is_a: CO_325:1000010 ! Computation
relationship: method_of CO_325:0000600 ! percentage of plants with yellowing leaves caused by fusarium wilt

[Term]
id: CO_325:0010135
name: percentage of plants with a splitting pseudostem base caused by fusarium wilt - computation
namespace: BananaMethod
def: "Calculate as: the sum of the number of values for Presence of splitting pseudostem base caused by Fusarium wilt scored as Present, divided by the Number of plants planted, multiplied by 100, e.g. 24 / 300 * 100 = 8%." []
is_a: CO_325:1000010 ! Computation
relationship: method_of CO_325:0000602 ! percentage of plants with a splitting pseudostem base caused by fusarium wilt

[Term]
id: CO_325:0010136
name: percentage of plants with changes in new leaves caused by fusarium wilt - computation
namespace: BananaMethod
def: "Calculate as: the sum of the number of values for Presence of changes in new leaves caused by Fusarium wilt scored as Present, divided by the Number of plants planted, multiplied by 100, e.g. 67 / 300 * 100 = 22%." []
is_a: CO_325:1000010 ! Computation
relationship: method_of CO_325:0000604 ! percentage of plants with changes in new leaves caused by fusarium wilt

[Term]
id: CO_325:0010137
name: percentage of plants with petiole collapse caused by fusarium wilt - computation
namespace: BananaMethod
def: "Calculate as: the sum of the number of values for Presence of petiole collapse caused by Fusarium wilt scored as Present, divided by the Number of plants planted, multiplied by 100, e.g. 84 / 300 * 100 = 28%." []
is_a: CO_325:1000010 ! Computation
relationship: method_of CO_325:0000606 ! percentage of plants with petiole collapse caused by fusarium wilt

[Term]
id: CO_325:0010138
name: percentage of plants with external disease symptoms caused by fusarium wilt - computation
namespace: BananaMethod
def: "Calculate as: the sum of the number of plants with any or multiple of the external disease symptoms caused by Fusarium wilt - yellowing leaves, splitting of pseudostem base, changes in new leaves, petiole collapse - divided by the Number of plants planted * 100, e.g. 112 / 300 * 100 = 37%." []
is_a: CO_325:1000010 ! Computation
relationship: method_of CO_325:0000078 ! percentage of plants with external disease symptoms caused by fusarium wilt

[Term]
id: CO_325:0010139
name: percentage of plants with internal disease symptoms caused by fusarium wilt - computation
namespace: BananaMethod
def: "Calculate as: the sum of the number of plants with any or multiple of the internal disease symptoms caused by Fusarium wilt - discolouration in the corm, and/or discolouration in the pseudostem - divided by the Number of plants planted * 100, e.g. 108 / 300 * 100 = 36%." []
is_a: CO_325:1000010 ! Computation
relationship: method_of CO_325:0000081 ! percentage of plants with internal disease symptoms caused by fusarium wilt

[Term]
id: CO_325:0010140
name: damage to upper inner corm weevils - measurement
namespace: BananaMethod
def: "Cut a transverse cross section of the corm at the collar (upper cross-section). Score weevil damage (galleries) as percentage damage on the side of the cross-section that was facing the ground, downwards." []
is_a: CO_325:1000008 ! Measurement
relationship: method_of CO_325:0000650 ! percentage damage to upper cross-section inner corm caused by weevils

[Term]
id: CO_325:0010141
name: damage to upper outer corm weevils - measurement
namespace: BananaMethod
def: "Cut a transverse cross section of the corm at the collar (upper cross-section). Score weevil damage (galleries) as percentage damage on the side of the cross-section that was facing the ground, downwards." []
is_a: CO_325:1000008 ! Measurement
relationship: method_of CO_325:0000648 ! percentage damage to upper cross-section outer corm caused by weevils

[Term]
id: CO_325:0010142
name: damage to lower inner corm weevils - measurement
namespace: BananaMethod
def: "Cut a transverse cross section of the corm at 10 cm below the collar (lower cross-section). Score weevil damage (galleries) as percentage damage on the side of the cross-section that was facing the ground, downwards." []
is_a: CO_325:1000008 ! Measurement
relationship: method_of CO_325:0000677 ! percentage damage to lower cross-section inner corm caused by weevils

[Term]
id: CO_325:0010143
name: damage to lower outer corm weevils - measurement
namespace: BananaMethod
def: "Cut a transverse cross section of the corm at 10 cm below the collar (lower cross-section). Score weevil damage (galleries) as percentage damage on the side of the cross-section that was facing the ground, downwards." []
is_a: CO_325:1000008 ! Measurement
relationship: method_of CO_325:0000679 ! percentage damage to lower cross-section outer corm caused by weevils

[Term]
id: CO_325:0010144
name: number of adult weevil trap - counting
namespace: BananaMethod
def: "Visual counting method of Weevil traps (the trap should be minimum 30 cm long)." []
is_a: CO_325:1000009 ! Counting
relationship: method_of CO_325:0000612 ! number of banana weevil traps used

[Term]
id: CO_325:0010145
name: number of adult weevils - counting
namespace: BananaMethod
def: "Visual counting method of Weevils per trap (the trap should be minimum 30 cm long)" []
is_a: CO_325:1000009 ! Counting
relationship: method_of CO_325:0000610 ! number of banana weevil adults per trap
relationship: method_of CO_325:0000614 ! average number of banana weevil adults per trap

[Term]
id: CO_325:0010146
name: number of weevil larvae - counting
namespace: BananaMethod
def: "Visual counting method" []
is_a: CO_325:1000009 ! Counting
relationship: method_of CO_325:0000616 ! number of banana weevil larvae per trap
relationship: method_of CO_325:0000618 ! average number of banana weevil larvae per trap
relationship: method_of CO_325:0000622 ! number of banana weevil larvae measured

[Term]
id: CO_325:0010147
name: number of adult larvae - counting
namespace: BananaMethod
def: "Visual counting method" []
is_a: CO_325:1000009 ! Counting
relationship: method_of CO_325:0000620 ! number of banana weevil adults measured

[Term]
id: CO_325:0010148
name: adult weevil head capsule - measurement
namespace: BananaMethod
def: "Measurement under microscope" []
is_a: CO_325:1000008 ! Measurement
relationship: method_of CO_325:0000624 ! banana weevil adult head capsule width
relationship: method_of CO_325:0000626 ! banana weevil adult average head capsule width

[Term]
id: CO_325:0010149
name: adult weevil body - measurement
namespace: BananaMethod
def: "Measurement under microscope" []
is_a: CO_325:1000008 ! Measurement
relationship: method_of CO_325:0000628 ! banana weevil adult body length
relationship: method_of CO_325:0000630 ! banana weevil adult average body length
relationship: method_of CO_325:0000632 ! banana weevil adult body weight
relationship: method_of CO_325:0000634 ! banana weevil adult average body weight

[Term]
id: CO_325:0010150
name: weevil larvae head capsule - measurement
namespace: BananaMethod
def: "Measurement under microscope" []
is_a: CO_325:1000008 ! Measurement
relationship: method_of CO_325:0000636 ! banana weevil larvae head capsule width
relationship: method_of CO_325:0000638 ! banana weevil larvae average head capsule width

[Term]
id: CO_325:0010151
name: weevil larvae body length - measurement
namespace: BananaMethod
def: "Measurement under microscope" []
is_a: CO_325:1000008 ! Measurement
relationship: method_of CO_325:0000640 ! banana weevil larvae body length
relationship: method_of CO_325:0000642 ! banana weevil larvae average body length

[Term]
id: CO_325:0010152
name: weevil larvae body weight - measurement
namespace: BananaMethod
def: "Measurement under microscope" []
is_a: CO_325:1000008 ! Measurement
relationship: method_of CO_325:0000644 ! banana weevil larvae body weight
relationship: method_of CO_325:0000646 ! banana weevil larvae average body weight

[Term]
id: CO_325:0010153
name: peripheral damage - measurement
namespace: BananaMethod
def: "Visual observation" []
is_a: CO_325:1000008 ! Measurement
relationship: method_of CO_325:0000516 ! damage to periphery of peeled corm caused by weevils

[Term]
id: CO_325:0010154
name: weevil damage -estimation
namespace: BananaMethod
def: "Visual observation (potted trials)" []
is_a: CO_325:1000011 ! Estimation
relationship: method_of CO_325:0000516 ! damage to periphery of peeled corm caused by weevils
relationship: method_of CO_325:0000841 ! damage to the corm of the mother plant caused by weevils

[Term]
id: CO_325:0010155
name: corm size - measurement
namespace: BananaMethod
def: "slice the corm measure the diameter using a tape (cm) 35 and 66 days after weevil introduction (experiement done in potted plant)" []
is_a: CO_325:1000008 ! Measurement
relationship: method_of CO_325:0000843 ! size of corm inner diameter after weevils introduction
relationship: method_of CO_325:0000845 ! size of corm outter diameter after weevils introduction

[Term]
id: CO_325:0010156
name: number of dead roots - counting
namespace: BananaMethod
def: "Collect all roots from a standard-size excavation of 20 x 20 x 20 cm extending outwards from the corm of the plant. Take only roots from the selected plant. Divide the collected roots into two categories: dead roots, functional roots. Dead roots are completely rotten or shrivelled whereas functional roots show at least some healthy tissue. Count the number of dead roots." []
is_a: CO_325:1000009 ! Counting
relationship: method_of CO_325:0000108 ! number of dead roots

[Term]
id: CO_325:0010157
name: number of functional roots - counting
namespace: BananaMethod
def: "Collect all roots from a standard-size excavation of 20 x 20 x 20 cm extending outwards from the corm of the plant. Take only roots from the selected plant. Divide the collected roots into two categories: dead roots, functional roots. Dead roots are completely rotten or shrivelled whereas functional roots show at least some healthy tissue. Count the number of functional roots." []
is_a: CO_325:1000009 ! Counting
relationship: method_of CO_325:0000111 ! number of functional roots

[Term]
id: CO_325:0010158
name: root nematode density - computation
namespace: BananaMethod
def: "Collect all roots from a standard-size excavation of 20 x 20 x 20 cm extending outwards from the corm of the plant. Take only roots from the selected plant; do not include roots from adjacent plants. Carefully wash the soil from the roots with tap water. Cut the roots into 10 cm long pieces and dry with paper tissue. Take a subsample of 15 g, add 100 ml distilled water and store the roots at 4 degrees Celsius. Put the roots in 100 ml of distilled water in a kitchen blender. Macerate the roots 3 times for 10 secs (separated by 5 sec intervals). Pour the macerated suspension through 250, 106 and 40 micro-metre sieves and rinse the sieves with tap water. Using distilled water, collect in a beaker the nematodes from the 40 micro-metre sieve. Using distilled water, dilute to 200 ml the nematode suspension in a graduated cylinder. Blow air through the nematode suspension with a pipette (to homogenise the suspension). Take a subsample of 6 ml (counting dish) or 2 ml (counting slide). Count the nematodes in the counting dish (stereo microscope) or in the counting slide (light microscope). Calculate the final nematode population per unit of fresh root weight." []
is_a: CO_325:1000010 ! Computation
relationship: method_of CO_325:0000531 ! root nematode density

[Term]
id: CO_325:0010159
name: pseudostem height - estimation
namespace: BananaMethod
def: "Recorded from the base of the pseudostem to the emerging point of the peduncle." []
is_a: CO_325:1000011 ! Estimation
relationship: method_of CO_325:0000425 ! pseudostem height

[Term]
id: CO_325:0010160
name: pseudostem colour - estimation
namespace: BananaMethod
def: "Detach the outermost sheath from the pseudostem (the sheath should not be too dry). Record the overall impression of colour of the exposed surface of the underlying pseudostem. Note that this 'main colour' should cover more than 75% of the underlying pseudostem surface. Use colour chart A and observe out of direct sunlight." []
is_a: CO_325:1000011 ! Estimation
relationship: method_of CO_325:0000243 ! main underlying colour of pseudostem

[Term]
id: CO_325:0010161
name: blotches area - estimation
namespace: BananaMethod
def: "Record the relative surface area coverage by blotches. [x Look at several plants if possible to get an overall idea. Observe at flowering time]." []
is_a: CO_325:1000011 ! Estimation
relationship: method_of CO_325:0000427 ! blotches relative area at petiole base

[Term]
id: CO_325:0010162
name: blotches colour - estimation
namespace: BananaMethod
def: "Observe visually the colour of the blotches on the upper leaf sheath." []
is_a: CO_325:1000011 ! Estimation
relationship: method_of CO_325:0000430 ! blotches colour at the petiole base

[Term]
id: CO_325:0010163
name: margin behaviour on petiole canal of third leaf - estimation
namespace: BananaMethod
def: "The third leaf (Leaf III) is counted from the last leaf produced before [x bunch emergence] [shooting]. Cut the petiole halfway between the pseudostem and the leaf blade and examine the cross section. [x Observe at flowering time]." []
is_a: CO_325:1000011 ! Estimation
relationship: method_of CO_325:0000433 ! margin behaviour on petiole canal of third leaf

[Term]
id: CO_325:0010164
name: winged petiole margin - estimation
namespace: BananaMethod
def: "Observations on the margins and petiole wings should be made where the petiole and pseudostem meet at shooting. Margin is the part of the petiole that can be bent outwards/inwards. [x Observe at flowering time.]" []
is_a: CO_325:1000011 ! Estimation
relationship: method_of CO_325:0000256 ! petiole margins winged

[Term]
id: CO_325:0010165
name: petiole margin clasping - estimation
namespace: BananaMethod
def: "Observations on the margins and petiole wings should be made where the petiole and pseudostem meet at shooting. Observation should be made at shooting on the neck, where the petiole and pseudostem meet. Margin is the part of the petiole that can be bent outwards/inwards. [x Observe at flowering time.]" []
is_a: CO_325:1000011 ! Estimation
relationship: method_of CO_325:0000260 ! petiole margins clasping

[Term]
id: CO_325:0010166
name: petiole margin colour - estimation
namespace: BananaMethod
def: "Observations on the margins and petiole wings should be made where the petiole and pseudostem meet at shooting. Use colour chart A and observe out of direct sunlight. Record the colour of the margin (general colour is below the rim). [x Observe at flowering time.]" []
is_a: CO_325:1000011 ! Estimation
relationship: method_of CO_325:0000264 ! petiole margin colour

[Term]
id: CO_325:0010167
name: colour line along edge of petiole margin - estimation
namespace: BananaMethod
def: "Observations on the margins and petiole wings should be made where the petiole and pseudostem meet at shooting. Record on the last developed leaf at [x flowering stage] [shooting]." []
is_a: CO_325:1000011 ! Estimation
relationship: method_of CO_325:0000248 ! colour line along edge of petiole margin

[Term]
id: CO_325:0010168
name: pigmentation of outer surface of cigar leaf - estimation
namespace: BananaMethod
def: "Visually observe the pigmentation of the outer surface of the cigar leaf of a developed sucker or on another plant of the same accession. [x Observation should be made before shooting, on a developed sucker or on another plant of the same accession.]" []
is_a: CO_325:1000011 ! Estimation
relationship: method_of CO_325:0000252 ! pigmentation of outer surface of cigar leaf on sucker

[Term]
id: CO_325:0010169
name: bunch position - estimation
namespace: BananaMethod
def: "Visually observe the angle of the bunch and choose the option that is most similar, from the 5 schematic drawings of descriptor 6.4.6 in the reference material." []
is_a: CO_325:1000011 ! Estimation
relationship: method_of CO_325:0000438 ! bunch position

[Term]
id: CO_325:0010170
name: bunch shape - estimation
namespace: BananaMethod
def: "Visually observe the shape of the mature bunch on a fully developed plant that is not experiencing environmental stress and choose the option that is most similar, from the 4 photos of descriptor 6.4.7. in the reference material." []
is_a: CO_325:1000011 ! Estimation
relationship: method_of CO_325:0000440 ! bunch shape

[Term]
id: CO_325:0010171
name: male rachis type - estimation
namespace: BananaMethod
def: "Visually observe the part of the rachis between the last hand and the male bud. Truncated means there is no bract scar below the last hand. Present means there is a degenerated or persistent male bud" []
is_a: CO_325:1000011 ! Estimation
relationship: method_of CO_325:0000442 ! male rachis type

[Term]
id: CO_325:0010172
name: male rachis position - estimation
namespace: BananaMethod
def: "Visually observe the male rachis position (the part between the last hand and the male bud) and choose the option that is most similar, from the 5 schematic drawings of descriptor 6.4.12 in the reference material." []
is_a: CO_325:1000011 ! Estimation
relationship: method_of CO_325:0000444 ! male rachis position

[Term]
id: CO_325:0010173
name: male rachis appearance - estimation
namespace: BananaMethod
def: "Visually observe the male rachis appearance and choose the option that is most similar." []
is_a: CO_325:1000011 ! Estimation
relationship: method_of CO_325:0000446 ! male rachis appearance

[Term]
id: CO_325:0010174
name: male bud shape - computation
namespace: BananaMethod
def: "Calculate the ratio w/y, i.e. the broadest width of the male bud to the total length of the male bud. Do not measure the dimensions along the bud but rather on a projection/outline of the bud (e.g. trace the outline of the bud on paper) and use ruler or measuring tape." []
is_a: CO_325:1000010 ! Computation
relationship: method_of CO_325:0000448 ! male bud shape

[Term]
id: CO_325:0010175
name: male bud length - measurement
namespace: BananaMethod
def: "Measure the length (y) of a projection/outline of the male bud on paper, with a measuring tape or ruler." []
is_a: CO_325:1000008 ! Measurement
relationship: method_of CO_325:0000451 ! male bud length

[Term]
id: CO_325:0010176
name: male bud size - measurement
namespace: BananaMethod
def: "Length and maximum diamter of male bud at harvest." []
is_a: CO_325:1000008 ! Measurement
relationship: method_of CO_325:0000451 ! male bud length

[Term]
id: CO_325:0010177
name: male bud metric length - measurement
namespace: BananaMethod
def: "Length of male bud at harvest." []
is_a: CO_325:1000008 ! Measurement
relationship: method_of CO_325:0000451 ! male bud length

[Term]
id: CO_325:0010178
name: male bud width - measurement
namespace: BananaMethod
def: "Width of male bud at harvest." []
is_a: CO_325:1000008 ! Measurement
relationship: method_of CO_325:0000857 ! male bud width

[Term]
id: CO_325:0010179
name: male bud shoulder - computation
namespace: BananaMethod
def: "Calculate the ratio w/y, i.e. the broadest width of the male bud to the total length of the male bud. Do not measure the dimensions along the bud but rather on a projection/outline of the bud (e.g. trace the outline of the bud on paper) and use ruler or measuring tape" []
is_a: CO_325:1000010 ! Computation
relationship: method_of CO_325:0000454 ! male bud shoulder

[Term]
id: CO_325:0010180
name: bract apex shape - estimation
namespace: BananaMethod
def: "Refers to the first external unlifted bract. Visually observe the apex shape of flattened bracts to determine shape and choose the option that is most similar, from the 4 photos of descriptor 6.5.2. in the reference material." []
is_a: CO_325:1000011 ! Estimation
relationship: method_of CO_325:0000456 ! bract apex shape

[Term]
id: CO_325:0010181
name: bract imbrication at apex of male bud - estimation
namespace: BananaMethod
def: "Visually observe the bract imbrication of the apex of the male bud and choose the option that is most similar, from the 3 photos of descriptor 6.5.3 in the reference material." []
is_a: CO_325:1000011 ! Estimation
relationship: method_of CO_325:0000459 ! bract imbrication at apex of male bud

[Term]
id: CO_325:0010182
name: bract behaviour before falling - estimation
namespace: BananaMethod
def: "Visually observe the last bract to lift from the hands, ideally when the bract has lifted to a horizontal position, and choose the option that is most similar, from the 2 photos of descriptpr 6.5.12 in the reference material." []
is_a: CO_325:1000011 ! Estimation
relationship: method_of CO_325:0000461 ! bract behaviour before falling

[Term]
id: CO_325:0010183
name: colour of bract external face - estimation
namespace: BananaMethod
def: "Visually observe the colour of the external face of the first unlifted bract. Use colour chart A and observe out of direct sunlight." []
is_a: CO_325:1000011 ! Estimation
relationship: method_of CO_325:0000463 ! colour of bract external face

[Term]
id: CO_325:0010184
name: colour of bract internal face - estimation
namespace: BananaMethod
def: "Visually observe the colour of the internal face of the first unlifted bract. Use colour chart A and observe out of direct sunlight." []
is_a: CO_325:1000011 ! Estimation
relationship: method_of CO_325:0000466 ! colour of bract internal face

[Term]
id: CO_325:0010185
name: compound tepal main colour - estimation
namespace: BananaMethod
def: "The following flower descriptors refer to the flowers at the axil of the first external unlifted bract. Fresh material must be used (make the observation as soon as you detach the bract/flower from the rachis). Visually observe the colour of the backside middle of tepal. Use colour chart B and observe out of direct sunlight." []
is_a: CO_325:1000011 ! Estimation
relationship: method_of CO_325:0000469 ! compound tepal main colour

[Term]
id: CO_325:0010186
name: lobe colour of tip of compound tepal - estimation
namespace: BananaMethod
def: "The following flower descriptors refer to the flowers at the axil of the first external unlifted bract. Fresh material must be used (make the observation as soon as you detach the bract/flower from the rachis). Visually observe the colour of the lobe at the tip of the tepal. Use colour chart B and observe out of direct sunlight." []
is_a: CO_325:1000011 ! Estimation
relationship: method_of CO_325:0000472 ! lobe colour of tip of compound tepal

[Term]
id: CO_325:0010187
name: anther colour - estimation
namespace: BananaMethod
def: "The following flower descriptors refer to the flowers at the axil of the first external unlifted bract. Fresh material must be used (make the observation as soon as you detach the bract/flower from the rachis). Visually observe the anther colour on the face opposite to the dehiscence split of the anther. Use colour chart B and observe out of direct sunlight." []
is_a: CO_325:1000011 ! Estimation
relationship: method_of CO_325:0000475 ! anther colour

[Term]
id: CO_325:0010188
name: number of hands on whole bunch - counting
namespace: BananaMethod
def: "On a bunch with mostly hands of > 10 fingers, a possible ultimate hand with 1-5 (rather smaller) fingers should not be counted." []
is_a: CO_325:1000009 ! Counting
relationship: method_of CO_325:0000478 ! number of hands on whole bunch

[Term]
id: CO_325:0010189
name: number of fruits on mid-hand of the bunch - counting
namespace: BananaMethod
def: "Count only fully developed fruit. If there is an even number of hands, there will be two middle hands. Count the middle hand that developed first." []
is_a: CO_325:1000009 ! Counting
relationship: method_of CO_325:0000480 ! number of fruits on mid-hand of the bunch

[Term]
id: CO_325:0010190
name: fruit length - exact value - measurement
namespace: BananaMethod
def: "Measure the length of the internal arc of a fruit, without pedicel. Record on the inner fruit in the middle of the mid-hand of the bunch. If there is an even number of hands, there will be two middle hands so use the upper hand that developed first. Record the exact value." []
is_a: CO_325:1000008 ! Measurement
relationship: method_of CO_325:0000482 ! fruit length

[Term]
id: CO_325:0010191
name: fruit length - range - measurement
namespace: BananaMethod
def: "Measure the length of the internal arc of a fruit, without pedicel. Record on the inner fruit in the middle of the mid-hand of the bunch. If there is an even number of hands, there will be two middle hands so use the upper hand that developed first. Record the range." []
is_a: CO_325:1000008 ! Measurement
relationship: method_of CO_325:0000482 ! fruit length

[Term]
id: CO_325:0010192
name: fruit shape of curve - estimation
namespace: BananaMethod
def: "Visually observe the shape of the curve of the fruit and choose the option that is most similar, from the 5 photos of descriptor 6.7.4. in the reference material. Observe the inner fruit in the middle of the mid-hand of the bunch. In case of an asymmetric bunch that has straight and curved fruits, please indicate it in the note section and score only the fruit on the upper side of the bunch." []
is_a: CO_325:1000011 ! Estimation
relationship: method_of CO_325:0000485 ! fruit shape of curve

[Term]
id: CO_325:0010193
name: fruit apex point - estimation
namespace: BananaMethod
def: "Visually observe the fruit apex point and choose the option that is most similar, from the 5 photos of descriptor 6.7.6 in the reference material." []
is_a: CO_325:1000011 ! Estimation
relationship: method_of CO_325:0000488 ! fruit apex point

[Term]
id: CO_325:0010194
name: remains of flower relicts at fruit apex - estimation
namespace: BananaMethod
def: "Visually observe the remains, or not, of flower relicts at the finger apex, and choose the option that is most similar, from the 4 photos of descriptor 6.7.7 in the reference materials." []
is_a: CO_325:1000011 ! Estimation
relationship: method_of CO_325:0000490 ! remains of flower relicts at fruit apex

[Term]
id: CO_325:0010195
name: fruit pedicel length - exact value - measurement
namespace: BananaMethod
def: "Measure from the scar on the rachis until the beginning of the fruit. Record on the inner fruit in the middle of the mid-hand of the bunch. Tip: use string to measure or trace outline of fruit on paper. Record the exact value." []
is_a: CO_325:1000008 ! Measurement
relationship: method_of CO_325:0000493 ! fruit pedicel length

[Term]
id: CO_325:0010196
name: fruit pedical length - range - measurement
namespace: BananaMethod
def: "Measure from the scar on the rachis until the beginning of the fruit. Record on the inner fruit in the middle of the mid-hand of the bunch. Tip: use string to measure or trace outline of fruit on paper. Record the range." []
is_a: CO_325:1000008 ! Measurement
relationship: method_of CO_325:0000493 ! fruit pedicel length

[Term]
id: CO_325:0010197
name: fusion of pedicels - estimation
namespace: BananaMethod
def: "Visually observe the fusion of pedicels and choose the option that is most similar, from the 3 photos of descriptor 6.7.11. in the reference materials. Observe before they join the rachis at the bract scar. Look upwards from the bottom of the bunch." []
is_a: CO_325:1000011 ! Estimation
relationship: method_of CO_325:0000496 ! fusion of pedicels

[Term]
id: CO_325:0010198
name: visual appearance - estimation
namespace: BananaMethod
def: "Subjective visual assessment of smashed and unsmashed fruit pulp" []
is_a: CO_325:1000011 ! Estimation
relationship: method_of CO_325:0000498 ! fruit smashed pulp colour
relationship: method_of CO_325:0000500 ! fruit unsmashed pulp colour

[Term]
id: CO_325:0010199
name: taste - estimation
namespace: BananaMethod
def: "Subjective taste assessment of smashed and unsmashed fruit pulp" []
is_a: CO_325:1000011 ! Estimation
relationship: method_of CO_325:0000502 ! fruit smashed pulp taste
relationship: method_of CO_325:0000504 ! fruit unsmashed pulp taste

[Term]
id: CO_325:0010200
name: finger feel - estimation
namespace: BananaMethod
def: "Finger feel assessment of smashed and unsmashed fruit pulp" []
is_a: CO_325:1000011 ! Estimation
relationship: method_of CO_325:0000506 ! fruit smashed pulp texture
relationship: method_of CO_325:0000508 ! fruit unsmashed pulp texture

[Term]
id: CO_325:0010201
name: smoothness-mouth feel - estimation
namespace: BananaMethod
def: "Mouth feel assessment of smashed and unsmashed fruit pulp" []
is_a: CO_325:1000011 ! Estimation
relationship: method_of CO_325:0000510 ! fruit smashed pulp smoothness-mouth feel
relationship: method_of CO_325:0000512 ! fruit unsmashed pulp smoothness-mouth feel

[Term]
id: CO_325:0010202
name: nosal smell - estimation
namespace: BananaMethod
def: "Nosal smell assessment of smashed and unsmashed fruit pulp aromas" []
is_a: CO_325:1000011 ! Estimation
relationship: method_of CO_325:0000514 ! fruit smashed pulp aroma/smell

[Term]
id: CO_325:0010203
name: dry matter content- calculation
namespace: BananaMethod
def: "Take a standard fresh weigth in grams (i.e. 100 g.) of fruit pulp and oven dry it 24hrs at 50 centigrade (measured from the middle finger of second hand), calculate the ratio fresh weight (g.)/dry weight (g.)measured from the middle finger of second hand)" []
is_a: CO_325:1000008 ! Measurement
relationship: method_of CO_325:0000859 ! fruit dry matter content

[Term]
id: CO_325:0010204
name: leaf area - measurement
namespace: BananaMethod
def: "top view image" []
is_a: CO_325:1000008 ! Measurement
relationship: method_of CO_325:0000921 ! projected top area
relationship: method_of CO_325:0000922 ! leaf area

[Term]
id: CO_325:0010205
name: leaf area ratio - computation
namespace: BananaMethod
def: "computation of top leaf area with total (loose) leaf area" []
is_a: CO_325:1000010 ! Computation
relationship: method_of CO_325:0000923 ! leaf area to plant area ratio

[Term]
id: CO_325:0010206
name: leaf length - measurement
namespace: BananaMethod
def: "the longest diagonal of a fitted ellips" []
is_a: CO_325:1000008 ! Measurement
relationship: method_of CO_325:0000924 ! total length of all leaves
relationship: method_of CO_325:0000925 ! single leaf length

[Term]
id: CO_325:0010207
name: leaf width - measurement
namespace: BananaMethod
def: "the shortest diagonal of a fitted ellips" []
is_a: CO_325:1000008 ! Measurement
relationship: method_of CO_325:0000926 ! single leaf width

[Term]
id: CO_325:0010208
name: leaf chlorosis - computation
namespace: BananaMethod
def: "ratio of non green to green plant pixels" []
is_a: CO_325:1000010 ! Computation
relationship: method_of CO_325:0000927 ! leaf chlorosis

[Term]
id: CO_325:0010209
name: dry weight - measurement
namespace: BananaMethod
def: "80?C, for 14 days, or longer untill dry" []
is_a: CO_325:1000008 ! Measurement
relationship: method_of CO_325:0000928 ! leaf dry weight
relationship: method_of CO_325:0000929 ! pseudostem dry weight
relationship: method_of CO_325:0000930 ! root dry weight
relationship: method_of CO_325:0000931 ! plant dry weight

[Term]
id: CO_325:0010210
name: ratio - computation
namespace: BananaMethod
def: "ratio of belowground (root) to aboveground (shoot) dry mass" []
is_a: CO_325:1000010 ! Computation
relationship: method_of CO_325:0000932 ! ratio root to shoot
relationship: method_of CO_325:0000947 ! leaf to whole plant mass ratio
relationship: method_of CO_325:0000948 ! pseudostem to whole plant mass ratio
relationship: method_of CO_325:0000949 ! root to whole plant mass ratio

[Term]
id: CO_325:0010211
name: water content - computation
namespace: BananaMethod
def: "leaf dry mass /leaf fresh mass" []
is_a: CO_325:1000010 ! Computation
relationship: method_of CO_325:0000933 ! leaf relative water content
relationship: method_of CO_325:0000934 ! pseudostem relative water content
relationship: method_of CO_325:0000935 ! root relative water content
relationship: method_of CO_325:0000936 ! plant relative water content

[Term]
id: CO_325:0010212
name: length - measurement
namespace: BananaMethod
def: "manual height measurement" []
is_a: CO_325:1000008 ! Measurement
relationship: method_of CO_325:0000937 ! pseudostem length

[Term]
id: CO_325:0010213
name: leaf number - counting
namespace: BananaMethod
def: "count the number of leaves" []
is_a: CO_325:1000009 ! Counting
relationship: method_of CO_325:0000938 ! leaf number
relationship: method_of CO_325:0000939 ! functional leaf number

[Term]
id: CO_325:0010214
name: water loss - measurement
namespace: BananaMethod
def: "weighing of water loss though system between timepoints (refer to experimental metadata)" []
is_a: CO_325:1000008 ! Measurement
relationship: method_of CO_325:0000940 ! system water loss
relationship: method_of CO_325:0000941 ! plant water loss
relationship: method_of CO_325:0000951 ! system water loss per leaf area

[Term]
id: CO_325:0010215
name: transpiration efficiency - computation
namespace: BananaMethod
def: "gram accumulated biomass per volume water transpired" []
is_a: CO_325:1000010 ! Computation
relationship: method_of CO_325:0000942 ! transpiration efficiency

[Term]
id: CO_325:0010216
name: fresh weight - measurement
namespace: BananaMethod
def: "weighing" []
is_a: CO_325:1000008 ! Measurement
relationship: method_of CO_325:0000943 ! leaf fresh weight
relationship: method_of CO_325:0000944 ! pseudostem fresh weight
relationship: method_of CO_325:0000945 ! root fresh weight
relationship: method_of CO_325:0000946 ! plant fresh weight

[Term]
id: CO_325:0010217
name: water loss rate - computation
namespace: BananaMethod
def: "measurement of system water loss between two timepoints (refer to experimental metadata)" []
is_a: CO_325:1000010 ! Computation
relationship: method_of CO_325:0000950 ! daily rate of water loss

[Term]
id: CO_325:0010218
name: growth - computation
namespace: BananaMethod
def: "dry weight difference between timepoints (refer to experimental metadata)" []
is_a: CO_325:1000010 ! Computation
relationship: method_of CO_325:0000952 ! dry plant growth
relationship: method_of CO_325:0000953 ! fresh plant growth
relationship: method_of CO_325:0000954 ! increase of leaf area
relationship: method_of CO_325:0000955 ! height increase of pseudostem
relationship: method_of CO_325:0000956 ! pseudostem height increase per leaf formed
relationship: method_of CO_325:0000957 ! leaves formed per pseudostem height increase

[Term]
id: CO_325:0010219
name: root necrosis caused by nematodes - estimation
namespace: BananaMethod
def: "Select at random five functional primary roots, at least 10 cm long. Reduce the length of the five selected roots to 10 cm and slice through the roots length-wise. Evaluate one half of each of the five roots for the percentage of root cortex showing necrosis. The maximum root necrosis per root half can be 20%, giving a maximum root necrosis of 100% for the five halves together. Mentally determine the necrosis of the individual roots (1 to 5) and sum these together to get the total root necrosis of the sample." []
is_a: CO_325:1000011 ! Estimation
relationship: method_of CO_325:0000123 ! root necrosis caused by nematodes

[Term]
id: CO_325:0010220
name: number of nematodes (unclassified spp.) per unit fresh root weight - method
namespace: BananaMethod
def: "Count from 100 ml of soil sample" []
is_a: CO_325:1000009 ! Counting
relationship: method_of CO_325:0000520 ! nematode population density per soil sample

[Term]
id: CO_325:0010221
name: nematode multiplication from single root inoculation - computation
namespace: BananaMethod
def: "calculation from count" []
is_a: CO_325:1000009 ! Counting
relationship: method_of CO_325:0000518 ! nematode reproduction factor (microplot screening)

[Term]
id: CO_325:0010222
name: number of nematodes (radopholus similis ) per unit of soil sample - method
namespace: BananaMethod
def: "Count from 100 ml of soil sample" []
is_a: CO_325:1000009 ! Counting
relationship: method_of CO_325:0000522 ! number of radopholus similis per soil sample

[Term]
id: CO_325:0010223
name: number of nematodes (helicotylenchus multicinctus) per unit of soil sample - method
namespace: BananaMethod
def: "Count from 100 ml of soil sample" []
is_a: CO_325:1000009 ! Counting
relationship: method_of CO_325:0000523 ! number of helicotylenchus multicinctus per soil sample

[Term]
id: CO_325:0010224
name: number of nematodes (rotylenchulus spp.) per unit of soil sample - method
namespace: BananaMethod
def: "Count from 100 ml of soil sample" []
is_a: CO_325:1000009 ! Counting
relationship: method_of CO_325:0000524 ! number of rotylenchulus spp.per soil sample

[Term]
id: CO_325:0010225
name: number of nematodes (meloidogyne spp.) per unit of soil sample - method
namespace: BananaMethod
def: "Count from 100 ml of soil sample" []
is_a: CO_325:1000009 ! Counting
relationship: method_of CO_325:0000526 ! number of meloidogyne spp. per soil sample

[Term]
id: CO_325:0010226
name: number of nematodes (pratylenchus spp.) per unit of soil sample - method
namespace: BananaMethod
def: "Count from 100 ml of soil sample" []
is_a: CO_325:1000009 ! Counting
relationship: method_of CO_325:0000527 ! number of pratylenchus spp. per soil sample

[Term]
id: CO_325:0010227
name: number of nematodes (hoplolaimus spp.) per unit of soil sample - method
namespace: BananaMethod
def: "Count from 100 ml of soil sample" []
is_a: CO_325:1000009 ! Counting
relationship: method_of CO_325:0000528 ! number of hoplolaimus spp. per soil sample

[Term]
id: CO_325:0010228
name: number of nematodes (pratylenchus goodeyi) per unit of soil sample - method
namespace: BananaMethod
def: "Count from 100 ml of soil sample" []
is_a: CO_325:1000009 ! Counting
relationship: method_of CO_325:0000529 ! number of pratylenchus goodeyi per soil sample

[Term]
id: CO_325:0010229
name: number of nematodes (pratylenchus coffeae) per unit of soil sample - method
namespace: BananaMethod
def: "Count from 100 ml of soil sample" []
is_a: CO_325:1000009 ! Counting
relationship: method_of CO_325:0000530 ! number of pratylenchus coffeae per soil sample

[Term]
id: CO_325:0010230
name: number of nematodes (radopholus similis ) per unit fresh root weight -method
namespace: BananaMethod
def: "Count from 10 g of chopped roots from the tested banana plant sample" []
is_a: CO_325:1000009 ! Counting
relationship: method_of CO_325:0000533 ! number of radopholus similis per fresh root weight

[Term]
id: CO_325:0010231
name: number of nematodes (meloidogyne spp.) per unit fresh root weight -method
namespace: BananaMethod
def: "Count from 10 g of chopped roots from the tested banana plant sample" []
is_a: CO_325:1000009 ! Counting
relationship: method_of CO_325:0000535 ! number of meloidogyne spp. per fresh root weight

[Term]
id: CO_325:0010232
name: number of nematodes (pratylenchus spp.) per unit fresh root weight -method
namespace: BananaMethod
def: "Count from 10 g of chopped roots from the tested banana plant sample" []
is_a: CO_325:1000009 ! Counting
relationship: method_of CO_325:0000537 ! number of pratylenchus spp. per fresh root weight

[Term]
id: CO_325:0010233
name: number of nematodes (hoplolaimus spp.) per unit fresh root weight -method
namespace: BananaMethod
def: "Count from 10 g of chopped roots from the tested banana plant sample" []
is_a: CO_325:1000009 ! Counting
relationship: method_of CO_325:0000539 ! number of hoplolaimus spp. per fresh root weight

[Term]
id: CO_325:0010234
name: number of nematodes (pratylenchus goodeyi) per unit fresh root weight -method
namespace: BananaMethod
def: "Count from 10 g of chopped roots from the tested banana plant sample" []
is_a: CO_325:1000009 ! Counting
relationship: method_of CO_325:0000541 ! number of pratylenchus goodeyi per fresh root weight

[Term]
id: CO_325:0010235
name: number of nematodes (pratylenchus coffeae) per unit fresh root weight -method
namespace: BananaMethod
def: "Count from 10 g of chopped roots from the tested banana plant sample" []
is_a: CO_325:1000009 ! Counting
relationship: method_of CO_325:0000543 ! number of pratylenchus coffeae per fresh root weight

[Term]
id: CO_325:0010237
name: percentage of pollen grain germinating - computation
namespace: BananaMethod
def: "Calculate as: number of germinated pollen grain divided by total number of pollen grain times 100" []
is_a: CO_325:1000010 ! Computation
relationship: method_of CO_325:0000967 ! pollen germination

[Term]
id: CO_325:0010238
name: percentage of pollen grain viable- computation
namespace: BananaMethod
is_a: CO_325:1000010 ! Computation

[Term]
id: CO_325:0010239
name: number of pollen grain per anther - counting
namespace: BananaMethod
def: "count under microscope number of pollen grain per anther" []
is_a: CO_325:1000009 ! Counting

[Term]
id: CO_325:0010240
name: percentage of leaf chlorosis - estimation
namespace: BananaMethod
def: "visual assement, in percentage, of the amount of leaf chlorosis, on a weekly basis of a detached leaf disk (usually until 50-60 days) on a petri dish" []
is_a: CO_325:1000011 ! Estimation

[Term]
id: CO_325:0010241
name: percentage of leaf necrosis - estimation
namespace: BananaMethod
def: "visual assessment, in percentage, of the amount of leaf necrosis, on a weekly basis of a detached leaf disk (usually until 50-60 days) on a petri dish" []
is_a: CO_325:1000011 ! Estimation

[Term]
id: CO_325:0010242
name: youngest leaf with black streak disease development stage  - estimation
namespace: BananaMethod
def: "Visually observe and record the amount of the surface area of a standing leaf that is affected by black leaf streak disease." []
is_a: CO_325:1000011 ! Estimation

[Term]
id: CO_325:0010243
name: PCR assay
namespace: BananaMethod
def: "polymerase chain reaction assay based estimation" []
is_a: CO_325:1000011 ! Estimation

[Term]
id: CO_325:0010245
name: fruit parthenocarpy - estimation
namespace: BananaMethod
def: "visual observation of seed presence in mature fruits" []
is_a: CO_325:1000011 ! Estimation

[Term]
id: CO_325:0010246
name: sucker behavior - estimation
namespace: BananaMethod
def: "On a banana plant evaluate the level of apical dominance of the sucker" []
is_a: CO_325:1000011 ! Estimation

[Term]
id: CO_325:0010247
name: bunch size - estimation
namespace: BananaMethod
def: "Visually observe the size of the mature green bunch and score its overall size" []
is_a: CO_325:1000011 ! Estimation

[Term]
id: CO_325:0010248
name: plant circumference at 100 cm - measurement
namespace: BananaMethod
def: "Measure the circumference of the pseudostem of the plant at 100 cm from the collar, or from the pseudostem base at the ground if the collar is not visible, using a tape measure." []
is_a: CO_325:0010025 ! plant circumference - measurement

[Term]
id: CO_325:0010249
name: plant circumference at 75 cm - measurement
namespace: BananaMethod
def: "Measure the circumference of the pseudostem of the plant at 75 cm from the collar, or from the pseudostem base at the ground if the collar is not visible, using a tape measure." []
is_a: CO_325:0010025 ! plant circumference - measurement

[Term]
id: CO_325:0010250
name: plant circumference at 20 cm - measurement
namespace: BananaMethod
def: "Measure the circumference of the pseudostem of the plant at 20 cm from the collar, or from the pseudostem base at the ground if the collar is not visible, using a tape measure." []
is_a: CO_325:0010025 ! plant circumference - measurement

[Term]
id: CO_325:0100002
name: open answer
namespace: BananaScale
is_a: CO_325:1000014 ! Text

[Term]
id: CO_325:0100003
name: day
namespace: BananaScale
is_a: CO_325:1000016 ! Duration
relationship: scale_of CO_325:0010011 ! time from planting to shooting - computation
relationship: scale_of CO_325:0010012 ! plant crop cycle - computation
relationship: scale_of CO_325:0010013 ! time from shooting to harvest - computation
relationship: scale_of CO_325:0010014 ! time from flowering to harvest - computation
relationship: scale_of CO_325:0010015 ! time from planting to death - computation
relationship: scale_of CO_325:0010016 ! time from harvest to death - computation
relationship: scale_of CO_325:0010017 ! ratoon crop cycle - computation
relationship: scale_of CO_325:0010104 ! time from planting to first youngest spotted leaf - computation
relationship: scale_of CO_325:0010122 ! black leaf streak disease incubation time - computation
relationship: scale_of CO_325:0010123 ! black leaf streak disease evolution time - computation
relationship: scale_of CO_325:0010133 ! time from start of crop cycle to first external disease symptoms caused by fusarium wilt - computation

[Term]
id: CO_325:0100004
name: leaf rank
namespace: BananaScale
is_a: CO_325:1000017 ! Numerical
relationship: scale_of CO_325:0010018 ! rank of marked youngest leaf - counting
relationship: scale_of CO_325:0010019 ! rank of previously marked leaf - counting
relationship: scale_of CO_325:0010102 ! youngest leaf spotted - counting
relationship: scale_of CO_325:0010108 ! rank of oldest standing leaf - counting

[Term]
id: CO_325:0100005
name: leaves/month
namespace: BananaScale
is_a: CO_325:1000017 ! Numerical
relationship: scale_of CO_325:0010020 ! monthly leaf emission rate - computation

[Term]
id: CO_325:0100006
name: leaves/week
namespace: BananaScale
is_a: CO_325:1000017 ! Numerical
relationship: scale_of CO_325:0010021 ! weekly leaf emission rate - computation

[Term]
id: CO_325:0100007
name: leaf
namespace: BananaScale
is_a: CO_325:1000017 ! Numerical
relationship: scale_of CO_325:0010022 ! number of functional leaves - counting
relationship: scale_of CO_325:0010105 ! number of spotted leaves - counting
relationship: scale_of CO_325:0010106 ! number of standing leaves - counting
relationship: scale_of CO_325:0010107 ! number of standing leaves - computation
relationship: scale_of CO_325:0010111 ! number of leaves with black leaf streak disease severity grade 0 - computation
relationship: scale_of CO_325:0010112 ! number of leaves with black leaf streak disease severity grade 1 - computation
relationship: scale_of CO_325:0010113 ! number of leaves with black leaf streak disease severity grade 2 - computation
relationship: scale_of CO_325:0010114 ! number of leaves with black leaf streak disease severity grade 3 - computation
relationship: scale_of CO_325:0010115 ! number of leaves with black leaf streak disease severity grade 4 - computation
relationship: scale_of CO_325:0010116 ! number of leaves with black leaf streak disease severity grade 5 - computation
relationship: scale_of CO_325:0010117 ! number of leaves with black leaf streak disease severity grade 6 - computation

[Term]
id: CO_325:0100008
name: cm
namespace: BananaScale
is_a: CO_325:1000017 ! Numerical
relationship: scale_of CO_325:0010023 ! plant height - petiole of two youngest leaves - measurement
relationship: scale_of CO_325:0010024 ! plant height - neck of peduncle - measurement
relationship: scale_of CO_325:0010025 ! plant circumference - measurement
relationship: scale_of CO_325:0010026 ! tallest sucker height - measurement
relationship: scale_of CO_325:0010034 ! bunch height - measurement
relationship: scale_of CO_325:0010035 ! bunch circumference - measurement
relationship: scale_of CO_325:0010056 ! finger external length - measurement
relationship: scale_of CO_325:0010057 ! average finger external length - computation
relationship: scale_of CO_325:0010058 ! finger internal length - measurement
relationship: scale_of CO_325:0010059 ! average finger internal length - computation
relationship: scale_of CO_325:0010060 ! finger circumference - measurement
relationship: scale_of CO_325:0010061 ! average finger circumference - computation
relationship: scale_of CO_325:0010062 ! finger lateral diameter - measurement
relationship: scale_of CO_325:0010063 ! average finger lateral diameter - computation
relationship: scale_of CO_325:0010064 ! fruit pulp lateral diameter - measurement
relationship: scale_of CO_325:0010065 ! average fruit pulp lateral diameter - computation
relationship: scale_of CO_325:0010124 ! extent of internal discolouration in corm of plant caused by fusarium wilt - estimation
relationship: scale_of CO_325:0010126 ! extent of internal discolouration in corm of tallest sucker caused by fusarium wilt - estimation
relationship: scale_of CO_325:0010155 ! corm size - measurement
relationship: scale_of CO_325:0010177 ! male bud metric length - measurement
relationship: scale_of CO_325:0010178 ! male bud width - measurement
relationship: scale_of CO_325:0010190 ! fruit length - exact value - measurement
relationship: scale_of CO_325:0010206 ! leaf length - measurement
relationship: scale_of CO_325:0010207 ! leaf width - measurement
relationship: scale_of CO_325:0010212 ! length - measurement
relationship: scale_of CO_325:0010218 ! growth - computation

[Term]
id: CO_325:0100009
name: maiden sucker
namespace: BananaScale
is_a: CO_325:1000017 ! Numerical
relationship: scale_of CO_325:0010027 ! number of maiden suckers - counting

[Term]
id: CO_325:0100010
name: sword sucker
namespace: BananaScale
is_a: CO_325:1000017 ! Numerical
relationship: scale_of CO_325:0010028 ! number of sword suckers - counting

[Term]
id: CO_325:0100011
name: peeper sucker
namespace: BananaScale
is_a: CO_325:1000017 ! Numerical
relationship: scale_of CO_325:0010029 ! number of peeper suckers - counting

[Term]
id: CO_325:0100012
name: water suckers
namespace: BananaScale
is_a: CO_325:1000017 ! Numerical
relationship: scale_of CO_325:0010030 ! number of water suckers - counting

[Term]
id: CO_325:0100013
name: sucker
namespace: BananaScale
is_a: CO_325:1000017 ! Numerical
relationship: scale_of CO_325:0010031 ! number of suckers - counting

[Term]
id: CO_325:0100014
name: bunch maturity
namespace: BananaScale
is_a: CO_325:1000015 ! Nominal
relationship: scale_of CO_325:0010032 ! bunch maturity stage - estimation

[Term]
id: CO_325:0100015
name: kg
namespace: BananaScale
is_a: CO_325:1000017 ! Numerical
relationship: scale_of CO_325:0010033 ! bunch weight - measurement
relationship: scale_of CO_325:0010036 ! rachis weight - measurement
relationship: scale_of CO_325:0010037 ! total finger weight - computation
relationship: scale_of CO_325:0010042 ! hand weight - measurement
relationship: scale_of CO_325:0010043 ! multiple hand weight - measurement
relationship: scale_of CO_325:0010044 ! average hand weight - computation
relationship: scale_of CO_325:0010045 ! average hand weight - all - computation

[Term]
id: CO_325:0100016
name: hand
namespace: BananaScale
is_a: CO_325:1000017 ! Numerical
relationship: scale_of CO_325:0010038 ! number of hands in bunch - counting
relationship: scale_of CO_325:0010048 ! number of hands measured - counting

[Term]
id: CO_325:0100017
name: finger
namespace: BananaScale
is_a: CO_325:1000017 ! Numerical
relationship: scale_of CO_325:0010039 ! number of fingers in bunch - counting
relationship: scale_of CO_325:0010040 ! number of fingers in bunch - estimation
relationship: scale_of CO_325:0010046 ! number of fingers in third hand - counting
relationship: scale_of CO_325:0010047 ! multiple number of fingers in hand - counting
relationship: scale_of CO_325:0010049 ! average number of fingers in hand - computation
relationship: scale_of CO_325:0010050 ! average number of fingers in bunch - bunch - computation
relationship: scale_of CO_325:0010051 ! average number of fingers in hand - hands - computation
relationship: scale_of CO_325:0010054 ! number of fingers measured - counting
relationship: scale_of CO_325:0010189 ! number of fruits on mid-hand of the bunch - counting

[Term]
id: CO_325:0100018
name: hand rank
namespace: BananaScale
is_a: CO_325:1000017 ! Numerical
relationship: scale_of CO_325:0010041 ! hand rank - counting

[Term]
id: CO_325:0100019
name: g
namespace: BananaScale
is_a: CO_325:1000017 ! Numerical
relationship: scale_of CO_325:0010052 ! finger weight - measurement
relationship: scale_of CO_325:0010053 ! multiple finger weight - measurement
relationship: scale_of CO_325:0010055 ! average finger weight - computation
relationship: scale_of CO_325:0010203 ! dry matter content- calculation
relationship: scale_of CO_325:0010209 ! dry weight - measurement
relationship: scale_of CO_325:0010216 ! fresh weight - measurement
relationship: scale_of CO_325:0010218 ! growth - computation

[Term]
id: CO_325:0100020
name: mm
namespace: BananaScale
is_a: CO_325:1000017 ! Numerical
relationship: scale_of CO_325:0010056 ! finger external length - measurement
relationship: scale_of CO_325:0010058 ! finger internal length - measurement
relationship: scale_of CO_325:0010060 ! finger circumference - measurement
relationship: scale_of CO_325:0010062 ! finger lateral diameter - measurement
relationship: scale_of CO_325:0010064 ! fruit pulp lateral diameter - measurement
relationship: scale_of CO_325:0010066 ! finger peel thickness - measurement
relationship: scale_of CO_325:0010067 ! average finger peel thickness - computation
relationship: scale_of CO_325:0010195 ! fruit pedicel length - exact value - measurement

[Term]
id: CO_325:0100021
name: plant
namespace: BananaScale
is_a: CO_325:1000017 ! Numerical
relationship: scale_of CO_325:0010068 ! number of plants planted - computation
relationship: scale_of CO_325:0010071 ! number of plants dead - computation
relationship: scale_of CO_325:0010072 ! number of plants harvested - computation
relationship: scale_of CO_325:0010073 ! number of plants not harvested - computation

[Term]
id: CO_325:0100022
name: m2
namespace: BananaScale
is_a: CO_325:1000017 ! Numerical
relationship: scale_of CO_325:0010069 ! plant spacing - computation

[Term]
id: CO_325:0100023
name: plants/unit of area
namespace: BananaScale
is_a: CO_325:1000017 ! Numerical
relationship: scale_of CO_325:0010070 ! plant density - computation
relationship: scale_of CO_325:0010075 ! death density - computation
relationship: scale_of CO_325:0010077 ! harvest density - computation
relationship: scale_of CO_325:0010079 ! non-harvest density - computation

[Term]
id: CO_325:0100024
name: plants dead/plants planted
namespace: BananaScale
is_a: CO_325:1000017 ! Numerical
relationship: scale_of CO_325:0010074 ! death proportion - computation

[Term]
id: CO_325:0100025
name: plants harvested/plants planted
namespace: BananaScale
is_a: CO_325:1000017 ! Numerical
relationship: scale_of CO_325:0010076 ! harvest proportion - computation

[Term]
id: CO_325:0100026
name: plants not harvested/plants planted
namespace: BananaScale
is_a: CO_325:1000017 ! Numerical
relationship: scale_of CO_325:0010078 ! non-harvest proportion - computation

[Term]
id: CO_325:0100027
name: crop cycle duration/year
namespace: BananaScale
is_a: CO_325:1000017 ! Numerical
relationship: scale_of CO_325:0010080 ! annual crop cycle proportion - computation

[Term]
id: CO_325:0100028
name: kg/plant/y
namespace: BananaScale
is_a: CO_325:1000017 ! Numerical
relationship: scale_of CO_325:0010081 ! annual plant productivity - computation

[Term]
id: CO_325:0100029
name: t/unit of area/y
namespace: BananaScale
is_a: CO_325:1000017 ! Numerical
relationship: scale_of CO_325:0010082 ! actual annual yield - computation
relationship: scale_of CO_325:0010083 ! potential annual yield - computation

[Term]
id: CO_325:0100030
name: bad good
namespace: BananaScale
is_a: CO_325:1000015 ! Nominal
relationship: scale_of CO_325:0010084 ! fruit pendulance - estimation
relationship: scale_of CO_325:0010085 ! bunch quality - estimation
relationship: scale_of CO_325:0010087 ! sucker quality - estimation

[Term]
id: CO_325:0100031
name: fruitfill
namespace: BananaScale
is_a: CO_325:1000015 ! Nominal
relationship: scale_of CO_325:0010086 ! fruitfill - estimation

[Term]
id: CO_325:0100032
name: dwarfism
namespace: BananaScale
is_a: CO_325:1000015 ! Nominal
relationship: scale_of CO_325:0010088 ! dwarfism - estimation

[Term]
id: CO_325:0100045
name: index of non-spotted leaves
namespace: BananaScale
is_a: CO_325:1000017 ! Numerical
relationship: scale_of CO_325:0010109 ! index of non-spotted leaves - computation

[Term]
id: CO_325:0100046
name: %
namespace: BananaScale
is_a: CO_325:1000017 ! Numerical
relationship: scale_of CO_325:0010110 ! black leaf streak disease severity - estimation
relationship: scale_of CO_325:0010134 ! percentage of plants with yellowing leaves caused by fusarium wilt - computation
relationship: scale_of CO_325:0010135 ! percentage of plants with a splitting pseudostem base caused by fusarium wilt - computation
relationship: scale_of CO_325:0010136 ! percentage of plants with changes in new leaves caused by fusarium wilt - computation
relationship: scale_of CO_325:0010137 ! percentage of plants with petiole collapse caused by fusarium wilt - computation
relationship: scale_of CO_325:0010138 ! percentage of plants with external disease symptoms caused by fusarium wilt - computation
relationship: scale_of CO_325:0010139 ! percentage of plants with internal disease symptoms caused by fusarium wilt - computation
relationship: scale_of CO_325:0010140 ! damage to upper inner corm weevils - measurement
relationship: scale_of CO_325:0010141 ! damage to upper outer corm weevils - measurement
relationship: scale_of CO_325:0010142 ! damage to lower inner corm weevils - measurement
relationship: scale_of CO_325:0010143 ! damage to lower outer corm weevils - measurement
relationship: scale_of CO_325:0010153 ! peripheral damage - measurement
relationship: scale_of CO_325:0010219 ! root necrosis caused by nematodes - estimation

[Term]
id: CO_325:0100047
name: gauhl's modification of stover's severity scoring system (yyyy)
namespace: BananaScale
is_a: CO_325:1000015 ! Nominal
relationship: scale_of CO_325:0010110 ! black leaf streak disease severity - estimation

[Term]
id: CO_325:0100048
name: Foure's stages of development of bls disease scale (1987)
namespace: BananaScale
is_a: CO_325:1000015 ! Nominal
relationship: scale_of CO_325:0010110 ! black leaf streak disease severity - estimation

[Term]
id: CO_325:0100049
name: meredith & lawrence (1969) - complete
namespace: BananaScale
is_a: CO_325:1000015 ! Nominal
relationship: scale_of CO_325:0010110 ! black leaf streak disease severity - estimation

[Term]
id: CO_325:0100050
name: meredith & lawrence (1969) - condensed
namespace: BananaScale
is_a: CO_325:1000015 ! Nominal
relationship: scale_of CO_325:0010110 ! black leaf streak disease severity - estimation

[Term]
id: CO_325:0100051
name: index of black leaf streak disease severity
namespace: BananaScale
is_a: CO_325:1000017 ! Numerical
relationship: scale_of CO_325:0010118 ! black leaf streak disease severity index - computation

[Term]
id: CO_325:0100052
name: 5 pt corm discolouration scale
namespace: BananaScale
is_a: CO_325:1000015 ! Nominal
relationship: scale_of CO_325:0010125 ! distance of internal discolouration in pseudostem of plant caused by fusarium wilt
relationship: scale_of CO_325:0010127 ! distance of internal discolouration in pseudostem of tallest sucker caused by fusarium wilt

[Term]
id: CO_325:0100053
name: presence absence 0
namespace: BananaScale
is_a: CO_325:1000015 ! Nominal
relationship: scale_of CO_325:0010128 ! presence of yellowing leaves caused by fusarium wilt - estimation
relationship: scale_of CO_325:0010129 ! presence of splitting pseudostem base caused by fusarium wilt - estimation
relationship: scale_of CO_325:0010130 ! presence of changes in new leaves caused by fusarium wilt - estimation
relationship: scale_of CO_325:0010131 ! presence of petiole collapse caused by fusarium wilt - estimation

[Term]
id: CO_325:0100054
name: presence absence 1
namespace: BananaScale
is_a: CO_325:1000015 ! Nominal
relationship: scale_of CO_325:0010128 ! presence of yellowing leaves caused by fusarium wilt - estimation
relationship: scale_of CO_325:0010129 ! presence of splitting pseudostem base caused by fusarium wilt - estimation
relationship: scale_of CO_325:0010130 ! presence of changes in new leaves caused by fusarium wilt - estimation
relationship: scale_of CO_325:0010131 ! presence of petiole collapse caused by fusarium wilt - estimation

[Term]
id: CO_325:0100055
name: weevil
namespace: BananaScale
is_a: CO_325:1000017 ! Numerical
relationship: scale_of CO_325:0010144 ! number of adult weevil trap - counting
relationship: scale_of CO_325:0010145 ! number of adult weevils - counting
relationship: scale_of CO_325:0010146 ! number of weevil larvae - counting
relationship: scale_of CO_325:0010147 ! number of adult larvae - counting

[Term]
id: CO_325:0100056
name: m
namespace: BananaScale
is_a: CO_325:1000017 ! Numerical
relationship: scale_of CO_325:0010148 ! adult weevil head capsule - measurement
relationship: scale_of CO_325:0010149 ! adult weevil body - measurement
relationship: scale_of CO_325:0010150 ! weevil larvae head capsule - measurement
relationship: scale_of CO_325:0010151 ! weevil larvae body length - measurement

[Term]
id: CO_325:0100057
name: mg
namespace: BananaScale
is_a: CO_325:1000017 ! Numerical
relationship: scale_of CO_325:0010149 ! adult weevil body - measurement
relationship: scale_of CO_325:0010152 ! weevil larvae body weight - measurement

[Term]
id: CO_325:0100058
name: weevil damage
namespace: BananaScale
is_a: CO_325:1000015 ! Nominal
relationship: scale_of CO_325:0010154 ! weevil damage -estimation

[Term]
id: CO_325:0100059
name: dead roots
namespace: BananaScale
is_a: CO_325:1000017 ! Numerical
relationship: scale_of CO_325:0010156 ! number of dead roots - counting

[Term]
id: CO_325:0100060
name: functional roots
namespace: BananaScale
is_a: CO_325:1000017 ! Numerical
relationship: scale_of CO_325:0010157 ! number of functional roots - counting

[Term]
id: CO_325:0100061
name: nematodes/unit of fresh root weight
namespace: BananaScale
is_a: CO_325:1000017 ! Numerical
relationship: scale_of CO_325:0010158 ! root nematode density - computation

[Term]
id: CO_325:0100062
name: height score (1 to 3)
namespace: BananaScale
is_a: CO_325:1000012 ! Ordinal
relationship: scale_of CO_325:0010159 ! pseudostem height - estimation

[Term]
id: CO_325:0100063
name: bd colour chart a - 2016
namespace: BananaScale
is_a: CO_325:1000015 ! Nominal
relationship: scale_of CO_325:0010160 ! pseudostem colour - estimation
relationship: scale_of CO_325:0010166 ! petiole margin colour - estimation
relationship: scale_of CO_325:0010168 ! pigmentation of outer surface of cigar leaf - estimation
relationship: scale_of CO_325:0010183 ! colour of bract external face - estimation
relationship: scale_of CO_325:0010184 ! colour of bract internal face - estimation

[Term]
id: CO_325:0100064
name: blotch pigmentation scale (1 to 4)
namespace: BananaScale
is_a: CO_325:1000015 ! Nominal
relationship: scale_of CO_325:0010161 ! blotches area - estimation

[Term]
id: CO_325:0100065
name: blotch pigmentation scale (1 to 5)
namespace: BananaScale
is_a: CO_325:1000015 ! Nominal
relationship: scale_of CO_325:0010161 ! blotches area - estimation

[Term]
id: CO_325:0100066
name: blotch color scale (1 to 4)
namespace: BananaScale
is_a: CO_325:1000015 ! Nominal
relationship: scale_of CO_325:0010162 ! blotches colour - estimation

[Term]
id: CO_325:0100067
name: blotch color scale (1 to 5)
namespace: BananaScale
is_a: CO_325:1000015 ! Nominal
relationship: scale_of CO_325:0010162 ! blotches colour - estimation

[Term]
id: CO_325:0100068
name: margin behaviour scale (1 to 4)
namespace: BananaScale
is_a: CO_325:1000015 ! Nominal
relationship: scale_of CO_325:0010163 ! margin behaviour on petiole canal of third leaf - estimation

[Term]
id: CO_325:0100069
name: margin behaviour scale (1 to 5)
namespace: BananaScale
is_a: CO_325:1000015 ! Nominal
relationship: scale_of CO_325:0010163 ! margin behaviour on petiole canal of third leaf - estimation

[Term]
id: CO_325:0100070
name: wing presence/absence
namespace: BananaScale
is_a: CO_325:1000015 ! Nominal
relationship: scale_of CO_325:0010164 ! winged petiole margin - estimation

[Term]
id: CO_325:0100071
name: wing presence/absence and clasping presence/absence scale 1 to 5
namespace: BananaScale
is_a: CO_325:1000015 ! Nominal
relationship: scale_of CO_325:0010164 ! winged petiole margin - estimation

[Term]
id: CO_325:0100072
name: clasping or not clasping
namespace: BananaScale
is_a: CO_325:1000015 ! Nominal
relationship: scale_of CO_325:0010165 ! petiole margin clasping - estimation

[Term]
id: CO_325:0100073
name: bd colour chart a - 1996
namespace: BananaScale
is_a: CO_325:1000015 ! Nominal
relationship: scale_of CO_325:0010166 ! petiole margin colour - estimation
relationship: scale_of CO_325:0010183 ! colour of bract external face - estimation
relationship: scale_of CO_325:0010184 ! colour of bract internal face - estimation

[Term]
id: CO_325:0100074
name: petiole-margin contrast
namespace: BananaScale
is_a: CO_325:1000015 ! Nominal
relationship: scale_of CO_325:0010167 ! colour line along edge of petiole margin - estimation

[Term]
id: CO_325:0100075
name: bunch position scale(1 to 5)
namespace: BananaScale
is_a: CO_325:1000015 ! Nominal
relationship: scale_of CO_325:0010169 ! bunch position - estimation

[Term]
id: CO_325:0100076
name: bunch shape scale (1 to 5)
namespace: BananaScale
is_a: CO_325:1000015 ! Nominal
relationship: scale_of CO_325:0010170 ! bunch shape - estimation

[Term]
id: CO_325:0100077
name: rachis type scale (1 to 2)
namespace: BananaScale
is_a: CO_325:1000015 ! Nominal
relationship: scale_of CO_325:0010171 ! male rachis type - estimation

[Term]
id: CO_325:0100078
name: rachis angle scale (1 to 2)
namespace: BananaScale
is_a: CO_325:1000015 ! Nominal
relationship: scale_of CO_325:0010172 ! male rachis position - estimation

[Term]
id: CO_325:0100079
name: rachis appearance scale (1 to 5)
namespace: BananaScale
is_a: CO_325:1000015 ! Nominal
relationship: scale_of CO_325:0010173 ! male rachis appearance - estimation

[Term]
id: CO_325:0100080
name: bud shape scale (1 to 3)
namespace: BananaScale
is_a: CO_325:1000015 ! Nominal
relationship: scale_of CO_325:0010174 ! male bud shape - computation

[Term]
id: CO_325:0100081
name: bud shape scale (1 to 5)
namespace: BananaScale
is_a: CO_325:1000015 ! Nominal
relationship: scale_of CO_325:0010174 ! male bud shape - computation

[Term]
id: CO_325:0100082
name: bud length scale (1 to 3)
namespace: BananaScale
is_a: CO_325:1000015 ! Nominal
relationship: scale_of CO_325:0010175 ! male bud length - measurement

[Term]
id: CO_325:0100083
name: bud size scale (1 to 3)
namespace: BananaScale
is_a: CO_325:1000015 ! Nominal
relationship: scale_of CO_325:0010176 ! male bud size - measurement

[Term]
id: CO_325:0100084
name: bud shoulder scale (1 to 3)
namespace: BananaScale
is_a: CO_325:1000015 ! Nominal
relationship: scale_of CO_325:0010179 ! male bud shoulder - computation

[Term]
id: CO_325:0100085
name: bract apex scale (1 to 4)
namespace: BananaScale
is_a: CO_325:1000015 ! Nominal
relationship: scale_of CO_325:0010180 ! bract apex shape - estimation

[Term]
id: CO_325:0100086
name: bract apex scale (1 to 5)
namespace: BananaScale
is_a: CO_325:1000015 ! Nominal
relationship: scale_of CO_325:0010180 ! bract apex shape - estimation

[Term]
id: CO_325:0100087
name: bract imbrication scale (1 to 3)
namespace: BananaScale
is_a: CO_325:1000015 ! Nominal
relationship: scale_of CO_325:0010181 ! bract imbrication at apex of male bud - estimation

[Term]
id: CO_325:0100088
name: bract behaviour scale (1 to 2)
namespace: BananaScale
is_a: CO_325:1000015 ! Nominal
relationship: scale_of CO_325:0010182 ! bract behaviour before falling - estimation

[Term]
id: CO_325:0100089
name: bd colour chart b - 2016
namespace: BananaScale
is_a: CO_325:1000015 ! Nominal
relationship: scale_of CO_325:0010185 ! compound tepal main colour - estimation
relationship: scale_of CO_325:0010186 ! lobe colour of tip of compound tepal - estimation
relationship: scale_of CO_325:0010187 ! anther colour - estimation

[Term]
id: CO_325:0100090
name: bd colour chart b - 1996
namespace: BananaScale
is_a: CO_325:1000015 ! Nominal
relationship: scale_of CO_325:0010185 ! compound tepal main colour - estimation
relationship: scale_of CO_325:0010186 ! lobe colour of tip of compound tepal - estimation
relationship: scale_of CO_325:0010187 ! anther colour - estimation

[Term]
id: CO_325:0100091
name: hands
namespace: BananaScale
is_a: CO_325:1000017 ! Numerical
relationship: scale_of CO_325:0010188 ! number of hands on whole bunch - counting

[Term]
id: CO_325:0100092
name: fruit length scale (1 to 5)
namespace: BananaScale
is_a: CO_325:1000012 ! Ordinal
relationship: scale_of CO_325:0010191 ! fruit length - range - measurement

[Term]
id: CO_325:0100093
name: fruit curve shape (scale 1 to 6)
namespace: BananaScale
is_a: CO_325:1000015 ! Nominal
relationship: scale_of CO_325:0010192 ! fruit shape of curve - estimation

[Term]
id: CO_325:0100094
name: fruit curve shape (scale 1 to 5)
namespace: BananaScale
is_a: CO_325:1000015 ! Nominal
relationship: scale_of CO_325:0010192 ! fruit shape of curve - estimation

[Term]
id: CO_325:0100095
name: fruit apex scale (1 to 5)
namespace: BananaScale
is_a: CO_325:1000015 ! Nominal
relationship: scale_of CO_325:0010193 ! fruit apex point - estimation

[Term]
id: CO_325:0100096
name: fruit relicts scale (1 to 4)
namespace: BananaScale
is_a: CO_325:1000015 ! Nominal
relationship: scale_of CO_325:0010194 ! remains of flower relicts at fruit apex - estimation

[Term]
id: CO_325:0100097
name: fruit relicts scale (1 to 3)
namespace: BananaScale
is_a: CO_325:1000015 ! Nominal
relationship: scale_of CO_325:0010194 ! remains of flower relicts at fruit apex - estimation

[Term]
id: CO_325:0100098
name: fruit pedicel scale (1 to 3)
namespace: BananaScale
is_a: CO_325:1000012 ! Ordinal
relationship: scale_of CO_325:0010196 ! fruit pedical length - range - measurement

[Term]
id: CO_325:0100099
name: fusion of pedicel scale (1 to 2)
namespace: BananaScale
is_a: CO_325:1000015 ! Nominal
relationship: scale_of CO_325:0010197 ! fusion of pedicels - estimation

[Term]
id: CO_325:0100100
name: 1 to 5 acceptability score
namespace: BananaScale
is_a: CO_325:1000015 ! Nominal
relationship: scale_of CO_325:0010198 ! visual appearance - estimation
relationship: scale_of CO_325:0010199 ! taste - estimation
relationship: scale_of CO_325:0010200 ! finger feel - estimation
relationship: scale_of CO_325:0010201 ! smoothness-mouth feel - estimation
relationship: scale_of CO_325:0010202 ! nosal smell - estimation

[Term]
id: CO_325:0100101
name: cm2
namespace: BananaScale
is_a: CO_325:1000017 ! Numerical
relationship: scale_of CO_325:0010204 ! leaf area - measurement
relationship: scale_of CO_325:0010218 ! growth - computation

[Term]
id: CO_325:0100102
name: unitless
namespace: BananaScale
is_a: CO_325:1000017 ! Numerical
relationship: scale_of CO_325:0010205 ! leaf area ratio - computation
relationship: scale_of CO_325:0010208 ! leaf chlorosis - computation
relationship: scale_of CO_325:0010210 ! ratio - computation
relationship: scale_of CO_325:0010211 ! water content - computation
relationship: scale_of CO_325:0010213 ! leaf number - counting

[Term]
id: CO_325:0100103
name: ml
namespace: BananaScale
is_a: CO_325:1000017 ! Numerical
relationship: scale_of CO_325:0010214 ! water loss - measurement
relationship: scale_of CO_325:0010217 ! water loss rate - computation

[Term]
id: CO_325:0100104
name: g / ml
namespace: BananaScale
is_a: CO_325:1000017 ! Numerical
relationship: scale_of CO_325:0010215 ! transpiration efficiency - computation

[Term]
id: CO_325:0100105
name: ml / cm2
namespace: BananaScale
is_a: CO_325:1000017 ! Numerical
relationship: scale_of CO_325:0010214 ! water loss - measurement

[Term]
id: CO_325:0100106
name: []/cm
namespace: BananaScale
is_a: CO_325:1000017 ! Numerical
relationship: scale_of CO_325:0010218 ! growth - computation

[Term]
id: CO_325:0100107
name: no. per 100ml
namespace: BananaScale
is_a: CO_325:1000017 ! Numerical
relationship: scale_of CO_325:0010220 ! number of nematodes (unclassified spp.) per unit fresh root weight - method

[Term]
id: CO_325:0100108
name: multiplication factor
namespace: BananaScale
is_a: CO_325:1000017 ! Numerical
relationship: scale_of CO_325:0010221 ! nematode multiplication from single root inoculation - computation

[Term]
id: CO_325:0100109
name: no. per 100 ml
namespace: BananaScale
is_a: CO_325:1000017 ! Numerical
relationship: scale_of CO_325:0010222 ! number of nematodes (radopholus similis ) per unit of soil sample - method
relationship: scale_of CO_325:0010223 ! number of nematodes (helicotylenchus multicinctus) per unit of soil sample - method
relationship: scale_of CO_325:0010224 ! number of nematodes (rotylenchulus spp.) per unit of soil sample - method
relationship: scale_of CO_325:0010225 ! number of nematodes (meloidogyne spp.) per unit of soil sample - method
relationship: scale_of CO_325:0010226 ! number of nematodes (pratylenchus spp.) per unit of soil sample - method
relationship: scale_of CO_325:0010227 ! number of nematodes (hoplolaimus spp.) per unit of soil sample - method
relationship: scale_of CO_325:0010228 ! number of nematodes (pratylenchus goodeyi) per unit of soil sample - method
relationship: scale_of CO_325:0010229 ! number of nematodes (pratylenchus coffeae) per unit of soil sample - method

[Term]
id: CO_325:0100110
name: no. per 10g
namespace: BananaScale
is_a: CO_325:1000017 ! Numerical
relationship: scale_of CO_325:0010230 ! number of nematodes (radopholus similis ) per unit fresh root weight -method
relationship: scale_of CO_325:0010231 ! number of nematodes (meloidogyne spp.) per unit fresh root weight -method
relationship: scale_of CO_325:0010232 ! number of nematodes (pratylenchus spp.) per unit fresh root weight -method
relationship: scale_of CO_325:0010233 ! number of nematodes (hoplolaimus spp.) per unit fresh root weight -method
relationship: scale_of CO_325:0010234 ! number of nematodes (pratylenchus goodeyi) per unit fresh root weight -method
relationship: scale_of CO_325:0010235 ! number of nematodes (pratylenchus coffeae) per unit fresh root weight -method

[Term]
id: CO_325:0100111
name: fully green
namespace: BananaScale
synonym: "1" EXACT []
is_a: CO_325:0100014 ! bunch maturity

[Term]
id: CO_325:0100112
name: one yellow finger
namespace: BananaScale
synonym: "2" EXACT []
is_a: CO_325:0100014 ! bunch maturity

[Term]
id: CO_325:0100113
name: bad
namespace: BananaScale
synonym: "1" EXACT []
is_a: CO_325:0100030 ! bad good

[Term]
id: CO_325:0100114
name: good
namespace: BananaScale
synonym: "2" EXACT []
is_a: CO_325:0100030 ! bad good

[Term]
id: CO_325:0100115
name: fruitfilled
namespace: BananaScale
synonym: "1" EXACT []
is_a: CO_325:0100031 ! fruitfill

[Term]
id: CO_325:0100116
name: not fruitfilled
namespace: BananaScale
synonym: "2" EXACT []
is_a: CO_325:0100031 ! fruitfill

[Term]
id: CO_325:0100117
name: dwarf
namespace: BananaScale
synonym: "1" EXACT []
is_a: CO_325:0100032 ! dwarfism

[Term]
id: CO_325:0100118
name: not dwarf
namespace: BananaScale
synonym: "2" EXACT []
is_a: CO_325:0100032 ! dwarfism

[Term]
id: CO_325:0100119
name: no symptoms
namespace: BananaScale
synonym: "0" EXACT []
is_a: CO_325:0100047 ! gauhl's modification of stover's severity scoring system (yyyy)

[Term]
id: CO_325:0100120
name: less than 1% of lamina with symptoms, only streaks and/or up to 10 spots
namespace: BananaScale
synonym: "1" EXACT []
is_a: CO_325:0100047 ! gauhl's modification of stover's severity scoring system (yyyy)

[Term]
id: CO_325:0100121
name: 1-5% of lamina with symptoms
namespace: BananaScale
synonym: "2" EXACT []
is_a: CO_325:0100047 ! gauhl's modification of stover's severity scoring system (yyyy)

[Term]
id: CO_325:0100122
name: 6-15% of lamina with symptoms
namespace: BananaScale
synonym: "3" EXACT []
is_a: CO_325:0100047 ! gauhl's modification of stover's severity scoring system (yyyy)

[Term]
id: CO_325:0100123
name: 16-33% of lamina with symptoms
namespace: BananaScale
synonym: "4" EXACT []
is_a: CO_325:0100047 ! gauhl's modification of stover's severity scoring system (yyyy)

[Term]
id: CO_325:0100124
name: 34-50% of lamina with symptoms
namespace: BananaScale
synonym: "5" EXACT []
is_a: CO_325:0100047 ! gauhl's modification of stover's severity scoring system (yyyy)

[Term]
id: CO_325:0100125
name: 51-100% of lamina with symptoms
namespace: BananaScale
synonym: "6" EXACT []
is_a: CO_325:0100047 ! gauhl's modification of stover's severity scoring system (yyyy)

[Term]
id: CO_325:0100126
name: Stage 1 appears as a small depigmentation spot whose whitish or yellow colour resembles stage 1 of Yellow Sigatoka disease. These symptoms are not visible in transmitted light and can be observed only on the underside of the leaf.
namespace: BananaScale
synonym: "1" EXACT []
is_a: CO_325:0100048 ! Foure's stages of development of bls disease scale (1987)

[Term]
id: CO_325:0100127
name: Stage 2 appears as a stripe, generally brown in colour and visible on the underside of the leaf; later the symptom also appears on the upper part of the limb as a stripe, the yellow colour of which resembles the stripe at stage 1 of Yellow Sigatoka. The colour of this stripe will change progressively from brown and later to black on the upper side of the limb, but will retain the brown colour on the underside.
namespace: BananaScale
synonym: "2" EXACT []
is_a: CO_325:0100048 ! Foure's stages of development of bls disease scale (1987)

[Term]
id: CO_325:0100128
name: Stage 3 differs from the previous one by its dimensions. The stripe becomes longer, is enlarged and in certain conditions (weak inoculum and unfavourable climatic conditions) can reach 2 or 3 cm.
namespace: BananaScale
synonym: "3" EXACT []
is_a: CO_325:0100048 ! Foure's stages of development of bls disease scale (1987)

[Term]
id: CO_325:0100129
name: Stage 4 appears on the underside as a brown spot and on the upper side as a black spot.
namespace: BananaScale
synonym: "4" EXACT []
is_a: CO_325:0100048 ! Foure's stages of development of bls disease scale (1987)

[Term]
id: CO_325:0100130
name: Stage 5 is when the elliptical spot is totally black and has spread to the underside of the limb. It is surrounded by a yellow halo with the centre beginning to flatten out.
namespace: BananaScale
synonym: "5" EXACT []
is_a: CO_325:0100048 ! Foure's stages of development of bls disease scale (1987)

[Term]
id: CO_325:0100131
name: Stage 6 is when the centre of the spot dries out, turns clear gray and is surrounded by a well-defined black ring, which is, in turn, surrounded by a bright yellow halo. These spots remain visible after the leaf has dried out because the ring persists.
namespace: BananaScale
synonym: "6" EXACT []
is_a: CO_325:0100048 ! Foure's stages of development of bls disease scale (1987)

[Term]
id: CO_325:0100132
name: Initial speck stage: symptoms are first visible to the naked eye as faint, minute (less than 0.25 mm diam), reddish brown specks on the lower surface of the leaf. Specks are often most abundant near the margin of the left side of the leaf, particularly towards the tip. Where leaf spot is severe, specks have been observed on the second leaf of plants that have not yet produced a bunch. Elsewhere they usually appear on the third, fourth, or older leaves.
namespace: BananaScale
synonym: "1" EXACT []
is_a: CO_325:0100049 ! meredith & lawrence (1969) - complete

[Term]
id: CO_325:0100133
name: First streak stage: the initial speck elongates, becoming slightly wider, to form a characteristic narrow, reddish brown streak up to 20 mm long and 2.0 mm wide, with the long axis parallel to the leaf venation. At this stage, streaks are more clearly visible on the lower surface of the leaf than on the upper one. The distribution of streaks is variable. Sometimes they are most numerous near the edge of the left side of the leaf. At other times they are equally numerous on both sides of the leaf, and more or less evenly distributed. Frequently they are densely aggregated in a band several cm wide on one side or both sides of the mid-rib, becoming less numerous towards the edge of the leaf. Streaks may be so numerous that every cm2 of leaf surface bears one or more. There is considerable variation in the length of individual streaks on a given leaf, and they frequently overlap to form larger, compound streaks.
namespace: BananaScale
synonym: "2" EXACT []
is_a: CO_325:0100049 ! meredith & lawrence (1969) - complete

[Term]
id: CO_325:0100134
name: Second-streak stage: the streaks may elongate slightly, but the most notable change is that in colour from reddish brown to dark brown or almost black, sometimes with a purplish tinge. The streak is now clearly visible on the upper surface of the leaf. The distribution of streaks at this stage of development varies in the same way as mentioned above. When streaks are very numerous, and more or less evenly distributed, the entire leaf blackens.
namespace: BananaScale
synonym: "3" EXACT []
is_a: CO_325:0100049 ! meredith & lawrence (1969) - complete

[Term]
id: CO_325:0100135
name: First-spot stage: the streak broadens and becomes more or less fusiform and elliptical in outline and similar to the 'first-spot stage' of Sigatoka (Leach 1946). The transition from streak to spot is further characterised by the development of a light brown, water-soaked border around the spot. This water-soaked effect is especially clear in the early morning, when dew is still present on the leaf, or after rain.
namespace: BananaScale
synonym: "4" EXACT []
is_a: CO_325:0100049 ! meredith & lawrence (1969) - complete

[Term]
id: CO_325:0100136
name: Second-spot stage: the dark brown or black central area of the spot becomes slightly depressed and the water-soaked border becomes more pronounced due to darkening. At this stage, a slight yellowing of the leaf tissue immediately surrounding the water-soaked border may occur.
namespace: BananaScale
synonym: "5" EXACT []
is_a: CO_325:0100049 ! meredith & lawrence (1969) - complete

[Term]
id: CO_325:0100137
name: Third or mature spot stage: the centre of the spot dries out, becoming light grey or buff-coloured, and further depressed. The spot is surrounded by a narrow, well-defined, dark brown or black border. between the latter and the normal green colour of the leaf, there is often a bright yellow transitional zone. After the leaf has collapsed and withered, spots remain clearly visible because of the light-coloured centre and dark border.
namespace: BananaScale
synonym: "6" EXACT []
is_a: CO_325:0100049 ! meredith & lawrence (1969) - complete

[Term]
id: CO_325:0100138
name: Initial speck stage: faint, minute, reddish-brown specks on the lower surface of the leaf.
namespace: BananaScale
synonym: "1" EXACT []
is_a: CO_325:0100050 ! meredith & lawrence (1969) - condensed

[Term]
id: CO_325:0100139
name: First streak stage: specks elongate, becoming slightly wider to form narrow reddish-brown streaks.
namespace: BananaScale
synonym: "2" EXACT []
is_a: CO_325:0100050 ! meredith & lawrence (1969) - condensed

[Term]
id: CO_325:0100140
name: Second-streak stage: streaks change colour from reddish brown to dark brown or black, sometimes with a purplish tinge, clearly visible at the upper surface of the leaf.
namespace: BananaScale
synonym: "3" EXACT []
is_a: CO_325:0100050 ! meredith & lawrence (1969) - condensed

[Term]
id: CO_325:0100141
name: First-spot stage: the streaks broaden and become more or less fusiform or elliptical in outline and a water soaked border appears around each lesion.
namespace: BananaScale
synonym: "4" EXACT []
is_a: CO_325:0100050 ! meredith & lawrence (1969) - condensed

[Term]
id: CO_325:0100142
name: Second-spot stage: the dark brown or black centre of each lesion becomes slightly depressed and water soaked border becomes more pronounced.
namespace: BananaScale
synonym: "5" EXACT []
is_a: CO_325:0100050 ! meredith & lawrence (1969) - condensed

[Term]
id: CO_325:0100143
name: Third or mature spot stage: the centres of the lesions dry out becoming light grey or buff coloured and a bright yellow transitional zone appears between them and the normal green colour of the leaf. The lesions remain clearly visible after the leaf has collapsed or withered because of their light coloured centre and dark border.
namespace: BananaScale
synonym: "6" EXACT []
is_a: CO_325:0100050 ! meredith & lawrence (1969) - condensed

[Term]
id: CO_325:0100144
name: corm completely clean, no vascular discolouration
namespace: BananaScale
synonym: "1" EXACT []
is_a: CO_325:0100052 ! 5 pt corm discolouration scale

[Term]
id: CO_325:0100145
name: isolated points of discolouration in vascular tissue
namespace: BananaScale
synonym: "2" EXACT []
is_a: CO_325:0100052 ! 5 pt corm discolouration scale

[Term]
id: CO_325:0100146
name: discolouration of up to one-third of vascular tissue
namespace: BananaScale
synonym: "3" EXACT []
is_a: CO_325:0100052 ! 5 pt corm discolouration scale

[Term]
id: CO_325:0100147
name: discolouration of between one-third and two-thirds of vascular tissue
namespace: BananaScale
synonym: "4" EXACT []
is_a: CO_325:0100052 ! 5 pt corm discolouration scale

[Term]
id: CO_325:0100148
name: discolouration greater than two-thirds of vascular tissue
namespace: BananaScale
synonym: "5" EXACT []
is_a: CO_325:0100052 ! 5 pt corm discolouration scale

[Term]
id: CO_325:0100149
name: total discolouration of vascular tissue
namespace: BananaScale
synonym: "6" EXACT []
is_a: CO_325:0100052 ! 5 pt corm discolouration scale

[Term]
id: CO_325:0100150
name: absent
namespace: BananaScale
synonym: "0" EXACT []
is_a: CO_325:0100053 ! presence absence 0

[Term]
id: CO_325:0100151
name: present
namespace: BananaScale
synonym: "1" EXACT []
is_a: CO_325:0100053 ! presence absence 0

[Term]
id: CO_325:0100152
name: absent
namespace: BananaScale
synonym: "1" EXACT []
is_a: CO_325:0100054 ! presence absence 1

[Term]
id: CO_325:0100153
name: present
namespace: BananaScale
synonym: "2" EXACT []
is_a: CO_325:0100054 ! presence absence 1

[Term]
id: CO_325:0100154
name: no weevil damage
namespace: BananaScale
synonym: "1" EXACT []
is_a: CO_325:0100058 ! weevil damage

[Term]
id: CO_325:0100155
name: partial damage
namespace: BananaScale
synonym: "2" EXACT []
is_a: CO_325:0100058 ! weevil damage

[Term]
id: CO_325:0100156
name: severe damage
namespace: BananaScale
synonym: "3" EXACT []
is_a: CO_325:0100058 ! weevil damage

[Term]
id: CO_325:0100157
name: less than or equal to 2 m
namespace: BananaScale
synonym: "1" EXACT []
is_a: CO_325:0100062 ! height score (1 to 3)

[Term]
id: CO_325:0100158
name: 2.1-2.9 m
namespace: BananaScale
synonym: "2" EXACT []
is_a: CO_325:0100062 ! height score (1 to 3)

[Term]
id: CO_325:0100159
name: equal to or more than 3 m
namespace: BananaScale
synonym: "3" EXACT []
is_a: CO_325:0100062 ! height score (1 to 3)

[Term]
id: CO_325:0100160
name: cream
namespace: BananaScale
synonym: "1" EXACT []
is_a: CO_325:0100063 ! bd colour chart a - 2016

[Term]
id: CO_325:0100161
name: orange red
namespace: BananaScale
synonym: "10" EXACT []
is_a: CO_325:0100063 ! bd colour chart a - 2016

[Term]
id: CO_325:0100162
name: red
namespace: BananaScale
synonym: "11" EXACT []
is_a: CO_325:0100063 ! bd colour chart a - 2016

[Term]
id: CO_325:0100163
name: pink-purple
namespace: BananaScale
synonym: "12" EXACT []
is_a: CO_325:0100063 ! bd colour chart a - 2016

[Term]
id: CO_325:0100164
name: purple-brown
namespace: BananaScale
synonym: "13" EXACT []
is_a: CO_325:0100063 ! bd colour chart a - 2016

[Term]
id: CO_325:0100165
name: red-purple
namespace: BananaScale
synonym: "14" EXACT []
is_a: CO_325:0100063 ! bd colour chart a - 2016

[Term]
id: CO_325:0100166
name: purple
namespace: BananaScale
synonym: "15" EXACT []
is_a: CO_325:0100063 ! bd colour chart a - 2016

[Term]
id: CO_325:0100167
name: yellow
namespace: BananaScale
synonym: "2" EXACT []
is_a: CO_325:0100063 ! bd colour chart a - 2016

[Term]
id: CO_325:0100168
name: watery green
namespace: BananaScale
synonym: "3" EXACT []
is_a: CO_325:0100063 ! bd colour chart a - 2016

[Term]
id: CO_325:0100169
name: green yellow
namespace: BananaScale
synonym: "4" EXACT []
is_a: CO_325:0100063 ! bd colour chart a - 2016

[Term]
id: CO_325:0100170
name: light green
namespace: BananaScale
synonym: "5" EXACT []
is_a: CO_325:0100063 ! bd colour chart a - 2016

[Term]
id: CO_325:0100171
name: medium green
namespace: BananaScale
synonym: "6" EXACT []
is_a: CO_325:0100063 ! bd colour chart a - 2016

[Term]
id: CO_325:0100172
name: green
namespace: BananaScale
synonym: "7" EXACT []
is_a: CO_325:0100063 ! bd colour chart a - 2016

[Term]
id: CO_325:0100173
name: dark green
namespace: BananaScale
synonym: "8" EXACT []
is_a: CO_325:0100063 ! bd colour chart a - 2016

[Term]
id: CO_325:0100174
name: whitish
namespace: BananaScale
synonym: "9" EXACT []
is_a: CO_325:0100063 ! bd colour chart a - 2016

[Term]
id: CO_325:0100175
name: no pigmentation
namespace: BananaScale
synonym: "1" EXACT []
is_a: CO_325:0100064 ! blotch pigmentation scale (1 to 4)

[Term]
id: CO_325:0100176
name: sparse blotching (<20%)
namespace: BananaScale
synonym: "2" EXACT []
is_a: CO_325:0100064 ! blotch pigmentation scale (1 to 4)

[Term]
id: CO_325:0100177
name: moderate blotching (20-50%)
namespace: BananaScale
synonym: "3" EXACT []
is_a: CO_325:0100064 ! blotch pigmentation scale (1 to 4)

[Term]
id: CO_325:0100178
name: extensive pigmentation (>50%)
namespace: BananaScale
synonym: "4" EXACT []
is_a: CO_325:0100064 ! blotch pigmentation scale (1 to 4)

[Term]
id: CO_325:0100179
name: sparse blotching
namespace: BananaScale
synonym: "1" EXACT []
is_a: CO_325:0100065 ! blotch pigmentation scale (1 to 5)

[Term]
id: CO_325:0100180
name: small blotches
namespace: BananaScale
synonym: "2" EXACT []
is_a: CO_325:0100065 ! blotch pigmentation scale (1 to 5)

[Term]
id: CO_325:0100181
name: large blotches
namespace: BananaScale
synonym: "3" EXACT []
is_a: CO_325:0100065 ! blotch pigmentation scale (1 to 5)

[Term]
id: CO_325:0100182
name: extensive pigmentation
namespace: BananaScale
synonym: "4" EXACT []
is_a: CO_325:0100065 ! blotch pigmentation scale (1 to 5)

[Term]
id: CO_325:0100183
name: without pigmentation
namespace: BananaScale
synonym: "5" EXACT []
is_a: CO_325:0100065 ! blotch pigmentation scale (1 to 5)

[Term]
id: CO_325:0100184
name: orange-brown (mahogany, like in Pisang Mas)
namespace: BananaScale
synonym: "1" EXACT []
is_a: CO_325:0100066 ! blotch color scale (1 to 4)

[Term]
id: CO_325:0100185
name: brown
namespace: BananaScale
synonym: "2" EXACT []
is_a: CO_325:0100066 ! blotch color scale (1 to 4)

[Term]
id: CO_325:0100186
name: black-purple
namespace: BananaScale
synonym: "3" EXACT []
is_a: CO_325:0100066 ! blotch color scale (1 to 4)

[Term]
id: CO_325:0100187
name: other
namespace: BananaScale
synonym: "4" EXACT []
is_a: CO_325:0100066 ! blotch color scale (1 to 4)

[Term]
id: CO_325:0100188
name: brown
namespace: BananaScale
synonym: "1" EXACT []
is_a: CO_325:0100067 ! blotch color scale (1 to 5)

[Term]
id: CO_325:0100189
name: dark brown
namespace: BananaScale
synonym: "2" EXACT []
is_a: CO_325:0100067 ! blotch color scale (1 to 5)

[Term]
id: CO_325:0100190
name: brown-black
namespace: BananaScale
synonym: "3" EXACT []
is_a: CO_325:0100067 ! blotch color scale (1 to 5)

[Term]
id: CO_325:0100191
name: black-purple
namespace: BananaScale
synonym: "4" EXACT []
is_a: CO_325:0100067 ! blotch color scale (1 to 5)

[Term]
id: CO_325:0100192
name: other
namespace: BananaScale
synonym: "5" EXACT []
is_a: CO_325:0100067 ! blotch color scale (1 to 5)

[Term]
id: CO_325:0100193
name: margins spreading
namespace: BananaScale
synonym: "1" EXACT []
is_a: CO_325:0100068 ! margin behaviour scale (1 to 4)

[Term]
id: CO_325:0100194
name: margins erect
namespace: BananaScale
synonym: "2" EXACT []
is_a: CO_325:0100068 ! margin behaviour scale (1 to 4)

[Term]
id: CO_325:0100195
name: margins curved inward
namespace: BananaScale
synonym: "3" EXACT []
is_a: CO_325:0100068 ! margin behaviour scale (1 to 4)

[Term]
id: CO_325:0100196
name: margins overlapping
namespace: BananaScale
synonym: "4" EXACT []
is_a: CO_325:0100068 ! margin behaviour scale (1 to 4)

[Term]
id: CO_325:0100197
name: open with margins spreading
namespace: BananaScale
synonym: "1" EXACT []
is_a: CO_325:0100069 ! margin behaviour scale (1 to 5)

[Term]
id: CO_325:0100198
name: wide with erect margins
namespace: BananaScale
synonym: "2" EXACT []
is_a: CO_325:0100069 ! margin behaviour scale (1 to 5)

[Term]
id: CO_325:0100199
name: straight with erect margins
namespace: BananaScale
synonym: "3" EXACT []
is_a: CO_325:0100069 ! margin behaviour scale (1 to 5)

[Term]
id: CO_325:0100200
name: margins curved inward
namespace: BananaScale
synonym: "4" EXACT []
is_a: CO_325:0100069 ! margin behaviour scale (1 to 5)

[Term]
id: CO_325:0100201
name: margins overlapping
namespace: BananaScale
synonym: "5" EXACT []
is_a: CO_325:0100069 ! margin behaviour scale (1 to 5)

[Term]
id: CO_325:0100202
name: winged
namespace: BananaScale
synonym: "1" EXACT []
is_a: CO_325:0100070 ! wing presence/absence

[Term]
id: CO_325:0100203
name: not winged
namespace: BananaScale
synonym: "2" EXACT []
is_a: CO_325:0100070 ! wing presence/absence

[Term]
id: CO_325:0100204
name: winged and undulating
namespace: BananaScale
synonym: "1" EXACT []
is_a: CO_325:0100071 ! wing presence/absence and clasping presence/absence scale 1 to 5

[Term]
id: CO_325:0100205
name: winged and not clasping the pseudostem
namespace: BananaScale
synonym: "2" EXACT []
is_a: CO_325:0100071 ! wing presence/absence and clasping presence/absence scale 1 to 5

[Term]
id: CO_325:0100206
name: winged and clasping the pseudostem
namespace: BananaScale
synonym: "3" EXACT []
is_a: CO_325:0100071 ! wing presence/absence and clasping presence/absence scale 1 to 5

[Term]
id: CO_325:0100207
name: not winged and clasping the pseudostem
namespace: BananaScale
synonym: "4" EXACT []
is_a: CO_325:0100071 ! wing presence/absence and clasping presence/absence scale 1 to 5

[Term]
id: CO_325:0100208
name: not winged and not clasping the pseudostem
namespace: BananaScale
synonym: "5" EXACT []
is_a: CO_325:0100071 ! wing presence/absence and clasping presence/absence scale 1 to 5

[Term]
id: CO_325:0100209
name: clasping
namespace: BananaScale
synonym: "1" EXACT []
is_a: CO_325:0100072 ! clasping or not clasping

[Term]
id: CO_325:0100210
name: not clasping
namespace: BananaScale
synonym: "2" EXACT []
is_a: CO_325:0100072 ! clasping or not clasping

[Term]
id: CO_325:0100211
name: green
namespace: BananaScale
synonym: "1" EXACT []
is_a: CO_325:0100073 ! bd colour chart a - 1996

[Term]
id: CO_325:0100212
name: pink-purple to red
namespace: BananaScale
synonym: "2" EXACT []
is_a: CO_325:0100073 ! bd colour chart a - 1996

[Term]
id: CO_325:0100213
name: purple to blue
namespace: BananaScale
synonym: "3" EXACT []
is_a: CO_325:0100073 ! bd colour chart a - 1996

[Term]
id: CO_325:0100214
name: other
namespace: BananaScale
synonym: "4" EXACT []
is_a: CO_325:0100073 ! bd colour chart a - 1996

[Term]
id: CO_325:0100215
name: no contrast between margin and petiole (without a colour line along)
namespace: BananaScale
synonym: "1" EXACT []
is_a: CO_325:0100074 ! petiole-margin contrast

[Term]
id: CO_325:0100216
name: contrast between margin and petiole (with a contrasting colour line along)
namespace: BananaScale
synonym: "2" EXACT []
is_a: CO_325:0100074 ! petiole-margin contrast

[Term]
id: CO_325:0100217
name: hanging vertically
namespace: BananaScale
synonym: "1" EXACT []
is_a: CO_325:0100075 ! bunch position scale(1 to 5)

[Term]
id: CO_325:0100218
name: slightly angled
namespace: BananaScale
synonym: "2" EXACT []
is_a: CO_325:0100075 ! bunch position scale(1 to 5)

[Term]
id: CO_325:0100219
name: hanging at a 45 degree angle
namespace: BananaScale
synonym: "3" EXACT []
is_a: CO_325:0100075 ! bunch position scale(1 to 5)

[Term]
id: CO_325:0100220
name: horizontal
namespace: BananaScale
synonym: "4" EXACT []
is_a: CO_325:0100075 ! bunch position scale(1 to 5)

[Term]
id: CO_325:0100221
name: erect
namespace: BananaScale
synonym: "5" EXACT []
is_a: CO_325:0100075 ! bunch position scale(1 to 5)

[Term]
id: CO_325:0100222
name: cylindrical
namespace: BananaScale
synonym: "1" EXACT []
is_a: CO_325:0100076 ! bunch shape scale (1 to 5)

[Term]
id: CO_325:0100223
name: cone shaped
namespace: BananaScale
synonym: "2" EXACT []
synonym: "truncate (" EXACT []
is_a: CO_325:0100076 ! bunch shape scale (1 to 5)

[Term]
id: CO_325:0100224
name: asymmetrical
namespace: BananaScale
synonym: "3" EXACT []
is_a: CO_325:0100076 ! bunch shape scale (1 to 5)

[Term]
id: CO_325:0100225
name: spiral (all fruit are attached to a unique crown coiled around the stalk)
namespace: BananaScale
synonym: "4" EXACT []
is_a: CO_325:0100076 ! bunch shape scale (1 to 5)

[Term]
id: CO_325:0100226
name: other
namespace: BananaScale
synonym: "5" EXACT []
is_a: CO_325:0100076 ! bunch shape scale (1 to 5)

[Term]
id: CO_325:0100227
name: truncated
namespace: BananaScale
synonym: "1" EXACT []
is_a: CO_325:0100077 ! rachis type scale (1 to 2)

[Term]
id: CO_325:0100228
name: present
namespace: BananaScale
synonym: "2" EXACT []
is_a: CO_325:0100077 ! rachis type scale (1 to 2)

[Term]
id: CO_325:0100229
name: falling vertically
namespace: BananaScale
synonym: "1" EXACT []
is_a: CO_325:0100078 ! rachis angle scale (1 to 2)

[Term]
id: CO_325:0100230
name: at an angle
namespace: BananaScale
synonym: "2" EXACT []
is_a: CO_325:0100078 ! rachis angle scale (1 to 2)

[Term]
id: CO_325:0100231
name: with a curve
namespace: BananaScale
synonym: "3" EXACT []
is_a: CO_325:0100078 ! rachis angle scale (1 to 2)

[Term]
id: CO_325:0100232
name: horizontal or supra-horizontal
namespace: BananaScale
synonym: "4" EXACT []
is_a: CO_325:0100078 ! rachis angle scale (1 to 2)

[Term]
id: CO_325:0100233
name: erect
namespace: BananaScale
synonym: "5" EXACT []
is_a: CO_325:0100078 ! rachis angle scale (1 to 2)

[Term]
id: CO_325:0100234
name: bare
namespace: BananaScale
synonym: "1" EXACT []
is_a: CO_325:0100079 ! rachis appearance scale (1 to 5)

[Term]
id: CO_325:0100235
name: neutral flowers on one to few hands only near the bunch (rest of stalk is bare)
namespace: BananaScale
synonym: "2" EXACT []
is_a: CO_325:0100079 ! rachis appearance scale (1 to 5)

[Term]
id: CO_325:0100236
name: male flowers/bracts above the male bud (rest of stalk is bare)
namespace: BananaScale
synonym: "3" EXACT []
is_a: CO_325:0100079 ! rachis appearance scale (1 to 5)

[Term]
id: CO_325:0100237
name: neutral/male flowers and presence of withered bracts on the entire stalk
namespace: BananaScale
synonym: "4" EXACT []
is_a: CO_325:0100079 ! rachis appearance scale (1 to 5)

[Term]
id: CO_325:0100238
name: neutral/male flowers on the whole stalk without persistent bracts (still firmly attached to the rachis)
namespace: BananaScale
synonym: "5" EXACT []
is_a: CO_325:0100079 ! rachis appearance scale (1 to 5)

[Term]
id: CO_325:0100239
name: small bunch from neutral/hermaphrodite flowers just above the male bud
namespace: BananaScale
synonym: "6" EXACT []
is_a: CO_325:0100079 ! rachis appearance scale (1 to 5)

[Term]
id: CO_325:0100240
name: other
namespace: BananaScale
synonym: "7" EXACT []
is_a: CO_325:0100079 ! rachis appearance scale (1 to 5)

[Term]
id: CO_325:0100241
name: skinny (w/y less than or equal to 0.45)
namespace: BananaScale
synonym: "1" EXACT []
is_a: CO_325:0100080 ! bud shape scale (1 to 3)

[Term]
id: CO_325:0100242
name: medium (0.45 < w/y < 0.55)
namespace: BananaScale
synonym: "2" EXACT []
is_a: CO_325:0100080 ! bud shape scale (1 to 3)

[Term]
id: CO_325:0100243
name: fat (w/y equal to or more than 0.55)
namespace: BananaScale
synonym: "3" EXACT []
is_a: CO_325:0100080 ! bud shape scale (1 to 3)

[Term]
id: CO_325:0100244
name: like a top
namespace: BananaScale
synonym: "1" EXACT []
is_a: CO_325:0100081 ! bud shape scale (1 to 5)

[Term]
id: CO_325:0100245
name: lanceolate
namespace: BananaScale
synonym: "2" EXACT []
is_a: CO_325:0100081 ! bud shape scale (1 to 5)

[Term]
id: CO_325:0100246
name: intermediate
namespace: BananaScale
synonym: "3" EXACT []
is_a: CO_325:0100081 ! bud shape scale (1 to 5)

[Term]
id: CO_325:0100247
name: ovoid
namespace: BananaScale
synonym: "4" EXACT []
is_a: CO_325:0100081 ! bud shape scale (1 to 5)

[Term]
id: CO_325:0100248
name: rounded
namespace: BananaScale
synonym: "5" EXACT []
is_a: CO_325:0100081 ! bud shape scale (1 to 5)

[Term]
id: CO_325:0100249
name: short (y less than or equal to 20 cm)
namespace: BananaScale
synonym: "1" EXACT []
is_a: CO_325:0100082 ! bud length scale (1 to 3)

[Term]
id: CO_325:0100250
name: medium (20 cm < y < 30 cm)
namespace: BananaScale
synonym: "2" EXACT []
is_a: CO_325:0100082 ! bud length scale (1 to 3)

[Term]
id: CO_325:0100251
name: long (equal to or more than 30 cm)
namespace: BananaScale
synonym: "3" EXACT []
is_a: CO_325:0100082 ! bud length scale (1 to 3)

[Term]
id: CO_325:0100252
name: less than or equal to 20 cm
namespace: BananaScale
synonym: "1" EXACT []
is_a: CO_325:0100083 ! bud size scale (1 to 3)

[Term]
id: CO_325:0100253
name: 21-30 cm
namespace: BananaScale
synonym: "2" EXACT []
is_a: CO_325:0100083 ! bud size scale (1 to 3)

[Term]
id: CO_325:0100254
name: equal to or more than 31 cm
namespace: BananaScale
synonym: "3" EXACT []
is_a: CO_325:0100083 ! bud size scale (1 to 3)

[Term]
id: CO_325:0100255
name: High shouldered (x/y less than or equal to 0.28)
namespace: BananaScale
synonym: "1" EXACT []
is_a: CO_325:0100084 ! bud shoulder scale (1 to 3)

[Term]
id: CO_325:0100256
name: medium shouldered (0.28 < x/y < 0.30)
namespace: BananaScale
synonym: "2" EXACT []
is_a: CO_325:0100084 ! bud shoulder scale (1 to 3)

[Term]
id: CO_325:0100257
name: low shouldered (x/y more than or equal to 0.30)
namespace: BananaScale
synonym: "3" EXACT []
is_a: CO_325:0100084 ! bud shoulder scale (1 to 3)

[Term]
id: CO_325:0100258
name: pointed
namespace: BananaScale
synonym: "1" EXACT []
is_a: CO_325:0100085 ! bract apex scale (1 to 4)

[Term]
id: CO_325:0100259
name: intermeditae
namespace: BananaScale
synonym: "2" EXACT []
is_a: CO_325:0100085 ! bract apex scale (1 to 4)

[Term]
id: CO_325:0100260
name: obtuse
namespace: BananaScale
synonym: "3" EXACT []
is_a: CO_325:0100085 ! bract apex scale (1 to 4)

[Term]
id: CO_325:0100261
name: obtuse and split
namespace: BananaScale
synonym: "4" EXACT []
is_a: CO_325:0100085 ! bract apex scale (1 to 4)

[Term]
id: CO_325:0100262
name: pointed
namespace: BananaScale
synonym: "1" EXACT []
is_a: CO_325:0100086 ! bract apex scale (1 to 5)

[Term]
id: CO_325:0100263
name: slightly pointed
namespace: BananaScale
synonym: "2" EXACT []
is_a: CO_325:0100086 ! bract apex scale (1 to 5)

[Term]
id: CO_325:0100264
name: intermediate
namespace: BananaScale
synonym: "3" EXACT []
is_a: CO_325:0100086 ! bract apex scale (1 to 5)

[Term]
id: CO_325:0100265
name: obtuse
namespace: BananaScale
synonym: "4" EXACT []
is_a: CO_325:0100086 ! bract apex scale (1 to 5)

[Term]
id: CO_325:0100266
name: obtuse and split
namespace: BananaScale
synonym: "5" EXACT []
is_a: CO_325:0100086 ! bract apex scale (1 to 5)

[Term]
id: CO_325:0100267
name: convolute
namespace: BananaScale
synonym: "1" EXACT []
is_a: CO_325:0100087 ! bract imbrication scale (1 to 3)

[Term]
id: CO_325:0100268
name: moderately imbricate
namespace: BananaScale
synonym: "2" EXACT []
is_a: CO_325:0100087 ! bract imbrication scale (1 to 3)

[Term]
id: CO_325:0100269
name: highly imbricate
namespace: BananaScale
synonym: "3" EXACT []
is_a: CO_325:0100087 ! bract imbrication scale (1 to 3)

[Term]
id: CO_325:0100270
name: revolute (rolling)
namespace: BananaScale
synonym: "1" EXACT []
is_a: CO_325:0100088 ! bract behaviour scale (1 to 2)

[Term]
id: CO_325:0100271
name: not revolute (not rolling)
namespace: BananaScale
synonym: "2" EXACT []
is_a: CO_325:0100088 ! bract behaviour scale (1 to 2)

[Term]
id: CO_325:0100272
name: white
namespace: BananaScale
synonym: "1" EXACT []
is_a: CO_325:0100089 ! bd colour chart b - 2016

[Term]
id: CO_325:0100273
name: pink/pink-purple
namespace: BananaScale
synonym: "10" EXACT []
is_a: CO_325:0100089 ! bd colour chart b - 2016

[Term]
id: CO_325:0100274
name: brown/rusty-brown
namespace: BananaScale
synonym: "11" EXACT []
is_a: CO_325:0100089 ! bd colour chart b - 2016

[Term]
id: CO_325:0100275
name: beige-pink
namespace: BananaScale
synonym: "12" EXACT []
is_a: CO_325:0100089 ! bd colour chart b - 2016

[Term]
id: CO_325:0100276
name: silvery
namespace: BananaScale
synonym: "13" EXACT []
is_a: CO_325:0100089 ! bd colour chart b - 2016

[Term]
id: CO_325:0100277
name: light green
namespace: BananaScale
synonym: "14" EXACT []
is_a: CO_325:0100089 ! bd colour chart b - 2016

[Term]
id: CO_325:0100278
name: green
namespace: BananaScale
synonym: "15" EXACT []
is_a: CO_325:0100089 ! bd colour chart b - 2016

[Term]
id: CO_325:0100279
name: cream
namespace: BananaScale
synonym: "2" EXACT []
is_a: CO_325:0100089 ! bd colour chart b - 2016

[Term]
id: CO_325:0100280
name: ivory
namespace: BananaScale
synonym: "3" EXACT []
is_a: CO_325:0100089 ! bd colour chart b - 2016

[Term]
id: CO_325:0100281
name: yellow
namespace: BananaScale
synonym: "4" EXACT []
is_a: CO_325:0100089 ! bd colour chart b - 2016

[Term]
id: CO_325:0100282
name: bright yellow
namespace: BananaScale
synonym: "5" EXACT []
is_a: CO_325:0100089 ! bd colour chart b - 2016

[Term]
id: CO_325:0100283
name: orange
namespace: BananaScale
synonym: "6" EXACT []
is_a: CO_325:0100089 ! bd colour chart b - 2016

[Term]
id: CO_325:0100284
name: orange red
namespace: BananaScale
synonym: "7" EXACT []
is_a: CO_325:0100089 ! bd colour chart b - 2016

[Term]
id: CO_325:0100285
name: red
namespace: BananaScale
synonym: "8" EXACT []
is_a: CO_325:0100089 ! bd colour chart b - 2016

[Term]
id: CO_325:0100286
name: red-purple
namespace: BananaScale
synonym: "9" EXACT []
is_a: CO_325:0100089 ! bd colour chart b - 2016

[Term]
id: CO_325:0100287
name: white
namespace: BananaScale
synonym: "1" EXACT []
is_a: CO_325:0100090 ! bd colour chart b - 1996

[Term]
id: CO_325:0100288
name: cream
namespace: BananaScale
synonym: "2" EXACT []
is_a: CO_325:0100090 ! bd colour chart b - 1996

[Term]
id: CO_325:0100289
name: yellow
namespace: BananaScale
synonym: "3" EXACT []
is_a: CO_325:0100090 ! bd colour chart b - 1996

[Term]
id: CO_325:0100290
name: orange
namespace: BananaScale
synonym: "4" EXACT []
is_a: CO_325:0100090 ! bd colour chart b - 1996

[Term]
id: CO_325:0100291
name: pink/pink-purple
namespace: BananaScale
synonym: "5" EXACT []
is_a: CO_325:0100090 ! bd colour chart b - 1996

[Term]
id: CO_325:0100292
name: other
namespace: BananaScale
synonym: "6" EXACT []
is_a: CO_325:0100090 ! bd colour chart b - 1996

[Term]
id: CO_325:0100293
name: less than or equal to 15 cm
namespace: BananaScale
synonym: "1" EXACT []
is_a: CO_325:0100092 ! fruit length scale (1 to 5)

[Term]
id: CO_325:0100294
name: 16-20 cm
namespace: BananaScale
synonym: "2" EXACT []
is_a: CO_325:0100092 ! fruit length scale (1 to 5)

[Term]
id: CO_325:0100295
name: 21-25 cm
namespace: BananaScale
synonym: "3" EXACT []
is_a: CO_325:0100092 ! fruit length scale (1 to 5)

[Term]
id: CO_325:0100296
name: 26-30 cm
namespace: BananaScale
synonym: "4" EXACT []
is_a: CO_325:0100092 ! fruit length scale (1 to 5)

[Term]
id: CO_325:0100297
name: equal to or more than 31 cm
namespace: BananaScale
synonym: "5" EXACT []
is_a: CO_325:0100092 ! fruit length scale (1 to 5)

[Term]
id: CO_325:0100298
name: straight
namespace: BananaScale
synonym: "1" EXACT []
is_a: CO_325:0100093 ! fruit curve shape (scale 1 to 6)

[Term]
id: CO_325:0100299
name: slightly curved
namespace: BananaScale
synonym: "2" EXACT []
is_a: CO_325:0100093 ! fruit curve shape (scale 1 to 6)

[Term]
id: CO_325:0100300
name: straight in the distal part
namespace: BananaScale
synonym: "3" EXACT []
is_a: CO_325:0100093 ! fruit curve shape (scale 1 to 6)

[Term]
id: CO_325:0100301
name: curved (sharp curve)
namespace: BananaScale
synonym: "4" EXACT []
is_a: CO_325:0100093 ! fruit curve shape (scale 1 to 6)

[Term]
id: CO_325:0100302
name: curved in slight 'S' shape (double curvature)
namespace: BananaScale
synonym: "5" EXACT []
is_a: CO_325:0100093 ! fruit curve shape (scale 1 to 6)

[Term]
id: CO_325:0100303
name: other
namespace: BananaScale
synonym: "6" EXACT []
is_a: CO_325:0100093 ! fruit curve shape (scale 1 to 6)

[Term]
id: CO_325:0100304
name: straight (or slightly curved)
namespace: BananaScale
synonym: "1" EXACT []
is_a: CO_325:0100094 ! fruit curve shape (scale 1 to 5)

[Term]
id: CO_325:0100305
name: straight in the distal part
namespace: BananaScale
synonym: "2" EXACT []
is_a: CO_325:0100094 ! fruit curve shape (scale 1 to 5)

[Term]
id: CO_325:0100306
name: curved (sharp curve)
namespace: BananaScale
synonym: "3" EXACT []
is_a: CO_325:0100094 ! fruit curve shape (scale 1 to 5)

[Term]
id: CO_325:0100307
name: curved in 'S' shape (double curvature)
namespace: BananaScale
synonym: "4" EXACT []
is_a: CO_325:0100094 ! fruit curve shape (scale 1 to 5)

[Term]
id: CO_325:0100308
name: other
namespace: BananaScale
synonym: "5" EXACT []
is_a: CO_325:0100094 ! fruit curve shape (scale 1 to 5)

[Term]
id: CO_325:0100309
name: pointed
namespace: BananaScale
synonym: "1" EXACT []
is_a: CO_325:0100095 ! fruit apex scale (1 to 5)

[Term]
id: CO_325:0100310
name: lengthily pointed (like plantain)
namespace: BananaScale
synonym: "2" EXACT []
is_a: CO_325:0100095 ! fruit apex scale (1 to 5)

[Term]
id: CO_325:0100311
name: blunt-tipped (plateau at tip)
namespace: BananaScale
synonym: "3" EXACT []
is_a: CO_325:0100095 ! fruit apex scale (1 to 5)

[Term]
id: CO_325:0100312
name: strongly bottle-necked (wider under tip than number 2)
namespace: BananaScale
synonym: "4" EXACT []
is_a: CO_325:0100095 ! fruit apex scale (1 to 5)

[Term]
id: CO_325:0100313
name: rounded
namespace: BananaScale
synonym: "5" EXACT []
is_a: CO_325:0100095 ! fruit apex scale (1 to 5)

[Term]
id: CO_325:0100314
name: without flower relicts
namespace: BananaScale
synonym: "1" EXACT []
is_a: CO_325:0100096 ! fruit relicts scale (1 to 4)

[Term]
id: CO_325:0100315
name: few flower relicts (< 20% of the fruits with relicts)
namespace: BananaScale
synonym: "2" EXACT []
is_a: CO_325:0100096 ! fruit relicts scale (1 to 4)

[Term]
id: CO_325:0100316
name: persistent flower relicts (> 20% of the fruits with relicts)
namespace: BananaScale
synonym: "3" EXACT []
is_a: CO_325:0100096 ! fruit relicts scale (1 to 4)

[Term]
id: CO_325:0100317
name: only base of the style persists
namespace: BananaScale
synonym: "4" EXACT []
is_a: CO_325:0100096 ! fruit relicts scale (1 to 4)

[Term]
id: CO_325:0100318
name: without any floral relicts
namespace: BananaScale
synonym: "1" EXACT []
is_a: CO_325:0100097 ! fruit relicts scale (1 to 3)

[Term]
id: CO_325:0100319
name: persistent style
namespace: BananaScale
synonym: "2" EXACT []
is_a: CO_325:0100097 ! fruit relicts scale (1 to 3)

[Term]
id: CO_325:0100320
name: base of the style prominent
namespace: BananaScale
synonym: "3" EXACT []
is_a: CO_325:0100097 ! fruit relicts scale (1 to 3)

[Term]
id: CO_325:0100321
name: less than or equal to 10 mm
namespace: BananaScale
synonym: "1" EXACT []
is_a: CO_325:0100098 ! fruit pedicel scale (1 to 3)

[Term]
id: CO_325:0100322
name: 11-20 mm
namespace: BananaScale
synonym: "2" EXACT []
is_a: CO_325:0100098 ! fruit pedicel scale (1 to 3)

[Term]
id: CO_325:0100323
name: equal to or more than 21 mm
namespace: BananaScale
synonym: "3" EXACT []
is_a: CO_325:0100098 ! fruit pedicel scale (1 to 3)

[Term]
id: CO_325:0100324
name: no visible sign of fusion
namespace: BananaScale
synonym: "1" EXACT []
is_a: CO_325:0100099 ! fusion of pedicel scale (1 to 2)

[Term]
id: CO_325:0100325
name: partially fused (up to 50% of the length of the pedicel)
namespace: BananaScale
synonym: "2" EXACT []
is_a: CO_325:0100099 ! fusion of pedicel scale (1 to 2)

[Term]
id: CO_325:0100326
name: totally fused (more than 50% of the length of the pedicel)
namespace: BananaScale
synonym: "3" EXACT []
is_a: CO_325:0100099 ! fusion of pedicel scale (1 to 2)

[Term]
id: CO_325:0100327
name: dislike very much
namespace: BananaScale
synonym: "1" EXACT []
is_a: CO_325:0100100 ! 1 to 5 acceptability score

[Term]
id: CO_325:0100328
name: dislike
namespace: BananaScale
synonym: "2" EXACT []
is_a: CO_325:0100100 ! 1 to 5 acceptability score

[Term]
id: CO_325:0100329
name: like fairly
namespace: BananaScale
synonym: "3" EXACT []
is_a: CO_325:0100100 ! 1 to 5 acceptability score

[Term]
id: CO_325:0100330
name: like very much
namespace: BananaScale
synonym: "4" EXACT []
is_a: CO_325:0100100 ! 1 to 5 acceptability score

[Term]
id: CO_325:0100331
name: like extremely
namespace: BananaScale
synonym: "5" EXACT []
is_a: CO_325:0100100 ! 1 to 5 acceptability score

[Term]
id: CO_325:0100332
name: suckering behavior (1 to 3)
namespace: BananaScale
is_a: CO_325:1000015 ! Nominal

[Term]
id: CO_325:0100333
name: high apical dominance
namespace: BananaScale
is_a: CO_325:0100332 ! suckering behavior (1 to 3)

[Term]
id: CO_325:0100334
name: medium apical dominance
namespace: BananaScale
is_a: CO_325:0100332 ! suckering behavior (1 to 3)

[Term]
id: CO_325:0100335
name: low apical dominance
namespace: BananaScale
is_a: CO_325:0100332 ! suckering behavior (1 to 3)

[Term]
id: CO_325:0100336
name: bunch size (scale 1 to 3)
namespace: BananaScale
is_a: CO_325:1000015 ! Nominal

[Term]
id: CO_325:0100337
name: small
namespace: BananaScale
synonym: "1" EXACT []
is_a: CO_325:0100336 ! bunch size (scale 1 to 3)

[Term]
id: CO_325:0100338
name: medium
namespace: BananaScale
synonym: "2" EXACT []
is_a: CO_325:0100336 ! bunch size (scale 1 to 3)

[Term]
id: CO_325:0100339
name: large
namespace: BananaScale
synonym: "3" EXACT []
is_a: CO_325:0100336 ! bunch size (scale 1 to 3)

[Term]
id: CO_325:0101100
name: black streak scale (1 to 3)
is_a: CO_325:1000015 ! Nominal

[Term]
id: CO_325:1000001
name: Agronomical
namespace: BananaTrait
is_a: CO_325:0000000 ! CGIAR banana trait ontology

[Term]
id: CO_325:1000002
name: Biotic_stress
namespace: BananaTrait
is_a: CO_325:0000000 ! CGIAR banana trait ontology

[Term]
id: CO_325:1000003
name: Morphological
namespace: BananaTrait
is_a: CO_325:0000000 ! CGIAR banana trait ontology

[Term]
id: CO_325:1000004
name: Phenological
namespace: BananaTrait
is_a: CO_325:0000000 ! CGIAR banana trait ontology

[Term]
id: CO_325:1000005
name: Physiological
namespace: BananaTrait
is_a: CO_325:0000000 ! CGIAR banana trait ontology

[Term]
id: CO_325:1000006
name: Quality_traits
namespace: BananaTrait
is_a: CO_325:0000000 ! CGIAR banana trait ontology

[Term]
id: CO_325:1000008
name: Measurement
namespace: BananaMethod
is_a: CO_325:1000021 ! Method

[Term]
id: CO_325:1000009
name: Counting
namespace: BananaMethod
is_a: CO_325:1000021 ! Method

[Term]
id: CO_325:1000010
name: Computation
namespace: BananaMethod
is_a: CO_325:1000021 ! Method

[Term]
id: CO_325:1000011
name: Estimation
namespace: BananaMethod
is_a: CO_325:1000021 ! Method

[Term]
id: CO_325:1000012
name: Ordinal
namespace: BananaScale
is_a: CO_325:1000022 ! Scale

[Term]
id: CO_325:1000014
name: Text
namespace: BananaScale
is_a: CO_325:1000022 ! Scale

[Term]
id: CO_325:1000015
name: Nominal
namespace: BananaScale
is_a: CO_325:1000022 ! Scale

[Term]
id: CO_325:1000016
name: Duration
namespace: BananaScale
is_a: CO_325:1000022 ! Scale

[Term]
id: CO_325:1000017
name: Numerical
namespace: BananaScale
is_a: CO_325:1000022 ! Scale

[Term]
id: CO_325:1000018
name: Time
namespace: BananaScale
is_a: CO_325:1000022 ! Scale

[Term]
id: CO_325:1000021
name: Method
namespace: BananaMethod

[Term]
id: CO_325:1000022
name: Scale
namespace: BananaScale

[Term]
id: CO_325:1000024
name: Variable
namespace: BananaTrait
is_a: CO_325:0000000 ! CGIAR banana trait ontology

[Typedef]
id: method_of
name: method_of

[Typedef]
id: scale_of
name: scale_of

[Typedef]
id: variable_of
name: variable_of

